theorem OnePlusOneEqualsTwo() {
  let P: PeanoStructure;
  let s: P → P;  // successor function
  let zero = P \ s(P);  // definition of 0
  let one = s(zero);    // definition of 1
  let two = s(one);     // definition of 2
  
  assert(
    one + one = two
  )
} ↔

proof OnePlusOneEqualsTwo() {
  lemma AdditionSuccessor() {
    assert(
      ∀m,n ∈ P: m + s(n) = s(m + n)
    )
  } →
  
  lemma AdditionZero() {
    assert(
      ∀m ∈ P: m + zero = m
    )
  } →
  
  // Step 1: Apply AdditionSuccessor with m = s(zero), n = zero
  let step1 = s(zero) + s(zero) = s(s(zero) + zero) →
  
  // Step 2: Apply AdditionZero to s(zero) + zero
  let step2 = s(zero) + zero = s(zero) →
  
  // Step 3: Take successor of both sides in step2
  let step3 = s(s(zero) + zero) = s(s(zero)) →
  
  // Final step: Transitive property
  apply(TransitiveEquality(step1, step3)) →
  assert(s(zero) + s(zero) = s(s(zero)))
} ↔

// Alternative proof
proof OnePlusOneEqualsTwo_Alt() {
  // Direct application of addition definitions
  apply(AdditionSuccessor(), m = s(zero), n = zero) →
  apply(AdditionZero(), m = s(zero)) →
  apply(SuccessorEquality()) →
  assert(s(zero) + s(zero) = s(s(zero)))
}