theorem SymmetricSequenceSum() {
  assert(
    ∀n ∈ ℕ ⇒ 1 + 2 + ... + n + (n-1) + ... + 1 = n²
  )
} ↔

proof SymmetricSequenceSum_Direct1() {
  setVar(n: ℕ) →
  assert(1 + 2 + ... + (n-1) + n + (n-1) + ... + 1) →
  rearrange() →
  assert(1 + 2 + ... + (n-1) + (n-1) + ... + 1 + n) →
  factor() →
  assert(2(1 + 2 + ... + (n-1)) + n) →
  apply(TriangularNumberTheorem) →
  assert(2((n-1)n/2) + n) →
  simplify() →
  assert((n-1)n + n) →
  assert(n² - n + n) →
  assert(n²)
} ∧

proof SymmetricSequenceSum_Direct2() {
  setVar(n: ℕ) →
  assert(1 + 2 + ... + (n-1) + n + (n-1) + ... + 1) →
  split() →
  assert((1 + 2 + ... + (n-1)) + (1 + 2 + ... + (n-1) + n)) →
  apply(TriangularNumberTheorem) →
  assert(((n-1)n/2) + (n(n+1)/2)) →
  simplify() →
  assert((n² - n + n² + n)/2) →
  assert(n²)
} ∧

proof SymmetricSequenceSum_Induction() {
  baseCase() {
    assert(n = 1 ⇒ 1 = 1²) ∧
    assert(n = 2 ⇒ 1 + 2 + 1 = 2²)
  } →
  inductiveHypothesis(k: ℕ) {
    assert(1 + 2 + ... + k + (k-1) + ... + 1 = k²)
  } →
  inductiveStep() {
    assert(1 + 2 + ... + (k+1) + k + (k-1) + ... + 1) →
    assert((1 + 2 + ... + k + (k-1) + ... + 1) + k + (k+1)) →
    apply(inductiveHypothesis) →
    assert(k² + k + (k+1)) →
    assert(k² + 2k + 1) →
    assert((k+1)²)
  }
} ∧

proof SymmetricSequenceSum_Recurrence() {
  define(Tn = 1 + 2 + ... + n + (n-1) + ... + 1) →
  assert(T₁ = 1) →
  setVar(n: ℕ) →
  assert(Tn - Tn₋₁ = 2n - 1) →
  unroll() →
  assert(Tn = (Tn - Tn₋₁) + (Tn₋₁ - Tn₋₂) + ... + (T₂ - T₁) + T₁) →
  substitute() →
  assert(Tn = (2n - 1) + (2(n-1) - 1) + ... + (2×2 - 1) + 1) →
  apply(SumOfOddNumbers) →
  assert(Tn = n²)
}