theorem NumericPattern() {
  assert(
    ∀n,b ∈ ℤ_{>0}, b ≥ 3 →
    (b-1)∑_{j=1}^n j b^{n-j} + n + 1 = ∑_{j=0}^n b^j
  )
} ↔

proof NumericPattern() {
  setVar(n: ℤ_{>0}, b: ℤ_{>0} | b ≥ 3) →
  
  lemma BaseCase() {
    assert(
      (b-1)∑_{j=1}^1 j b^{1-j} + 2 
      = (b-1)b^0 + 2
      = b + 1 
      = ∑_{j=0}^1 b^j
    )
  } →

  lemma InductiveStep() {
    assume(
      P(k): (b-1)∑_{j=1}^k j b^{k-j} + k + 1 = ∑_{j=0}^k b^j
    ) →
    
    assert(
      (b-1)∑_{j=1}^{k+1} j b^{k+1-j} + k + 2
      = (b-1)∑_{j=1}^k j b^{k+1-j} + k + 2 + (b-1)(k+1)
      = (b-1)b∑_{j=1}^k j b^{k-j} + (b(k+1) - b(k+1)) + k + 2 + (b-1)(k+1)
      = b((b-1)∑_{j=1}^k j b^{k-j} + k + 1) + 1
      = b(∑_{j=0}^k b^j) + 1
      = ∑_{j=1}^{k+1} b^j + 1
      = ∑_{j=0}^{k+1} b^j
    )
  } →

  apply(BaseCase()) →
  apply(InductiveStep()) →
  apply(MathematicalInduction()) →
  
  conclude(
    ∀n,b ∈ ℤ_{>0}, b ≥ 3 →
    (b-1)∑_{j=1}^n j b^{n-j} + n + 1 = ∑_{j=0}^n b^j
  )
}