theorem PatternIdentity() {
  assert(
    ∀n,b ∈ ℤ_{>0}, b ≥ 3 ⇒ 
    (b-2)∑_{j=1}^n j·b^{n-j} + n = ∑_{j=1}^n (b-j)·b^{n-j}
  )
} ↔

proof PatternIdentity() {
  setVar(n,b: ℤ_{>0}, b ≥ 3) →
  setVar(P(n): proposition) →
  
  // Base case P(1)
  lemma BaseCase() {
    assert((b-2)∑_{j=1}^1 j·b^{1-j} + 1) →
    assert((b-2)·b^0 + 1) →
    assert(b-1) →
    assert(∑_{j=1}^1 (b-j)·b^{1-j})
  } →

  // Inductive step
  lemma InductiveStep() {
    assume(k ≥ 2 ∧ P(k)) →
    setInductiveHypothesis(
      (b-2)∑_{j=1}^k j·b^{k-j} + k = ∑_{j=1}^k (b-j)·b^{k-j}
    ) →
    
    // Show P(k) → P(k+1)
    assert((b-2)∑_{j=1}^{k+1} j·b^{k+1-j} + (k+1)) →
    assert((b-2)∑_{j=1}^k j·b^{k+1-j} + k + 1 + (b-2)(k+1)) →
    assert((b-2)b∑_{j=1}^k j·b^{k-j} + (bk-bk) + k + 1 + bk - 2k + b - 2) →
    assert(b((b-2)∑_{j=1}^k j·b^{k-j} + k) + b - k - 1) →
    applyInductiveHypothesis() →
    assert(b(∑_{j=1}^k (b-j)·b^{k-j}) + b - k - 1) →
    assert(∑_{j=1}^k (b-j)·b^{k+1-j} + b - (k+1)) →
    assert(∑_{j=1}^{k+1} (b-j)·b^{k+1-j})
  } →

  applyMathematicalInduction(BaseCase(), InductiveStep()) →
  assert((b-2)∑_{j=1}^n j·b^{n-j} + n = ∑_{j=1}^n (b-j)·b^{n-j})
}