theorem Adjugate_Matrix_Example() {
  assert(
    let A = [[−1, 2, 0], [0, 1, 3], [2, −3, 3]] ∈ ℝ^{3×3} →
    adj(A) = [[12, 6, −2], [−6, −3, 1], [6, 3, −1]]
  )
} ↔

proof Adjugate_Matrix_Example() {
  setMatrix(A: ℝ^{3×3}) →
  
  lemma Cofactor_Definition() {
    assert(
      ∀i,j ∈ {1,2,3} →
      A_{i,j} = (-1)^{i+j} × det(minor(A,i,j))
    )
  } →

  calc_cofactors() {
    A_{1,1} = (+1) × det([[1,3], [-3,3]]) = (+1)(3+9) = 12 →
    A_{1,2} = (-1) × det([[0,3], [2,3]]) = (-1)(0-6) = 6 →
    A_{1,3} = (+1) × det([[0,1], [2,-3]]) = (+1)(0-2) = -2 →
    A_{2,1} = (-1) × det([[2,0], [-3,3]]) = (-1)(6-0) = -6 →
    A_{2,2} = (+1) × det([[-1,0], [2,3]]) = (+1)(-3-0) = -3 →
    A_{2,3} = (-1) × det([[-1,2], [2,-3]]) = (-1)(3-4) = 1 →
    A_{3,1} = (+1) × det([[2,0], [1,3]]) = (+1)(6-0) = 6 →
    A_{3,2} = (-1) × det([[-1,0], [0,3]]) = (-1)(-3-0) = 3 →
    A_{3,3} = (+1) × det([[-1,2], [0,1]]) = (+1)(-1-0) = -1
  } →

  assert(
    adj(A) = [
      [A_{1,1}, A_{1,2}, A_{1,3}],
      [A_{2,1}, A_{2,2}, A_{2,3}],
      [A_{3,1}, A_{3,2}, A_{3,3}]
    ] = [[12, 6, -2], [-6, -3, 1], [6, 3, -1]]
  )
}