theorem AmicableTriple_Example() {
  assert(
    let n₁ = 103340640 ∧
    let n₂ = 123228768 ∧
    let n₃ = 124015008 →
    AmicableTriple(n₁, n₂, n₃)
  )
} ↔

proof AmicableTriple_Example() {
  define(s(n) ≡ σ₁(n) - n) →
  
  // First number
  assert(s(n₁) = 
    σ₁(103340640) - 103340640) →
  assert(s(n₁) = 
    350584416 - 103340640) →
  assert(s(n₁) = 247243776) →
  assert(s(n₁) = n₂ + n₃) →

  // Second number
  assert(s(n₂) = 
    σ₁(123228768) - 123228768) →
  assert(s(n₂) = 
    350584416 - 123228768) →
  assert(s(n₂) = 227355648) →
  assert(s(n₂) = n₁ + n₃) →

  // Third number
  assert(s(n₃) = 
    σ₁(124015008) - 124015008) →
  assert(s(n₃) = 
    350584416 - 124015008) →
  assert(s(n₃) = 226569408) →
  assert(s(n₃) = n₁ + n₂) →

  conclude(
    s(n₁) = n₂ + n₃ ∧
    s(n₂) = n₁ + n₃ ∧
    s(n₃) = n₁ + n₂ →
    AmicableTriple(n₁, n₂, n₃)
  )
}