theorem BanachAlgebraWithUnity() {
  let(ğ”½ âˆˆ {â„, â„‚})
  let((X, â€–Â·â€–): NonTrivialBanachAlgebra(ğ”½))
  let(1â‚“: IdentityElement(X))
  assert(
    âˆƒâ€–Â·â€–': Norm(X) â‡’
    (1): â€–Â·â€–' â‰¡ â€–Â·â€– âˆ§
    (2): (X, â€–Â·â€–') is BanachAlgebra âˆ§
    (3): â€–1â‚“â€–' = 1
  )
}

proof BanachAlgebraWithUnity() {
  define(â€–Â·â€–': X â†’ [0,âˆ], a â†¦ sup{â€–abâ€–: â€–bâ€– â‰¤ 1}) â†’
  
  // Prove norm properties
  lemma NormWellDefined() {
    âˆ€a,b âˆˆ X: â€–bâ€– â‰¤ 1 â‡’ â€–abâ€– â‰¤ â€–aâ€–â€–bâ€– â‰¤ â€–aâ€– â†’
    assert(â€–aâ€–' âˆˆ [0,âˆ])
  } â†’

  lemma PositiveDefinite() {
    assert(â€–0â€–' = 0) â†’
    assume(â€–aâ€–' = 0 for a âˆˆ X) â†’
    assert(âˆ€b: â€–bâ€– â‰¤ 1 â‡’ ab = 0) â†’
    apply(b = 1â‚“/â€–1â‚“â€–) â†’
    conclude(a = 0)
  } â†’

  lemma Homogeneous() {
    âˆ€Î» âˆˆ ğ”½, a âˆˆ X:
    â€–Î»aâ€–' = sup{â€–Î»abâ€–: â€–bâ€– â‰¤ 1} =
    |Î»|sup{â€–abâ€–: â€–bâ€– â‰¤ 1} =
    |Î»|â€–aâ€–'
  } â†’

  lemma Triangle() {
    âˆ€x,y âˆˆ X:
    âˆ€b: â€–bâ€– â‰¤ 1 â‡’
    â€–(x+y)bâ€– â‰¤ â€–xbâ€– + â€–ybâ€– â‰¤ â€–xâ€–' + â€–yâ€–'
  } â†’

  // Prove norm equivalence
  lemma NormEquivalence() {
    âˆ€a âˆˆ X:
    assert(â€–aâ€–' â‰¤ â€–aâ€–) â†’
    assert(â€–aâ€–/â€–1â‚“â€– â‰¤ â€–aâ€–' â‰¤ â€–aâ€–)
  } â†’

  // Prove Banach algebra properties
  lemma BanachAlgebraProperties() {
    assert((X,â€–Â·â€–') is BanachSpace) â†’
    âˆ€x,y âˆˆ X:
    case(x = 0 âˆ¨ y = 0): â€–xyâ€–' â‰¤ â€–xâ€–'â€–yâ€–' â†’
    case(x,y â‰  0):
      âˆ€b: â€–bâ€– â‰¤ 1 â‡’
      â€–(xy)bâ€– = â€–x(yb)â€– = â€–ybâ€–â€–x(yb/â€–ybâ€–)â€– â‰¤ â€–xâ€–'â€–yâ€–'
  } â†’

  // Prove unity norm
  lemma UnityNorm() {
    assert(â€–1â‚“â€–' = sup{â€–bâ€–: â€–bâ€– â‰¤ 1} = 1)
  } â†’

  conclude()
}