theorem Barber_Paradox() {
  let(ğ•Œ: Set) â†’
  let(S: ğ•Œ â†’ {T,F}) â†’
  let(B: ğ•Œ â†’ {T,F}) â†’
  let(b âˆˆ ğ•Œ) â†’
  assert(
    âˆ€x âˆˆ ğ•Œ: S(x) â†” "x shaves x" âˆ§
    âˆ€x âˆˆ ğ•Œ: B(x) â†” "x is shaved by b"
  )
}

proof Barber_Contradiction() {
  premise1(âˆ€x âˆˆ ğ•Œ: (Â¬S(x)) â†” B(x)) â†’
  premise2(B(b) â†” S(b)) â†’
  
  chain_equivalence() {
    S(b) â†” B(b) â†” (Â¬S(b))
  } â†’
  
  apply(Biconditional_Transitive) {
    S(b) â†” (Â¬S(b))
  } â†’
  
  assert(contradiction)
}

theorem Barber_Resolution() {
  let(ğ•Œ: Set) â†’
  let(S: ğ•Œ â†’ {T,F}) â†’
  let(B: ğ•Œ â†’ {T,F}) â†’
  let(b âˆˆ ğ•Œ) â†’
  assert(
    âˆ€x âˆˆ ğ•Œ: (Â¬S(x)) â†’ B(x) âˆ§
    B(b) â†” S(b)
  )
}

proof Barber_Resolution() {
  premise1(âˆ€x âˆˆ ğ•Œ: (Â¬S(x)) â†’ B(x)) â†’
  premise2(B(b) â†” S(b)) â†’
  
  assert(Â¬(B(x) â†’ (Â¬S(x)))) â†’
  conclude(
    âˆƒx âˆˆ ğ•Œ: (B(x) âˆ§ S(x)) âˆ§
    (b must be such an x)
  )
}