theorem Basis_For_Topological_Subspace() {
  let(T = âŸ¨A,Ï„âŸ©: TopologicalSpace) âˆ§
  let(O âŠ† H âŠ† A) âˆ§
  let(T_H = âŸ¨H,Ï„_HâŸ©: Subspace(T)) âˆ§
  let(ğ”¹: SyntheticBasis(T)) âˆ§
  let(ğ”¹_H = {U âˆ© H: U âˆˆ ğ”¹}) â†’
  assert(ğ”¹_H: SyntheticBasis(T_H))
}

proof Basis_For_Topological_Subspace() {
  lemma SyntheticBasisDefinition() {
    assert(ğ”¹ âŠ† ğ’«(A) â†” (
      (B1: A = âˆª{B: B âˆˆ ğ”¹}) âˆ§
      (B2: âˆ€Bâ‚,Bâ‚‚ âˆˆ ğ”¹ â†’ Bâ‚ âˆ© Bâ‚‚ = âˆª{B: B âˆˆ ğ”¹'} for some ğ”¹' âŠ† ğ”¹)
    ))
  } â†’

  // Prove B1 for ğ”¹_H
  let(A = âˆª{S: S âˆˆ ğ•Š} where ğ•Š âŠ† ğ”¹) â†’
  assert(
    H = A âˆ© H â†’
    H = (âˆª{S: S âˆˆ ğ•Š}) âˆ© H â†’
    H = âˆª{S âˆ© H: S âˆˆ ğ•Š}
  ) â†’
  assert(âˆ€S âˆˆ ğ”¹ â†’ S âˆ© H âˆˆ ğ”¹_H) â†’

  // Prove B2 for ğ”¹_H
  let(Uâ‚,Uâ‚‚ âˆˆ ğ”¹_H) â†’
  assert(âˆƒBâ‚,Bâ‚‚ âˆˆ ğ”¹: Uâ‚ = Bâ‚ âˆ© H âˆ§ Uâ‚‚ = Bâ‚‚ âˆ© H) â†’
  assert(Uâ‚ âˆ© Uâ‚‚ = (Bâ‚ âˆ© Bâ‚‚) âˆ© H) â†’
  let(Bâ‚ âˆ© Bâ‚‚ = âˆª{S: S âˆˆ ğ•Š} where ğ•Š âŠ† ğ”¹) â†’
  assert(
    Uâ‚ âˆ© Uâ‚‚ = (âˆª{S: S âˆˆ ğ•Š}) âˆ© H â†’
    Uâ‚ âˆ© Uâ‚‚ = âˆª{S âˆ© H: S âˆˆ ğ•Š}
  ) â†’
  assert(âˆ€S âˆˆ ğ”¹ â†’ S âˆ© H âˆˆ ğ”¹_H) â†’
  conclude(ğ”¹_H: SyntheticBasis(T_H))
}