theorem NotSurjectivePowerSet() {
  assert(
    âˆ€S:Set â‡’ Â¬âˆƒf:Function(S â†’ ğ’«(S)) [Surjective(f)]
  )
} â†”

proof NotSurjectivePowerSet() {
  setVar(S: Set) â†’
  setVar(f: Function(S â†’ ğ’«(S))) â†’
  define(T := {x âˆˆ S : x âˆ‰ f(x)}) â†’
  assert(T âŠ† S) â†’
  assert(T âˆˆ ğ’«(S)) â†’

  lemma ProveNotSurjective() {
    assume(âˆƒa âˆˆ S : T = f(a)) â†’
    case(a âˆˆ T) {
      assert(a âˆ‰ f(a)) [by T definition] â†’
      assert(a âˆ‰ T) [since T = f(a)] â†’
      contradiction()
    } â†’
    conclude(a âˆ‰ T) â†’
    assert(a âˆ‰ f(a)) [since T = f(a)] â†’
    assert(a âˆˆ T) [by T definition] â†’
    contradiction()
  } â†’

  apply(ProveNotSurjective()) â†’
  assert(Â¬âˆƒa âˆˆ S : T = f(a)) â†’
  conclude(Â¬Surjective(f))
}