theorem Cardinality_Of_Set_Of_Subsets() {
  let(S: Set, n: â„•, m: â„•) â†’
  assert(card(S) = n âˆ§ m â‰¤ n) â†’
  assert(
    card({T âŠ† S : card(T) = m}) = (n!/(m!(n-m)!))
  )
} â†”

proof Cardinality_Of_Set_Of_Subsets_1() {
  let(Nn: Set) â†’ assert(Nn = {1,...,n}) â†’
  let(B: Function) â†’ assert(âˆ€XâŠ†Nn, âˆ€YâŠ†S: B(X,Y) = {f: Xâ†’Y | f is bijective}) â†’
  let(ğ•Š: Set) â†’ assert(ğ•Š = {T âŠ† S : card(T) = m}) â†’
  let(s: â„•) â†’ assert(s = card(ğ•Š)) â†’
  let(Î²: Function) â†’ assert(
    Î²: B(Nn,S) â†’ ğ•Š,
    âˆ€fâˆˆB(Nn,S): Î²(f) = f(Nm)
  ) â†’

  lemma Bijection_Decomposition() {
    âˆ€Yâˆˆğ•Š: assert(
      âˆƒÎ¦Y: Î²â»Â¹(Y) â†’ B(Nm,Y) Ã— B(Nn-Nm,S-Y),
      Î¦Y is bijective
    )
  } â†’

  apply(Cardinality_Of_Bijections) â†’
  assert(âˆ€Yâˆˆğ•Š: card(B(Nm,Y)) = m!) â†’
  assert(âˆ€Yâˆˆğ•Š: card(B(Nn-Nm,S-Y)) = (n-m)!) â†’
  apply(Cardinality_Of_Cartesian_Product) â†’
  assert(âˆ€Yâˆˆğ•Š: card(Î²â»Â¹(Y)) = m!(n-m)!) â†’
  apply(Number_Of_Elements_In_Partition) â†’
  assert(card(B(Nn,S)) = m!(n-m)!s) â†’
  assert(card(B(Nn,S)) = n!) â†’
  conclude(s = n!/(m!(n-m)!))
}

proof Cardinality_Of_Set_Of_Subsets_2() {
  let(P: Function) â†’ assert(P(n,m) = n!/(n-m)!) â†’
  assert(P(n,m) = card({Ï€: subset(S,m) â†’ subset(S,m) | Ï€ is permutation})) â†’
  assert(P(n,m) = (n choose m) Ã— m!) â†’
  conclude((n choose m) = n!/(m!(n-m)!))
}

proof Cardinality_Of_Set_Of_Subsets_3() {
  let(Sn: Group) â†’ assert(Sn = SymmetricGroup(Nn)) â†’
  let(Br: Set) â†’ assert(Br = {S âŠ† Nn : card(S) = r}) â†’
  let(*: Function) â†’ assert(*: Sn Ã— Br â†’ Br) â†’
  apply(Group_Action_Properties) â†’
  assert(âˆ€UâˆˆBr: card(Stab(U)) = r!(n-r)!) â†’
  apply(Orbit_Stabilizer_Theorem) â†’
  conclude(card(Br) = n!/(r!(n-r)!))
}

proof Cardinality_Of_Set_Of_Subsets_4() {
  let(P: Predicate) â†’ 
  assert(P(n) â†” âˆ€mâ‰¤n: (n choose m) = n!/(m!(n-m)!)) â†’
  
  base_case {
    assert(P(1)) â†’
    verify(
      (1 choose m) = 
      case(m=0: 1) âˆ§
      case(m=1: 1) âˆ§
      case(else: 0)
    )
  } â†’

  inductive_step {
    assume(P(k)) â†’
    assert((k+1 choose m) = (k choose m) + (k choose m-1)) â†’
    apply(Algebra) â†’
    verify((k+1 choose m) = (k+1)!/(m!(k+1-m)!))
  } â†’

  apply(Mathematical_Induction) â†’
  conclude(âˆ€nâˆˆâ„•: P(n))
}