theorem NormalDistribution_CharacteristicFunction_Lemma1() {
  let Ï†(t) := CharacteristicFunction(NormalDist(Î¼, ÏƒÂ²))
  let k := Î¼ + itÏƒÂ²
  let c := exp(Î¼it - (1/2)tÂ²ÏƒÂ²)
  
  assert(
    Ï†(t) = c * (1/âˆš(2Ï€ÏƒÂ²)) * âˆ«[xâˆˆâ„](exp(-(((x-k)/(âˆš2Ïƒ))Â²)))dx
  )
} â†”

proof NormalDistribution_CharacteristicFunction_Lemma1() {
  // Definition of characteristic function
  assert(Ï†(t) = ğ”¼[exp(itX)]) â†’
  
  // Expand expectation using PDF of normal distribution
  assert(
    Ï†(t) = âˆ«[xâˆˆâ„](exp(itx) * (1/âˆš(2Ï€ÏƒÂ²)) * exp(-(((x-Î¼)Â²)/(2ÏƒÂ²))))dx
  ) â†’
  
  // Combine exponential terms
  assert(
    Ï†(t) = (1/âˆš(2Ï€ÏƒÂ²)) * âˆ«[xâˆˆâ„](exp(itx - ((x-Î¼)Â²)/(2ÏƒÂ²)))dx
  ) â†’
  
  lemma ExponentIdentity() {
    assert(
      itx - ((x-Î¼)Â²)/(2ÏƒÂ²) = 
      -((x-k)Â² + 2Î¼itÏƒÂ² - tÂ²Ïƒâ´)/(2ÏƒÂ²)
    )
  } â†’
  
  apply(ExponentIdentity()) â†’
  
  // Separate constant terms from integral
  assert(
    Ï†(t) = (1/âˆš(2Ï€ÏƒÂ²)) * exp((2Î¼itÏƒÂ² - tÂ²Ïƒâ´)/(2ÏƒÂ²)) * 
    âˆ«[xâˆˆâ„](exp(-((x-k)Â²)/(2ÏƒÂ²)))dx
  ) â†’
  
  // Simplify exponential term
  assert(
    exp((2Î¼itÏƒÂ² - tÂ²Ïƒâ´)/(2ÏƒÂ²)) = exp(Î¼it - (1/2)tÂ²ÏƒÂ²)
  ) â†’
  
  // Substitute c definition
  assert(
    Ï†(t) = c * (1/âˆš(2Ï€ÏƒÂ²)) * âˆ«[xâˆˆâ„](exp(-(((x-k)/(âˆš2Ïƒ))Â²)))dx
  )
}