theorem Character_Hermitian_Real() {
  assert(
    âˆ€A: CStarAlgebra âˆ§ âˆ€Ï†: Character(A) âˆ§ âˆ€x: Hermitian(A) â‡’
    Ï†(x) âˆˆ â„
  )
} â†”

proof Character_Hermitian_Real() {
  setVar(A: CStarAlgebra) â†’
  setVar(Ï†: Character(A)) â†’
  setVar(x: Hermitian(A)) â†’
  
  letExist(Î±,Î²: â„ | Ï†(x) = Î± + iÎ²) â†’
  
  define(x_t := x + itğŸ™_A, t: â„) â†’
  
  lemma CharacterUnital() {
    assert(Ï†(ğŸ™_A) = 1)
  } â†’
  
  apply(CharacterUnital()) â†’
  assert(Ï†(x_t) = Ï†(x) + it = Î± + i(Î² + t)) â†’
  assert(|Ï†(x_t)|Â² = Î±Â² + (Î² + t)Â²) â†’
  
  assert(|Ï†(x_t)|Â² â‰¤ â€–x_tâ€–Â²) by CharacterContinuous â†’
  assert(â€–x_tâ€–Â² = â€–x_t x_t*â€–) by CStarDef â†’
  assert(â€–x_t x_t*â€– = â€–(x + itğŸ™_A)(x - itğŸ™_A)â€–) by InvolutionDef â†’
  assert(â€–(x + itğŸ™_A)(x - itğŸ™_A)â€– = â€–xÂ² + tÂ²ğŸ™_Aâ€–) â†’
  assert(â€–xÂ² + tÂ²ğŸ™_Aâ€– â‰¤ â€–xÂ²â€– + tÂ²) by NormTriangle â†’
  assert(â€–xÂ²â€– + tÂ² â‰¤ â€–xâ€–Â² + tÂ²) by NormPower â†’
  
  assert(âˆ€t: â„ â‡’ Î±Â² + Î²Â² + 2Î²t â‰¤ â€–xâ€–Â²) â†’
  
  byContradiction(Î² â‰  0) {
    case(Î² > 0) {
      letExist(t > â€–xâ€–Â²/(2Î²)) â†’
      assert(Î±Â² + Î²Â² + 2Î²t > â€–xâ€–Â²) â†’
      contradiction()
    } â†’
    case(Î² < 0) {
      letExist(t < -â€–xâ€–Â²/(2Î²)) â†’
      assert(Î±Â² + Î²Â² + 2Î²t > â€–xâ€–Â²) â†’
      contradiction()
    }
  } â†’
  
  assert(Î² = 0) â†’
  conclude(Ï†(x) = Î± âˆˆ â„)
}