((inverse_sine_series(S) ↔ (S = {t : t = Σ_{n=0}^∞ [(1 * 3 * ... * (2n-1)) / (2 * 4 * ... * (2n)) * x^(2n+1) / (2n+1)] ∧ |x| ≤ 1})) ∧
(let T = {t : t = sin^(-1)(x) ∧ t ∈ [0, π/2]} →
(T = {t : t = Σ_{n=0}^∞ [(1 * 3 * ... * (2n-1)) / (2 * 4 * ... * (2n)) * sin(t)^(2n+1) / (2n+1)]}))) →

((let I = {I_{2n+1} : I_{2n+1} = ∫_0^(π/2) (sin(x)^(2n+1)) dx} ∧
(recursion_formula ↔ (I_{2n+1} ∈ I ∧ I_{2n+1} = I_{2n-1} - ∫_0^(π/2) (sin(x)^(2n-1) * cos(x)) dx))) →

((integration_by_parts ↔ (∀I_{2n+1} ∈ I ((2n+1)/(2n) * I_{2n+1} = I_{2n-1}))) →
(recursive_relation ↔ (∀I_{2n+1} ∈ I (I_{2n+1} = (2n / (2n+1)) * (2(n-1) / (2n-1)) * I_{2n-3})))) →

((explicit_formula ↔ (∀I_{2n+1} ∈ I (I_{2n+1} = [(2 * 4 * ... * (2n)) / (3 * 5 * ... * (2n+1))]))) →

((relation_to_series ↔ ({π^2 / 8} = {∫_0^(π/2) t dt : t ∈ T} = {Σ_{n=0}^∞ (1 / (2n+1)^2)})) →

({ζ(2)} = {Σ_{n=1}^∞ (1 / n^2) : ζ(2) = π^2 / 6}))))
