((monotone_convergence(J) ↔ (1 / j^2 = ∫_0^1 ∫_0^1 x^(j-1) y^(j-1) dx dy)) ∧
(sum_to_integral(K) ↔ (Σ_{k=1}^∞ (1 / k^2) = ∫_0^1 ∫_0^1 (Σ_{n=1}^∞ (x y)^(n-1)) dx dy = ∫_0^1 ∫_0^1 dx dy / (1 - x y))) →

((variable_change(U, V) ↔ (u = (x + y) / 2 ∧ v = (x - y) / 2)) →
(integral_relation(ζ) ↔ (ζ(2) = 2 * ∫∫_S (du dv) / (1 - u^2 v^2))) →

((symmetric_square(S) ↔ (S = {(0, 0), (1/2, -1/2), (1, 0), (1/2, 1/2)} ∧ symmetry(S, line = y = 0))) →
(triangle_decomposition(T) ↔ (T = {(0, 0), (1/2, 1/2), (1/2, 0)} ∨ {(1/2, 1/2), (1, 0), (1/2, 0)})) →

((rewritten_integral(ζ) ↔ (ζ(2) = 4 * {∫_0^(1/2) ∫_0^(1-u) du dv / (1 - u^2 + v^2)})) →
(split_integral(U) ↔ (ζ(2) = 4 * ({∫_0^(1/2) (1 / √(1-u^2) * tan^(-1)(u / √(1-u^2))) du} ∪ {∫_(1/2)^1 (1 / √(1-u^2) * tan^(-1)((1-u) / √(1-u^2))) du})))) →

((substitution(T) ↔ (tan^2(θ) = (1 - u) / (1 + u) ∧ sec^2(θ) = 2 / (1+u))) →
(u_change(θ) ↔ (u = 2 * cos(2θ) - 1))) →

((final_integral(ζ) ↔ (ζ(2) = 4 * ({π^2 / 4} ∪ {π^2 / 36}))) →
({ζ(2)} = {Σ_{n=1}^∞ (1 / n^2) : ζ(2) = π^2 / 6})))
