theorem_definition(Taylor_Theorem) ↔
    ∀f, a, b, n (a < b ∧ n ∈ ℕ ∧ Differentiable(f, n, (a, b)) ∧ Continuous(f, n, [a, b]) →
        ∃c ∈ (a, b) (f(b) = Σ_{k=0}^{n-1} f^(k)(a) / k! * (b - a)^k + f^(n)(c) / n! * (b - a)^n)).
→

[generalization(Rolle_Theorem_Extended) ↔
    ∀F, a, b, n (a < b ∧ n ∈ ℕ ∧ Differentiable(F, n, (a, b)) ∧ Continuous(F, n, [a, b]) ∧
        F(a) = F'(a) = ... = F^(n-1)(a) = F(b) →
        ∃c ∈ (a, b) (F^(n)(c) = 0))].
→

[polynomial_construction(Coefficient_Definition) ↔
    ∀f, P, a, b, n (a < b ∧ Polynomial(P, n) ∧ ∀k ∈ {0, ..., n-1} 
        (P^(k)(a) = f^(k)(a) ∧ P^(n)(a) = 0) →
        Coefficients(P) = {f^(k)(a) / k! ∀k ∈ {0, ..., n-1}, (f(b) - Σ_{k=0}^{n-1} f^(k)(a) / k! * (b - a)^k) / (b - a)^n})].
→

[first_proof(Linear_Reduction) ↔
    ∀f, a, b, n (a < b ∧ n ∈ ℕ ∧ f(b) - P(b) satisfies Rolle_Theorem_Extended →
        ∃c ∈ (a, b) (f(b) = Σ_{k=0}^{n-1} f^(k)(a) / k! * (b - a)^k + f^(n)(c) / n! * (b - a)^n))].
→

[second_proof(Cauchy_Mean_Value) ↔
    ∀f, a, b, n (a < b ∧ n ∈ ℕ ∧ Construct_G(f, n, a) →
        ∃c ∈ (a, b) (f(b) = Σ_{k=0}^{n-1} f^(k)(a) / k! * (b - a)^k + f^(n)(c) / n! * (b - a)^n))].
→

[conclusion(C) ↔
    ∀f, a, b, n (a < b ∧ n ∈ ℕ ∧ Differentiable(f, n, (a, b)) ∧ Continuous(f, n, [a, b]) →
        ∃c ∈ (a, b) (f(b) = Σ_{k=0}^{n-1} f^(k)(a) / k! * (b - a)^k + f^(n)(c) / n! * (b - a)^n)).
    ∴ Proved. )]