# 

Source: https://proofwiki.org/wiki/0.999...%3D1



Theorem
$0.999 \ldots = 1$


Proof using Geometric Series
By Sum of Infinite Geometric Sequence:

$0.999 \ldots = \dfrac a {1 - r}$
where $a = \dfrac 9 {10}$ and $r = \dfrac 1 {10}$.
Since our ratio is less than $1$, then we know that $\ds \sum_{n \mathop = 0}^\infty \frac 9 {10} \paren {\frac 1 {10} }^n$ must converge to:

$\dfrac a {1 - r} = \dfrac {\frac 9 {10} } {1 - \frac 1 {10} } = \dfrac {\frac 9 {10} } {\frac 9 {10} } = 1$
$\blacksquare$


Proof using Fractions













\(\ds 0.333 \ldots\)

\(=\)







\(\ds 1 / 3\)














\(\ds \leadsto \ \ \)





\(\ds 3 \paren {0.333 \ldots}\)

\(=\)







\(\ds 3 \paren {1 / 3}\)














\(\ds \leadsto \ \ \)





\(\ds 0.999 \ldots\)

\(=\)







\(\ds 3 / 3\)




















\(\ds \)

\(=\)







\(\ds 1\)









$\blacksquare$


Proof using Multiplication by 10
Let  $c = 0.999 \ldots$
Then:














\(\ds c\)

\(=\)







\(\ds 0.999 \ldots\)














\(\ds \leadsto \ \ \)





\(\ds 10 c\)

\(=\)







\(\ds \paren {9.999 \ldots}\)





multiplying $c$ by $10$








\(\ds \leadsto \ \ \)





\(\ds 10 c - c\)

\(=\)







\(\ds \paren {9.999 \ldots} - \paren {0.999 \ldots}\)





subtracting $c$ from each side








\(\ds \leadsto \ \ \)





\(\ds 9 c\)

\(=\)







\(\ds 9\)














\(\ds \leadsto \ \ \)





\(\ds c\)

\(=\)







\(\ds 1\)









It follows that:

$0.999 \ldots = 1$
$\blacksquare$


Proof using Long Division
We begin with the knowledge that:














\(\ds \frac 9 9\)

\(=\)







\(\ds \frac 1 1 = 1\)









Now we divide $9$ by $9$ using the standard process of long division, only instead of stating that $90$ divided by $9$ is $10$, we say that it is "$9$ remainder $9$," yielding the following result:

     0.9999...
    -----------
   9)9.0000...
     8.1
     ---
       90
       81
       --
        90
        81
        --
         9...

Thus, we are compelled to believe that:

$0.999\ldots = \dfrac 9 9 = 1$
$\blacksquare$


Proof using Sequences



\(\text {(1)}: \quad\)









\(\ds 0 . \underset n {\underbrace {999 \cdots 9} }\)

\(=\)







\(\ds 1 - 0.1^n\)




















\(\ds 0.999 \cdots\)

\(=\)







\(\ds \eqclass {\sequence {0.9, \, 0.99, \, 0.999, \, \cdots} } {}\)





Definition of Real Numbers














\(\ds \)

\(=\)







\(\ds \eqclass {\sequence {1 - 0.1^1, \, 1 - 0.1^2, \, 1 - 0.1^3, \, \cdots} } {}\)





from $(1)$














\(\ds \)

\(=\)







\(\ds \eqclass {\sequence {1, \, 1, \, 1, \, \cdots} } {} - \eqclass {\sequence {0.1^1, \, 0.1^2, \, 0.1^3, \, \cdots} } {}\)




















\(\ds \)

\(=\)







\(\ds 1 - 0\)





Sequence of Powers of Number less than One, Definition of Real Numbers














\(\ds \)

\(=\)







\(\ds 1\)









$\blacksquare$


Also see
For a video presentation of the contents of this page, visit the Khan Academy.




