# 

Source: https://proofwiki.org/wiki/1%2B2%2B...%2Bn%2B(n-1)%2B...%2B1_%3D_n%5E2/Proof_2

Theorem
$\forall n \in \N: 1 + 2 + \cdots + n + \paren {n - 1} + \cdots + 1 = n^2$


Proof













\(\ds \)

\(\)







\(\ds 1 + 2 + \cdots + \paren {n - 1} + n + \paren {n - 1} + \cdots + 1\)




















\(\ds \)

\(=\)







\(\ds \paren {1 + 2 + \cdots + \paren {n - 1} } + \paren {1 + 2 + \cdots + \paren {n - 1} + n}\)




















\(\ds \)

\(=\)







\(\ds \frac {\paren {n - 1} n} 2 + \frac {n \paren {n + 1} } 2\)





Closed Form for Triangular Numbers














\(\ds \)

\(=\)







\(\ds \frac {n^2 - n + n^2 + n} 2\)




















\(\ds \)

\(=\)







\(\ds n^2\)









$\blacksquare$





