# 

Source: https://proofwiki.org/wiki/1%2B2%2B...%2Bn%2B(n-1)%2B...%2B1_%3D_n%5E2



Theorem
$\forall n \in \N: 1 + 2 + \cdots + n + \paren {n - 1} + \cdots + 1 = n^2$


Direct Proof 1













\(\ds \)

\(\)







\(\ds 1 + 2 + \cdots + \paren {n - 1} + n + \paren {n - 1} + \cdots + 1\)




















\(\ds \)

\(=\)







\(\ds 1 + 2 + \cdots + \paren {n - 1} + \paren {n - 1} + \cdots + 1 + n\)




















\(\ds \)

\(=\)







\(\ds 2 \paren {1 + 2 + \cdots + \paren {n - 1} } + n\)




















\(\ds \)

\(=\)







\(\ds 2 \paren {\frac {\paren {n - 1} n} 2} + n\)





Closed Form for Triangular Numbers














\(\ds \)

\(=\)







\(\ds \paren {n - 1} n + n\)




















\(\ds \)

\(=\)







\(\ds n^2 - n + n\)




















\(\ds \)

\(=\)







\(\ds n^2\)









$\blacksquare$


Direct Proof 2













\(\ds \)

\(\)







\(\ds 1 + 2 + \cdots + \paren {n - 1} + n + \paren {n - 1} + \cdots + 1\)




















\(\ds \)

\(=\)







\(\ds \paren {1 + 2 + \cdots + \paren {n - 1} } + \paren {1 + 2 + \cdots + \paren {n - 1} + n}\)




















\(\ds \)

\(=\)







\(\ds \frac {\paren {n - 1} n} 2 + \frac {n \paren {n + 1} } 2\)





Closed Form for Triangular Numbers














\(\ds \)

\(=\)







\(\ds \frac {n^2 - n + n^2 + n} 2\)




















\(\ds \)

\(=\)







\(\ds n^2\)









$\blacksquare$


Proof by Induction
Proof by induction:

Basis for the Induction
$n = 1$ holds trivially.
Just to make sure, we try $n = 2$:

$1 + 2 + 1 = 4$
Likewise $n^2 = 2^2 = 4$.
So shown for basis for the induction.


Induction Hypothesis
This is the induction hypothesis:

$1 + 2 + \cdots + k + \paren {k - 1} + \cdots + 1 = k^2$
Now we need to show true for $n = k + 1$:

$1 + 2 + \cdots + \paren {k + 1} + k + \paren {k - 1} + \cdots + 1 = \paren {k + 1}^2$


Induction Step
This is the induction step:














\(\ds \)

\(\)







\(\ds 1 + 2 + \cdots + \paren {k + 1} + k + \paren {k - 1} + \cdots + 1\)




















\(\ds \)

\(=\)







\(\ds \paren {1 + 2 + \cdots + k + \paren {k - 1} + \cdots + 1} + k + \paren {k + 1}\)




















\(\ds \)

\(=\)







\(\ds k^2 + k + \paren {k + 1}\)





from induction hypothesis














\(\ds \)

\(=\)







\(\ds k^2 + 2k + 1\)




















\(\ds \)

\(=\)







\(\ds \paren {k + 1}^2\)









The result follows by induction.
$\blacksquare$


Proof 4
Let $T_n = 1 + 2 + \cdots + n + \paren {n - 1} + \cdots + 1$.
We have $T_1 = 1$
and














\(\ds T_n - T_{n - 1}\)

\(=\)







\(\ds \paren {1 + 2 + \cdots + n + \paren {n - 1} + \cdots + 1 }\)





Definition of $T_n$














\(\ds \)

\(\)





\(\, \ds - \, \)

\(\ds \paren {1 + 2 + \cdots + \paren {n - 1} + \paren {n - 2} + \cdots + 1}\)




















\(\ds \)

\(=\)







\(\ds \paren {\paren {1 + 2 + \cdots + n} - \paren {1 + 2 + \cdots + \paren {n - 1} } }\)





Integer Addition is Associative














\(\ds \)

\(\)





\(\, \ds + \, \)

\(\ds \paren {\paren {\paren {n - 1} + \paren {n - 2} + \cdots + 1} - \paren {\paren {n - 2} + \paren {n - 3} + \cdots + 1} }\)





Integer Addition is Commutative














\(\ds \)

\(=\)







\(\ds n + \paren {n - 1}\)





simplifying














\(\ds \)

\(=\)







\(\ds 2 n - 1\)









Thus we have:














\(\ds T_n\)

\(=\)







\(\ds \paren {T_n - T_{n - 1} } + \paren {T_{n - 1} - T_{n - 2} } + \cdots + \paren {T_2 - T_1} + T_1\)




















\(\ds \)

\(=\)







\(\ds \paren {2 n - 1} + \paren {2 \paren {n - 1} - 1} + \cdots + \paren {2 \times 2 - 1} + 1\)




















\(\ds \)

\(=\)







\(\ds \sum_{k \mathop = 1}^n 2 k - 1\)




















\(\ds \)

\(=\)







\(\ds n^2\)





Odd Number Theorem



$\blacksquare$


Illustration



Sources
1986: David Wells: Curious and Interesting Numbers ... (previous) ... (next): $25$
1997: David Wells: Curious and Interesting Numbers (2nd ed.) ... (previous) ... (next): $25$




