# 

Source: https://proofwiki.org/wiki/123456789_x_8_%2B_9_%3D_987654321



Theorem













\(\ds 1 \times 8 + 1\)

\(=\)







\(\ds 9\)




















\(\ds 12 \times 8 + 2\)

\(=\)







\(\ds 98\)




















\(\ds 123 \times 8 + 3\)

\(=\)







\(\ds 987\)




















\(\ds 1234 \times 8 + 4\)

\(=\)







\(\ds 9876\)




















\(\ds 12345 \times 8 + 5\)

\(=\)







\(\ds 98765\)




















\(\ds 123456 \times 8 + 6\)

\(=\)







\(\ds 987654\)




















\(\ds 1234567 \times 8 + 7\)

\(=\)







\(\ds 9876543\)




















\(\ds 12345678 \times 8 + 8\)

\(=\)







\(\ds 98765432\)




















\(\ds 123456789 \times 8 + 9\)

\(=\)







\(\ds 987654321\)










The above pattern is an instance of the identity:

$\ds \paren {b - 2} \sum_{j \mathop = 1}^n j b^{n - j} + n = \sum_{j \mathop = 1}^n \paren {b - j} b^{n - j}$
where $b = 10$ and $n$ goes from $1$ to $9$.


Proof
The proof proceeds by induction.
Let $n, b \in \Z_{>0}$, where $b \ge 3$.
For all $n \in \Z_{\ge 1}$, let $\map P n$ be the proposition:

$\ds \paren {b - 2} \sum_{j \mathop = 1}^n j b^{n - j} + n = \sum_{j \mathop = 1}^n \paren {b - j} b^{n - j}$


Basis for the Induction
$\map P 1$ is the case:














\(\ds \paren {b - 2} \sum_{j \mathop = 1}^1 j b^{1 - j} + 1\)

\(=\)







\(\ds \paren {b - 2} b^0 + 1\)




















\(\ds \)

\(=\)







\(\ds b - 1\)




















\(\ds \)

\(=\)







\(\ds \sum_{j \mathop = 1}^1 \paren {b - j} b^{1 - j}\)









Thus $\map P 1$ is seen to hold.

This is the basis for the induction.


Induction Hypothesis
Now it needs to be shown that, if $\map P k$ is true, where $k \ge 2$, then it logically follows that $\map P {k + 1}$ is true.

So this is the induction hypothesis:

$\ds \paren {b - 2} \sum_{j \mathop = 1}^k j b^{k - j} + k = \sum_{j \mathop = 1}^k \paren {b - j} b^{k - j}$

from which it is to be shown that:

$\ds \paren {b - 2} \sum_{j \mathop = 1}^{k + 1} j b^{k + 1 - j} + \paren {k + 1} = \sum_{j \mathop = 1}^{k + 1} \paren {b - j} b^{k + 1 - j}$


Induction Step
This is the induction step:














\(\ds \paren {b - 2} \sum_{j \mathop = 1}^{k + 1} j b^{k + 1 - j} + \paren {k + 1}\)

\(=\)







\(\ds \paren {b - 2} \sum_{j \mathop = 1}^k j b^{k + 1 - j} + k + 1 + \paren {b - 2} \paren {k + 1}\)




















\(\ds \)

\(=\)







\(\ds \paren {b - 2} b \sum_{j \mathop = 1}^k j b^{k - j} + \paren {b k - b k} + k + 1 + b k - 2 k + b - 2\)




















\(\ds \)

\(=\)







\(\ds b \paren {\paren {b - 2} \sum_{j \mathop = 1}^k j b^{k - j} + k} + b - k - 1\)




















\(\ds \)

\(=\)







\(\ds b \paren {\sum_{j \mathop = 1}^k \paren {b - j} b^{k - j} } + b - k - 1\)





Induction Hypothesis














\(\ds \)

\(=\)







\(\ds \sum_{j \mathop = 1}^k \paren {b - j} b^{k + 1 - j} + b - \paren {k + 1}\)




















\(\ds \)

\(=\)







\(\ds \sum_{j \mathop = 1}^{k + 1} \paren {b - j} b^{k + 1 - j}\)









So $\map P k \implies \map P {k + 1}$ and the result follows by the Principle of Mathematical Induction.

Therefore:

$\ds \paren {b - 2} \sum_{j \mathop = 1}^n j b^{n - j} + n = \sum_{j \mathop = 1}^n \paren {b - j} b^{n - j}$
$\blacksquare$





