# 

Source: https://proofwiki.org/wiki/123456789_x_9_%2B_10_%3D_1111111111



Theorem













\(\ds 1 \times 9 + 2\)

\(=\)







\(\ds 11\)




















\(\ds 12 \times 9 + 3\)

\(=\)







\(\ds 111\)




















\(\ds 123 \times 9 + 4\)

\(=\)







\(\ds 1111\)




















\(\ds 1234 \times 9 + 5\)

\(=\)







\(\ds 11111\)




















\(\ds 12345 \times 9 + 6\)

\(=\)







\(\ds 111111\)




















\(\ds 123456 \times 9 + 7\)

\(=\)







\(\ds 1111111\)




















\(\ds 1234567 \times 9 + 8\)

\(=\)







\(\ds 11111111\)




















\(\ds 12345678 \times 9 + 9\)

\(=\)







\(\ds 111111111\)




















\(\ds 123456789 \times 9 + 10\)

\(=\)







\(\ds 1111111111\)










The above pattern is an instance of the identity:

$\ds \paren {b - 1} \sum_{j \mathop = 1}^n j b^{n - j} + n + 1 = \sum_{j \mathop = 0}^n b^j$
where $b = 10$ and $n$ goes from $1$ to $9$.


Proof
The proof proceeds by induction.
Let $n, b \in \Z_{>0}$, where $b \ge 3$.
For all $n \in \Z_{\ge 1}$, let $\map P n$ be the proposition:

$\ds \paren {b - 1} \sum_{j \mathop = 1}^n j b^{n - j} + n + 1 = \sum_{j \mathop = 0}^n b^j$


Basis for the Induction
$\map P 1$ is the case:














\(\ds \paren {b - 1} \sum_{j \mathop = 1}^1 j b^{1 - j} + 2\)

\(=\)







\(\ds \paren {b - 1} b^0 + 2\)




















\(\ds \)

\(=\)







\(\ds b + 1\)




















\(\ds \)

\(=\)







\(\ds \sum_{j \mathop = 0}^1 b^j\)









Thus $\map P 1$ is seen to hold.

This is the basis for the induction.


Induction Hypothesis
Now it needs to be shown that, if $\map P k$ is true, where $k \ge 2$, then it logically follows that $\map P {k + 1}$ is true.

So this is the induction hypothesis:

$\ds \paren {b - 1} \sum_{j \mathop = 1}^k j b^{k - j} + k + 1 = \sum_{j \mathop = 0}^k b^j$

from which it is to be shown that:

$\ds \paren {b - 1} \sum_{j \mathop = 1}^{k + 1} j b^{k + 1 - j} + k + 2 = \sum_{j \mathop = 0}^{k + 1} b^j$


Induction Step
This is the induction step:














\(\ds \)

\(\)







\(\ds \paren {b - 1} \sum_{j \mathop = 1}^{k + 1} j b^{k + 1 - j} + k + 2\)




















\(\ds \)

\(=\)







\(\ds \paren {b - 1} \sum_{j \mathop = 1}^k j b^{k + 1 - j} + k + 2 + \paren {b - 1} \paren {k + 1}\)




















\(\ds \)

\(=\)







\(\ds \paren {b - 1} b \sum_{j \mathop = 1}^k j b^{k - j} + \paren {b \paren {k + 1} - b \paren {k + 1} } + k + 2 + \paren {b - 1} \paren {k + 1}\)




















\(\ds \)

\(=\)







\(\ds b \paren {\paren {b - 1} \sum_{j \mathop = 1}^k j b^{k - j} + k + 1} + 1\)




















\(\ds \)

\(=\)







\(\ds b \paren {\sum_{j \mathop = 0}^k b^j} + 1\)





Induction Hypothesis














\(\ds \)

\(=\)







\(\ds \sum_{j \mathop = 0}^k b^{j + 1} + 1\)




















\(\ds \)

\(=\)







\(\ds \sum_{j \mathop = 1}^{k + 1} b^j + 1\)





Translation of Index Variable of Summation: Corollary














\(\ds \)

\(=\)







\(\ds \sum_{j \mathop = 0}^{k + 1} b^j\)









So $\map P k \implies \map P {k + 1}$ and the result follows by the Principle of Mathematical Induction.

Therefore:

$\ds \paren {b - 1} \sum_{j \mathop = 1}^n j b^{n - j} + n + 1 = \sum_{j \mathop = 0}^n b^j$
$\blacksquare$





