# 

Source: https://proofwiki.org/wiki/Absolute_Value_Function_is_Even_Function

Theorem
Let $\size {\, \cdot \,} : \R \to \R$ denote the absolute value function on $\R$:

Then $\size {\, \cdot \,}$ is an even function.


Proof
Recall the definition of the absolute value function:

$\size x = \begin{cases}
x & : x > 0 \\
0 & : x = 0 \\
-x & : x < 0
\end{cases}$
Testing the $3$ cases in turn:














\(\ds x\)

\(>\)







\(\ds 0\)














\(\ds \leadsto \ \ \)





\(\ds -x\)

\(<\)







\(\ds 0\)














\(\ds \leadsto \ \ \)





\(\ds \size {-x}\)

\(=\)







\(\ds x\)





Definition of Absolute Value














\(\ds \)

\(=\)







\(\ds \size x\)





Definition of Absolute Value



$\Box$















\(\ds x\)

\(=\)







\(\ds 0\)














\(\ds \leadsto \ \ \)





\(\ds -x\)

\(=\)







\(\ds 0\)














\(\ds \leadsto \ \ \)





\(\ds \size {-x}\)

\(=\)







\(\ds 0\)





Definition of Absolute Value














\(\ds \)

\(=\)







\(\ds \size x\)





Definition of Absolute Value



$\Box$















\(\ds x\)

\(<\)







\(\ds 0\)














\(\ds \leadsto \ \ \)





\(\ds -x\)

\(>\)







\(\ds 0\)














\(\ds \leadsto \ \ \)





\(\ds \size {-x}\)

\(=\)







\(\ds -x\)





Definition of Absolute Value: as $-x > 0$














\(\ds \)

\(=\)







\(\ds \size x\)





Definition of Absolute Value: as $x < 0$



$\Box$

Hence the result by definition of even function.
$\blacksquare$





