# 

Source: https://proofwiki.org/wiki/Absolute_Value_Function_is_Completely_Multiplicative/Proof_1

Theorem
Let $x, y \in \R$ be real numbers.

Then:

$\size {x y} = \size x \size y$
where $\size x$ denotes the absolute value of $x$.

Thus the absolute value function is completely multiplicative.


Proof
Let either $x = 0$ or $y = 0$, or both.
We have that $\size 0 = 0$ by definition of absolute value.
Hence:

$\size x \size y = 0 = x y = \size {x y}$

Let $x > 0$ and $y > 0$.
Then:














\(\ds x y\)

\(>\)







\(\ds 0\)














\(\ds \leadsto \ \ \)





\(\ds \size {x y}\)

\(=\)







\(\ds x y\)





Definition of Absolute Value



and:














\(\ds x\)

\(=\)







\(\ds \size x\)





Definition of Absolute Value














\(\ds y\)

\(=\)







\(\ds \size y\)














\(\ds \leadsto \ \ \)





\(\ds \size x \size y\)

\(=\)







\(\ds x y\)




















\(\ds \)

\(=\)







\(\ds \size {x y}\)










Let $x < 0$ and $y < 0$.
Then:














\(\ds x y\)

\(>\)







\(\ds 0\)














\(\ds \leadsto \ \ \)





\(\ds \size {x y}\)

\(=\)







\(\ds x y\)





Definition of Absolute Value



and:














\(\ds -x\)

\(=\)







\(\ds \size x\)





Definition of Absolute Value














\(\ds -y\)

\(=\)







\(\ds \size y\)














\(\ds \leadsto \ \ \)





\(\ds \size x \size y\)

\(=\)







\(\ds \paren {-x} \paren {-y}\)




















\(\ds \)

\(=\)







\(\ds xy\)




















\(\ds \)

\(=\)







\(\ds \size {x y}\)










The final case is where one of $x$ and $y$ is positive, and one is negative.
Without loss of generality, let $x < 0$ and $y > 0$.
Then:














\(\ds x y\)

\(<\)







\(\ds 0\)














\(\ds \leadsto \ \ \)





\(\ds \size {x y}\)

\(=\)







\(\ds -\paren {x y}\)





Definition of Absolute Value



and:














\(\ds -x\)

\(=\)







\(\ds \size x\)





Definition of Absolute Value














\(\ds y\)

\(=\)







\(\ds \size y\)














\(\ds \leadsto \ \ \)





\(\ds \size x \size y\)

\(=\)







\(\ds \paren {-x} y\)




















\(\ds \)

\(=\)







\(\ds -\paren {x y}\)




















\(\ds \)

\(=\)







\(\ds \size {x y}\)









The case where $x > 0$ and $y < 0$ is the same.
$\blacksquare$





