# 

Source: https://proofwiki.org/wiki/Algebraic_Number/Examples/Cube_Root_of_2_plus_Root_3

Example of Algebraic Number
$\sqrt [3] 2 + \sqrt 3$ is an algebraic number.


Proof
Let $x = \sqrt [3] 2 + \sqrt 3$.
We have that:














\(\ds x - \sqrt 3\)

\(=\)







\(\ds \sqrt [3] 2\)














\(\ds \leadsto \ \ \)





\(\ds \paren {x - \sqrt 3}^3\)

\(=\)







\(\ds 2\)














\(\ds \leadsto \ \ \)





\(\ds \paren {x - \sqrt 3} \paren {x - \sqrt 3}^2\)

\(=\)







\(\ds 2\)














\(\ds \leadsto \ \ \)





\(\ds \paren {x - \sqrt 3} \paren {x^2 - 2 x \sqrt 3 + 3}\)

\(=\)







\(\ds 2\)














\(\ds \leadsto \ \ \)





\(\ds x^3 - 3 \sqrt 3 x^2 + 9 x - 3 \sqrt 3\)

\(=\)







\(\ds 2\)














\(\ds \leadsto \ \ \)





\(\ds x^3 + 9 x - 2\)

\(=\)







\(\ds 3 \sqrt 3 x^2 + 3 \sqrt 3\)




















\(\ds \)

\(=\)







\(\ds 3 \sqrt 3 \paren {x^2 + 1}\)














\(\ds \leadsto \ \ \)





\(\ds \paren {x^3 + 9 x - 2}^2\)

\(=\)







\(\ds 3^2 {\sqrt 3}^2 \paren {x^2 + 1}^2\)














\(\ds \leadsto \ \ \)





\(\ds x^6 + 18 x^4 - 4 x^3 + 81 x^2 - 36 x + 4\)

\(=\)







\(\ds 27 \paren {x^4 + 2 x^2 + 1}\)




















\(\ds \)

\(=\)







\(\ds 27 x^4 + 54 x^2 + 27\)














\(\ds \leadsto \ \ \)





\(\ds x^6 - 9 x^4 - 4 x^3 + 27 x^2 - 36 x - 23\)

\(=\)







\(\ds 0\)










Thus $\sqrt [3] 2 + \sqrt 3$ is a root of a non-zero polynomial with rational coefficients, namely $x^6 - 9 x^4 - 4 x^3 + 27 x^2 - 36 x - 23 = 0$.
Hence the result by definition of algebraic number.
$\blacksquare$


Sources
1981: Murray R. Spiegel: Theory and Problems of Complex Variables (SI ed.) ... (previous) ... (next): $1$: Complex Numbers: Supplementary Problems: Miscellaneous Problems: $158 \ \text{(a)}$




