# 

Source: https://proofwiki.org/wiki/Alternating_Sum_and_Difference_of_r_Choose_k_up_to_n/Proof_1

Theorem
$\ds \sum_{k \mathop \le n} \paren {-1}^k \binom r k = \paren {-1}^n \binom {r - 1} n$


Proof













\(\ds \sum_{k \mathop \le n} \paren {-1}^k \binom r k\)

\(=\)







\(\ds \sum_{k \mathop \le n} \binom {k - r - 1} k\)





Negated Upper Index of Binomial Coefficient














\(\ds \)

\(=\)







\(\ds \binom {-r + n} n\)





Sum of r+k Choose k up to n














\(\ds \)

\(=\)







\(\ds \paren {-1}^n \binom {r - 1} n\)





Negated Upper Index of Binomial Coefficient



$\blacksquare$


Sources
1997: Donald E. Knuth: The Art of Computer Programming: Volume 1: Fundamental Algorithms (3rd ed.) ... (previous) ... (next): $\S 1.2.6$: Binomial Coefficients: $(18)$




