# 

Source: https://proofwiki.org/wiki/Arccotangent_Logarithmic_Formulation

Theorem
For any real number $x$:

$\arccot x = \dfrac 1 2 i \, \map \ln {\dfrac {1 + i x} {1 - i x} }$
where $\arccot x$ is the arccotangent and $i^2 = -1$.


Proof

This article needs proofreading.Please check it for mathematical errors.If you believe there are none, please remove {{Proofread}} from the code.To discuss this page in more detail, feel free to use the talk page.When this work has been completed, you may remove this instance of {{Proofread}} from the code.
Assume $y \in \R$, $ -\dfrac \pi 2 \le y \le \dfrac \pi 2 $.














\(\ds y\)

\(=\)







\(\ds \arccot x\)














\(\ds \leadstoandfrom \ \ \)





\(\ds x\)

\(=\)







\(\ds \cot y\)














\(\ds \leadstoandfrom \ \ \)





\(\ds x\)

\(=\)







\(\ds i \frac {1 + e^{2 i y} } {1 - e^{2 i y} }\)





Euler's Cotangent Identity








\(\ds \leadstoandfrom \ \ \)





\(\ds i x\)

\(=\)







\(\ds \frac {e^{2 i y} + 1} {e^{2 i y} - 1}\)





$ i^2 = -1 $








\(\ds \leadstoandfrom \ \ \)





\(\ds i x \paren {e^{2 i y} - 1}\)

\(=\)







\(\ds e^{2 i y} + 1\)














\(\ds \leadstoandfrom \ \ \)





\(\ds i x e^{2 i y} - i x\)

\(=\)







\(\ds e^{2 i y} + 1\)














\(\ds \leadstoandfrom \ \ \)





\(\ds e^{2 i y} - i x e^{2 i y}\)

\(=\)







\(\ds 1 + i x\)














\(\ds \leadstoandfrom \ \ \)





\(\ds e^{2 i y}\)

\(=\)







\(\ds \frac {1 + i x} {1 - i x}\)














\(\ds \leadstoandfrom \ \ \)





\(\ds y\)

\(=\)







\(\ds \frac 1 2 i \map \ln {\frac {1 + i x} {1 - i x} }\)









$\blacksquare$


Also see
Arcsine Logarithmic Formulation
Arccosine Logarithmic Formulation
Arctangent Logarithmic Formulation
Arcsecant Logarithmic Formulation
Arccosecant Logarithmic Formulation




