# 

Source: https://proofwiki.org/wiki/Asymptotes_to_Hyperbola_in_Reduced_Form

Theorem
Let $\KK$ be a hyperbola embedded in a cartesian plane in reduced form with the equation:

$\dfrac {x^2} {a^2} - \dfrac {y^2} {b^2} = 1$

$\KK$ has two asymptotes which can be described by the equation:

$\dfrac {x^2} {a^2} - \dfrac {y^2} {b^2} = 0$
that is: 

$y = \pm \dfrac b a x$


Proof
From Equation of Hyperbola in Reduced Form: Polar Frame, $\KK$ can be described in polar coordinates as:

$\dfrac {\cos^2 \theta} {a^2} - \dfrac {\sin^2 \theta} {b^2} = \dfrac 1 {r^2}$
When $\theta = 0$ we have that $r = a$.
As $\theta$ increases, $\cos^2 \theta$ decreases and $\sin^2 \theta$ increases.
Hence $\dfrac 1 {r^2}$ decreases and $r$ increases as a consequence.
This continues until:

$\dfrac {\cos^2 \theta} {a^2} - \dfrac {\sin^2 \theta} {b^2} = 0$
that is:














\(\ds \tan^2 \theta\)

\(=\)







\(\ds \dfrac {b^2} {a^2}\)




















\(\ds \dfrac {y^2} {x^2}\)

\(=\)







\(\ds \dfrac {b^2} {a^2}\)




















\(\ds \dfrac {x^2} {a^2} - \dfrac {y^2} {b^2}\)

\(=\)







\(\ds 0\)









This can be expressed in the form:

$b^2 x^2 - a^2 y^2 = 0$
This is a homogeneous quadratic equation in $2$ variables of the form:

$a' x^2 + 2 h' x y + b' y^2 0 $
where:

$h' = 0$
$a' = b^2$
$b' = a^2$
From Homogeneous Quadratic Equation represents Two Straight Lines through Origin, this is the equation for $2$ straight lines through the origin:

$y = \pm \dfrac b a x$
$\blacksquare$


Sources
1933: D.M.Y. Sommerville: Analytical Conics (3rd ed.) ... (previous) ... (next): Chapter $\text {V}$. The Hyperbola: $3$. Asymptotes
1998: David Nelson: The Penguin Dictionary of Mathematics (2nd ed.) ... (previous) ... (next): hyperbola
2008: David Nelson: The Penguin Dictionary of Mathematics (4th ed.) ... (previous) ... (next): hyperbola




