# 

Source: https://proofwiki.org/wiki/Binomial_Coefficient_with_Self_minus_One/Proof_1

Theorem
$\forall n \in \N_{>0}: \dbinom n {n - 1} = n$


Proof
The case where $n = 1$ can be taken separately.
From Binomial Coefficient with Zero:

$\dbinom 1 0 = 1$
demonstrating that the result holds for $n = 1$.

Let $n \in \N: n > 1$.
From the definition of binomial coefficients:

$\dbinom n {n - 1} = \dfrac {n!} {\paren {n - 1}! \paren {n - \paren {n - 1} }!} = \dfrac {n!} {\paren {n - 1}! \ 1!}$
the result following directly from the definition of the factorial.
$\blacksquare$





