# 

Source: https://proofwiki.org/wiki/Cancellation_Laws/Proof_1

Theorem
Let $G$ be a group.
Let $a, b, c \in G$.

Then the following hold:

Right cancellation law
$b a = c a \implies b = c$
Left cancellation law
$a b = a c \implies b = c$


Proof
Let $a, b, c \in G$ and let $a^{-1}$ be the inverse of $a$.
Suppose $b a = c a$.
Then:














\(\ds \paren {b a} a^{-1}\)

\(=\)







\(\ds \paren {c a} a^{-1}\)














\(\ds \leadsto \ \ \)





\(\ds b \paren {a a^{-1} }\)

\(=\)







\(\ds c \paren {a a^{-1} }\)





Definition of Associative Operation








\(\ds \leadsto \ \ \)





\(\ds b e\)

\(=\)







\(\ds c e\)





Definition of Inverse Element








\(\ds \leadsto \ \ \)





\(\ds b\)

\(=\)







\(\ds c\)





Definition of Identity Element




Thus, the right cancellation law holds.
The proof of the left cancellation law is analogous.
$\blacksquare$


Sources
1978: Thomas A. Whitelaw: An Introduction to Abstract Algebra ... (previous) ... (next): $\S 35.1$: Elementary consequences of the group axioms




