# 

Source: https://proofwiki.org/wiki/Cancellation_of_Meet_in_Boolean_Algebra

Theorem
Let $\struct {S, \vee, \wedge, \neg}$ be a Boolean algebra.
Let $a, b, c \in S$.
Let:














\(\ds a \wedge c\)

\(=\)







\(\ds b \wedge c\)




















\(\ds a \wedge \neg c\)

\(=\)







\(\ds b \wedge \neg c\)










Then:

$a = b$


Proof
Follows from Cancellation of Join in Boolean Algebra through the Duality Principle
$\blacksquare$


Also see
Cancellation of Join in Boolean Algebra




