# 

Source: https://proofwiki.org/wiki/Cayley-Hamilton_Theorem/Finitely_Generated_Module


This article needs to be linked to other articles.You can help $\mathsf{Pr} \infty \mathsf{fWiki}$ by adding these links.To discuss this page in more detail, feel free to use the talk page.When this work has been completed, you may remove this instance of {{MissingLinks}} from the code.
Theorem
Let $A$ be a commutative ring with unity.
Let $M$ be a finitely generated $A$-module.
Let $\mathfrak a$ be an ideal of $A$.
Let $\phi$ be an endomorphism of $M$ such that $\phi \sqbrk M \subseteq \mathfrak a M$.

Then $\phi$ satisfies an equation of the form:

$\phi^n + a_{n - 1} \phi^{n-1} + \cdots + a_1 \phi + a_0 = 0$
with the $a_i \in \mathfrak a$.


Proof
Recall that the set of endomorphisms $\operatorname{End}_A(M)$ is an $A$-module with unity.
Let $R \subseteq \operatorname{End}_A(M)$ be the $A$-submudole generated by $\set {\phi^n : n \in \N}$.
That is:

$R = \set {a_0 + a_1 \phi + \cdots + a_k \phi^k : k \in \N, a_1,\ldots ,a_k \in A}$
Note that $R$ is a commutative ring with unity.
Recall also the ring of $n$-matrices $\map {\MM_R} n$.

Let $\set {m_1, \ldots, m_n}$ be a generator for $M$.
Then for each $i \in \set {1, \ldots, n}$, as $\map \phi {m_i} \in \mathfrak a M$, we can write:

$\ds \map \phi {m_i} = \sum_{j \mathop = 1}^n a_j m_j$
where $a_j \in A$ for $j \in \set {1, \ldots, n}$.
Thus for each $i \in \set {1, \ldots, n}$:

$(1): \quad \ds \sum_{j \mathop = 1}^n \sqbrk{\delta_{ij} \phi - a_{ij} \mathbf 1_R } m_i = 0$
where:

$\delta_{i j}$ is the Kronecker delta with values in $A$
Now let $\Delta \in \map {\MM_R} n$ defined as:

$\Delta := \paren {\phi \delta_{i j} - a_{i j} \mathbf 1_R }$
Then $\paren 1$ can be written as:

$\Delta \cdot \begin{bmatrix} m_1 \\ \vdots \\ m_n \end{bmatrix} = \mathbf 0_{R^n}$

Let $\adj \Delta \in \map {\MM_R } n$ be the adjugate matrix of $\Delta$.
By Matrix Product with Adjugate Matrix:














\(\ds \adj \Delta \cdot \Delta\)

\(=\)







\(\ds \Delta \cdot \adj \Delta\)




















\(\ds \)

\(=\)







\(\ds \map \det \Delta \mathbf I_n\)




















\(\ds \)

\(=\)







\(\ds \begin{bmatrix}
\map \det \Delta & 0 & \cdots & 0 \\
0 & \map \det \Delta & \cdots & 0 \\
\vdots & \vdots & \ddots & \vdots \\
0 & 0 & \cdots & \map \det \Delta \\
\end{bmatrix}\)










where $\map \det \Delta \in R$ denotes the determinant of $\Delta$.

Multiplying the above equality by $\adj \Delta$ and applying Cramer's Rule:

$\ds \map \det \Delta m_i = 0$
for each $i \in \set {1, \ldots , n}$.
Therefore:

$\map \det \Delta = \mathbf 0_R$
On the other hand, $\map \det \Delta$ is a monic polynomial in $\phi$, since:














\(\ds \map \det \Delta\)

\(=\)







\(\ds \map \det {\delta_{i j} \phi - a_{i j} \mathbf 1_R }\)




















\(\ds \)

\(=\)







\(\ds \sum_{\lambda} \paren {\map \sgn \lambda \prod_{k \mathop = 1}^n \paren {\delta_{k \map \lambda k} \phi - a_{k \map \lambda k} \mathbf 1_R } }\)





Definition 1 of Determinant














\(\ds \)

\(=\)







\(\ds \phi^n + a_{n - 1} \phi^{n-1} + \cdots + a_1 \phi + a_0 \mathbf 1_R\)









where:

$\lambda$ goes over all permutations of $\set {1, 2, \ldots, n}$
$\map \sgn \lambda$ is the sign of the permutation $\lambda$
$a_0, a_1, \ldots, a_{n-1} \in \mathfrak a$
As $R \subseteq \operatorname{End}_A(M)$, this means:

$\phi^n + a_{n - 1} \phi^{n-1} + \cdots + a_1 \phi + a_0 = 0$
$\blacksquare$


Source of Name
This entry was named for Arthur Cayley and William Rowan Hamilton.





