# 

Source: https://proofwiki.org/wiki/Change_of_Base_of_Logarithm/Base_e_to_Base_10/Form_1

Theorem
Let $\log_{10} x$ be the common (base $10$) logarithm of $x$.
Let $\ln x$ be the natural (base $e$) logarithm of $x$.

Then:

$\log_{10} x = \paren {\log_{10} e} \paren {\ln x} = 0 \cdotp 43429 \, 44819 \, 03 \ldots \ln x$


Proof
From Change of Base of Logarithm:

$\log_a x = \log_a b \, \log_b x$
Substituting $a = 10$ and $b = e$ gives:

$\log_{10} x = \paren {\log_{10} e} \paren {\ln x}$

The Common Logarithm of e:

$\log_{10} e = 0 \cdotp 43429 \, 44819 \, 03 \ldots$
can be calculated or looked up.
$\blacksquare$


Sources
1968: Murray R. Spiegel: Mathematical Handbook of Formulas and Tables ... (previous) ... (next): $\S 7$: Change of Base of Logarithms: $7.15$
1983: François Le Lionnais and Jean Brette: Les Nombres Remarquables ... (previous) ... (next): $0,43429 44819 \ldots$




