# 

Source: https://proofwiki.org/wiki/Change_of_Base_of_Logarithm/Base_2_to_Base_8

Theorem
Let $\log_8 x$ be the logarithm base $8$ of $x$.
Let $\lg x$ be the binary (base $2$) logarithm of $x$.

Then:

$\log_8 x = \dfrac {\lg x} 3$


Proof
From Change of Base of Logarithm:

$\log_a x = \dfrac {\log_b x} {\log_b a}$
Substituting $a = 8$ and $b = 2$ gives:

$\log_8 x = \dfrac {\log_2 x} {\log_2 8}$

We have that:














\(\ds 2^3\)

\(=\)







\(\ds 8\)














\(\ds \leadsto \ \ \)





\(\ds \lg 8\)

\(=\)







\(\ds \log_2 2^3\)




















\(\ds \)

\(=\)







\(\ds 3 \log_2 2\)




















\(\ds \)

\(=\)







\(\ds 3\)





Logarithm to Own Base equals 1



The result follows.
$\blacksquare$


Sources
1997: Donald E. Knuth: The Art of Computer Programming: Volume 1: Fundamental Algorithms (3rd ed.) ... (previous) ... (next): $\S 1.2.2$: Numbers, Powers, and Logarithms: Exercise $18$




