# 

Source: https://proofwiki.org/wiki/Change_of_Base_of_Logarithm/Proof_1

Theorem
$\log_b x = \dfrac {\log_a x} {\log_a b}$


Proof
Let:

$y = \log_b x \iff b^y = x$
$z = \log_a x \iff a^z = x$
Then:














\(\ds z\)

\(=\)







\(\ds \map {\log_a} {b^y}\)




















\(\ds \)

\(=\)







\(\ds y \log_a b\)





Logarithms of Powers














\(\ds \)

\(=\)







\(\ds \log_b x \log_a b\)









Hence the result.
$\blacksquare$


Sources

This page may be the result of a refactoring operation.As such, the following source works, along with any process flow, will need to be reviewed.When this has been completed, the citation of that source work (if it is appropriate that it stay on this page) is to be placed above this message, into the usual chronological ordering.If you have access to any of these works, then you are invited to review this list, and make any necessary corrections.To discuss this page in more detail, feel free to use the talk page.When this work has been completed, you may remove this instance of {{SourceReview}} from the code.
1968: Murray R. Spiegel: Mathematical Handbook of Formulas and Tables ... (previous) ... (next): $\S 7$: Change of Base of Logarithms: $7.13$
1997: Donald E. Knuth: The Art of Computer Programming: Volume 1: Fundamental Algorithms (3rd ed.) ... (previous) ... (next): $\S 1.2.2$: Numbers, Powers, and Logarithms: $(14)$




