# 

Source: https://proofwiki.org/wiki/Chebyshev%27s_Sum_Inequality/Discrete/Proof



Theorem
Let $a_1, a_2, \ldots, a_n$ be real numbers such that:

$a_1 \ge a_2 \ge \cdots \ge a_n$
Let $b_1, b_2, \ldots, b_n$ be real numbers such that:

$b_1 \ge b_2 \ge \cdots \ge b_n$
Then:

$\ds \dfrac 1 n \sum_{k \mathop = 1}^n a_k b_k \ge \paren {\dfrac 1 n \sum_{k \mathop = 1}^n a_k} \paren {\dfrac 1 n \sum_{k \mathop = 1}^n b_k}$


Proof
We have by hypothesis that the sequences $\sequence {a_k}$ and $\sequence {b_k}$ are both decreasing.
For $j, k \in \set {1, 2, \ldots, n}$, consider:

$\paren {a_j - a_k} \paren {b_j - b_k}$
Therefore $a_j - a_k$ and $b_j - b_k$ have the same sign for all $j, k \in \set {1, 2, \ldots, n}$.
So:

$\forall j, k \in \set {1, 2, \ldots, n}: \paren {a_j - a_k} \paren {b_j - b_k} \ge 0$

Hence:














\(\ds 0\)

\(\le\)







\(\ds \sum_{j \mathop = 1}^n \sum_{k \mathop = 1}^n \paren {a_j - a_k} \paren {b_j - b_k}\)




















\(\ds \)

\(=\)







\(\ds \sum_{j \mathop = 1}^n \sum_{k \mathop = 1}^n \paren {a_j b_j - a_k b_j - a_j b_k + a_k b_k}\)




















\(\ds \)

\(=\)







\(\ds \sum_{j \mathop = 1}^n \sum_{k \mathop = 1}^n a_j b_j - \sum_{j \mathop = 1}^n \sum_{k \mathop = 1}^n a_k b_j - \sum_{j \mathop = 1}^n \sum_{k \mathop = 1}^n a_j b_k + \sum_{j \mathop = 1}^n \sum_{k \mathop = 1}^n a_k b_k\)




















\(\ds \)

\(=\)







\(\ds n \sum_{j \mathop = 1}^n a_j b_j - \sum_{k \mathop = 1}^n a_k \sum_{j \mathop = 1}^n b_j - \sum_{j \mathop = 1}^n a_j \sum_{k \mathop = 1}^n b_k + n \sum_{k \mathop = 1}^n a_k b_k\)





General Distributivity Theorem














\(\ds \)

\(=\)







\(\ds 2 n \sum_{k \mathop = 1}^n a_k b_k - 2 \sum_{k \mathop = 1}^n a_k \sum_{k \mathop = 1}^n b_k\)





renaming and gathering equal terms














\(\ds \)

\(=\)







\(\ds n \sum_{k \mathop = 1}^n a_k b_k - \sum_{k \mathop = 1}^n a_k \sum_{k \mathop = 1}^n b_k\)





dividing through by $2$




Then we may manipulate it into the required form:












\(\ds \)

\(=\)







\(\ds \dfrac 1 n \sum_{k \mathop = 1}^n a_k b_k - \dfrac 1 {n^2} \sum_{k \mathop = 1}^n a_k \sum_{k \mathop = 1}^n b_k\)





dividing through by $n^2$








\(\ds \leadsto \ \ \)





\(\ds \dfrac 1 n \sum_{k \mathop = 1}^n a_k b_k\)

\(\ge\)







\(\ds \paren {\dfrac 1 n \sum_{k \mathop = 1}^n a_k} \paren {\dfrac 1 n \sum_{k \mathop = 1}^n b_k}\)









The result follows.
$\blacksquare$


Also presented as
Some sources present Chebyshev's sum inequality as:

$\ds n \sum_{k \mathop = 1}^n a_k b_k \ge \paren {\sum_{k \mathop = 1}^n a_k} \paren {\sum_{k \mathop = 1}^n b_k}$


Also known as
Chebyshev's Sum Inequality is also known as Chebyshev's Inequality.
However, some sources use this name to mean the Bienaym√©-Chebyshev Inequality, which is a completely different result.
Hence, to avoid confusion, the name Chebyshev's Inequality is not used on $\mathsf{Pr} \infty \mathsf{fWiki}$.


Source of Name
This entry was named for Pafnuty Lvovich Chebyshev.





