# 

Source: https://proofwiki.org/wiki/Closed_Form_for_Centered_Hexagonal_Numbers

Theorem
Let $C_n$ be the $n$th centered hexagonal number.

Then:

$C_n = 3 n \paren {n - 1} + 1$


Proof
By the definition of centered hexagonal number:














\(\ds C_n\)

\(=\)







\(\ds 1 + \sum_{k \mathop = 1}^{n - 1} 6 k\)





Definition of Centered Hexagonal Number














\(\ds \)

\(=\)







\(\ds 1 + 6 \sum_{k \mathop = 1}^{n - 1} k\)




















\(\ds \)

\(=\)







\(\ds 6 \paren {\dfrac {n \paren {n - 1} } 2} + 1\)





Closed Form for Triangular Numbers














\(\ds \)

\(=\)







\(\ds 3 n \paren {n - 1} + 1\)









$\blacksquare$


Sources
1986: David Wells: Curious and Interesting Numbers ... (previous) ... (next): $37$
1997: David Wells: Curious and Interesting Numbers (2nd ed.) ... (previous) ... (next): $37$




