# 

Source: https://proofwiki.org/wiki/Closed_Form_for_Triangular_Numbers/Proof_by_Arithmetic_Sequence

Theorem
The closed-form expression for the $n$th triangular number is:

$\ds T_n = \sum_{i \mathop = 1}^n i = \frac {n \paren {n + 1} } 2$


Proof













\(\ds \sum_{i \mathop = 0}^{m - 1} \paren {a + i d}\)

\(=\)







\(\ds m \paren {a + \frac {m - 1} 2 d}\)





Sum of Arithmetic Sequence














\(\ds \sum_{i \mathop = 0}^n \paren {a + i d}\)

\(=\)







\(\ds \paren {n + 1} \paren {a + \frac n 2 d}\)





Let $n = m - 1$














\(\ds \sum_{i \mathop = 0}^n i\)

\(=\)







\(\ds \paren {n + 1} \paren {\frac n 2}\)





Let $a = 0$ and $d = 1$














\(\ds 0 + \sum_{i \mathop = 1}^n i\)

\(=\)







\(\ds \frac {n \paren {n + 1} } 2\)




















\(\ds \sum_{i \mathop = 1}^n i\)

\(=\)







\(\ds \frac {n \paren {n + 1} } 2\)









$\blacksquare$





