# 

Source: https://proofwiki.org/wiki/Closed_Form_for_Triangular_Numbers/Proof_using_Odd_Number_Theorem

Theorem
The closed-form expression for the $n$th triangular number is:

$\ds T_n = \sum_{i \mathop = 1}^n i = \frac {n \paren {n + 1} } 2$


Proof













\(\ds \sum_{j \mathop = 1}^n \paren {2 j - 1}\)

\(=\)







\(\ds n^2\)





Odd Number Theorem








\(\ds \leadsto \ \ \)





\(\ds \sum_{j \mathop = 1}^n \paren {2 j - 1} + \sum_{j \mathop = 1}^n 1\)

\(=\)







\(\ds n^2 + n\)














\(\ds \leadsto \ \ \)





\(\ds \sum_{j \mathop = 1}^n \paren {2 j}\)

\(=\)







\(\ds n \paren {n + 1}\)














\(\ds \leadsto \ \ \)





\(\ds \sum_{j \mathop = 1}^n j\)

\(=\)







\(\ds \frac {n \paren {n + 1} } 2\)









$\blacksquare$


Sources
1992: George F. Simmons: Calculus Gems ... (previous) ... (next): Chapter $\text {A}.2$: Pythagoras (ca. $\text {580}$ – $\text {500}$ B.C.)




