# 

Source: https://proofwiki.org/wiki/Closed_Form_for_Hexagonal_Pyramidal_Numbers

Theorem
The closed-form expression for the $n$th hexagonal pyramidal number is:

$S_n = \dfrac {n \paren {n + 1} \paren {4 n - 1} } 6$


Proof













\(\ds S_n\)

\(=\)







\(\ds \sum_{k \mathop = 1}^n H_k\)





Definition of Hexagonal Pyramidal Number














\(\ds \)

\(=\)







\(\ds \sum_{k \mathop = 1}^n k \paren {2 k - 1}\)





Closed Form for Hexagonal Numbers














\(\ds \)

\(=\)







\(\ds 3 \sum_{k \mathop = 1}^n 2 k^2 - \sum_{k \mathop = 1}^n k\)




















\(\ds \)

\(=\)







\(\ds \frac {2 n \paren {n + 1} \paren {2 n + 1} } 6 - \sum_{k \mathop = 1}^n k\)





Sum of Sequence of Squares














\(\ds \)

\(=\)







\(\ds \frac {2 n \paren {n + 1} \paren {2 n + 1} } 6 - \dfrac {n \paren {n + 1} } 2\)





Closed Form for Triangular Numbers














\(\ds \)

\(=\)







\(\ds \frac {2 n \paren {n + 1} \paren {2 n + 1} - 3 n \paren {n + 1} } 6\)




















\(\ds \)

\(=\)







\(\ds \frac {n \paren {n + 1} \paren {4 n + 2 - 3} } 6\)




















\(\ds \)

\(=\)







\(\ds \frac {n \paren {n + 1} \paren {4 n - 1} } 6\)









$\blacksquare$





