# 

Source: https://proofwiki.org/wiki/Closed_Form_for_Heptagonal_Pyramidal_Numbers

Theorem
The closed-form expression for the $n$th heptagonal pyramidal number is:

$Q_n = \dfrac {n \paren {n + 1} \paren {5 n - 2} } 6$


Proof













\(\ds Q_n\)

\(=\)







\(\ds \sum_{k \mathop = 1}^n H_n\)





Definition of Heptagonal Pyramidal Number














\(\ds \)

\(=\)







\(\ds \sum_{k \mathop = 1}^n \dfrac {k \paren {5 k - 3} } 2\)





Closed Form for Heptagonal Numbers














\(\ds \)

\(=\)







\(\ds \dfrac 1 2 \paren {5 \sum_{k \mathop = 1}^n k^2 - 3 \sum_{k \mathop = 1}^n k}\)




















\(\ds \)

\(=\)







\(\ds \dfrac 1 2 \paren {5 \frac {n \paren {n + 1} \paren {2 n + 1} } 6 - 3 \sum_{k \mathop = 1}^n k}\)





Sum of Sequence of Squares














\(\ds \)

\(=\)







\(\ds \dfrac 1 2 \paren {5 \frac {n \paren {n + 1} \paren {2 n + 1} } 6 - 3 \dfrac {n \paren {n + 1} } 2}\)





Closed Form for Triangular Numbers














\(\ds \)

\(=\)







\(\ds \dfrac 1 2 \paren {\frac {5 n \paren {n + 1} \paren {2 n + 1} - 9 n \paren {n + 1} } 6}\)




















\(\ds \)

\(=\)







\(\ds \dfrac 1 2 \paren {\frac {n \paren {n + 1} \paren {5 \paren {2 n + 1} - 9} } 6}\)




















\(\ds \)

\(=\)







\(\ds \dfrac 1 2 \paren {\frac {n \paren {n + 1} \paren {10 n + 5 - 9} } 6}\)




















\(\ds \)

\(=\)







\(\ds \dfrac 1 2 \paren {\frac {n \paren {n + 1} \paren {10 n - 4} } 6}\)




















\(\ds \)

\(=\)







\(\ds \frac {n \paren {n + 1} \paren {5 n - 2} } 6\)









$\blacksquare$


Sources
1997: David Wells: Curious and Interesting Numbers (2nd ed.) ... (previous) ... (next): $196$




