# 

Source: https://proofwiki.org/wiki/Closed_Form_for_Pentagonal_Pyramidal_Numbers

Theorem
The closed-form expression for the $n$th pentagonal pyramidal number is:

$Q_n = \dfrac {n^2 \paren {n + 1} } 2$


Proof













\(\ds Q_n\)

\(=\)







\(\ds \sum_{k \mathop = 1}^n P_k\)





Definition of Pentagonal Pyramidal Number














\(\ds \)

\(=\)







\(\ds \sum_{k \mathop = 1}^n \dfrac {k \paren {3 k - 1} } 2\)





Closed Form for Pentagonal Numbers














\(\ds \)

\(=\)







\(\ds \dfrac 1 2 \paren {3 \sum_{k \mathop = 1}^n k^2 - \sum_{k \mathop = 1}^n k}\)




















\(\ds \)

\(=\)







\(\ds \dfrac 1 2 \paren {3 \frac {n \paren {n + 1} \paren {2 n + 1} } 6 - \sum_{k \mathop = 1}^n k}\)





Sum of Sequence of Squares














\(\ds \)

\(=\)







\(\ds \dfrac 1 2 \paren {3 \frac {n \paren {n + 1} \paren {2 n + 1} } 6 - \dfrac {n \paren {n + 1} } 2}\)





Closed Form for Triangular Numbers














\(\ds \)

\(=\)







\(\ds \dfrac 1 2 \paren {\frac {n \paren {n + 1} \paren {2 n + 1} - n \paren {n + 1} } 2}\)




















\(\ds \)

\(=\)







\(\ds \dfrac 1 2 \paren {\frac {n \paren {n + 1} \paren {2 n} } 2}\)




















\(\ds \)

\(=\)







\(\ds \frac {n^2 \paren {n + 1} } 2\)









$\blacksquare$


Sources
1986: David Wells: Curious and Interesting Numbers ... (previous) ... (next): $55$
1997: David Wells: Curious and Interesting Numbers (2nd ed.) ... (previous) ... (next): $55$




