# 

Source: https://proofwiki.org/wiki/Closed_Form_for_Triangular_Numbers/Proof_using_Binomial_Coefficients

Theorem
The closed-form expression for the $n$th triangular number is:

$\ds T_n = \sum_{i \mathop = 1}^n i = \frac {n \paren {n + 1} } 2$


Proof
From Binomial Coefficient with One:

$\forall k \in \Z, k > 0: \dbinom k 1 = k$
Thus:














\(\ds \sum_{k \mathop = 1}^n k\)

\(=\)







\(\ds \sum_{k \mathop = 1}^n \binom k 1\)





Binomial Coefficient with One














\(\ds \)

\(=\)







\(\ds \binom {n + 1} 2\)





Sum of k Choose m up to n‎














\(\ds \)

\(=\)







\(\ds \frac {\paren {n + 1} n} 2\)





Definition of Binomial Coefficient



$\blacksquare$


Sources
1997: Donald E. Knuth: The Art of Computer Programming: Volume 1: Fundamental Algorithms (3rd ed.) ... (previous) ... (next): $\S 1.2.6$: Binomial Coefficients




