# 

Source: https://proofwiki.org/wiki/Combination_Theorem_for_Sequences/Normed_Division_Ring/Combined_Sum_Rule

Theorem
Let $\struct {R, \norm {\, \cdot \,} }$ be a normed division ring.
Let $\sequence {x_n}$,  $\sequence {y_n}$ be sequences in $R$.
Let $\sequence {x_n}$ and $\sequence {y_n}$ be convergent in the norm $\norm {\, \cdot \,}$ to the following limits:

$\ds \lim_{n \mathop \to \infty} x_n = l$
$\ds \lim_{n \mathop \to \infty} y_n = m$

Let $\lambda, \mu \in R$.
Then:

$\sequence {\lambda x_n + \mu y_n }$ is convergent and $\ds \lim_{n \mathop \to \infty} \paren {\lambda x_n + \mu y_n} = \lambda l + \mu m$


Proof
From the Multiple Rule for Sequences in Normed Division Ring, we have:

$\ds \lim_{n \mathop \to \infty} \paren {\lambda x_n} = \lambda l$
$\ds \lim_{n \mathop \to \infty} \paren {\mu y_n} = \mu m$
The result now follows directly from the Sum Rule for Sequences in Normed Division Ring:

$\ds \lim_{n \mathop \to \infty} \paren {\lambda x_n + \mu y_n} = \lambda l + \mu m$
$\blacksquare$


Also see
Multiple Rule for Sequences in Normed Division Ring
Sum Rule for Sequences in Normed Division Ring




