# 

Source: https://proofwiki.org/wiki/Combination_Theorem_for_Sequences/Real/Combined_Sum_Rule

Theorem
Let $\sequence {x_n}$ and $\sequence {y_n}$ be sequences in $\R$.
Let $\sequence {x_n}$ and $\sequence {y_n}$ be convergent to the following limits:

$\ds \lim_{n \mathop \to \infty} x_n = l$
$\ds \lim_{n \mathop \to \infty} y_n = m$

Let $\lambda, \mu \in \R$.

Then:

$\ds \lim_{n \mathop \to \infty} \paren {\lambda x_n + \mu y_n} = \lambda l + \mu m$


Proof
From the Multiple Rule for Real Sequences, we have:

$\ds \lim_{n \mathop \to \infty} \paren {\lambda x_n} = \lambda l$
$\ds \lim_{n \mathop \to \infty} \paren {\mu y_n} = \mu m$
The result now follows directly from the Sum Rule for Real Sequences:

$\ds \lim_{n \mathop \to \infty} \paren {\lambda x_n + \mu y_n} = \lambda l + \mu m$
$\blacksquare$


Sources
1977: K.G. Binmore: Mathematical Analysis: A Straightforward Approach ... (previous) ... (next): $\S 4$: Convergent Sequences: $\S 4.8 \ \text {(i)}$: Criteria for convergence




