# 

Source: https://proofwiki.org/wiki/Complex_Algebra/Examples/2x_-_3iy_%2B_4ix_-_2y_-_5_-_10i_%3D_(x_%2B_y_%2B_2)_-_(y_-_x_%2B_3)i

Example of Complex Algebra
Let:

$2 x - 3 i y + 4 i x - 2 y - 5 - 10 i = \paren {x + y + 2} - \paren {y - x + 3} i$
Then:














\(\ds x\)

\(=\)







\(\ds 1\)




















\(\ds y\)

\(=\)







\(\ds -2\)











Proof
Separating the real parts from the imaginary parts:














\(\ds 2 x - 2 y - 5\)

\(=\)







\(\ds x + y + 2\)










\(\text {(1)}: \quad\)



\(\ds \leadsto \ \ \)





\(\ds x\)

\(=\)







\(\ds 3 y + 7\)
























\(\ds -3 i y + 4 i x - 10 i\)

\(=\)







\(\ds \paren {y - x + 3} i\)














\(\ds \leadsto \ \ \)





\(\ds -3 y + 4 x - 10\)

\(=\)







\(\ds y - x + 3\)










\(\text {(2)}: \quad\)



\(\ds \leadsto \ \ \)





\(\ds 5 x - 4 y\)

\(=\)







\(\ds 13\)










Substituting for $x$ from $(1)$ into $(2)$:














\(\ds 5 \paren {3 y + 7} - 4 y\)

\(=\)







\(\ds 13\)














\(\ds \leadsto \ \ \)





\(\ds 15 y + 35 - 4 y\)

\(=\)







\(\ds 13\)














\(\ds \leadsto \ \ \)





\(\ds 11 y\)

\(=\)







\(\ds -22\)










\(\text {(3)}: \quad\)



\(\ds \leadsto \ \ \)





\(\ds y\)

\(=\)







\(\ds -2\)














\(\ds \leadsto \ \ \)





\(\ds x\)

\(=\)







\(\ds 3 \times {-2} + 7\)





substituting for $y$ from $(3)$ into $(1)$














\(\ds \)

\(=\)







\(\ds 1\)









$\blacksquare$


Sources
1981: Murray R. Spiegel: Theory and Problems of Complex Variables (SI ed.) ... (previous) ... (next): $1$: Complex Numbers: Supplementary Problems: Fundamental Operations with Complex Numbers: $57$




