# 

Source: https://proofwiki.org/wiki/Completely_Multiplicative_Function_of_Quotient

Theorem
Let $f: \R \to \R$ be a completely multiplicative function.
Then:

$\forall x, y \in \R, y \ne 0: \map f {\dfrac x y} = \dfrac {\map f x} {\map f y}$
whenever $\map f y \ne 0$.


Proof
Let $z = \dfrac x y$.
Then:














\(\ds z\)

\(=\)







\(\ds \dfrac x y\)














\(\ds \leadsto \ \ \)





\(\ds x\)

\(=\)







\(\ds y z\)














\(\ds \leadsto \ \ \)





\(\ds \map f x\)

\(=\)







\(\ds \map f y \map f z\)





Definition of Completely Multiplicative Function








\(\ds \leadsto \ \ \)





\(\ds \frac {\map f x} {\map f y}\)

\(=\)







\(\ds \map f z\)





dividing by $\map f y$








\(\ds \leadsto \ \ \)





\(\ds \frac {\map f x} {\map f y}\)

\(=\)







\(\ds \map f {\frac x y}\)





Definition of $z$



$\blacksquare$





