# 

Source: https://proofwiki.org/wiki/Complex_Arithmetic/Examples/(3i%5E30_-_i%5E19)_(2i_-_1)%5E-1

Example of Complex Arithmetic
$\dfrac {3 i^{30} - i^{19} } {2 i - 1} = 1 + i$


Proof













\(\ds \dfrac {3 i^{30} - i^{19} } {2 i - 1}\)

\(=\)







\(\ds \dfrac {3 \paren {-1}^{15} - \paren {-1}^9 i} {2 i - 1}\)





as $i^2 = -1$














\(\ds \)

\(=\)







\(\ds \dfrac {-3 + i} {2 i - 1}\)





as $\paren {-1}^n = -1$ for odd $n$














\(\ds \)

\(=\)







\(\ds \dfrac {\paren {-3 + i}\paren {-1 - 2 i} } {\paren {2 i - 1}\paren {-1 - 2 i} }\)





multiplying top and bottom by $-1 - 2 i$














\(\ds \)

\(=\)







\(\ds \dfrac {3 - i + 6 i - 2 i^2} {2^2 + 1^2}\)





Definition of Complex Multiplication














\(\ds \)

\(=\)







\(\ds \dfrac {5 + 5 i} 5\)





simplifying














\(\ds \)

\(=\)







\(\ds 1 + i\)





simplifying



$\blacksquare$


Sources
1981: Murray R. Spiegel: Theory and Problems of Complex Variables (SI ed.) ... (previous) ... (next): $1$: Complex Numbers: Solved Problems: Fundamental Operations with Complex Numbers: $1 \ \text{(m)}$




