# 

Source: https://proofwiki.org/wiki/Complex_Division/Examples/(3_-_2i)_(-1_%2B_i)%5E-1/Proof_2

Example of Complex Division
$\dfrac {3 - 2 i} {-1 + i} = \dfrac {-5 - i} 2$


Proof













\(\ds \dfrac {3 - 2 i} {-1 + i}\)

\(=\)







\(\ds a + b i\)





where $a, b \in \R$








\(\ds \leadsto \ \ \)





\(\ds 3 - 2 i\)

\(=\)







\(\ds \paren {-1 + i} \paren {a + b i}\)




















\(\ds \)

\(=\)







\(\ds -a + b i + a i + b i^2\)





Definition of Complex Multiplication














\(\ds \)

\(=\)







\(\ds -a - b + \paren {a - b} i\)





simplifying




Then:














\(\ds -a - b\)

\(=\)







\(\ds 3\)




















\(\ds a - b\)

\(=\)







\(\ds -1\)














\(\ds \leadsto \ \ \)





\(\ds a\)

\(=\)







\(\ds -\frac 5 2\)




















\(\ds b\)

\(=\)







\(\ds -\frac 1 2\)









Hence the result.
$\blacksquare$


Sources
1981: Murray R. Spiegel: Theory and Problems of Complex Variables (SI ed.) ... (previous) ... (next): $1$: Complex Numbers: Solved Problems: Fundamental Operations with Complex Numbers: $1 \ \text{(k)}$




