# 

Source: https://proofwiki.org/wiki/Conditions_under_which_Commutative_Semigroup_is_Group/Lemma_2

Lemma for Conditions under which Commutative Semigroup is Group
Suppose the following:
Let $\struct {S, \circ}$ be a commutative semigroup.

Let $\struct {S, \circ}$ have the following properties:




\((1)\)  

$:$  





  \(\ds \forall x \in S: \exists y \in S:\)

\(\ds y \circ x = x \)   







  


\((2)\)  

$:$  





  \(\ds \forall x, y \in S:\)

\(\ds y \circ x = x \implies \exists z \in S: z \circ x = y \)   







  


Then:

If $y \circ x = x$, then $y \circ y = y$.


Proof













\(\ds y \circ x\)

\(=\)







\(\ds x\)





by hypothesis








\(\ds \leadsto \ \ \)





\(\ds y \circ \paren {y \circ x}\)

\(=\)







\(\ds y \circ x\)





premultiplying both sides by $y$














\(\ds \)

\(=\)







\(\ds x\)





by hypothesis








\(\ds \leadsto \ \ \)





\(\ds \paren {y \circ y} \circ x\)

\(=\)







\(\ds x\)





Semigroup Axiom $\text S 1$: Associativity








\(\ds \leadsto \ \ \)





\(\ds y \circ y\)

\(=\)







\(\ds y\)





Lemma 1



$\blacksquare$


Sources
1965: Seth Warner: Modern Algebra ... (previous) ... (next): Chapter $\text I$: Algebraic Structures: $\S 7$: Semigroups and Groups: Exercise $7.16 \ \text {(b)}$




