# 

Source: https://proofwiki.org/wiki/Conjugates_of_Transpositions


This article needs to be linked to other articles.You can help $\mathsf{Pr} \infty \mathsf{fWiki}$ by adding these links.To discuss this page in more detail, feel free to use the talk page.When this work has been completed, you may remove this instance of {{MissingLinks}} from the code.
Theorem
Let $k_1, k_2, k_3 \in \left\{{1, 2, \ldots, n}\right\}$.
Then:

$(1): \quad \begin{bmatrix} k_1 & k_2 \end{bmatrix} = \begin{bmatrix} k_3 & k_2 \end{bmatrix} \begin{bmatrix} k_1 & k_3 \end{bmatrix} \begin{bmatrix} k_3 & k_2 \end{bmatrix}$
$(2): \quad \begin{bmatrix} k_1 & k_2 \end{bmatrix} = \begin{bmatrix} k_3 & k_1 \end{bmatrix} \begin{bmatrix} k_3 & k_2 \end{bmatrix} \begin{bmatrix} k_3 & k_1 \end{bmatrix}$


Proof
$(1):$ Calculating the product of $\begin{bmatrix} k_3 & k_2 \end{bmatrix} \begin{bmatrix} k_1 & k_3 \end{bmatrix} \begin{bmatrix} k_3 & k_2 \end{bmatrix}$:

$k_1 \to k_3 \to k_2$
$k_2 \to k_3 \to k_1$
$k_3 \to k_2 \to k_3$
hence the result.
$\Box$

$(2):$ Calculating the product of $\begin{bmatrix} k_3 & k_1 \end{bmatrix} \begin{bmatrix} k_3 & k_2 \end{bmatrix} \begin{bmatrix} k_3 & k_1 \end{bmatrix}$:

$k_1 \to k_3 \to k_2$
$k_2 \to k_3 \to k_1$
$k_3 \to k_1 \to k_3$
hence the result.
$\blacksquare$





