# 

Source: https://proofwiki.org/wiki/Coset/Examples/Dihedral_Group_D3/Cosets_of_Subgroup_Generated_by_b/Left_Cosets

Examples of Left Cosets
Consider the dihedral group $D_3$.

$D_3 = \gen {a, b: a^3 = b^2 = e, a b = b a^{-1} }$

Let $H \subseteq D_3$ be defined as:

$H = \gen b$
where $\gen b$ denotes the subgroup generated by $b$.

As $b$ has order $2$, it follows that:

$\gen b = \set {e, b}$

The left cosets of $H$ are:














\(\ds e H\)

\(=\)







\(\ds \set {e, b}\)




















\(\ds \)

\(=\)







\(\ds b H\)




















\(\ds \)

\(=\)







\(\ds H\)
























\(\ds a H\)

\(=\)







\(\ds \set {a, a b}\)




















\(\ds \)

\(=\)







\(\ds a b H\)
























\(\ds a^2 H\)

\(=\)







\(\ds \set {a^2, a^2 b}\)




















\(\ds \)

\(=\)







\(\ds a^2 b H\)











Proof
The Cayley table of $D_3$ is presented as:

$\begin{array}{c|cccccc}      & e     & a     & a^2   & b     & a b   & a^2 b \\ \hline e     & e     & a     & a^2   & b     & a b   & a^2 b \\ a     & a     & a^2   & e     & a b   & a^2 b & b     \\ a^2   & a^2   & e     & a     & a^2 b & b     & a b   \\ b     & b     & a^2 b & a b   & e     & a^2   & a     \\ a b   & a b   & b     & a^2 b & a     & e     & a^2   \\ a^2 b & a^2 b & a b   & b     & a^2   & a     & e     \\ \end{array}$

Thus:














\(\ds e H\)

\(=\)







\(\ds e \set {e, b}\)




















\(\ds \)

\(=\)







\(\ds \set {e^2, e b}\)




















\(\ds \)

\(=\)







\(\ds \set {e, b}\)




















\(\ds \)

\(=\)







\(\ds H\)
























\(\ds b H\)

\(=\)







\(\ds b \set {e, b}\)




















\(\ds \)

\(=\)







\(\ds \set {b e, b^2}\)




















\(\ds \)

\(=\)







\(\ds \set {b, e}\)




















\(\ds \)

\(=\)







\(\ds H\)
























\(\ds a H\)

\(=\)







\(\ds a \set {e, b}\)




















\(\ds \)

\(=\)







\(\ds \set {a e, a b}\)




















\(\ds \)

\(=\)







\(\ds \set {a, a b}\)
























\(\ds a^2 H\)

\(=\)







\(\ds a^2 \set {e, b}\)




















\(\ds \)

\(=\)







\(\ds \set {a^2 e, a^2 b}\)




















\(\ds \)

\(=\)







\(\ds \set {a^2, a^2 b}\)
























\(\ds a b H\)

\(=\)







\(\ds a b \set {e, b}\)




















\(\ds \)

\(=\)







\(\ds \set {a b e, a b b}\)




















\(\ds \)

\(=\)







\(\ds \set {a b, a}\)




















\(\ds \)

\(=\)







\(\ds a H\)
























\(\ds a^2 b H\)

\(=\)







\(\ds a^2 b \set {e, b}\)




















\(\ds \)

\(=\)







\(\ds \set {a^2 b e, a^2 b b}\)




















\(\ds \)

\(=\)







\(\ds \set {a^2 b, a^2}\)




















\(\ds \)

\(=\)







\(\ds a^2 H\)









$\blacksquare$


Sources
1996: John F. Humphreys: A Course in Group Theory ... (previous) ... (next): Chapter $5$: Cosets and Lagrange's Theorem: Example $5.2$




