# 

Source: https://proofwiki.org/wiki/Cosecant_of_i/Proof_2

Theorem
$\csc i = \paren {\dfrac {2 e} {1 - e^2} } i$


Proof













\(\ds \csc i\)

\(=\)







\(\ds -i \csch 1\)





Hyperbolic Cosecant in terms of Cosecant














\(\ds \)

\(=\)







\(\ds -\paren {\frac 2 {e^1 - e^{-1} } } i\)





Definition of Hyperbolic Cosecant














\(\ds \)

\(=\)







\(\ds -\paren {\frac {2 e} {e^2 - 1} } i\)





multiplying denominator and numerator by $e$














\(\ds \)

\(=\)







\(\ds \paren {\frac {2 e} {1 - e^2} } i\)









$\blacksquare$





