# 

Source: https://proofwiki.org/wiki/Coset/Examples/Dihedral_Group_D3/Cosets_of_Subgroup_Generated_by_b/Right_Cosets

Examples of Right Cosets
Consider the dihedral group $D_3$.

$D_3 = \gen {a, b: a^3 = b^2 = e, a b = b a^{-1} }$

Let $H \subseteq D_3$ be defined as:

$H = \gen b$
where $\gen b$ denotes the subgroup generated by $b$.

As $b$ has order $2$, it follows that:

$\gen b = \set {e, b}$

The right cosets of $H$ are:














\(\ds H e\)

\(=\)







\(\ds \set {e, b}\)




















\(\ds \)

\(=\)







\(\ds H b\)




















\(\ds \)

\(=\)







\(\ds H\)
























\(\ds H a\)

\(=\)







\(\ds \set {a, a^2 b}\)




















\(\ds \)

\(=\)







\(\ds H a^2 b\)
























\(\ds H a^2\)

\(=\)







\(\ds \set {a^2, a b}\)




















\(\ds \)

\(=\)







\(\ds H a b\)











Proof
The Cayley table of $D_3$ is presented as:

$\begin{array}{c|cccccc}      & e     & a     & a^2   & b     & a b   & a^2 b \\ \hline e     & e     & a     & a^2   & b     & a b   & a^2 b \\ a     & a     & a^2   & e     & a b   & a^2 b & b     \\ a^2   & a^2   & e     & a     & a^2 b & b     & a b   \\ b     & b     & a^2 b & a b   & e     & a^2   & a     \\ a b   & a b   & b     & a^2 b & a     & e     & a^2   \\ a^2 b & a^2 b & a b   & b     & a^2   & a     & e     \\ \end{array}$

Thus:














\(\ds H\)

\(=\)







\(\ds \set {e, b} e\)




















\(\ds \)

\(=\)







\(\ds \set {e^2, b e}\)




















\(\ds \)

\(=\)







\(\ds \set {e, b}\)




















\(\ds \)

\(=\)







\(\ds H\)
























\(\ds H b\)

\(=\)







\(\ds \set {e, b} b\)




















\(\ds \)

\(=\)







\(\ds \set {e b, b^2}\)




















\(\ds \)

\(=\)







\(\ds \set {b, e}\)




















\(\ds \)

\(=\)







\(\ds H\)
























\(\ds H a\)

\(=\)







\(\ds \set {e, b} a\)




















\(\ds \)

\(=\)







\(\ds \set {e a, b a}\)




















\(\ds \)

\(=\)







\(\ds \set {a, a^2 b}\)
























\(\ds H a^2\)

\(=\)







\(\ds \set {e, b} a^2\)




















\(\ds \)

\(=\)







\(\ds \set {e a^2, b a^2}\)




















\(\ds \)

\(=\)







\(\ds \set {a^2, a b}\)
























\(\ds H a b\)

\(=\)







\(\ds \set {e, b} a b\)




















\(\ds \)

\(=\)







\(\ds \set {e a b, b a b}\)




















\(\ds \)

\(=\)







\(\ds \set {a b, a^2}\)




















\(\ds \)

\(=\)







\(\ds H a^2\)
























\(\ds H a^2 b\)

\(=\)







\(\ds \set {e, b} a^2 b\)




















\(\ds \)

\(=\)







\(\ds \set {e a^2 b, b a^2 b}\)




















\(\ds \)

\(=\)







\(\ds \set {a^2 b, a}\)




















\(\ds \)

\(=\)







\(\ds H a\)









$\blacksquare$


Sources
1996: John F. Humphreys: A Course in Group Theory ... (previous) ... (next): Chapter $5$: Cosets and Lagrange's Theorem: Proposition $5.15$




