# 

Source: https://proofwiki.org/wiki/Cosine_of_Angle_plus_Straight_Angle/Proof_3

Theorem
$\map \cos {x + \pi} = -\cos x$


Proof













\(\ds \map \cos {x + \pi}\)

\(=\)







\(\ds \frac 1 2 \paren {e^{i \paren {x + \pi} } + e^{-i \paren {x + \pi} } }\)





Euler's Cosine Identity














\(\ds \)

\(=\)







\(\ds \frac 1 2 \paren {e^{i x} e^{i \pi} + e^{-i x} e^{-i \pi} }\)





Exponential of Sum: Complex Numbers














\(\ds \)

\(=\)







\(\ds \frac 1 2 \paren {-e^{i x} - e^{-i x} }\)





Euler's Identity














\(\ds \)

\(=\)







\(\ds -\frac 1 2 \paren {e^{i x} + e^{-i x} }\)




















\(\ds \)

\(=\)







\(\ds -\cos x\)





Euler's Cosine Identity



$\blacksquare$





