# 

Source: https://proofwiki.org/wiki/Cosine_of_36_Degrees/Proof_1

Theorem
$\cos 36 \degrees = \cos \dfrac \pi 5 = \dfrac \phi 2 = \dfrac {1 + \sqrt 5} 4$
where $\phi$ denotes the golden mean.


Proof
Let $u = \cos 72 \degrees, v = \cos 36 \degrees$.
Recall from Cosine of Complement equals Sine that $\map \cos {\dfrac \pi 2 - \theta} = \sin \theta$
Therefore:














\(\ds \map \cos {90 \degrees - 18 \degrees}\)

\(=\)







\(\ds \map \sin {18 \degrees}\)














\(\ds \leadsto \ \ \)





\(\ds \map \cos {72 \degrees}\)

\(=\)







\(\ds \map \sin {18 \degrees}\)










Therefore:














\(\ds \cos 36 \degrees\)

\(=\)







\(\ds 1 - 2 \sin^2 18 \degrees\)





Double Angle Formula for Cosine: Corollary $2$








\(\ds \leadsto \ \ \)





\(\ds v\)

\(=\)







\(\ds 1 - 2 u^2\)





substituting for $u$ and $v$














\(\ds \cos 72 \degrees\)

\(=\)







\(\ds 2 \cos^2 36 \degrees - 1\)





Double Angle Formula for Cosine: Corollary $1$








\(\ds \leadsto \ \ \)





\(\ds u\)

\(=\)







\(\ds 2 v^2 - 1\)





substituting for $u$ and $v$








\(\ds \leadsto \ \ \)





\(\ds u + v\)

\(=\)







\(\ds 2 \paren {v^2 - u^2}\)




















\(\ds \)

\(=\)







\(\ds 2 \paren {v + u} \paren {v - u}\)














\(\ds \leadsto \ \ \)





\(\ds 1\)

\(=\)







\(\ds 2 \paren {v - u}\)





dividing both sides by $\paren {v + u}$














\(\ds \)

\(=\)







\(\ds 2 v - 4 v^2 + 2\)





substituting $u = 2 v^2 - 1$








\(\ds \leadsto \ \ \)





\(\ds \paren {2 v}^2\)

\(=\)







\(\ds 2 v + 1\)














\(\ds \leadsto \ \ \)





\(\ds 2 v\)

\(=\)







\(\ds \phi\)





Square of Golden Mean equals One plus Golden Mean



$\blacksquare$


Sources
1997: Donald E. Knuth: The Art of Computer Programming: Volume 1: Fundamental Algorithms (3rd ed.) ... (previous) ... (next): $\S 1.2.8$: Fibonacci Numbers: Exercise $19$




