# 

Source: https://proofwiki.org/wiki/Cosine_of_Sum/Proof_5

Theorem
$\map \cos {a + b} = \cos a \cos b - \sin a \sin b$


Proof


We begin by enclosing a right-angled triangle $BEF$ with hypotenuse $BF$ of length $1$, inside Rectangle $ABCD$.
Let $\angle EBF = a$ and $\angle ABE = b$.
Therefore:














\(\ds BF\)

\(=\)







\(\ds 1\)





Given














\(\ds BE\)

\(=\)







\(\ds \cos a\)





Definition of Cosine of Angle














\(\ds EF\)

\(=\)







\(\ds \sin a\)





Definition of Sine of Angle














\(\ds AB\)

\(=\)







\(\ds \cos a \cos b\)




















\(\ds AE\)

\(=\)







\(\ds \cos a \sin b\)




















\(\ds ED\)

\(=\)







\(\ds \sin a \cos b\)




















\(\ds DF\)

\(=\)







\(\ds \sin a \sin b\)




















\(\ds \map \cos {a + b }\)

\(=\)







\(\ds FC\)




















\(\ds \)

\(=\)







\(\ds AB - DF\)




















\(\ds \)

\(=\)







\(\ds \cos a \cos b - \sin a \sin b\)









$\blacksquare$





