# 

Source: https://proofwiki.org/wiki/Cotangent_of_i/Proof_2

Theorem
$\cot i = \paren {\dfrac {1 + e^2} {1 - e^2} } i$


Proof













\(\ds \cot i\)

\(=\)







\(\ds -i \coth 1\)





Hyperbolic Cotangent in terms of Cotangent














\(\ds \)

\(=\)







\(\ds -\paren {\frac {e^1 + e^{-1} } {e^1 - e^{-1} } } i\)





DefinitionÂ 1 of Hyperbolic Cotangent














\(\ds \)

\(=\)







\(\ds -\paren {\frac {e^2 + 1} {e^2 - 1} } i\)





multiplying denominator and numerator by $e$














\(\ds \)

\(=\)







\(\ds \paren {\frac {1 + e^2} {1 - e^2} } i\)









$\blacksquare$





