# 

Source: https://proofwiki.org/wiki/Cube_Number_as_Difference_between_Squares_of_Triangular_Numbers/Proof_2

Theorem
Let $n \in \Z_{>0}$ be a positive integer.
Then:

$n^3 = {T_n}^2 - {T_{n - 1} }^2$
where $T_n$ denotes the $n$th triangular number.


Proof













\(\ds n^3\)

\(=\)







\(\ds \sum_{k \mathop = 1}^n k^3 - \sum_{k \mathop = 1}^{n - 1} k^3\)




















\(\ds \)

\(=\)







\(\ds \paren {\frac {n^2 \paren {n + 1}^2} 4} - \paren {\frac {\paren {n - 1}^2 n^2} 4}\)





Sum of Sequence of Cubes














\(\ds \)

\(=\)







\(\ds \frac {n^2 \paren {\paren {n + 1}^2 - \paren {n - 1}^2} } 4\)




















\(\ds \)

\(=\)







\(\ds \paren {\frac {n \paren {n + 1} } 2}^2 - \paren {\frac {n \paren {n - 1} } 2}^2\)




















\(\ds \)

\(=\)







\(\ds {T_n}^2 - {T_{n - 1} }^2\)





Closed Form for Triangular Numbers



$\blacksquare$





