# 

Source: https://proofwiki.org/wiki/Cube_Number_as_Difference_between_Squares_of_Triangular_Numbers/Proof_1

Theorem
Let $n \in \Z_{>0}$ be a positive integer.
Then:

$n^3 = {T_n}^2 - {T_{n - 1} }^2$
where $T_n$ denotes the $n$th triangular number.


Proof













\(\ds {T_n}^2 - {T_{n - 1} }^2\)

\(=\)







\(\ds \paren {\frac {n \paren {n + 1} } 2}^2 - \paren {\frac {\paren {n - 1} n} 2}^2\)





Closed Form for Triangular Numbers














\(\ds \)

\(=\)







\(\ds \frac {\paren {n^2 + n}^2 - \paren {n^2 - n}^2} 4\)




















\(\ds \)

\(=\)







\(\ds \frac {\paren {n^4 + 2 n^3 + n^2} - \paren {n^4 - 2 n^3 + n^2} } 4\)




















\(\ds \)

\(=\)







\(\ds \frac {4 n^3} 4\)




















\(\ds \)

\(=\)







\(\ds n^3\)









$\blacksquare$





