# 

Source: https://proofwiki.org/wiki/Curved_Mirror_producing_Parallel_Rays_is_Paraboloid

Theorem
Let $M$ be a curved mirror embedded in a real cartesian $3$- space.
Let there be a source of light at the origin.
Let $M$ reflect the light in a beam parallel to the $x$-axis.

Then $M$ is the solid of revolution produced by rotating about the $x$-axis the parabola whose equation is:

$y^2 = 2 c x + c^2$


Proof
The mirror will have the shape of a surface of revolution generated by revolving a curve $APB$ in the cartesian plane around the $x$-axis.
Let $P = \tuple {x, y}$ be an arbitrary point on $APB$.




From the Law of Reflection:

$\alpha = \beta$
By the geometry of the situation:

$\phi = \beta$
$\theta = \alpha + \phi = 2 \beta$
By definition of tangent:

$\tan \theta = \dfrac y x$
and so:














\(\ds \tan \theta\)

\(=\)







\(\ds \tan 2 \beta\)




















\(\ds \)

\(=\)







\(\ds \dfrac {2 \tan \beta} {1 - \tan^2 \beta}\)





Double Angle Formula for Tangent








\(\ds \leadsto \ \ \)





\(\ds \frac y x\)

\(=\)







\(\ds \dfrac {2 \dfrac {\d y} {\d x} } {1 - \paren {\dfrac {\d y} {\d x} }^2}\)





Double Angle Formula for Tangent



Using the Quadratic Formula:

$\dfrac {\d y} {\d x} = \dfrac {-x \pm \sqrt {x^2 + y^2} \rd x} y$
which can be expressed as:

$x \rd x + y \rd y = \pm \sqrt {x^2 + y^2} \rd x$
Using Differential of Sum of Squares:

$\pm \dfrac {\map \d {x^2 + y^2} } {2 \sqrt {x^2 + y^2} } = \d x$
and so:

$\pm \sqrt {x^2 + y^2} = x + c$
Hence the result.
$\blacksquare$


Sources
1972: George F. Simmons: Differential Equations ... (previous) ... (next): $\S 2.9$: Integrating Factors: Example $2$




