# 

Source: https://proofwiki.org/wiki/De_Morgan%27s_Laws_(Logic)/Conjunction_of_Negations/Formulation_2/Reverse_Implication

Theorem
$\paren {\neg \paren {p \lor q} } \implies \paren {\neg p \land \neg q}$


Proof
By the tableau method of natural deduction:


$\vdash \paren {\neg \paren {p \lor q} } \implies \paren {\neg p \land \neg q} $


Line


Pool

Formula

Rule

Depends upon

Notes


1


1

$\neg \paren {p \lor q}$

Assumption

(None)




2


1

$\neg p \land \neg q$

Sequent Introduction

1

De Morgan's Laws (Logic): Conjunction of Negations: Formulation 1


3




$\paren {\neg \paren {p \lor q} } \implies \paren {\neg p \land \neg q}$

Rule of Implication: $\implies \II$

1 â€“ 2

Assumption 1 has been discharged
$\blacksquare$




