# 

Source: https://proofwiki.org/wiki/Derivative_of_Composite_Function/Examples/Exponential_of_3_x%5E2_%2B_4

Example of Derivative of Composite Function
$\map {\dfrac \d {\d x} } {e^{3 x^2 + 4} } = 6 x e^{3 x^2 + 4}$


Proof
Let $u = 3 x^2 + 4$.
Let $y = e^u$.
Thus we have:

$y = e^{3 x^2 + 4}$
and so:














\(\ds \dfrac {\d y} {\d x}\)

\(=\)







\(\ds \dfrac {\d y} {\d u} \dfrac {\d u} {\d x}\)





Derivative of Composite Function














\(\ds \)

\(=\)







\(\ds e^u \paren {\map {\dfrac \d {\d x} } {3 x^2} + \map {\dfrac \d {\d x} } 4}\)





Derivative of Exponential Function, Sum Rule for Derivatives














\(\ds \)

\(=\)







\(\ds e^u \paren {6 x}\)





Derivative of Exponential Function, Power Rule for Derivatives, Derivative of Constant














\(\ds \)

\(=\)







\(\ds 6 x e^{3 x^2 + 4}\)





simplification



$\blacksquare$


Sources
1953: L. Harwood Clarke: A Note Book in Pure Mathematics ... (previous) ... (next): $\text {II}$. Calculus: Differentiation: Exercises $\text {IX}$: $23$.




