# 

Source: https://proofwiki.org/wiki/Derivative_of_Cosecant_Function/Proof_1

Theorem
$\map {\dfrac \d {\d x} } {\csc x} = -\csc x \cot x$
where $\sin x \ne 0$.


Proof
From the definition of the cosecant function:

$\csc x = \dfrac 1 {\sin x}$
From Derivative of Sine Function:

$\map {\dfrac \d {\d x} } {\sin x} = \cos x$

Then:














\(\ds \map {\dfrac \d {\d x} } {\csc x}\)

\(=\)







\(\ds \cos x \frac {-1} {\sin^2 x}\)





Chain Rule for Derivatives














\(\ds \)

\(=\)







\(\ds \frac {-1} {\sin x} \frac {\cos x} {\sin x}\)




















\(\ds \)

\(=\)







\(\ds -\csc x \cot x\)





Definition of Real Cosecant Function and Definition of Real Cotangent Function



This is valid only when $\sin x \ne 0$.
$\blacksquare$





