# 

Source: https://proofwiki.org/wiki/Derivative_of_Composite_Function/Examples/(3x%2B1)%5E2

Example of Derivative of Composite Function
$\map {\dfrac \d {\d x} } {\paren {3 x + 1}^2} = 6 \paren {3 x + 1}$


Proof
Let $u = 3 x + 1$.
Let $y = u^2$.
Then we have:

$y = \paren {3 x + 1}^2$
and so:














\(\ds \dfrac {\d y} {\d x}\)

\(=\)







\(\ds \dfrac {\d y} {\d u} \dfrac {\d u} {\d x}\)





Derivative of Composite Function














\(\ds \)

\(=\)







\(\ds 2 u \cdot 3\)





Derivative of Square Function, Derivative of Identity Function: Corollary














\(\ds \)

\(=\)







\(\ds 6 \paren {3 x + 1}\)





simplification



$\blacksquare$


Sources
1998: David Nelson: The Penguin Dictionary of Mathematics (2nd ed.) ... (previous) ... (next): chain rule (for differentiation)
2008: David Nelson: The Penguin Dictionary of Mathematics (4th ed.) ... (previous) ... (next): chain rule (for differentiation)




