# 

Source: https://proofwiki.org/wiki/Derivative_of_Hyperbolic_Sine/Proof_1

Theorem
$\map {\dfrac \d {\d x} } {\sinh x} = \cosh x$


Proof













\(\ds \map {\frac \d {\d x} } {\sinh x}\)

\(=\)







\(\ds \map {\frac \d {\d x} } {\dfrac {e^x - e ^{-x} } 2}\)





Definition of Hyperbolic Sine














\(\ds \)

\(=\)







\(\ds \frac 1 2 \paren {\map {\frac \d {\d x} } {e^x} - \map {\frac \d {\d x} } {e^{-x} } }\)





Linear Combination of Derivatives














\(\ds \)

\(=\)







\(\ds \frac 1 2 \paren {e^x - \paren {-e^{-x} } }\)





Derivative of Exponential Function, Chain Rule for Derivatives














\(\ds \)

\(=\)







\(\ds \frac {e^x + e^{-x} } 2\)





simplification














\(\ds \)

\(=\)







\(\ds \cosh x\)





Definition of Hyperbolic Cosine



$\blacksquare$





