# 

Source: https://proofwiki.org/wiki/Derivative_of_Composite_Function/Examples/Reciprocal_of_(2x%2B1)%5E3

Example of Derivative of Composite Function
$\map {\dfrac \d {\d x} } {\dfrac 1 {\paren {2 x + 1}^3} } = -\dfrac 6 {\paren {2 x + 1}^4}$


Proof
Let $u = 2 x + 1$.
Let $y = u^{-3}$.
Then we have:

$y = \paren {2 x + 1}^{-3}$
and so:














\(\ds \dfrac {\d y} {\d x}\)

\(=\)







\(\ds \dfrac {\d y} {\d u} \dfrac {\d u} {\d x}\)





Derivative of Composite Function














\(\ds \)

\(=\)







\(\ds 2 \cdot \paren {-3} \paren {2 x + 1}^{-4}\)





Power Rule for Derivatives, Derivative of Identity Function: Corollary














\(\ds \)

\(=\)







\(\ds -\dfrac 6 {\paren {2 x + 1}^4}\)





simplification



$\blacksquare$


Sources
1953: L. Harwood Clarke: A Note Book in Pure Mathematics ... (previous) ... (next): $\text {II}$. Calculus: Differentiation: Exercises $\text {IX}$: $4$.




