# 

Source: https://proofwiki.org/wiki/Derivative_of_Composite_Function/Examples/Root_of_x%5E2_%2B_x_%2B_1

Example of Derivative of Composite Function
$\map {\dfrac \d {\d x} } {\sqrt {x^2 + x + 1} } = \dfrac {2 x + 1} {2 \sqrt {x^2 + x + 1} }$


Proof
Let $u = x^2 + x + 1$.
Let $y = u^{1/2}$.
Then we have:

$y = \paren {x^2 + x + 1}^{1/2}$
and so:














\(\ds \dfrac {\d y} {\d x}\)

\(=\)







\(\ds \dfrac {\d y} {\d u} \dfrac {\d u} {\d x}\)





Derivative of Composite Function














\(\ds \)

\(=\)







\(\ds \dfrac 1 2 \paren {x^2 + x + 1}^{-1/2} \cdot \paren {2 x + 1}\)





Power Rule for Derivatives














\(\ds \)

\(=\)







\(\ds \dfrac {2 x + 1} {2 \sqrt {x^2 + x + 1} }\)





simplification



$\blacksquare$


Sources
1953: L. Harwood Clarke: A Note Book in Pure Mathematics ... (previous) ... (next): $\text {II}$. Calculus: Differentiation: Exercises $\text {IX}$: $5$.




