# 

Source: https://proofwiki.org/wiki/Derivative_of_Composite_Function/Examples/Logarithm_of_Cosecant_of_x

Example of Derivative of Composite Function
$\map {\dfrac \d {\d x} } {\ln \cosec x} = -\cot x$


Proof
Let $u = \cosec x$.
Let $y = \ln u$.
Thus we have:

$y = \ln \cosec x$
and so:














\(\ds \dfrac {\d y} {\d x}\)

\(=\)







\(\ds \dfrac {\d y} {\d u} \dfrac {\d u} {\d x}\)





Derivative of Composite Function














\(\ds \)

\(=\)







\(\ds \dfrac 1 u \paren {-\cosec x \cot x}\)





Derivative of Cosecant Function, Derivative of Natural Logarithm














\(\ds \)

\(=\)







\(\ds \dfrac 1 {\cosec x} \paren {-\cosec x \cot x}\)





simplification














\(\ds \)

\(=\)







\(\ds -\cot x\)





simplification



$\blacksquare$


Sources
1953: L. Harwood Clarke: A Note Book in Pure Mathematics ... (previous) ... (next): $\text {II}$. Calculus: Differentiation: Exercises $\text {IX}$: $15$.




