# 

Source: https://proofwiki.org/wiki/Derivative_of_Exponential_Function/Proof_2

Theorem
Let $\exp$ be the exponential function.
Then:

$\map {\dfrac \d {\d x} } {\exp x} = \exp x$


Proof
We use the fact that the exponential function is the inverse of the natural logarithm function:

$y = e^x \iff x = \ln y$













\(\ds \dfrac {\d x} {\d y}\)

\(=\)







\(\ds \dfrac 1 y\)





Derivative of Natural Logarithm Function








\(\ds \leadsto \ \ \)





\(\ds \dfrac {\d y} {\d x}\)

\(=\)







\(\ds \dfrac 1 {1 / y}\)





Derivative of Inverse Function














\(\ds \)

\(=\)







\(\ds y\)




















\(\ds \)

\(=\)







\(\ds e^x\)









$\blacksquare$


Sources
1977: K.G. Binmore: Mathematical Analysis: A Straightforward Approach ... (previous) ... (next): $\S 14.4$




