# 

Source: https://proofwiki.org/wiki/Derivative_of_Exponential_at_Zero/Proof_3

Theorem
Let $\exp x$ be the exponential of $x$ for real $x$.

Then:

$\ds \lim_{x \mathop \to 0} \frac {\exp x - 1} x = 1$


Proof













\(\ds \frac {e^x - 1} x\)

\(=\)







\(\ds \frac {e^x - e^0} x\)





Exponential of Zero














\(\ds \)

\(\to\)







\(\ds \valueat {\dfrac \d {\d x} e^x} {x \mathop = 0} {}\)





Definition of Derivative of Real Function at Point, as $x \to 0$














\(\ds \)

\(=\)







\(\ds \valueat {e^x} {x \mathop = 0} {}\)





Derivative of Exponential Function














\(\ds \)

\(=\)







\(\ds 1\)





Exponential of Zero



$\blacksquare$





