# 

Source: https://proofwiki.org/wiki/Derivative_of_Composite_Function/Examples/Reciprocal_of_Arctangent_of_x

Example of Derivative of Composite Function
$\map {\dfrac \d {\d x} } {\dfrac 1 {\arctan x} } = -\dfrac 1 {\paren {1 + x^2} \arctan^2 x}$


Proof
Let $u = \arctan x$.
Let $y = u^{-1}$.
Thus we have:

$y = \dfrac 1 {\arctan x}$
and so:














\(\ds \dfrac {\d y} {\d x}\)

\(=\)







\(\ds \dfrac {\d y} {\d u} \dfrac {\d u} {\d x}\)





Derivative of Composite Function














\(\ds \)

\(=\)







\(\ds \dfrac {-1} {u^2} \cdot \dfrac 1 {1 + x^2}\)





Power Rule for Derivatives, Derivative of Arctangent Function














\(\ds \)

\(=\)







\(\ds -\dfrac 1 {\paren {1 + x^2} \arctan^2 x}\)





simplification



$\blacksquare$


Sources
1953: L. Harwood Clarke: A Note Book in Pure Mathematics ... (previous) ... (next): $\text {II}$. Calculus: Differentiation: Exercises $\text {IX}$: $12$.




