# 

Source: https://proofwiki.org/wiki/Derivative_of_Logarithm_over_Power

Theorem
$\dfrac \d {\d x} \dfrac {\ln x} {x^n} = \dfrac {1 - n \ln x} {x^{n + 1} }$


Proof













\(\ds \dfrac \d {\d x} \dfrac {\ln x} {x^n}\)

\(=\)







\(\ds \dfrac \d {\d x} x^{-n} \ln x\)




















\(\ds \)

\(=\)







\(\ds \ln x \dfrac \d {\d x} x^{-n} + x^{-n} \dfrac \d {\d x} \ln x\)





Product Rule for Derivatives














\(\ds \)

\(=\)







\(\ds - n x^{-n - 1} \ln x + x^{-n} \dfrac 1 x\)





Primitive of Reciprocal, Primitive of Power














\(\ds \)

\(=\)







\(\ds -n x^{-n - 1} \ln x + x^{-n - 1}\)




















\(\ds \)

\(=\)







\(\ds \frac {1 - n \ln x} {x^{n + 1} }\)









$\blacksquare$





