# 

Source: https://proofwiki.org/wiki/Derivative_of_Tangent_Function/Proof_1

Theorem
$\map {\dfrac \d {\d x} } {\tan x} = \sec^2 x = \dfrac 1 {\cos^2 x}$
when $\cos x \ne 0$.


Proof
From the definition of the tangent function:

$\tan x = \dfrac {\sin x} {\cos x}$
From Derivative of Sine Function:

$\map {\dfrac \d {\d x} } {\sin x} = \cos x$
From Derivative of Cosine Function:

$\map {\dfrac \d {\d x} } {\cos x} = -\sin x$

Then:














\(\ds \map {\dfrac \d {\d x} } {\tan x}\)

\(=\)







\(\ds \frac {\cos x \cos x - \sin x \paren {-\sin x} } {\cos^2 x}\)





Quotient Rule for Derivatives














\(\ds \)

\(=\)







\(\ds \frac {\cos^2 x + \sin^2 x} {\cos^2 x}\)




















\(\ds \)

\(=\)







\(\ds \frac 1 {\cos^2 x}\)





Sum of Squares of Sine and Cosine



This is valid only when $\cos x \ne 0$.
The result follows from the Secant is Reciprocal of Cosine.
$\blacksquare$


Proof
1953: L. Harwood Clarke: A Note Book in Pure Mathematics ... (previous) ... (next): $\text {II}$. Calculus: Differentiation: Quotient




