# 

Source: https://proofwiki.org/wiki/Derivative_of_Reciprocal

Theorem
Let $f: \R_{\ne 0} \to \R$ be the reciprocal function defined as:

$\map f x = \dfrac 1 x$

Then its derivative is given by:

$\map {f'} x = -\dfrac 1 {x^2}$


Proof
We have:














\(\ds \dfrac 1 x\)

\(=\)







\(\ds x^{-1}\)














\(\ds \leadsto \ \ \)





\(\ds \map {\dfrac \d {\d x} } {\dfrac 1 x}\)

\(=\)







\(\ds \paren {-1} x^{-2}\)





Power Rule for Derivatives














\(\ds \)

\(=\)







\(\ds -\dfrac 1 {x^2}\)









$\blacksquare$


Sources
1989: Ephraim J. Borowski and Jonathan M. Borwein: Dictionary of Mathematics ... (previous) ... (next): Appendix $2$: Table of derivatives and integrals of common functions




