# 

Source: https://proofwiki.org/wiki/Difference_of_Fourth_Powers_of_Cosine_and_Sine/Proof_1

Theorem
$\sin^4 x - \cos^4 x = \sin^2 x - \cos^2 x$


Proof













\(\ds \sin^4 x - \cos^4 x\)

\(=\)







\(\ds \sin^2 x \left({1 - \cos^2 x}\right) - \cos^2 x \left({1 - \sin^2 x}\right)\)





Sum of Squares of Sine and Cosine














\(\ds \)

\(=\)







\(\ds \sin^2 x - \sin^2 x \ \cos^2 x - \cos^2 x + \sin^2 x \ \cos^2 x\)




















\(\ds \)

\(=\)







\(\ds \sin^2 x - \cos^2 x\)









$\blacksquare$





