# 

Source: https://proofwiki.org/wiki/Difference_of_Arccotangents

Theorem
$\arccot a - \arccot b = \arccot \dfrac {a b + 1} {a - b}$
where $\arccot$ denotes the arccotangent.


Proof
Let $x = \arccot a$ and $y = \arccot b$.
Then:




\(\text {(1)}: \quad\)









\(\ds \cot x\)

\(=\)







\(\ds a\)










\(\text {(2)}: \quad\)









\(\ds \cot y\)

\(=\)







\(\ds b\)




















\(\ds \map \cot {\arccot a - \arccot b}\)

\(=\)







\(\ds \map \cot {x - y}\)




















\(\ds \)

\(=\)







\(\ds \frac {\cot x \cot y + 1} {\cot x - \cot y}\)





Cotangent of Difference














\(\ds \)

\(=\)







\(\ds \frac {a - b} {1 + a b}\)





by $(1)$ and $(2)$








\(\ds \leadsto \ \ \)





\(\ds \arccot a - \arccot b\)

\(=\)







\(\ds \arccot \frac {a b + 1} {a - b}\)









$\blacksquare$


Also see
Sum of Arccotangents




