# 

Source: https://proofwiki.org/wiki/Difference_of_Squares_of_Sum_and_Difference/Algebraic_Proof

Theorem
$\forall a, b \in \R: \paren {a + b}^2 - \paren {a - b}^2 = 4 a b$


Proof













\(\ds \)

\(\)







\(\ds \left({a + b}\right)^2 - \left({a - b}\right)^2\)




















\(\ds \)

\(=\)







\(\ds \left({a^2 + 2 a b + b^2}\right) - \left({a^2 - 2 a b + b^2}\right)\)





Square of Sum and Square of Difference














\(\ds \)

\(=\)







\(\ds a^2 + 2 a b + b^2 - a^2 + 2 a b - b^2\)




















\(\ds \)

\(=\)







\(\ds 2 a b + 2 a b\)




















\(\ds \)

\(=\)







\(\ds 4 a b\)









$\blacksquare$





