# 

Source: https://proofwiki.org/wiki/Difference_of_Absolutely_Convergent_Series

Theorem
Let $\ds \sum_{n \mathop = 1}^\infty a_n$ and $\ds \sum_{n \mathop = 1}^\infty b_n$ be two real or complex series that are absolutely convergent.

Then the series $\ds \sum_{n \mathop = 1}^\infty \paren {a_n - b_n}$ is absolutely convergent, and:

$\ds \sum_{n \mathop = 1}^\infty \paren {a_n - b_n} = \sum_{n \mathop = 1}^\infty a_n - \sum_{n \mathop = 1}^\infty b_n$


Proof
The series $\ds \sum_{n \mathop = 1}^\infty \paren {-b_n}$ is absolutely convergent, as $\cmod {-b_n} = \cmod {b_n}$ for all $n \in \N$.
Then:














\(\ds \sum_{n \mathop = 1}^\infty a_n - \sum_{n \mathop = 1}^\infty b_n\)

\(=\)







\(\ds \sum_{n \mathop = 1}^\infty a_n + \paren {-1} \sum_{n \mathop = 1}^\infty b_n\)




















\(\ds \)

\(=\)







\(\ds \sum_{n \mathop = 1}^\infty a_n + \sum_{n \mathop = 1}^\infty \paren {-1} b_n\)





Manipulation of Absolutely Convergent Series: Scale Factor














\(\ds \)

\(=\)







\(\ds \sum_{n \mathop = 1}^\infty \paren {a_n - b_n}\)





Sum of Absolutely Convergent Series



$\blacksquare$


Sources
1960: Walter Ledermann: Complex Numbers ... (previous) ... (next): $\S 4.4$. Power Series




