# 

Source: https://proofwiki.org/wiki/Difference_of_Logarithms/Proof_1

Theorem
$\log_b x - \log_b y = \map {\log_b} {\dfrac x y}$


Proof













\(\ds \log_b x - \log_b y\)

\(=\)







\(\ds \map {\log_b} {b^{\log_b x - \log_b y} }\)





Definition of General Logarithm














\(\ds \)

\(=\)







\(\ds \map {\log_b} {\frac {\paren {b^{\log_b x} } } {\paren {b^{\log_b y} } } }\)





Quotient of Powers














\(\ds \)

\(=\)







\(\ds \map {\log_b} {\frac x y}\)





Definition of General Logarithm



$\blacksquare$





