# 

Source: https://proofwiki.org/wiki/Difference_of_Logarithms/Proof_2

Theorem
$\log_b x - \log_b y = \map {\log_b} {\dfrac x y}$


Proof













\(\ds \log_b x - \log_b y\)

\(=\)







\(\ds \frac {\log_e x} {\log_e b} - \frac {\log_e y} {\log_e b}\)





Change of Base of Logarithm














\(\ds \)

\(=\)







\(\ds \frac {\log_e x - \log_e y} {\log_e b}\)




















\(\ds \)

\(=\)







\(\ds \frac {\log_e \left({\frac x y}\right)} {\log_e b}\)





Difference of Logarithms: Proof for Natural Logarithm














\(\ds \)

\(=\)







\(\ds \log_b \left({\frac x y}\right)\)





Change of Base of Logarithm



$\blacksquare$





