# 

Source: https://proofwiki.org/wiki/Difference_of_Fourth_Powers_of_Secant_and_Tangent

Theorem
$\sec^4 x - \tan^4 x = \sec^2 x + \tan^2 x$


Proof













\(\ds \sec^4 x - \tan^4 x\)

\(=\)







\(\ds \sec^4 x - \frac {\sin^4 x} {\cos^4 x}\)





Tangent is Sine divided by Cosine














\(\ds \)

\(=\)







\(\ds \frac 1 {\cos^4 x} - \frac {\sin^4 x} {\cos^4 x}\)





Secant is Reciprocal of Cosine














\(\ds \)

\(=\)







\(\ds \frac {1 - \sin^4 x} {\cos^4x}\)




















\(\ds \)

\(=\)







\(\ds \frac {1 - \sin^2 x \paren {1 - \cos^2 x} } {\cos^2 x \paren {1 - \sin^2 x} }\)





Sum of Squares of Sine and Cosine














\(\ds \)

\(=\)







\(\ds \frac {1 - \sin^2 x + \sin^2 x \ \cos^2 x} {\cos^2 x - \sin^2 x \ \cos^2 x}\)




















\(\ds \)

\(=\)







\(\ds \frac {\cos^2 x + \sin^2 x \ \cos^2 x} {\cos^2 x - \sin^2 x \ \cos^2 x}\)





Sum of Squares of Sine and Cosine














\(\ds \)

\(=\)







\(\ds \frac {\cos^2 x \paren {1 + \sin^2 x} } {\cos^2 x \paren {1 - \sin^2 x} }\)




















\(\ds \)

\(=\)







\(\ds \frac {1 + \sin^2 x} {1 - \sin^2 x}\)




















\(\ds \)

\(=\)







\(\ds \frac {1 + \sin^2 x} {\cos^2 x}\)





Sum of Squares of Sine and Cosine














\(\ds \)

\(=\)







\(\ds \frac 1 {\cos^2 x} + \frac {\sin^2 x} {\cos^2 x}\)




















\(\ds \)

\(=\)







\(\ds \frac 1 {\cos^2 x} x + \tan^2 x\)





Tangent is Sine divided by Cosine














\(\ds \)

\(=\)







\(\ds \sec^2 x + \tan^2 x\)





Secant is Reciprocal of Cosine



$\blacksquare$





