# 

Source: https://proofwiki.org/wiki/Difference_of_Arctangents/Proof

Theorem
Let $\arctan a - \arctan b \in \openint {-\dfrac \pi 2} {\dfrac \pi 2}$ 
Then:

$\arctan a - \arctan b = \arctan \dfrac {a - b} {1 + a b}$
where $\arctan$ denotes the arctangent.


Proof
Let $x = \arctan a$ and $y = \arctan b$.
Then:




\(\text {(1)}: \quad\)









\(\ds \tan x\)

\(=\)







\(\ds a\)










\(\text {(2)}: \quad\)









\(\ds \tan y\)

\(=\)







\(\ds b\)




















\(\ds \map \tan {\arctan a - \arctan b}\)

\(=\)







\(\ds \map \tan {x - y}\)




















\(\ds \)

\(=\)







\(\ds \frac {\tan x - \tan y} {1 + \tan x \tan y}\)





Tangent of Difference














\(\ds \)

\(=\)







\(\ds \frac {a - b} {1 + a b}\)





by $(1)$ and $(2)$








\(\ds \leadsto \ \ \)





\(\ds \arctan a - \arctan b\)

\(=\)







\(\ds \arctan \frac {a - b} {1 + a b}\)









$\blacksquare$


Sources
1953: L. Harwood Clarke: A Note Book in Pure Mathematics ... (previous) ... (next): $\text V$. Trigonometry: Inverse ratios




