# 

Source: https://proofwiki.org/wiki/Difference_of_Two_Fourth_Powers/Proof_2

Theorem
$x^4 - y^4 = \paren {x - y} \paren {x + y} \paren {x^2 + y^2}$


Proof













\(\ds x^4 - y^4\)

\(=\)







\(\ds \paren {x - y} \paren {x^3 + x^2 y + x y^2 + y^3}\)





Difference of Two Powers














\(\ds \)

\(=\)







\(\ds \paren {x - y} \paren {\paren {x^3 + y^3} + x y \paren {x + y} }\)





rearranging














\(\ds \)

\(=\)







\(\ds \paren {x - y} \paren {\paren {x + y} \paren {x^2 - x y + y^2} + x y \paren {x + y} }\)





Sum of Two Cubes














\(\ds \)

\(=\)







\(\ds \paren {x - y} \paren {x + y} \paren {\paren {x^2 - x y + y^2} + x y}\)





extracting common factor














\(\ds \)

\(=\)







\(\ds \paren {x - y} \paren {x + y} \paren {x^2 + y^2}\)





simplifying



$\blacksquare$





