# 

Source: https://proofwiki.org/wiki/Digamma_Function/Examples/Digamma_Function_of_Two

Example of Use of Recurrence Relation for Digamma Function
$\map \psi 2 = -\gamma + 1$


Proof













\(\ds \map \psi {z + 1}\)

\(=\)







\(\ds \map \psi z + \frac 1 z\)





Recurrence Relation for Digamma Function








\(\ds \leadsto \ \ \)





\(\ds \map \psi {1 + 1}\)

\(=\)







\(\ds \map \psi 1 + 1\)





$zÂ := 1$








\(\ds \leadsto \ \ \)





\(\ds \map \psi 2\)

\(=\)







\(\ds -\gamma + 1\)





Digamma Function of One



$\blacksquare$





