# 

Source: https://proofwiki.org/wiki/Digamma_Function_of_One_Third/Proof_2

Theorem
$\map \psi {\dfrac 1 3} = -\gamma - \dfrac 3 2 \ln 3 - \dfrac \pi {2 \sqrt 3}$


Proof













\(\ds \sum_{k \mathop = 1}^{n - 1} \map \psi {\frac k n}\)

\(=\)







\(\ds -\paren {n - 1} \gamma - n \ln n\)





Digamma Additive Formula: Corollary








\(\ds \leadsto \ \ \)





\(\ds \sum_{k \mathop = 1}^{3 - 1} \map \psi {\frac k 3}\)

\(=\)







\(\ds -\paren {3 - 1} \gamma - 3 \ln 3\)










\(\text {(1)}: \quad\)



\(\ds \leadsto \ \ \)





\(\ds \map \psi {\frac 1 3} + \map \psi {\frac 2 3}\)

\(=\)







\(\ds -2 \gamma - 3 \ln 3\)










\(\text {(2)}: \quad\)









\(\ds \map \psi {\frac 1 3} - \map \psi {\frac 2 3}\)

\(=\)







\(\ds -\pi \map \cot {\frac \pi 3}\)





Digamma Reflection Formula








\(\ds \leadsto \ \ \)





\(\ds 2 \map \psi {\frac 1 3}\)

\(=\)







\(\ds -2 \gamma - 3 \ln 3 - \pi \map \cot {\frac \pi 3}\)





adding lines $1$ and $2$








\(\ds \leadsto \ \ \)





\(\ds \map \psi {\frac 1 3}\)

\(=\)







\(\ds -\gamma - \dfrac 3 2 \ln 3 - \dfrac \pi {2 \sqrt 3}\)





dividing by $2$ and Cotangent of $60 \degrees$



$\blacksquare$





