# 

Source: https://proofwiki.org/wiki/Double_Angle_Formulas/Hyperbolic_Sine/Proof_3

Theorem
$\sinh 2 x = 2 \sinh x \cosh x$


Proof













\(\ds \sinh 2 x\)

\(=\)







\(\ds -i \sin 2 i x\)





Hyperbolic Sine in terms of Sine














\(\ds \)

\(=\)







\(\ds -2 i \sin i x \cos i x\)





Double Angle Formula for Sine














\(\ds \)

\(=\)







\(\ds 2 \sinh x \cosh x\)





Hyperbolic Sine in terms of Sine, Hyperbolic Cosine in terms of Cosine



$\blacksquare$





