# 

Source: https://proofwiki.org/wiki/Double_Negation/Double_Negation_Introduction/Sequent_Form/Formulation_2

Theorem
$\vdash p \implies \neg \neg p$


Proof
By the tableau method of natural deduction:


$\vdash p \implies \neg \neg p$


Line


Pool

Formula

Rule

Depends upon

Notes


1


1

$p$

Assumption

(None)




2


1

$\neg \neg p$

Double Negation Introduction: $\neg \neg \II$

1




3




$p \implies \neg \neg p$

Rule of Implication: $\implies \II$

1 – 2

Assumption 1 has been discharged
$\blacksquare$


Sources
1959: A.H. Basson and D.J. O'Connor: Introduction to Symbolic Logic (3rd ed.) ... (previous) ... (next): $\S 4.7$: The Derivation of Formulae: $D \, 15$
1964: Donald Kalish and Richard Montague: Logic: Techniques of Formal Reasoning ... (previous) ... (next): $\text{I}$: 'NOT' and 'IF': $\S 5$: Theorem $\text{T12}$
1965: E.J. Lemmon: Beginning Logic ... (previous) ... (next): Chapter $2$: The Propositional Calculus $2$: $2$: Theorems and Derived Rules: Theorem $39$




