# 

Source: https://proofwiki.org/wiki/Double_Angle_Formulas/Hyperbolic_Sine/Proof_2

Theorem
$\sinh 2 x = 2 \sinh x \cosh x$


Proof













\(\ds \sinh 2 x\)

\(=\)







\(\ds \frac 1 2 \paren {e^{2 x} - e^{-2 x} }\)





Definition of Hyperbolic Sine














\(\ds \)

\(=\)







\(\ds \frac 1 2 \paren {e^x + e^{-x} } \paren {e^x - e^{-x} }\)





Difference of Two Squares














\(\ds \)

\(=\)







\(\ds 2 \paren {\frac{e^x + e^{-x} } 2 \cdot \frac {e^x - e^{-x} } 2}\)




















\(\ds \)

\(=\)







\(\ds 2 \sinh x \cosh x\)





Definition of Hyperbolic Sine, Definition of Hyperbolic Cosine



$\blacksquare$





