# 

Source: https://proofwiki.org/wiki/Elementary_Symmetric_Function/Examples/m_%3D_1

Example of Elementary Symmetric Function: $m = 1$
Let $e_1 \left({\left\{ {x_1, x_2, \ldots, x_n}\right\} }\right)$ be an elementary symmetric function in $n$ variables of degree $1$.

Then:














\(\ds e_1 \left({\left\{ {x_1, x_2, \ldots, x_n}\right\} }\right)\)

\(=\)







\(\ds x_1 + x_2 + \cdots + x_n\)











Proof
By definition:














\(\ds e_1 \left({\left\{ {x_1, x_2, \ldots, x_n}\right\} }\right)\)

\(=\)







\(\ds \sum_{1 \mathop \le j_1 \mathop \le n} \left({\prod_{i \mathop = 1}^1 x_{j_i} }\right)\)




















\(\ds \)

\(=\)







\(\ds \sum_{1 \mathop \le j_1 \mathop \le n} x_{j_1}\)




















\(\ds \)

\(=\)







\(\ds \sum_{j \mathop = 1}^n x_j\)




















\(\ds \)

\(=\)







\(\ds x_1 + x_2 + \cdots + x_n\)









$\blacksquare$





