# 

Source: https://proofwiki.org/wiki/Elementary_Symmetric_Function/Examples/m_%3D_2

Example of Elementary Symmetric Function: $m = 2$
Let $e_2 \left({\left\{ {x_1, x_2, \ldots, x_n}\right\} }\right)$ be an elementary symmetric function in $n$ variables of degree $2$.

Then:














\(\ds e_2 \left({\left\{ {x_1, x_2, \ldots, x_n}\right\} }\right)\)

\(=\)







\(\ds x_1 x_2 + x_1 x_3 + \cdots + x_1 x_n\)




















\(\ds \)

\(\)





\(\, \ds + \, \)

\(\ds x_2 x_3 + \cdots + x_2 x_n\)




















\(\ds \)

\(\)





\(\, \ds + \, \)

\(\ds \cdots\)




















\(\ds \)

\(\)





\(\, \ds + \, \)

\(\ds x_{n - 1} x_n\)











Proof
By definition:














\(\ds e_2 \left({\left\{ {x_1, x_2, \ldots, x_n}\right\} }\right)\)

\(=\)







\(\ds \sum_{1 \mathop \le j_1 < j_2 \mathop \le n} \left({\prod_{i \mathop = 1}^2 x_{j_i} }\right)\)




















\(\ds \)

\(=\)







\(\ds \sum_{1 \mathop \le j_1 < j_2 \mathop \le n} x_{j_1} x_{j_2}\)




















\(\ds \)

\(=\)







\(\ds x_1 x_2 + x_1 x_3 + \cdots + x_1 x_n\)




















\(\ds \)

\(\)





\(\, \ds + \, \)

\(\ds x_2 x_3 + \cdots + x_2 x_n\)




















\(\ds \)

\(\)





\(\, \ds + \, \)

\(\ds \cdots\)




















\(\ds \)

\(\)





\(\, \ds + \, \)

\(\ds x_{n - 1} x_n\)









$\blacksquare$





