# 

Source: https://proofwiki.org/wiki/Equation_of_Straight_Line_in_Plane/Two-Intercept_Form/Proof_1

Theorem
Let $\LL$ be a straight line which intercepts the $x$-axis and $y$-axis respectively at $\tuple {a, 0}$ and $\tuple {0, b}$, where $a b \ne 0$.

Then $\LL$ can be described by the equation:

$\dfrac x a + \dfrac y b = 1$


Proof


From the General Equation of Straight Line in Plane, $\LL$ can be expressed in the form:

$(1): \quad \alpha_1 x + \alpha_2 y = \beta$
where $\alpha_1, \alpha_2, \beta \in \R$ are given, and not both $\alpha_1, \alpha_2$ are zero.

Substituting for the two points whose coordinates we know about:










\(\ds x = a, y = 0: \, \)



\(\ds \alpha_1 \times a + \alpha_2 \times 0\)

\(=\)







\(\ds \beta\)














\(\ds \leadsto \ \ \)





\(\ds \alpha_1\)

\(=\)







\(\ds \dfrac \beta a\)









and: 










\(\ds x = 0, y = b: \, \)



\(\ds \alpha_1 \times 0 + \alpha_2 \times b\)

\(=\)







\(\ds \beta\)














\(\ds \leadsto \ \ \)





\(\ds \alpha_2\)

\(=\)







\(\ds \dfrac \beta b\)









We know that $\beta \ne 0$ because none of $a, b, \alpha_1, \alpha_2$ are equal to $0$.

Hence:














\(\ds \dfrac \beta a x + \dfrac \beta b y\)

\(=\)







\(\ds \beta\)





substituting for $\alpha_1$ and $\alpha_2$ in $(1)$








\(\ds \leadsto \ \ \)





\(\ds \dfrac x a + \dfrac y b\)

\(=\)







\(\ds 1\)





dividing both sides by $\beta$



$\blacksquare$





