# 

Source: https://proofwiki.org/wiki/Equation_of_Straight_Line_in_Plane/Two-Point_Form/Parametric_Form

Theorem
Let $\LL$ be a straight line embedded in a cartesian plane, given in two-point form as:

$\dfrac {x - x_1} {x_2 - x_1} = \dfrac {y - y_1} {y_2 - y_1}$

Then $\LL$ can be expressed by the parametric equations:

$\begin {cases} x = x_1 + t \paren {x_2 - x_1} \\ y = y_1 + t \paren {y_2 - y_1} \end {cases}$


Proof
Let $P = \tuple {x, y}$ be an arbitrary point on $\LL$.
Let $t = \dfrac {x - x_1} {x_2 - x_1} = \dfrac {y - y_1} {y_2 - y_1}$.

We then have:














\(\ds t\)

\(=\)







\(\ds \dfrac {x - x_1} {x_2 - x_1}\)














\(\ds \leadsto \ \ \)





\(\ds x - x_1\)

\(=\)







\(\ds t \paren {x_2 - x_1}\)














\(\ds \leadsto \ \ \)





\(\ds x\)

\(=\)







\(\ds x_1 + t \paren {x_2 - x_1}\)






















\(\ds t\)

\(=\)







\(\ds \dfrac {y - y_1} {y_2 - y_1}\)














\(\ds \leadsto \ \ \)





\(\ds y - y_1\)

\(=\)







\(\ds t \paren {y_2 - y_1}\)














\(\ds \leadsto \ \ \)





\(\ds y\)

\(=\)







\(\ds y_1 + t \paren {y_2 - y_1}\)









The result follows.
$\blacksquare$


Sources
1933: D.M.Y. Sommerville: Analytical Conics (3rd ed.) ... (previous) ... (next): Chapter $\text {II}$. The Straight Line: $4$. Special forms of the equation of a straight line: $(3)$ Line through two points




