# 

Source: https://proofwiki.org/wiki/Equation_of_Straight_Line_through_Intersection_of_Two_Straight_Lines



Theorem
Let $\LL_1$ and $\LL_2$ be straight lines embedded in a cartesian plane $\CC$, expressed using the general equations:






\(\ds \LL_1: \ \ \)







\(\ds l_1 x + m_1 y + n_1\)

\(=\)







\(\ds 0\)












\(\ds \LL_2: \ \ \)







\(\ds l_2 x + m_2 y + n_2\)

\(=\)







\(\ds 0\)










Let $\LL_3$ be a third straight line embedded in $\CC$, passing through the point of intersection of $\LL_1$ and $\LL_2$.

$\LL_3$ can be expressed using the general equation:

$(1): \quad \paren {l_1 x + m_1 y + n_1} - k \paren {l_2 x + m_2 y + n_2} = 0$


Proof
Let $P = \tuple {x, y}$ be the point of intersection of $\LL_1$ and $\LL_2$.
We have that:














\(\ds l_1 x + m_1 y + n_1\)

\(=\)







\(\ds 0\)




















\(\ds l_2 x + m_2 y + n_2\)

\(=\)







\(\ds 0\)














\(\ds \leadsto \ \ \)





\(\ds k \paren {l_2 x + m_2 y + n_2}\)

\(=\)







\(\ds 0\)














\(\ds \leadsto \ \ \)





\(\ds \paren {l_1 x + m_1 y + n_1} - k \paren {l_2 x + m_2 y + n_2}\)

\(=\)







\(\ds 0\)









and so equation $(1)$:

$\paren {l_1 x + m_1 y + n_1} - k \paren {l_2 x + m_2 y + n_2} = 0$
is satisfied by the point $P$.

Then:














\(\ds \paren {l_1 x + m_1 y + n_1} - k \paren {l_2 x + m_2 y + n_2}\)

\(=\)







\(\ds 0\)














\(\ds \leadsto \ \ \)





\(\ds \paren {l_1 - k l_2} x + \paren {m_1 - k m_2} y + \paren {n_1 - k n_2}\)

\(=\)







\(\ds 0\)










Each of $l_1 - k l_2$, $m_1 - k m_2$ and $n_1 - k n_2$ is a real number.
Hence $(1)$ is the equation of a straight line.
$\blacksquare$


Also presented as
This result can also be conveniently presented as follows:
Let $u = l_1 x + m_1 y + n_1$.
Let $v = l_2 x + m_2 y + n_2$.

Let $\LL_1$ be defined by the equation $u = 0$.
Let $\LL_2$ be defined by the equation $v = 0$.

Then the equation of the straight line passing through the point of intersection of $\LL_1$ and $\LL_2$ can be written as:

$u - k v = 0$


Sources
1933: D.M.Y. Sommerville: Analytical Conics (3rd ed.) ... (previous) ... (next): Chapter $\text {II}$. The Straight Line: $10$. Equation of a straight line through the intersection of two given lines




