# 

Source: https://proofwiki.org/wiki/Equivalence_of_Definitions_of_Folium_of_Descartes



Theorem
The following definitions of the concept of Folium of Descartes are equivalent:

Cartesian Form
The folium of Descartes is the locus of the equation:

$x^3 + y^3 - 3 a x y = 0$
Parametric Form
The folium of Descartes is the locus of the equation given in parametric form as:

$\begin {cases} x = \dfrac {3 a t} {1 + t^3} \\ y = \dfrac {3 a t^2} {1 + t^3} \end {cases}$


Proof
Let $F$ be a folium of Descartes expressed in parametric form.
Then by definition:
The folium of Descartes is the locus of the equation given in parametric form as:

$\begin {cases} x = \dfrac {3 a t} {1 + t^3} \\ y = \dfrac {3 a t^2} {1 + t^3} \end {cases}$

Hence:














\(\ds x^3 + y^3\)

\(=\)







\(\ds \dfrac {\paren {3 a t}^3} {\paren {1 + t^3}^3} + \dfrac {\paren {3 a t^2}^3} {\paren {1 + t^3}^3}\)




















\(\ds \)

\(=\)







\(\ds \dfrac {\paren {3 a t}^3 \paren {1 + t^3} } {\paren {1 + t^3}^3}\)




















\(\ds \)

\(=\)







\(\ds \dfrac {3 a \paren {3 a t} \paren {3 a t^2} } {\paren {1 + t^3}^2}\)




















\(\ds \)

\(=\)







\(\ds 3 a \dfrac {3 a t} {1 + t^3} \dfrac {3 a t^2} {1 + t^3}\)




















\(\ds \)

\(=\)







\(\ds 3 a x y\)









Thus $F$ is a folium of Descartes expressed in Cartesian form.
$\blacksquare$





