# 

Source: https://proofwiki.org/wiki/Equivalence_of_Definitions_of_Octagonal_Number



Theorem
The following definitions of the concept of Octagonal Number are equivalent:

Definition 1
$O_n = \begin {cases} 0 & : n = 0 \\ O_{n - 1} + 6 n - 5 & : n > 0 \end {cases}$
Definition 2
$\ds O_n = \sum_{i \mathop = 1}^n \paren {6 i - 5} = 1 + 7 + \cdots + \paren {6 \paren {n - 1} - 5} + \paren {6 n - 5}$
Definition 3
$\forall n \in \N: O_n = \map P {8, n} = \begin{cases} 0 & : n = 0 \\ \map P {8, n - 1} + 6 \paren {n - 1} + 1 & : n > 0 \end{cases}$
where $\map P {k, n}$ denotes the $k$-gonal numbers.


Proof
Definition 1 implies Definition 2
Let $O_n$ be an octagonal number by definition 1.
Let $n = 0$.
By definition:

$O_0 = 0$
By vacuous summation:

$\ds O_0 = \sum_{i \mathop = 1}^0 \paren {6 i - 5} = 0$

By definition of summation:














\(\ds O_{n - 1}\)

\(=\)







\(\ds \sum_{i \mathop = 1}^{n - 1} \paren {6 i - 5}\)




















\(\ds \)

\(=\)







\(\ds 1 + 7 + \cdots + 6 \paren {n - 1} - 5\)









and so:














\(\ds O_n\)

\(=\)







\(\ds O_{n - 1} + 6 n - 5\)




















\(\ds \)

\(=\)







\(\ds \sum_{i \mathop = 1}^n \paren {6 i - 5}\)




















\(\ds \)

\(=\)







\(\ds 1 + 7 + \cdots + \paren {6 n - 5}\)









Thus $O_n$ is an octagonal number by definition 2.
$\Box$


Definition 2 implies Definition 1
Let $O_n$ be an octagonal number by definition 2.
Then:














\(\ds O_n\)

\(=\)







\(\ds \sum_{i \mathop = 1}^n \paren {6 i - 5}\)




















\(\ds \)

\(=\)







\(\ds 1 + 7 + \cdots + \paren {6 \paren {n - 1} - 5} + \paren {6 n - 5}\)




















\(\ds \)

\(=\)







\(\ds O_{n - 1} + 6 n - 5\)










Then:

$\ds O_0 = \sum_{i \mathop = 1}^0 \paren {6 i - 5}$
is a vacuous summation and so:

$O_0 = 0$
Thus $O_n$ is an octagonal number by definition 1.
$\Box$


Definition 1 equivalent to Definition 3
We have by definition that $O_n = 0 = \map P {8, n}$.
Then:










\(\ds \forall n \in \N_{>0}: \, \)



\(\ds \map P {8, n}\)

\(=\)







\(\ds \map P {8, n - 1} + \paren {8 - 2} \paren {n - 1} + 1\)




















\(\ds \)

\(=\)







\(\ds \map P {8, n - 1} + 6 \paren {n - 1} + 1\)




















\(\ds \)

\(=\)







\(\ds \map P {8, n - 1} + 6 n - 6 + 1\)




















\(\ds \)

\(=\)







\(\ds \map P {8, n - 1} + 6 n - 5\)









Thus $\map P {8, n}$ and $O_n$ are generated by the same recurrence relation.
$\blacksquare$





