# 

Source: https://proofwiki.org/wiki/Equivalence_of_Definitions_of_Normal_Subset/2_implies_3

Theorem
Let $\left({G, \circ}\right)$ be a group.
Let $S \subseteq G$.

Let $S$ be a normal subset of $G$ by Definition 2.
Then $S$ is a normal subset of $G$ by Definition 3.
That is, if:

$\forall g \in G: g \circ S \circ g^{-1} = S$
or:

$\forall g \in G: g^{-1} \circ S \circ g = S$
then:

$\forall g \in G: g \circ S \circ g^{-1} \subseteq S$
and:

$\forall g \in G: g^{-1} \circ S \circ g \subseteq S$


Proof
We have that:

$\left({\forall g \in G: g \circ S \circ g^{-1} = S}\right) \iff \left({\forall g \in G: g^{-1} \circ S \circ g = S}\right)$
The result follows by definition of set equality.
$\blacksquare$





