# 

Source: https://proofwiki.org/wiki/Equivalence_of_Definitions_of_Pentagonal_Number



Theorem
The following definitions of the concept of Pentagonal Number are equivalent:

Definition 1
$P_n = \begin{cases}
0 & : n = 0 \\
P_{n - 1} + 3 n - 2 & : n > 0 \end{cases}$
Definition 2
$\ds P_n = \sum_{i \mathop = 1}^n \paren {3 i - 2} = 1 + 4 + \cdots + \paren {3 \paren {n - 1} - 2} + \paren {3 n - 2}$
Definition 3
$\forall n \in \N: P_n = \map P {5, n} = \begin {cases} 0 & : n = 0 \\ \map P {5, n - 1} + 3 \paren {n - 1} + 1 & : n > 0 \end {cases}$
where $\map P {k, n}$ denotes the $k$-gonal numbers.


Proof
Definition 1 implies Definition 2
Let $P_n$ be a pentagonal number by definition 1.
Let $n = 0$.
By definition:

$P_0 = 0$
By vacuous summation:

$P_0 = \ds \sum_{i \mathop = 1}^0 \paren {3 i - 2} = 0$

By definition of summation:














\(\ds P_{n - 1}\)

\(=\)







\(\ds \sum_{i \mathop = 1}^{n - 1} \paren {3 i - 2}\)




















\(\ds \)

\(=\)







\(\ds 1 + 4 + \cdots + 3 \paren {n - 1} - 2\)









and so:














\(\ds P_n\)

\(=\)







\(\ds P_{n - 1} + 3 n - 2\)




















\(\ds \)

\(=\)







\(\ds \sum_{i \mathop = 1}^n \paren {3 i - 2}\)




















\(\ds \)

\(=\)







\(\ds 1 + 4 + \cdots + 3 n - 2\)









Thus $P_n$ is a pentagonal number by definition 2.
$\Box$


Definition 2 implies Definition 1
Let $P_n$ be a pentagonal number by definition 2.
Then:














\(\ds P_n\)

\(=\)







\(\ds \sum_{i \mathop = 1}^n \paren {3 i - 2}\)




















\(\ds \)

\(=\)







\(\ds 1 + 4 + \cdots + \paren {3 \paren {n - 1} - 2} + \paren {3 n - 2}\)




















\(\ds \)

\(=\)







\(\ds P_{n - 1} + 3 n - 2\)










Then:

$P_0 = \ds \sum_{i \mathop = 1}^0 \paren {3 n - 2}$
is a vacuous summation and so:

$P_0 = 0$
Thus $P_n$ is a pentagonal number by definition 1.
$\Box$


Definition 1 equivalent to Definition 3
We have by definition that $P_n = 0 = \map P {5, n}$.
Then:










\(\ds \forall n \in \N_{>0}: \, \)



\(\ds \map P {5, n}\)

\(=\)







\(\ds \map P {5, n - 1} + \paren {5 - 2} \paren {n - 1} + 1\)




















\(\ds \)

\(=\)







\(\ds \map P {5, n - 1} + 3 \paren {n - 1} + 1\)




















\(\ds \)

\(=\)







\(\ds \map P {5, n - 1} + 3 n - 2\)









Thus $\map P {5, n}$ and $P_n$ are generated by the same recurrence relation.
$\blacksquare$





