# 

Source: https://proofwiki.org/wiki/Equivalence_of_Definitions_of_Heptagonal_Number



Theorem
The following definitions of the concept of Heptagonal Number are equivalent:

Definition 1
$H_n = \begin{cases}
0 & : n = 0 \\
H_{n - 1} + 5 n - 4 & : n > 0 \end{cases}$

Definition 2
$\ds H_n = \sum_{i \mathop = 1}^n \paren {5 i - 4} = 1 + 6 + \cdots + \paren {5 \paren {n - 1} - 4} + \paren {5 n - 4}$
Definition 3
$\forall n \in \N: H_n = \map P {7, n} = \begin{cases} 0 & : n = 0 \\ \map P {7, n - 1} + 5 \paren {n - 1} + 1 & : n > 0 \end{cases}$
where $\map P {k, n}$ denotes the $k$-gonal numbers.


Proof
Definition 1 implies Definition 2
Let $H_n$ be a heptagonal number by definition 1.
Let $n = 0$.
By definition:

$H_0 = 0$
By vacuous summation:

$\ds H_0 = \sum_{i \mathop = 1}^0 \paren {5 i - 4} = 0$

By definition of summation:














\(\ds H_{n - 1}\)

\(=\)







\(\ds \sum_{i \mathop = 1}^{n - 1} \paren {5 i - 4}\)




















\(\ds \)

\(=\)







\(\ds 1 + 6 + \cdots + 5 \paren {n - 1} + 4\)









and so:














\(\ds H_n\)

\(=\)







\(\ds H_{n - 1} + 5 n - 4\)




















\(\ds \)

\(=\)







\(\ds \sum_{i \mathop = 1}^n \paren {5 n - 4}\)




















\(\ds \)

\(=\)







\(\ds 1 + 6 + \cdots + 5 n - 4\)









Thus $H_n$ is a heptagonal number by definition 2.
$\Box$


Definition 2 implies Definition 1
Let $H_n$ be a heptagonal number by definition 2.
Then:














\(\ds H_n\)

\(=\)







\(\ds \sum_{i \mathop = 1}^n \paren {5 i - 4}\)




















\(\ds \)

\(=\)







\(\ds 1 + 6 + \cdots + \paren {5 \paren {n - 1} - 4} + \paren {5 n - 4}\)




















\(\ds \)

\(=\)







\(\ds H_{n - 1} + 5 n - 4\)










Then:

$\ds H_0 = \sum_{i \mathop = 1}^0 \paren {5 i - 4}$
is a vacuous summation and so:

$H_0 = 0$
Thus $H_n$ is a heptagonal number by definition 1.
$\Box$


Definition 1 equivalent to Definition 3
We have by definition that $H_0 = 0 = \map P {7, 0}$.
Then:










\(\ds \forall n \in \N_{>0}: \, \)



\(\ds \map P {7, n}\)

\(=\)







\(\ds \map P {7, n - 1} + \paren {7 - 2} \paren {n - 1} + 1\)




















\(\ds \)

\(=\)







\(\ds \map P {7, n - 1} + 5 \paren {n - 1} + 1\)




















\(\ds \)

\(=\)







\(\ds \map P {7, n - 1} + 5 n - 4\)









Thus $\map P {7, n}$ and $H_n$ are generated by the same recurrence relation.
$\blacksquare$





