# 

Source: https://proofwiki.org/wiki/Equivalence_of_Definitions_of_Triangular_Number



Theorem
The following definitions of the concept of Triangular Number are equivalent:

Definition 1
$T_n = \begin {cases} 0 & : n = 0 \\ n + T_{n - 1} & : n > 0 \end {cases}$
Definition 2
$\ds T_n = \sum_{i \mathop = 1}^n i = 1 + 2 + \cdots + \paren {n - 1} + n$
Definition 3
$\forall n \in \N: T_n = \map P {3, n} = \begin {cases} 0 & : n = 0 \\ \map P {3, n - 1} + \paren {n - 1} + 1 & : n > 0 \end {cases}$
where $\map P {k, n}$ denotes the $k$-gonal numbers.


Proof
Definition 1 implies Definition 2
Let $T_n$ be a triangular number by definition 1.
Let $n = 0$.
By definition:

$T_0 = 0$
By vacuous summation:

$\ds T_0 = \sum_{i \mathop = 1}^0 i = 0$

By definition of summation:

$\ds T_{n - 1} = \sum_{i \mathop = 1}^{n - 1} i = 1 + 2 + \cdots + \paren {n - 1}$
and so:














\(\ds T_n\)

\(=\)







\(\ds T_{n - 1} + n\)




















\(\ds \)

\(=\)







\(\ds \sum_{i \mathop = 1}^n i = 1 + 2 + \cdots + \paren {n - 1} + n\)









Thus $T_n$ is a triangular number by definition 2.
$\Box$


Definition 2 implies Definition 1
Let $T_n$ be a triangular number by definition 2.

$\ds T_n = \sum_{i \mathop = 1}^n i = 1 + 2 + \cdots + \paren {n - 1} + n$
Thus:

$\ds T_{n - 1} = \sum_{i \mathop = 1}^{n - 1} i = 1 + 2 + \cdots + \paren {n - 1}$
and so:

$T_n = T_{n - 1} + n$

Then:

$\ds T_0 = \sum_{i \mathop = 1}^0 i$
is a vacuous summation and so:

$T_0 = 0$
Thus $T_n$ is a triangular number by definition 1.
$\Box$


Definition 1 equivalent to Definition 3
We have by definition that $T_n = 0 = \map P {3, n}$.
Then:










\(\ds \forall n \in \N_{>0}: \, \)



\(\ds \map P {3, n}\)

\(=\)







\(\ds \map P {3, n - 1} + \paren {n - 1} + 1\)




















\(\ds \)

\(=\)







\(\ds \map P {3, n - 1} + n\)









Thus $\map P {3, n}$ and $T_n$ are generated by the same recurrence relation.
$\blacksquare$





