# 

Source: https://proofwiki.org/wiki/Equivalence_of_Definitions_of_Hyperbolic_Secant



Theorem
The following definitions of the concept of Hyperbolic Secant are equivalent:

Definition 1
The hyperbolic secant function is defined on the complex numbers as:

$\sech: X \to \C$:
$\forall z \in X: \sech z := \dfrac 2 {e^z + e^{-z} }$
where:

$X = \set {z: z \in \C, \ e^z + e^{-z} \ne 0}$
Definition 2
The hyperbolic secant function is defined on the complex numbers as:

$\sech: X \to \C$:
$\forall z \in X: \sech z := \dfrac 1 {\cosh z}$
where:

$\cosh$ is the hyperbolic cosine
$X = \set {z: z \in \C, \ \cosh z \ne 0}$


Proof









\(\ds \forall z \in \set {z \in \C: \ e^z + e^{-z} \ne 0}: \, \)



\(\ds \)

\(\)







\(\ds \frac 2 {e^z + e^{-z} }\)





Definition 1 of Hyperbolic Secant










\(\ds \forall z \in \set {z \in \C: \ \frac {e^z + e^{-z} } 2 \ne 0}: \, \)



\(\ds \)

\(=\)







\(\ds 1 / \frac {e^z + e^{-z} } 2\)
















\(\ds \forall z \in \set {z \in \C: \ \cosh z \ne 0}: \, \)



\(\ds \)

\(=\)







\(\ds 1 / \cosh z\)





Definition 2 of Hyperbolic Secant



$\blacksquare$





