# 

Source: https://proofwiki.org/wiki/Euclidean_Algorithm/Examples/9n%2B8_and_6n%2B5

Examples of Use of Euclidean Algorithm
The GCD of $9 n + 8$ and $6 n + 5$ is found to be:

$\gcd \set {9 n + 8, 6 n + 5} = 1$
Hence:

$2 \paren {9 n + 8} - 3 \paren {6 n + 5} = 1$


Proof



\(\text {(1)}: \quad\)









\(\ds 9 n + 8\)

\(=\)







\(\ds \paren {6 n + 5} + \paren {3 n + 3}\)










\(\text {(2)}: \quad\)









\(\ds 6 n + 5\)

\(=\)







\(\ds \paren {3 n + 3} + \paren {3 n + 2}\)










\(\text {(3)}: \quad\)









\(\ds 3 n + 3\)

\(=\)







\(\ds \paren {3 n + 2} + 1\)









Thus:

$\gcd \set {9 n + 8, 6 n + 5} = 1$

Then we have:














\(\ds 1\)

\(=\)







\(\ds \paren {3 n + 3} - \paren {3 n + 2}\)





from $(3)$














\(\ds \)

\(=\)







\(\ds \paren {3 n + 3} - \paren {\paren {6 n + 5} - \paren {3 n + 3} }\)





from $(2)$














\(\ds \)

\(=\)







\(\ds 2 \paren {3 n + 3} - \paren {6 n + 5}\)




















\(\ds \)

\(=\)







\(\ds 2 \paren {\paren {9 n + 8} - \paren {6 n + 5} } - \paren {6 n + 5}\)





from $(1)$














\(\ds \)

\(=\)







\(\ds 2 \paren {9 n + 8} - 3 \paren {6 n + 5}\)









$\blacksquare$


Sources
1978: Thomas A. Whitelaw: An Introduction to Abstract Algebra ... (previous) ... (next): Chapter $2$: Some Properties of $\Z$: Exercise $2.3$




