# 

Source: https://proofwiki.org/wiki/Euler_Triangle_Formula/Lemma_2/Proof_1

Lemma to Euler Triangle Formula


Let the bisector of angle $C$ of triangle $\triangle ABC$ be produced to the circumcircle at $P$.
Let $I$ be the incenter of $\triangle ABC$.
Then:

$AP = BP = IP$


Proof
Without loss of generality, it will be demonstrated that $BP = IP$.
Let $CP$ be the bisector of $\angle ACB$.

$\angle ACP$ and $\angle ICB$ both subtend $AP$.
Hence indirectly by the Inscribed Angle Theorem:

$\angle ACP = \angle ICB$
From Angles on Equal Arcs are Equal:

$\angle ACP = \angle ABP$
and so:

$\angle ABP = \angle ICB$
By the construction of the incircle, $IB$ is the bisector of $B$.
Then:

$\angle IBA = \angle IBC$
and so:














\(\ds \angle IBP\)

\(=\)







\(\ds \angle IBA + \angle ABP\)




















\(\ds \)

\(=\)







\(\ds \angle IBC + \angle ICB\)










By Sum of Angles of Triangle equals Two Right Angles:

$\angle CIB + \angle IBC + \angle ICB = \angle CIB + \angle PIB$
as $\angle CIB$ and $\angle PIB$ are supplementary.
Thus:














\(\ds \angle PIB\)

\(=\)







\(\ds \angle IBC + \angle ICB\)




















\(\ds \)

\(=\)







\(\ds \angle IBP\)









and from Triangle with Two Equal Angles is Isosceles:

$IP = BP$

The proof that $IP = AP$ follows the same lines.
$\blacksquare$





