# 

Source: https://proofwiki.org/wiki/Euler%27s_Cosine_Identity/Proof_2

Theorem
$\cos z = \dfrac {e^{i z} + e^{-i z} } 2$


Proof
Recall Euler's Formula:

$e^{i z} = \cos z + i \sin z$

Then, starting from the right hand side:














\(\ds \frac {e^{i z} + e^{-i z} } 2\)

\(=\)







\(\ds \frac {\cos z + i \sin z + \map \cos {-z} + i \map \sin {-z} } 2\)




















\(\ds \)

\(=\)







\(\ds \frac {\cos z + \map \cos {-z} } 2\)





Sine Function is Odd














\(\ds \)

\(=\)







\(\ds \frac {2 \cos z} 2\)





Cosine Function is Even














\(\ds \)

\(=\)







\(\ds \cos z\)









$\blacksquare$





