# 

Source: https://proofwiki.org/wiki/Even_Number_minus_Odd_Number_is_Odd



Theorem
In the words of Euclid:

If from an even number an odd number be subtracted, the remainder will be odd.
(The Elements: Book $\text{IX}$: Proposition $25$)


Proof
Let $a$ be even and $b$ be odd.
Then by definition of even number:

$\exists c \in \Z: a = 2 c$
and by definition of odd number:

$\exists d \in \Z: b = 2 d + 1$
So:














\(\ds a - b\)

\(=\)







\(\ds 2 c - \left({2 d + 1}\right)\)




















\(\ds \)

\(=\)







\(\ds 2 \left({c - d}\right) - 1\)




















\(\ds \)

\(=\)







\(\ds 2 \left({c - d - 1}\right) + 1\)









Hence the result by definition of odd number.
$\blacksquare$


Historical Note
This proof is Proposition $25$ of Book $\text{IX}$ of Euclid's The Elements.


Sources
1926: Sir Thomas L. Heath: Euclid: The Thirteen Books of The Elements: Volume 2 (2nd ed.) ... (previous) ... (next): Book $\text{IX}$. Propositions




