# 

Source: https://proofwiki.org/wiki/Even_Number_minus_Even_Number_is_Even



Theorem
In the words of Euclid:

If from an even number an even number be subtracted, the remainder will be even.
(The Elements: Book $\text{IX}$: Proposition $24$)


Proof
Let $a$ and $b$ be even numbers.
Then by definition of even number:

$\exists c \in \Z: a = 2 c$
$\exists d \in \Z: b = 2 d$
So:














\(\ds a - b\)

\(=\)







\(\ds 2 c - 2 d\)




















\(\ds \)

\(=\)







\(\ds 2 \left({c - d}\right)\)









Hence the result by definition of even number.
$\blacksquare$


Historical Note
This proof is Proposition $24$ of Book $\text{IX}$ of Euclid's The Elements.


Sources
1926: Sir Thomas L. Heath: Euclid: The Thirteen Books of The Elements: Volume 2 (2nd ed.) ... (previous) ... (next): Book $\text{IX}$. Propositions




