# 

Source: https://proofwiki.org/wiki/Evolute_of_Parabola

Theorem
The evolute of the parabola $y = x^2$ is the curve:

$27 X^2 = 16 \paren {Y - \dfrac 1 2}^3$


Proof
From Parametric Equations for Evolute: Formulation 1:

$\begin {cases}
X = x - \dfrac {y' \paren {1 + y'^2} } {y} \\
Y = y + \dfrac {1 + y'^2} {y}
\end{cases}$
where:

$\tuple {x, y}$ denotes the Cartesian coordinates of a general point on $C$
$\tuple {X, Y}$ denotes the Cartesian coordinates of a general point on the evolute of $C$
$y'$ and $y$ denote the derivative and second derivative respectively of $y$ with respect to $x$.

Thus we have:














\(\ds y'\)

\(=\)







\(\ds 2 x\)




















\(\ds y\)

\(=\)







\(\ds 2\)










and so:














\(\ds X\)

\(=\)







\(\ds x - \dfrac {2 x \paren {1 + \paren {2 x}^2} } 2\)




















\(\ds \)

\(=\)







\(\ds x - x - 4 x^3\)




















\(\ds \)

\(=\)







\(\ds -4 x^3\)










and:














\(\ds Y\)

\(=\)







\(\ds x^2 + \dfrac {1 + \paren {2 x}^2} 2\)




















\(\ds \)

\(=\)







\(\ds \frac {2 x^2 + 1 + 4 x^2} 2\)




















\(\ds \)

\(=\)







\(\ds \frac {6 x^2 + 1} 2\)










Then:














\(\ds Y\)

\(=\)







\(\ds \frac {6 \paren {-\frac X 4}^{2/3} + 1} 2\)





substituting for $X$














\(\ds Y\)

\(=\)







\(\ds 3 \paren {-\frac X 4}^{2/3} + \frac 1 2\)





substituting for $X$








\(\ds \leadsto \ \ \)





\(\ds \frac 1 3 \paren {Y - \frac 1 2}\)

\(=\)







\(\ds \paren {\frac {X^2} {16} }^{1/3}\)














\(\ds \leadsto \ \ \)





\(\ds 27 X^2\)

\(=\)







\(\ds 16 \paren {Y - \dfrac 1 2}^3\)










The parabola (blue) and its evolute (red) are illustrated below:


$\blacksquare$


Sources
1992: George F. Simmons: Calculus Gems ... (previous) ... (next): Chapter $\text {B}.23$: Evolutes and Involutes. The Evolute of a Cycloid: Example $1$




