# 

Source: https://proofwiki.org/wiki/Example:Antiassociative_Structure

Theorem
Let $\left({\R_{>0}, \circ}\right)$ be an algebraic structure where $\R_{>0}$ denotes the strictly positive real numbers.
Define:

$\forall x, y \in \R_{>0}: x \circ y = x y + y$

Then $\circ$ is antiassociative on $\R_{>0}$:

$\forall x, y, z \in \R_{>0}: \left({x \circ y}\right) \circ z \ne x \circ \left({y \circ z}\right)$


Proof
Let $a, b, c \in \R_{>0}$:
Then:














\(\ds a \circ \left({b \circ c}\right)\)

\(=\)







\(\ds a \circ \left({b c + c}\right)\)




















\(\ds \)

\(=\)







\(\ds a \left({b c + c}\right) + b c + c\)




















\(\ds \)

\(=\)







\(\ds a b c + a c + b c + c\)










and:














\(\ds \left({a \circ b}\right) \circ c\)

\(=\)







\(\ds \left({a b + b}\right)\circ c\)




















\(\ds \)

\(=\)







\(\ds \left({a b + b}\right)c + c\)




















\(\ds \)

\(=\)







\(\ds a b c + b c + c\)









As $ac \ne 0$:

$\forall x, y, z \in \R_{>0}: \left({x \circ y}\right) \circ z \ne x \circ \left({y \circ z}\right)$

Hence the result.
$\blacksquare$





