# 

Source: https://proofwiki.org/wiki/Factorial_as_Product_of_Two_Factorials/Examples/3

Example of Factorial as Product of Two Factorials
$5! = 4 \times 5 \times 6 = \dfrac {6!} {3!}$


Proof
We have that:














\(\ds 6!\)

\(=\)







\(\ds \paren {3!}!\)




















\(\ds \)

\(=\)







\(\ds 3! \paren {3! - 1}!\)




















\(\ds \)

\(=\)







\(\ds 3! \, 5!\)














\(\ds \leadsto \ \ \)





\(\ds 5!\)

\(=\)







\(\ds \dfrac {6!} {3!}\)




















\(\ds \)

\(=\)







\(\ds \dfrac {1 \times 2 \times 3 \times 4 \times 5 \times 6} {1 \times 2 \times 3}\)




















\(\ds \)

\(=\)







\(\ds 4 \times 5 \times 6\)









$\blacksquare$


Sources
1997: David Wells: Curious and Interesting Numbers (2nd ed.) ... (previous) ... (next): $120$




