# 

Source: https://proofwiki.org/wiki/Fallacy/Examples/Arbitrary_Example_1

Example of Fallacy













\(\ds x\)

\(\ge\)







\(\ds y\)





by hypothesis














\(\ds y\)

\(\ge\)







\(\ds z\)





by hypothesis








\(\ds \leadsto \ \ \)





\(\ds x\)

\(>\)







\(\ds z\)









is a fallacy.


Proof
Let $x = y = z = 1$.
Then:

$1 \ge 1$
which satisfies both $x \ge y$ and $y \ge z$, but it is not the case that:

$1 > 1$
Hence the given argument is a fallacy.
$\blacksquare$


Sources
2008: David Nelson: The Penguin Dictionary of Mathematics (4th ed.) ... (previous) ... (next): fallacy




