# 

Source: https://proofwiki.org/wiki/False_Statement_implies_Every_Statement/Formulation_1/Proof_1

Theorem













\(\ds \neg p\)

\(\)







\(\ds \)














\(\ds \vdash \ \ \)





\(\ds p \implies q\)

\(\)







\(\ds \)











Proof
By the tableau method of natural deduction:


$\neg p \vdash p \implies q$


Line


Pool

Formula

Rule

Depends upon

Notes


1


1

$\neg p$

Premise

(None)




2


1

$\neg p \lor q$

Rule of Addition: $\lor \II_1$

1




3


1

$p \implies q$

Sequent Introduction

2

Rule of Material Implication
$\blacksquare$


Sources
1965: E.J. Lemmon: Beginning Logic ... (previous) ... (next): Chapter $2$: The Propositional Calculus $2$: $2$: Theorems and Derived Rules: Theorem $51$




