# 

Source: https://proofwiki.org/wiki/Fermat_Number_whose_Index_is_Sum_of_Integers

Theorem
Let $F_n = 2^{\left({2^n}\right)} + 1$ be the $n$th Fermat number.
Let $k \in \Z_{>0}$.

Then:

$F_{n + k} - 1 = \left({F_n - 1}\right)^{2^k}$


Proof
By the definition of Fermat number














\(\ds F_{n + k} - 1\)

\(=\)







\(\ds 2^{2^{n + k} }\)





Definition of Fermat Number














\(\ds \)

\(=\)







\(\ds 2^{2^n 2^k}\)




















\(\ds \)

\(=\)







\(\ds \left({2^{2^n} }\right)^{2^k}\)




















\(\ds \)

\(=\)







\(\ds \left({F_n - 1}\right)^{2^k}\)





Definition of Fermat Number



$\blacksquare$


Sources
1982: P.M. Cohn: Algebra Volume 1 (2nd ed.) ... (previous) ... (next): $\S 2.4$: The rational numbers and some finite fields: Further Exercises $9$




