# 

Source: https://proofwiki.org/wiki/Fibonacci_Number_n%2B1_Minus_Golden_Mean_by_Fibonacci_Number_n/Proof_1

Theorem
$F_{n + 1} - \phi F_n = \hat \phi^n$
where:

$F_n$ denotes the $n$th Fibonacci number
$\phi$ denotes the golden mean.


Proof













\(\ds F_{n + 1} - \phi F_n\)

\(=\)







\(\ds \dfrac 1 {\sqrt 5} \paren {\phi^{n + 1} - \hat \phi^{n + 1} } - \dfrac \phi {\sqrt 5} \paren {\phi^n - \hat \phi^n}\)





Euler-Binet Formula














\(\ds \)

\(=\)







\(\ds \dfrac 1 {\sqrt 5} \paren {\phi^{n + 1} - \hat \phi^{n + 1} - \phi^{n + 1} + \phi \hat \phi^n}\)




















\(\ds \)

\(=\)







\(\ds \hat \phi^n \dfrac {\phi - \hat \phi} {\sqrt 5}\)




















\(\ds \)

\(=\)







\(\ds \hat \phi^n F_1\)





Euler-Binet Formula














\(\ds \)

\(=\)







\(\ds \hat \phi^n\)





Definition of Fibonacci Number: $F_1 = 1$



$\blacksquare$





