# 

Source: https://proofwiki.org/wiki/First_Order_ODE/(1_%2B_x%5E2)_y%27_%2B_x_y_%3D_0

Theorem
The first order ODE:

$\paren {1 + x^2} y' + x y = 0$
has the general solution:

$y = \dfrac C {\sqrt {1 + x^2} }$


Proof













\(\ds \paren {1 + x^2} \dfrac {\d y} {\d x}\)

\(=\)







\(\ds -x y\)














\(\ds \leadsto \ \ \)





\(\ds \int \frac {\d y} y\)

\(=\)







\(\ds -\int \frac {x \rd x} {1 + x^2}\)





Solution to Separable Differential Equation








\(\ds \leadsto \ \ \)





\(\ds \ln y\)

\(=\)







\(\ds -\frac 1 2 \, \map \ln {1 + x^2} + C\)





Primitive of $\dfrac x {x^2 + a^2}$








\(\ds \leadsto \ \ \)





\(\ds \ln y\)

\(=\)







\(\ds \ln \frac {C_1} {\sqrt {1 + x^2} }\)














\(\ds \leadsto \ \ \)





\(\ds y\)

\(=\)







\(\ds \frac C {\sqrt {1 + x^2} }\)









$\blacksquare$





