# 

Source: https://proofwiki.org/wiki/First_Order_ODE/x_dy_-_y_dx_%3D_(1_%2B_y%5E2)_dy

Theorem
The first order ODE:

$(1): \quad x \rd y - y \rd x = \paren {1 + y^2} \rd y$
has the general solution:

$\dfrac x y = \dfrac 1 y - y + C$


Proof
Rearranging, we have:

$\dfrac {y \rd x - x \rd y} {y^2} = -\paren {\dfrac 1 {y^2} + 1} \rd y$
From the Quotient Rule for Derivatives:

$\map \d {\dfrac x y} = \dfrac {y \rd x - x \rd y} {y^2}$
from which:

$\map \d {\dfrac x y} = -\paren {\dfrac 1 {y^2} + 1} \rd y$
Hence the result:

$\dfrac x y = \dfrac 1 y - y + C$
$\blacksquare$


Sources
1972: George F. Simmons: Differential Equations ... (previous) ... (next): $\S 2.9$: Integrating Factors: Problem $4 \ \text{(a)}$




