# 

Source: https://proofwiki.org/wiki/First_Order_ODE/y_dx_%2B_x_dy_%3D_0

Theorem
The first order ODE:

$(1): \quad y \rd x + x \rd y = 0$
has the general solution:

$x y = C$


Proof
$(1)$ can be expressed as:














\(\ds x \rd y\)

\(=\)







\(\ds -y \rd x\)














\(\ds \leadsto \ \ \)





\(\ds y\)

\(=\)







\(\ds C x^{-1}\)





First Order ODE: $x \rd y = k y \rd x$








\(\ds \leadsto \ \ \)





\(\ds x y\)

\(=\)







\(\ds C\)





multiplying through by $x$



$\blacksquare$





