# 

Source: https://proofwiki.org/wiki/First_Order_ODE/y_dx_-_x_dy_%3D_x_y%5E3_dy

Theorem
The first order ODE:

$(1): \quad y rd x - x \rd y = x y^3 \rd y$
has the general solution:

$\ln \dfrac x y = \dfrac {y^3} 3 + C$


Proof
Rearranging, we have:

$\dfrac {y \rd x - x \rd y} {x y} = y^2 \rd y$
From Differential of Logarithm of Quotient:

$\map \d {\ln \dfrac y x} = \dfrac {y \rd x - x \rd y} {x y}$
from which:

$\map \d {\ln \dfrac x y} = y^2 \rd y$
Hence the result:

$\ln \dfrac x y = \dfrac {y^3} 3 + C$
$\blacksquare$


Sources
1972: George F. Simmons: Differential Equations ... (previous) ... (next): $\S 2.9$: Integrating Factors: Problem $4 \ \text{(b)}$




