# 

Source: https://proofwiki.org/wiki/First_Order_ODE/dy_%3D_k_y_dx/Proof_3

Theorem
Let $k \in \R$ be a real number.
The first order ODE:

$\dfrac {\d y} {\d x} = k y$
has the general solution:

$y = C e^{k x}$


Proof













\(\ds \dfrac {\d y} {\d x}\)

\(=\)







\(\ds k y\)














\(\ds \leadsto \ \ \)





\(\ds \dfrac {\d y} {\d x} - k y\)

\(=\)







\(\ds 0\)














\(\ds \leadsto \ \ \)





\(\ds e^{-k x} \paren {\dfrac {\d y} {\d x} - k y}\)

\(=\)







\(\ds 0\)





Solution to Linear First Order Ordinary Differential Equation: $e^{\int -k \rd x} = e^{-k x}$








\(\ds \leadsto \ \ \)





\(\ds \map {\dfrac \d {\d x} } {y e^{-k x} }\)

\(=\)







\(\ds 0\)





Solution to Linear First Order Ordinary Differential Equation continued








\(\ds \leadsto \ \ \)





\(\ds y e^{-k x}\)

\(=\)







\(\ds C\)














\(\ds \leadsto \ \ \)





\(\ds y\)

\(=\)







\(\ds C e^{k x}\)









$\blacksquare$


Sources
1958: G.E.H. Reuter: Elementary Differential Equations & Operators ... (previous) ... (next): Chapter $1$: Linear Differential Equations with Constant Coefficients: $\S 1$. The first order equation: $\S 1.2$ The integrating factor




