# 

Source: https://proofwiki.org/wiki/First_Order_ODE/y_dx_%2B_(x%5E2_y_-_x)_dy_%3D_0/Proof_2

Theorem
The first order ODE:

$(1): \quad y \rd x + \paren {x^2 y - x} \rd y = 0$
has the general solution:

$\dfrac {y^2} 2 - \dfrac y x = C$


Proof
Rearranging, we have:

$x^2 y \rd y - \paren {x \rd y - y \rd x} = 0$
Aiming to use Quotient Rule for Differentials, divide by $x^2$:

$y \rd y = \dfrac {x \rd y - y \rd x} {x^2}$
So from Quotient Rule for Differentials: Formulation 1

$y \rd y = \map \d {\dfrac y x}$
from which the solution immediately drops:

$\dfrac {y^2} 2 - \dfrac y x = C$
$\blacksquare$


Sources
1972: George F. Simmons: Differential Equations ... (previous) ... (next): $\S 2.9$: Integrating Factors: Example $1$




