# 

Source: https://proofwiki.org/wiki/First_Order_ODE/dy_%3D_k_y_dx/Proof_1

Theorem
Let $k \in \R$ be a real number.
The first order ODE:

$\dfrac {\d y} {\d x} = k y$
has the general solution:

$y = C e^{k x}$


Proof













\(\ds \dfrac {\d y} {\d x}\)

\(=\)







\(\ds k y\)














\(\ds \leadsto \ \ \)





\(\ds \int \dfrac {\d y} y\)

\(=\)







\(\ds \int k \rd x\)





Solution to Separable Differential Equation








\(\ds \leadsto \ \ \)





\(\ds \ln y\)

\(=\)







\(\ds k x + C'\)





Primitive of Reciprocal, Primitive of Constant








\(\ds \leadsto \ \ \)





\(\ds y\)

\(=\)







\(\ds e^{k x + C'}\)




















\(\ds \)

\(=\)







\(\ds e^{k x} e^{C'}\)




















\(\ds \)

\(=\)







\(\ds C e^{k x}\)





putting $C = e^{C'}$



$\blacksquare$


Sources
1958: G.E.H. Reuter: Elementary Differential Equations & Operators ... (previous) ... (next): Chapter $1$: Linear Differential Equations with Constant Coefficients: $\S 1$. The first order equation: $\S 1.1$ Introduction




