# 

Source: https://proofwiki.org/wiki/Forward_Difference_of_Power

Theorem
$\Delta c^x = \paren {c - 1} c^x$
where $\Delta$ denotes the forward difference operator.


Corollary
$\Delta 2^x = 2^x$


Proof
From the definitions:














\(\ds \Delta c^x\)

\(=\)







\(\ds c^{x + 1} - c^x\)





Definition of Forward Difference Operator














\(\ds \)

\(=\)







\(\ds c \cdot c^x - c^x\)




















\(\ds \)

\(=\)







\(\ds \paren {c - 1} c^x\)









$\blacksquare$





