# 

Source: https://proofwiki.org/wiki/Fourth_Power_is_Sum_of_2_Triangular_Numbers/Proof_2

Theorem
Let $n \in \Z$ be an integer.
Then:

$\exists a, b \in \Z_{\ge 0}: n^4 = T_a + T_b$
where $T_a$ and $T_b$ are triangular numbers.

That is, the $4$th power of an integer equals the sum of two triangular numbers.


Proof













\(\ds T_{n^2 - n - 1} + T_{n^2 + n - 1}\)

\(=\)







\(\ds \frac {\paren {n^2 - n - 1} \paren {n^2 - n} } 2 + \frac {\paren {n^2 + n - 1} \paren {n^2 + n} } 2\)





Closed Form for Triangular Numbers














\(\ds \)

\(=\)







\(\ds \frac {n \paren {n^2 - n - 1} \paren {n - 1} } 2 + \frac {n \paren {n^2 + n - 1} \paren {n + 1} } 2\)





factoring














\(\ds \)

\(=\)







\(\ds \frac {n \paren {n^3 - n^2 - n - n^2 + n + 1} } 2 + \frac {n \paren {n^3 + n^2 - n + n^2 + n - 1} } 2\)





multiplying out the numerators














\(\ds \)

\(=\)







\(\ds \frac {n \paren {\paren {n^3 - 2 n^2 + 1} + \paren {n^3 + 2 n^2 - 1} } } 2\)





simplifying














\(\ds \)

\(=\)







\(\ds n^4\)





simplifying



$\blacksquare$





