# 

Source: https://proofwiki.org/wiki/Gamma_Function_of_2

Theorem
Let $\Gamma$ denote the Gamma function.
Then:

$\map \Gamma 2 = 1$


Proof













\(\ds \map \Gamma 2\)

\(=\)







\(\ds \map \Gamma {1 + 1}\)




















\(\ds \)

\(=\)







\(\ds 1 \map \Gamma 1\)





Gamma Difference Equation














\(\ds \)

\(=\)







\(\ds 1 \times 0!\)





Gamma Function Extends Factorial














\(\ds \)

\(=\)







\(\ds 1\)





Definition of Factorial: $0! = 1$



$\blacksquare$





