# 

Source: https://proofwiki.org/wiki/GCD_of_Consecutive_Integers_of_General_Fibonacci_Sequence



Theorem
Let $\FF = \sequence {a_n}$ be a general Fibonacci sequence generated by the parameters $r, s, t, u$:

$a_n = \begin{cases}
r & : n = 0 \\
s & : n = 1 \\
t a_{n - 2} + u a_{n - 1} & : n > 1
\end{cases}$
Let:

$d = \gcd \set {r, s}$
where $\gcd$ denotes greatest common divisor.
Let $f = \gcd \set {a_m, a_{m - 1} }$ for some $m \in \N$.
Let $\gcd \set {f, t} = 1$.
Then:

$f \divides d$


Proof
Proof by induction:
Let $\map P m$ be the proposition:

$\gcd \set {f_m, t} = 1 \implies f_m = d$
where $f_m = \gcd \set {a_m, a_{m - 1} }$.
For clarity, we have indexed $f$.


Basis for the Induction
For $m = 1$:

$f_1 = \gcd \set {a_1, a_0} = \gcd \set {s, r} = d$
This is the basis for the induction.


Induction Hypothesis
Now we assume that $\map P k$ is true for some $k \in \N$.
In other words, this is our induction hypothesis:

$\gcd \set {f_k, t} = 1 \implies f_k = d$
where $f_k = \gcd \set {a_k, a_{k - 1} }$.
Now we need to show that $\map P {k + 1}$ is true, that is:

$\gcd \set {f_{k + 1}, t} = 1 \implies f_{k + 1} = d$
where $f_{k + 1} = \gcd \set {a_{k + 1}, a_k}$.


Induction Step
This is our induction step:














\(\ds f_{k + 1}\)

\(=\)







\(\ds \gcd \set {a_{k + 1}, a_k}\)




















\(\ds \)

\(=\)







\(\ds \gcd \set {t a_{k - 1} + u a_k, a_k}\)





Definition of $\sequence {a_n}$














\(\ds \)

\(=\)







\(\ds \gcd \set {t a_{k - 1}, a_k}\)





GCD with Remainder














\(\ds \)

\(=\)







\(\ds \gcd \set {t, a_k} \gcd \set {a_{k - 1}, a_k}\)





GCD with One Fixed Argument is Multiplicative Function














\(\ds \)

\(=\)







\(\ds \gcd \set {t, a_k} f_k\)









Suppose that $\gcd \set {f_{k + 1}, t} = 1$.
Then:














\(\ds 1\)

\(=\)







\(\ds \gcd \set {f_{k + 1}, t}\)




















\(\ds \)

\(=\)







\(\ds \gcd \set {\gcd \set {t, a_k}, t}\)





Divisor of One of Coprime Numbers is Coprime to Other














\(\ds \)

\(=\)







\(\ds \gcd \set {t, \gcd \set {t, a_k} }\)





Greatest Common Divisor is Symmetric














\(\ds \)

\(=\)







\(\ds \gcd \set {\gcd \set {t, t}, a_k}\)





Greatest Common Divisor is Associative














\(\ds \)

\(=\)







\(\ds \gcd \set {t, a_k}\)





GCD of Integer and Divisor



By the two results above, we have:

$f_{k + 1} = \gcd \set {t, a_k} f_k = f_k$
so we have $\gcd \set {f_k, t} = \gcd \set {f_{k + 1}, t} = 1$ as well.
By the induction hypothesis and Modus Ponendo Ponens:

$f_k = d$
and thus:

$f_{k + 1} = f_k = d$
so $\map P {k + 1}$ is true.

By the Principle of Mathematical Induction, $\map P m$ is true for all $m \in \N$.
Hence the result.
$\blacksquare$


Sources
1971: George E. Andrews: Number Theory ... (previous) ... (next): $\text {2-2}$ Divisibility: Exercise $12 \ \text{(b)}$




