# 

Source: https://proofwiki.org/wiki/General_Distributivity_Theorem/Examples/Sum_of_j_from_m_to_n_by_Sum_of_k_from_r_to_s

Example of General Distributivity Theorem
$\ds \sum_{j \mathop = m}^n \sum_{k \mathop = r}^s j k = \frac 1 4 \paren {n \paren {n + 1} - \paren {m - 1} m} \paren {s \paren {s + 1} - \paren {r - 1} r}$
for $m \le n, r \le s$.


Proof













\(\ds \sum_{j \mathop = m}^n \sum_{k \mathop = r}^s j k\)

\(=\)







\(\ds \paren {\sum_{j \mathop = m}^n j} \paren {\sum_{k \mathop = r}^s k}\)





General Distributivity Theorem














\(\ds \)

\(=\)







\(\ds \paren {\frac {n \paren {n + 1} } 2 - \frac {\paren {m - 1} m} 2} \paren {\frac {s \paren {s + 1} } 2 - \frac {\paren {r - 1} r} 2}\)





Sum of $j$ from $m$ to $n$














\(\ds \)

\(=\)







\(\ds \frac 1 4 \paren {n \paren {n + 1} - \paren {m - 1} m} \paren {s \paren {s + 1} - \paren {r - 1} r}\)





simplification



$\blacksquare$


Sources
1997: Donald E. Knuth: The Art of Computer Programming: Volume 1: Fundamental Algorithms (3rd ed.) ... (previous) ... (next): $\S 1.2.3$: Sums and Products: Exercise $14$




