# 

Source: https://proofwiki.org/wiki/Golden_Mean_by_One_Minus_Golden_Mean_equals_Minus_1

Theorem
$\phi \hat \phi = -1$
where:

$\phi$ denotes the golden mean
$\hat \phi := 1 - \phi$


Proof













\(\ds \phi\)

\(=\)







\(\ds \frac 1 {\phi - 1}\)





Definition 3 of Golden Mean








\(\ds \leadsto \ \ \)





\(\ds \phi \paren {\phi - 1}\)

\(=\)







\(\ds 1\)














\(\ds \leadsto \ \ \)





\(\ds \phi \paren {1 - \phi}\)

\(=\)







\(\ds -1\)














\(\ds \leadsto \ \ \)





\(\ds \phi \hat \phi\)

\(=\)







\(\ds -1\)





by definition



$\blacksquare$





