# 

Source: https://proofwiki.org/wiki/Group_Generated_by_Reciprocal_of_z_and_1_minus_z



Theorem
Let $\struct {S, \circ}$ denote the group generated by $\dfrac 1 z$ and $1 - z$.

Then $\struct {S, \circ}$ is a finite group of order $6$.


Proof
By definition:

$S = \set {f_1, f_2, f_3, f_4, f_5, f_6}$
where $f_1, f_2, \ldots, f_6$ are complex functions defined for all $z \in \C \setminus \set {0, 1}$ as:














\(\ds \map {f_1} z\)

\(=\)







\(\ds z\)




















\(\ds \map {f_2} z\)

\(=\)







\(\ds \dfrac 1 {1 - z}\)




















\(\ds \map {f_3} z\)

\(=\)







\(\ds \dfrac {z - 1} z\)




















\(\ds \map {f_4} z\)

\(=\)







\(\ds \dfrac 1 z\)




















\(\ds \map {f_5} z\)

\(=\)







\(\ds 1 - z\)




















\(\ds \map {f_6} z\)

\(=\)







\(\ds \dfrac z {z - 1}\)










Also by definition, $\circ$ denotes composition of functions.

First it is necessary to establish the Cayley table for $\struct {S, \circ}$.
First note that it is apparent by definition of composition of functions that:

$\forall n: f_1 \circ f_n = f_n = f_n \circ f_1$

It remains to establish the rest of the compositions














\(\ds f_2 \circ f_2\)

\(=\)







\(\ds \dfrac 1 {1 - \dfrac 1 {1 - z} }\)




















\(\ds \)

\(=\)







\(\ds \dfrac {1 - z} {1 - z - 1}\)




















\(\ds \)

\(=\)







\(\ds \dfrac {z - 1} z\)




















\(\ds \)

\(=\)







\(\ds f_3\)
























\(\ds f_2 \circ f_3\)

\(=\)







\(\ds \dfrac 1 {1 - \dfrac {z - 1} z}\)




















\(\ds \)

\(=\)







\(\ds \dfrac z {z - \paren {z - 1} }\)




















\(\ds \)

\(=\)







\(\ds z\)




















\(\ds \)

\(=\)







\(\ds f_1\)
























\(\ds f_2 \circ f_4\)

\(=\)







\(\ds \dfrac 1 {1 - \dfrac 1 z}\)




















\(\ds \)

\(=\)







\(\ds \dfrac z {z - 1}\)




















\(\ds \)

\(=\)







\(\ds f_6\)
























\(\ds f_2 \circ f_5\)

\(=\)







\(\ds \dfrac 1 {1 - \paren {1 - z} }\)




















\(\ds \)

\(=\)







\(\ds \dfrac 1 z\)




















\(\ds \)

\(=\)







\(\ds f_4\)
























\(\ds f_2 \circ f_6\)

\(=\)







\(\ds \dfrac 1 {1 - \dfrac z {z - 1} }\)




















\(\ds \)

\(=\)







\(\ds \dfrac {z - 1} {z - 1 - z}\)




















\(\ds \)

\(=\)







\(\ds 1 - z\)




















\(\ds \)

\(=\)







\(\ds f_5\)
























\(\ds f_3 \circ f_2\)

\(=\)







\(\ds \dfrac {\dfrac 1 {1 - z} - 1} {\dfrac 1 {1 - z} }\)




















\(\ds \)

\(=\)







\(\ds \paren {1 - z} \dfrac {1 - \paren {1 - z} } {1 - z}\)




















\(\ds \)

\(=\)







\(\ds z\)




















\(\ds \)

\(=\)







\(\ds f_1\)
























\(\ds f_3 \circ f_3\)

\(=\)







\(\ds \dfrac {\dfrac {z - 1} z - 1} {\dfrac {z - 1} z}\)




















\(\ds \)

\(=\)







\(\ds \dfrac {z - 1 - z} z \dfrac z {z - 1}\)




















\(\ds \)

\(=\)







\(\ds \dfrac 1 {1 - z}\)




















\(\ds \)

\(=\)







\(\ds f_2\)
























\(\ds f_3 \circ f_4\)

\(=\)







\(\ds \dfrac {\dfrac 1 z - 1} {\dfrac 1 z}\)




















\(\ds \)

\(=\)







\(\ds z \dfrac {1 - z} z\)




















\(\ds \)

\(=\)







\(\ds 1 - z\)




















\(\ds \)

\(=\)







\(\ds f_5\)
























\(\ds f_3 \circ f_5\)

\(=\)







\(\ds \dfrac {\paren {1 - z} - 1} {1 - z}\)




















\(\ds \)

\(=\)







\(\ds \dfrac z {z - 1}\)




















\(\ds \)

\(=\)







\(\ds f_6\)
























\(\ds f_3 \circ f_6\)

\(=\)







\(\ds \dfrac {\dfrac z {z - 1} - 1} {\dfrac z {z - 1} }\)




















\(\ds \)

\(=\)







\(\ds \dfrac {z - \paren {z - 1} } {z - 1} \dfrac {z - 1} z\)




















\(\ds \)

\(=\)







\(\ds \dfrac 1 z\)




















\(\ds \)

\(=\)







\(\ds f_4\)
























\(\ds f_4 \circ f_2\)

\(=\)







\(\ds \dfrac 1 {\dfrac 1 {1 - z} }\)




















\(\ds \)

\(=\)







\(\ds 1 - z\)




















\(\ds \)

\(=\)







\(\ds f_5\)
























\(\ds f_4 \circ f_3\)

\(=\)







\(\ds \dfrac 1 {\dfrac {z - 1} z}\)




















\(\ds \)

\(=\)







\(\ds \dfrac z {z - 1}\)




















\(\ds \)

\(=\)







\(\ds f_6\)
























\(\ds f_4 \circ f_4\)

\(=\)







\(\ds \dfrac 1 {1 / z}\)




















\(\ds \)

\(=\)







\(\ds z\)




















\(\ds \)

\(=\)







\(\ds f_1\)
























\(\ds f_4 \circ f_5\)

\(=\)







\(\ds \dfrac 1 {1 - z}\)




















\(\ds \)

\(=\)







\(\ds f_2\)
























\(\ds f_4 \circ f_6\)

\(=\)







\(\ds \dfrac 1 {\dfrac z {z - 1} }\)




















\(\ds \)

\(=\)







\(\ds \dfrac {z - 1} z\)




















\(\ds \)

\(=\)







\(\ds f_3\)
























\(\ds f_5 \circ f_2\)

\(=\)







\(\ds 1 - \dfrac 1 {1 - z}\)




















\(\ds \)

\(=\)







\(\ds \dfrac {1 - z - 1} {1 - z}\)




















\(\ds \)

\(=\)







\(\ds \dfrac z {z - 1}\)




















\(\ds \)

\(=\)







\(\ds f_6\)
























\(\ds f_5 \circ f_3\)

\(=\)







\(\ds 1 - \dfrac {z - 1} z\)




















\(\ds \)

\(=\)







\(\ds \dfrac {z - \paren {z - 1} } z\)




















\(\ds \)

\(=\)







\(\ds \dfrac 1 z\)




















\(\ds \)

\(=\)







\(\ds f_4\)
























\(\ds f_5 \circ f_4\)

\(=\)







\(\ds 1 - \dfrac 1 z\)




















\(\ds \)

\(=\)







\(\ds \dfrac {z - 1} z\)




















\(\ds \)

\(=\)







\(\ds f_3\)
























\(\ds f_5 \circ f_5\)

\(=\)







\(\ds 1 - \paren {1 - z}\)




















\(\ds \)

\(=\)







\(\ds z\)




















\(\ds \)

\(=\)







\(\ds f_1\)
























\(\ds f_5 \circ f_6\)

\(=\)







\(\ds 1 - \dfrac z {z - 1}\)




















\(\ds \)

\(=\)







\(\ds \dfrac {z - 1 - z} {z - 1}\)




















\(\ds \)

\(=\)







\(\ds \dfrac 1 {1 - z}\)




















\(\ds \)

\(=\)







\(\ds f_2\)
























\(\ds f_6 \circ f_2\)

\(=\)







\(\ds \dfrac {\dfrac 1 {1 - z} } {\dfrac 1 {1 - z} - 1}\)




















\(\ds \)

\(=\)







\(\ds \dfrac 1 {1 - z} \dfrac {1 - z} {1 - \paren {1 - z} }\)




















\(\ds \)

\(=\)







\(\ds \dfrac 1 z\)




















\(\ds \)

\(=\)







\(\ds f_4\)
























\(\ds f_6 \circ f_3\)

\(=\)







\(\ds \dfrac {\dfrac {z - 1} z} {\dfrac {z - 1} z - 1}\)




















\(\ds \)

\(=\)







\(\ds \dfrac {z - 1} z \dfrac z {z - 1 - z}\)




















\(\ds \)

\(=\)







\(\ds 1 - z\)




















\(\ds \)

\(=\)







\(\ds f_5\)
























\(\ds f_6 \circ f_4\)

\(=\)







\(\ds \dfrac {\dfrac 1 z} {\dfrac 1 z - 1}\)




















\(\ds \)

\(=\)







\(\ds \dfrac 1 z \dfrac z {1 - z}\)




















\(\ds \)

\(=\)







\(\ds \dfrac 1 {1 - z}\)




















\(\ds \)

\(=\)







\(\ds f_2\)
























\(\ds f_6 \circ f_5\)

\(=\)







\(\ds \dfrac {1 - z} {1 - z - 1}\)




















\(\ds \)

\(=\)







\(\ds \dfrac {z - 1} z\)




















\(\ds \)

\(=\)







\(\ds f_3\)
























\(\ds f_6 \circ f_6\)

\(=\)







\(\ds \dfrac {\dfrac z {z - 1} } {\dfrac z {z - 1} - 1}\)




















\(\ds \)

\(=\)







\(\ds \dfrac z {z - 1} \dfrac {z - 1} {z - 1 - z}\)




















\(\ds \)

\(=\)







\(\ds z\)




















\(\ds \)

\(=\)







\(\ds f_1\)










Hence the Cayley table is established:


$\begin{array}{r|rrrrrr}
\circ & f_1 & f_2 & f_3 & f_4 & f_5 & f_6 \\
\hline
f_1 & f_1 & f_2 & f_3 & f_4 & f_5 & f_6 \\
f_2 & f_2 & f_3 & f_1 & f_6 & f_4 & f_5 \\
f_3 & f_3 & f_1 & f_2 & f_5 & f_6 & f_4 \\
f_4 & f_4 & f_5 & f_6 & f_1 & f_2 & f_3 \\
f_5 & f_5 & f_6 & f_4 & f_3 & f_1 & f_2 \\
f_6 & f_6 & f_4 & f_5 & f_2 & f_3 & f_1 \\
\end{array}$

Expressing the elements in full:

$\begin{array}{c|cccccc}
\circ & z & \dfrac 1 {1 - z} & \dfrac {z - 1} z & \dfrac 1 z & 1 - z & \dfrac z {z - 1} \\
\hline
z & z & \dfrac 1 {1 - z} & \dfrac {z - 1} z & \dfrac 1 z & 1 - z & \dfrac z {z - 1} \\
\dfrac 1 {1 - z} & \dfrac 1 {1 - z} & \dfrac {z - 1} z & z & \dfrac z {z - 1} & \dfrac 1 z & 1 - z \\
\dfrac {z - 1} z & \dfrac {z - 1} z & z & \dfrac 1 {1 - z} & 1 - z & \dfrac z {z - 1} & \dfrac 1 z \\
\dfrac 1 z & \dfrac 1 z & 1 - z & \dfrac z {z - 1} & z & \dfrac 1 {1 - z} & \dfrac {z - 1} z \\
1 - z & 1 - z & \dfrac z {z - 1} & \dfrac 1 z & \dfrac {z - 1} z & z & \dfrac 1 {1 - z} \\
\dfrac z {z - 1} & \dfrac z {z - 1} & \dfrac 1 z & 1 - z & \dfrac 1 {1 - z} & \dfrac {z - 1} z & z \\
\end{array}$

Taking the group axioms in turn:


Group Axiom $\text G 0$: Closure
By inspection it can be seen that $\struct {S, \circ}$ is closed.
$\Box$


Group Axiom $\text G 1$: Associativity
From Composition of Mappings is Associative, it follows that $\struct {S, \circ}$ is associative.
$\Box$


Group Axiom $\text G 2$: Existence of Identity Element
We have that:

$\forall n: f_1 \circ f_n = f_n = f_n \circ f_1$
Thus $\struct {S, \circ}$ has an identity element.
$\Box$


Group Axiom $\text G 3$: Existence of Inverse Element
From the above analysis:














\(\ds f_1 \circ f_1\)

\(=\)







\(\ds f_1\)




















\(\ds f_2 \circ f_3\)

\(=\)







\(\ds f_1\)




















\(\ds f_3 \circ f_2\)

\(=\)







\(\ds f_1\)




















\(\ds f_4 \circ f_4\)

\(=\)







\(\ds f_1\)




















\(\ds f_5 \circ f_5\)

\(=\)







\(\ds f_1\)




















\(\ds f_6 \circ f_6\)

\(=\)







\(\ds f_1\)









Thus every element of $\struct {S, \circ}$ has an inverse.
$\Box$

All the group axioms are thus seen to be fulfilled, and so $\struct {S, \circ}$ is a group.

$\struct {S, \circ}$ has $6$ elements and so is a finite group of order $6$.
$\blacksquare$


Sources
1964: Walter Ledermann: Introduction to the Theory of Finite Groups (5th ed.) ... (previous) ... (next): Chapter $\text {I}$: The Group Concept: $\S 6$: Examples of Finite Groups: $\text{(ii)}$
1971: Allan Clark: Elements of Abstract Algebra ... (previous) ... (next): Introduction




