# 

Source: https://proofwiki.org/wiki/Half_Angle_Formulas/Hyperbolic_Tangent



Theorem
Let $x \in \R$.
Then:














\(\ds \tanh \frac x 2\)

\(=\)







\(\ds +\sqrt {\frac {\cosh x - 1} {\cosh x + 1} }\)





for $x \ge 1$














\(\ds \tanh \frac x 2\)

\(=\)







\(\ds -\sqrt {\frac {\cosh x - 1} {\cosh x + 1} }\)





for $x \le 1$



where $\tanh$ denotes hyperbolic tangent and $\cosh$ denotes hyperbolic cosine.


Corollary 1
$\tanh \dfrac x 2 = \dfrac {\sinh x} {\cosh x + 1}$


Corollary 2
For $x \ne 0$:

$\tanh \dfrac x 2 = \dfrac {\cosh x - 1} {\sinh x}$


Proof













\(\ds \tanh \frac x 2\)

\(=\)







\(\ds \frac {\sinh \frac x 2} {\cosh \frac x 2}\)





Definition 2 of Hyperbolic Tangent














\(\ds \)

\(=\)







\(\ds \frac {\pm \sqrt {\frac {\cosh x - 1} 2} } {\pm \sqrt {\frac {\cosh x + 1} 2} }\)





Half Angle Formula for Hyperbolic Sine and Half Angle Formula for Hyperbolic Cosine














\(\ds \)

\(=\)







\(\ds \pm \sqrt {\frac {\cosh x - 1} {\cosh x + 1} }\)










We also have that:

when $x \ge 0$, $\tanh \dfrac x 2 \ge 0$
when $x \le 0$, $\tanh \dfrac x 2 \le 0$.
$\blacksquare$


Also see
Half Angle Formula for Hyperbolic Sine
Half Angle Formula for Hyperbolic Cosine


Sources
1968: Murray R. Spiegel: Mathematical Handbook of Formulas and Tables ... (previous) ... (next): $\S 8$: Hyperbolic Functions: $8.29$: Double Angle Formulas




