# 

Source: https://proofwiki.org/wiki/Half_Angle_Formulas/Hyperbolic_Sine



Theorem
Let $x \in \R$.
Then:














\(\ds \sinh \frac x 2\)

\(=\)







\(\ds +\sqrt {\frac {\cosh x - 1} 2}\)





for $x \ge 0$














\(\ds \sinh \frac x 2\)

\(=\)







\(\ds -\sqrt {\dfrac {\cosh x - 1} 2}\)





for $x \le 0$



where $\sinh$ denotes hyperbolic sine and $\cosh$ denotes hyperbolic cosine.


Proof













\(\ds \cosh x\)

\(=\)







\(\ds 1 + 2 \ \sinh^2 \frac x 2\)





Double Angle Formula for Hyperbolic Cosine: Corollary $2$








\(\ds \leadsto \ \ \)





\(\ds 2 \ \sinh^2 \frac x 2\)

\(=\)







\(\ds \cosh x - 1\)














\(\ds \leadsto \ \ \)





\(\ds \sinh \frac x2\)

\(=\)







\(\ds \pm \sqrt {\frac {\cosh x - 1} 2}\)










We also have that:

when $x \ge 0$, $\sinh x \ge 0$
when $x \le 0$, $\sinh x \le 0$.
$\blacksquare$


Also see
Half Angle Formula for Hyperbolic Cosine
Half Angle Formula for Hyperbolic Tangent


Sources
1968: Murray R. Spiegel: Mathematical Handbook of Formulas and Tables ... (previous) ... (next): $\S 8$: Hyperbolic Functions: $8.27$: Double Angle Formulas




