# 

Source: https://proofwiki.org/wiki/Hypothetical_Syllogism/Formulation_1/Proof_2

Theorem













\(\ds p\)

\(\implies\)







\(\ds q\)




















\(\ds q\)

\(\implies\)







\(\ds r\)














\(\ds \vdash \ \ \)





\(\ds p\)

\(\implies\)







\(\ds r\)











Proof
This proof uses $\mathscr H_2$, Instance 2 of the Hilbert proof systems.
Recall the sequent form of the Hypothetical Syllogism:

$\vdash \paren {q \implies r} \implies \paren {\paren {p \implies q} \implies \paren {p \implies r} }$
Applying the Rule of Detachment $\text {RST} 3$ twice, we obtain:

$\vdash \paren {p \implies q} \implies \paren {p \implies r}$
and subsequently:

$\vdash p \implies r$
as desired.
$\blacksquare$


Sources
1959: A.H. Basson and D.J. O'Connor: Introduction to Symbolic Logic (3rd ed.) ... (previous) ... (next): $\S 4.7$: The Derivation of Formulae: $DR \, 1$




