# 

Source: https://proofwiki.org/wiki/Hypothetical_Syllogism/Formulation_2/Proof_2

Theorem













\(\ds p\)

\(\implies\)







\(\ds q\)




















\(\ds q\)

\(\implies\)







\(\ds r\)




















\(\ds p\)

\(\)







\(\ds \)














\(\ds \vdash \ \ \)





\(\ds r\)

\(\)







\(\ds \)











Proof
By the tableau method of natural deduction:


$p \implies q, q \implies r, p \vdash r$


Line


Pool

Formula

Rule

Depends upon

Notes


1


1

$p \implies q$

Premise

(None)




2


2

$q \implies r$

Premise

(None)




3


3

$p$

Premise

(None)




4


1, 3

$q$

Modus Ponendo Ponens: $\implies \mathcal E$

1, 3




5


1, 2, 3

$r$

Modus Ponendo Ponens: $\implies \mathcal E$

2, 4



$\blacksquare$


Sources
1965: E.J. Lemmon: Beginning Logic ... (previous) ... (next): Chapter $1$: The Propositional Calculus $1$: $2$ Conditionals and Negation: Theorem $3$




