# 

Source: https://proofwiki.org/wiki/If_n_is_Triangular_then_so_is_(2m%2B1)%5E2_n_%2B_m(m%2B1)/2

Theorem
Let $n$ be a triangular number.
Let $m \in \Z_{\ge 0}$ be a positive integer.

Then $\paren {2 m + 1}^2 n + \dfrac {m \paren {m + 1} } 2$ is also a triangular number.


Proof
Let $n$ be a triangular number.
Then:

$\exists k \in \Z: n = \dfrac {k \paren {k + 1} } 2$
So:














\(\ds \paren {2 m + 1}^2 n + \dfrac {m \paren {m + 1} } 2\)

\(=\)







\(\ds \paren {2 m + 1}^2 \dfrac {k \paren {k + 1} } 2 + \dfrac {m \paren {m + 1} } 2\)




















\(\ds \)

\(=\)







\(\ds \dfrac {\paren {2 m + 1}^2 k^2 + \paren {2 m + 1}^2 k + m \paren {m + 1} } 2\)




















\(\ds \)

\(=\)







\(\ds \dfrac {\paren {\paren {2 m + 1} k + m} \paren {\paren {2 m + 1} k + m + 1} } 2\)









which is of the form:

$\dfrac {t \paren {t + 1} } 2$
where $t = \paren {2 m + 1} k + m$.
$\blacksquare$





