# 

Source: https://proofwiki.org/wiki/Image_of_Element_under_Inverse_Mapping/Corollary_2

Theorem
Let $S$ and $T$ be sets.
Let $f: S \to T$ be a mapping such that its inverse $f^{-1}: T \to S$ is also a mapping.

Then:

$\forall y \in T: \map f {\map {f^{-1} } y} = y$


Proof









\(\ds \forall x \in S, y \in T: \, \)



\(\ds \map f x\)

\(=\)







\(\ds y\)


















\(\, \ds \iff \, \)

\(\ds \map {f^{-1} } y\)

\(=\)







\(\ds x\)





Image of Element under Inverse Mapping








\(\ds \leadsto \ \ \)

\(\ds \forall y \in T: \, \)



\(\ds \map f {\map {f^{-1} } y}\)

\(=\)







\(\ds y\)





substituting $\map {f^{-1} } y$ for $x$



$\blacksquare$


Sources
1998: David Nelson: The Penguin Dictionary of Mathematics (2nd ed.) ... (previous) ... (next): inverse: 1. (of a function)
2008: David Nelson: The Penguin Dictionary of Mathematics (4th ed.) ... (previous) ... (next): inverse: 1. (of a function)




