# 

Source: https://proofwiki.org/wiki/Inscribing_Equilateral_Triangle_inside_Square_with_a_Coincident_Vertex/Lemma



Lemma
Let $\Box ABCD$ be a square.
Let $\triangle DGH$ be an isosceles triangle inscribed within $\Box ABCD$ such that the apex $D$ of $\triangle DGH$ coincides with vertex $D$ of $\Box ABCD$.


Then:

$\triangle DGH$ is equilateral triangle
if and only if:

$\angle ADG = 15 \degrees \text { or } \angle CDH = 15 \degrees$ (and in fact both are the case).


Proof
First note that $\triangle DGH$ is isosceles.
First we note that:














\(\ds CD\)

\(=\)







\(\ds AD\)





as they are the sides of a square














\(\ds DH\)

\(=\)







\(\ds DG\)





as $\triangle DGH$ is isosceles














\(\ds \angle DCH\)

\(=\)







\(\ds \angle DAG = 90 \degrees\)





as $\Box ABCD$ is a square



Then:














\(\ds CH^2\)

\(=\)







\(\ds DH^2 - CD^2\)





Pythagoras's Theorem














\(\ds \)

\(=\)







\(\ds DG^2 - AD^2\)




















\(\ds \)

\(=\)







\(\ds AG^2\)














\(\ds \leadsto \ \ \)





\(\ds CH\)

\(=\)







\(\ds AG\)









So by Triangle Side-Side-Side Congruence:

$\triangle ADG = \triangle CDH$
and in particular:

$\angle ADG = \angle CDH$


Necessary Condition
Let $\angle ADG = \angle CDH = 15 \degrees$.
Then:

$\angle GDH = 90 \degrees - 2 \times 15 \degrees = 60 \degrees$
We have that $\triangle DGH$ is isosceles.
Hence from Isosceles Triangle has Two Equal Angles:

$\angle DGH = \angle DHG$
From Sum of Angles of Triangle equals Two Right Angles it follows that:

$\angle DGH + \angle DHG = 180 \degrees - 60 \degrees = 120 \degrees$
from which:

$\angle DGH = \angle DHG = 60 \degrees$
Hence all the vertices of $\triangle DGH$ equal $60 \degrees$.
It follows from Equiangular Triangle is Equilateral that $\triangle DGH$ is equilateral.
$\Box$


Sufficient Condition
Let $\triangle DGH$ be equilateral.
From Internal Angle of Equilateral Triangle:

$\angle GDH = 60 \degrees$
Because $\Box ABCD$ is a square:

$\angle ADC = 90 \degrees$
Thus:














\(\ds \angle ADG + \angle GDH + \angle CDH\)

\(=\)







\(\ds 90 \degrees\)














\(\ds \leadsto \ \ \)





\(\ds \angle ADG + \angle CDH\)

\(=\)







\(\ds 90 \degrees - \angle GDH\)




















\(\ds \)

\(=\)







\(\ds 90 \degrees - 60 \degrees\)




















\(\ds \)

\(=\)







\(\ds 30 \degrees\)









But we have that:

$\angle ADG = \angle CDH$
and so:

$\angle ADG = \angle CDH = 15 \degrees$
$\blacksquare$





