# 

Source: https://proofwiki.org/wiki/Integer_to_Power_of_Itself_Less_One_Falling_is_Factorial

Theorem
Let $n \in \Z_{\ge 0}$ be a positive integer.

$n^{\underline {n - 1} } = n!$
where:

$n^{\underline {n - 1} }$ denotes the falling factorial
$n!$ denotes the factorial.


Proof













\(\ds n^{\underline {n - 1} }\)

\(=\)







\(\ds \dfrac {n!} {\left({n - \left({n - 1}\right)}\right)!}\)





Falling Factorial as Quotient of Factorials














\(\ds \)

\(=\)







\(\ds \dfrac {n!} {1!}\)




















\(\ds \)

\(=\)







\(\ds n!\)





Factorial of $1$



$\blacksquare$





