# 

Source: https://proofwiki.org/wiki/Inverse_Hyperbolic_Cotangent_is_Odd_Function/Proof_1

Theorem
$\map {\coth^{-1} } {-x} = -\coth^{-1} x$


Proof













\(\ds \map {\coth^{-1} } {-x}\)

\(=\)







\(\ds y\)














\(\ds \leadstoandfrom \ \ \)





\(\ds -x\)

\(=\)







\(\ds \coth y\)





Definition 1 of Inverse Hyperbolic Cotangent








\(\ds \leadstoandfrom \ \ \)





\(\ds x\)

\(=\)







\(\ds -\coth y\)














\(\ds \leadstoandfrom \ \ \)





\(\ds x\)

\(=\)







\(\ds \map \coth {-y}\)





Hyperbolic Cotangent Function is Odd








\(\ds \leadstoandfrom \ \ \)





\(\ds \coth^{-1} x\)

\(=\)







\(\ds -y\)





Definition 1 of Inverse Hyperbolic Cotangent



$\blacksquare$





