# 

Source: https://proofwiki.org/wiki/Inverse_Tangent_of_Imaginary_Number



Theorem
$\map {\tan^{-1} } {i x} = i \tanh^{-1} x$


Proof 1













\(\ds y\)

\(=\)







\(\ds \map {\tan^{-1} } {i x}\)














\(\ds \leadsto \ \ \)





\(\ds \tan y\)

\(=\)







\(\ds i x\)





Definition of Inverse Tangent








\(\ds \leadsto \ \ \)





\(\ds i \tan y\)

\(=\)







\(\ds - x\)





$i^2 = -1$








\(\ds \leadsto \ \ \)





\(\ds \map \tanh {i y}\)

\(=\)







\(\ds -x\)





Tangent in terms of Hyperbolic Tangent








\(\ds \leadsto \ \ \)





\(\ds i y\)

\(=\)







\(\ds \map {\tanh^{-1} } {-x}\)





Definition of Inverse Hyperbolic Tangent








\(\ds \leadsto \ \ \)





\(\ds i y\)

\(=\)







\(\ds -\tanh^{-1} x\)





Inverse Hyperbolic Tangent is Odd Function








\(\ds \leadsto \ \ \)





\(\ds y\)

\(=\)







\(\ds i \tanh^{-1} x\)





multiplying both sides by $-i$



$\blacksquare$


Proof 2













\(\ds \map {\tan^{-1} } {i x}\)

\(=\)







\(\ds \frac i 2 \map \ln {\frac {1 - i \paren {i x} } {1 + i \paren {i x} } }\)





Arctangent Logarithmic Formulation














\(\ds \)

\(=\)







\(\ds \frac i 2 \map \ln {\frac {1 + x} {1 - x} }\)




















\(\ds \)

\(=\)







\(\ds i \tanh^{-1} x\)





Definition of Inverse Hyperbolic Tangent



$\blacksquare$


Sources
1968: Murray R. Spiegel: Mathematical Handbook of Formulas and Tables ... (previous) ... (next): $\S 8$: Hyperbolic Functions: $8.96$: Relationship between Inverse Hyperbolic and Inverse Trigonometric Functions




