# 

Source: https://proofwiki.org/wiki/Inverse_Hyperbolic_Cotangent_is_Odd_Function/Proof_2

Theorem
$\map {\coth^{-1} } {-x} = -\coth^{-1} x$


Proof













\(\ds \map {\coth^{-1} } {-x}\)

\(=\)







\(\ds \frac 1 2 \map \ln {\frac {-z + 1} {-z - 1} }\)





Definition 2 of Inverse Hyperbolic Cotangent














\(\ds \)

\(=\)







\(\ds \frac 1 2 \map \ln {\frac {z - 1} {z + 1} }\)





multiplying the argument by $\dfrac {-1} {-1}$














\(\ds \)

\(=\)







\(\ds \frac 1 2 \paren {\map \ln {z - 1} - \map \ln {z + 1} }\)





Difference of Logarithms














\(\ds \)

\(=\)







\(\ds -\frac 1 2 \paren {\map \ln {z + 1} - \map \ln {z - 1} }\)




















\(\ds \)

\(=\)







\(\ds -\frac 1 2 \map \ln {\frac {z + 1} {z - 1} }\)





Difference of Logarithms














\(\ds \)

\(=\)







\(\ds -\coth^{-1} x\)





Definition 2 of Inverse Hyperbolic Cotangent



$\blacksquare$





