# 

Source: https://proofwiki.org/wiki/Inverse_Hyperbolic_Tangent/Examples/i

Example of Inverse Hyperbolic Tangent
$\inv \tanh i = \dfrac {\paren {4 k + 1} \pi i} 4$


Proof
Recall the definition of Inverse Hyperbolic Tangent:

$\inv \tanh i := \set {z \in \C: \tanh z = i}$

Thus:














\(\ds \tanh z\)

\(=\)







\(\ds i\)














\(\ds \leadsto \ \ \)





\(\ds \dfrac {\map \exp {2 z} - 1} {\map \exp {2 z} + 1}\)

\(=\)







\(\ds i\)





Definition 3 of Hyperbolic Tangent








\(\ds \leadsto \ \ \)





\(\ds \map \exp {2 z} - 1\)

\(=\)







\(\ds i \paren {\map \exp {2 z} + 1}\)





rearranging














\(\ds \)

\(=\)







\(\ds i \map \exp {2 z} + i\)





rearranging








\(\ds \leadsto \ \ \)





\(\ds \map \exp {2 z} \paren {1 - i}\)

\(=\)







\(\ds 1 + i\)














\(\ds \leadsto \ \ \)





\(\ds \map \exp {2 z}\)

\(=\)







\(\ds \dfrac {1 + i} {1 - i}\)














\(\ds \leadsto \ \ \)





\(\ds z\)

\(=\)







\(\ds \dfrac 1 2 \ln \dfrac {1 + i} {1 - i}\)




















\(\ds \)

\(=\)







\(\ds \dfrac 1 2 \ln \dfrac {\paren {1 + i}^2 } {\paren {1 - i} \paren {1 + i} }\)




















\(\ds \)

\(=\)







\(\ds \dfrac 1 2 \ln \dfrac {2 i} 2\)




















\(\ds \)

\(=\)







\(\ds \dfrac 1 2 \ln i\)




















\(\ds \)

\(=\)







\(\ds \dfrac 1 2 \paren {\paren {4 k + 1} \dfrac {\pi i} 2}\)





Natural Logarithm of $i$














\(\ds \)

\(=\)







\(\ds \dfrac {\paren {4 k + 1} \pi i} 4\)





for all $k \in \Z$



$\blacksquare$


Sources
1960: Walter Ledermann: Complex Numbers ... (previous) ... (next): $\S 4$. Elementary Functions of a Complex Variable: Exercise $9 \ \text{(ii)}$




