# 

Source: https://proofwiki.org/wiki/Inverse_Hyperbolic_Tangent_is_Odd_Function/Proof_2

Theorem
$\map {\tanh^{-1} } {-x} = -\tanh^{-1} x$


Proof













\(\ds \map {\tanh^{-1} } {-x}\)

\(=\)







\(\ds \frac 1 2 \map \ln {\frac {1 + \paren {-x} } {1 - \paren {-x} } }\)





Definition 2 of Inverse Hyperbolic Tangent














\(\ds \)

\(=\)







\(\ds \frac 1 2 \map \ln {\frac {1 - x} {1 + x} }\)




















\(\ds \)

\(=\)







\(\ds \frac 1 2 \paren {\map \ln {1 - x} - \map \ln {1 + x} }\)





Difference of Logarithms














\(\ds \)

\(=\)







\(\ds -\frac 1 2 \paren {\map \ln {1 + x} - \map \ln {1 - x} }\)




















\(\ds \)

\(=\)







\(\ds -\frac 1 2 \map \ln {\frac {1 + x} {1 - x} }\)





Difference of Logarithms














\(\ds \)

\(=\)







\(\ds -\tanh^{-1} x\)





Definition 2 of Inverse Hyperbolic Tangent



$\blacksquare$





