# 

Source: https://proofwiki.org/wiki/Inverse_Element_is_Power_of_Order_Less_1

Theorem
Let $G$ be a group whose identity is $e$.
Let $g \in G$ be of finite order.
Then:

$\order g = n \implies g^{n - 1} = g^{-1}$


Proof













\(\ds \order g\)

\(=\)







\(\ds n\)














\(\ds \leadsto \ \ \)





\(\ds g^n\)

\(=\)







\(\ds e\)














\(\ds \leadsto \ \ \)





\(\ds g^n g^{-1}\)

\(=\)







\(\ds e g^{-1}\)














\(\ds \leadsto \ \ \)





\(\ds g^{n - 1}\)

\(=\)







\(\ds g^{-1}\)









$\blacksquare$


Sources
1965: J.A. Green: Sets and Groups ... (previous) ... (next): $\S 5.4$. Cyclic groups: Example $101$
1996: John F. Humphreys: A Course in Group Theory ... (previous) ... (next): Chapter $3$: Elementary consequences of the definitions: Definition $3.9$: Remark $2$




