# 

Source: https://proofwiki.org/wiki/Inverse_Hyperbolic_Tangent_of_Imaginary_Number

Theorem
$\map {\tanh^{-1} } {i x} = i \tan^{-1} x$


Proof













\(\ds y\)

\(=\)







\(\ds \map {\tanh^{-1} } {i x}\)














\(\ds \leadsto \ \ \)





\(\ds \tanh y\)

\(=\)







\(\ds i x\)





Definition of Inverse Hyperbolic Tangent








\(\ds \leadsto \ \ \)





\(\ds i \tanh y\)

\(=\)







\(\ds -x\)





$i^2 = -1$








\(\ds \leadsto \ \ \)





\(\ds \map \tan {i y}\)

\(=\)







\(\ds -x\)





Hyperbolic Tangent in terms of Tangent








\(\ds \leadsto \ \ \)





\(\ds i y\)

\(=\)







\(\ds \map {\tan^{-1} } {-x}\)





Definition of Inverse Tangent








\(\ds \leadsto \ \ \)





\(\ds i y\)

\(=\)







\(\ds -\tan^{-1} x\)





Inverse Tangent is Odd Function








\(\ds \leadsto \ \ \)





\(\ds y\)

\(=\)







\(\ds i \tan^{-1} x\)





multiplying both sides by $-i$



$\blacksquare$


Sources
1968: Murray R. Spiegel: Mathematical Handbook of Formulas and Tables ... (previous) ... (next): $\S 8$: Hyperbolic Functions: $8.97$: Relationship between Inverse Hyperbolic and Inverse Trigonometric Functions




