# 

Source: https://proofwiki.org/wiki/Inverse_of_Non-Symmetric_Relation_is_Non-Symmetric

Theorem
Let $\RR$ be a relation on a set $S$.

If $\RR$ is non-symmetric, then so is $\RR^{-1}$.


Proof
Let $\RR$ be non-symmetric.
Then:

$\exists \tuple {x_1, y_1} \in \RR \implies \tuple {y_1, x_1} \in \RR$
and also:

$\exists \tuple {x_2, y_2} \in \RR \implies \tuple {y_2, x_2} \notin \RR$
Thus:

$\exists \tuple {y_1, x_1} \in \RR^{-1} \implies \tuple {x_1, y_1} \in \RR^{-1}$
and also:

$\exists \tuple {y_2, x_2} \in \RR^{-1} \implies \tuple {x_2, y_2} \notin \RR^{-1}$
and so $\RR^{-1}$ is non-symmetric.
$\blacksquare$





