# 

Source: https://proofwiki.org/wiki/Inverse_Tangent_of_Imaginary_Number/Proof_2

Theorem
$\map {\tan^{-1} } {i x} = i \tanh^{-1} x$


Proof













\(\ds \map {\tan^{-1} } {i x}\)

\(=\)







\(\ds \frac i 2 \map \ln {\frac {1 - i \paren {i x} } {1 + i \paren {i x} } }\)





Arctangent Logarithmic Formulation














\(\ds \)

\(=\)







\(\ds \frac i 2 \map \ln {\frac {1 + x} {1 - x} }\)




















\(\ds \)

\(=\)







\(\ds i \tanh^{-1} x\)





Definition of Inverse Hyperbolic Tangent



$\blacksquare$





