# 

Source: https://proofwiki.org/wiki/Inverse_Hyperbolic_Tangent_is_Odd_Function/Proof_1

Theorem
$\map {\tanh^{-1} } {-x} = -\tanh^{-1} x$


Proof













\(\ds \map {\tanh^{-1} } {-x}\)

\(=\)







\(\ds y\)














\(\ds \leadstoandfrom \ \ \)





\(\ds -x\)

\(=\)







\(\ds \tanh y\)





Definition 1 of Inverse Hyperbolic Tangent








\(\ds \leadstoandfrom \ \ \)





\(\ds x\)

\(=\)







\(\ds -\tanh y\)














\(\ds \leadstoandfrom \ \ \)





\(\ds x\)

\(=\)







\(\ds \map \tanh {-y}\)





Hyperbolic Tangent Function is Odd








\(\ds \leadstoandfrom \ \ \)





\(\ds \tanh^{-1} x\)

\(=\)







\(\ds -y\)





Definition 1 of Inverse Hyperbolic Tangent



$\blacksquare$





