# 

Source: https://proofwiki.org/wiki/Inverse_Hyperbolic_Cotangent_of_Imaginary_Number

Theorem
$\map {\coth^{-1} } {i x} = i \cot^{-1} x$


Proof













\(\ds y\)

\(=\)







\(\ds \map {\coth^{-1} } {i x}\)














\(\ds \leadsto \ \ \)





\(\ds \coth y\)

\(=\)







\(\ds i x\)





Definition of Inverse Hyperbolic Cotangent








\(\ds \leadsto \ \ \)





\(\ds i \coth y\)

\(=\)







\(\ds - x\)





$i^2 = -1$








\(\ds \leadsto \ \ \)





\(\ds \map \cot {i y}\)

\(=\)







\(\ds x\)





Hyperbolic Cotangent in terms of Cotangent








\(\ds \leadsto \ \ \)





\(\ds i y\)

\(=\)







\(\ds \cot^{-1} x\)





Definition of Inverse Cotangent








\(\ds \leadsto \ \ \)





\(\ds y\)

\(=\)







\(\ds -i \cot^{-1} x\)





multiplying both sides by $-i$



$\blacksquare$


Sources
1968: Murray R. Spiegel: Mathematical Handbook of Formulas and Tables ... (previous) ... (next): $\S 8$: Hyperbolic Functions: $8.99$: Relationship between Inverse Hyperbolic and Inverse Trigonometric Functions




