# 

Source: https://proofwiki.org/wiki/Law_of_Cosines/Right_Triangle

Theorem
Let $\triangle ABC$ be a triangle whose sides $a, b, c$ are such that:

$a$ is opposite $A$
$b$ is opposite $B$
$c$ is opposite $C$.
Let $\triangle ABC$ be a right triangle such that $\angle A$ is right.

Then:

$c^2 = a^2 + b^2 - 2 a b \cos C$


Proof
Let $\triangle ABC$ be a right triangle such that $\angle A$ is right.















\(\ds a^2\)

\(=\)







\(\ds b^2 + c^2\)





Pythagoras's Theorem














\(\ds c^2\)

\(=\)







\(\ds a^2 - b^2\)





adding $-b^2$ to both sides and rearranging














\(\ds \)

\(=\)







\(\ds a^2 - 2 b^2 + b^2\)





adding $0 = b^2 - b^2$ to the right hand side














\(\ds \)

\(=\)







\(\ds a^2 - 2 a b \left({\frac b a}\right) + b^2\)





multiplying $2 b^2$ by $\dfrac a a$














\(\ds \)

\(=\)







\(\ds a^2 + b^2 - 2 a b \cos C\)





Definition of Cosine: $\cos C = \dfrac b a$



$\blacksquare$





