# 

Source: https://proofwiki.org/wiki/Law_of_Tangents



Theorem
Let $\triangle ABC$ be a triangle whose sides $a, b, c$ are such that $a$ is opposite $A$, $b$ is opposite $B$ and $c$ is opposite $C$.
Then:

$\dfrac {a + b} {a - b} = \dfrac {\tan \frac 1 2 \paren {A + B} } {\tan \frac 1 2 \paren {A - B} }$


Corollary
$\tan \dfrac {A - B} 2 = \dfrac {a - b} {a + b} \cot \dfrac C 2$


Proof
Let $d = \dfrac a {\sin A}$.
From the Law of Sines, let:

$d = \dfrac a {\sin A} = \dfrac b {\sin B}$
so that:














\(\ds a\)

\(=\)







\(\ds d \sin A\)




















\(\ds b\)

\(=\)







\(\ds d \sin B\)














\(\ds \leadsto \ \ \)





\(\ds \frac {a + b} {a - b}\)

\(=\)







\(\ds \frac {d \sin A + d \sin B} {d \sin A - d \sin B}\)




















\(\ds \)

\(=\)







\(\ds \frac {\sin A + \sin B} {\sin A - \sin B}\)










Let $C = \frac 1 2 \paren {A + B}$ and $D = \frac 1 2 \paren {A - B}$, and proceed as follows:






\(\ds \leadsto \ \ \)





\(\ds \frac {a + b} {a - b}\)

\(=\)







\(\ds \frac {2 \sin C \cos D} {\sin A - \sin B}\)





Sine plus Sine














\(\ds \)

\(=\)







\(\ds \frac {2 \sin C \cos D} {2 \sin D \cos C}\)





Sine minus Sine














\(\ds \)

\(=\)







\(\ds \frac {\frac {\sin C} {\cos C} } {\frac {\sin D} {\cos D} }\)





dividing top and bottom by $\cos C \cos D$














\(\ds \)

\(=\)







\(\ds \frac {\tan C} {\tan D}\)





Tangent is Sine divided by Cosine














\(\ds \)

\(=\)







\(\ds \frac {\tan \frac 1 2 \paren {A + B} } {\tan \frac 1 2 \paren {A - B} }\)





substituting back for $C$ and $D$



$\blacksquare$


Also see
Law of Sines
Law of Cosines


Sources
1968: Murray R. Spiegel: Mathematical Handbook of Formulas and Tables ... (previous) ... (next): $\S 5$: Trigonometric Functions: $5.94$




