# 

Source: https://proofwiki.org/wiki/Law_of_Cosines/Proof_3/Obtuse_Triangle

Theorem
Let $\triangle ABC$ be a triangle whose sides $a, b, c$ are such that:

$a$ is opposite $A$
$b$ is opposite $B$
$c$ is opposite $C$.
Let $\triangle ABC$ be an obtuse triangle such that $A$ is obtuse

Then:

$c^2 = a^2 + b^2 - 2a b \cos C$


Proof
Let $\triangle ABC$ be an obtuse triangle.


Let $AC$ be extended and $BD$ be dropped perpendicular to $AC$.
Let:














\(\ds h\)

\(=\)







\(\ds BD\)




















\(\ds e\)

\(=\)







\(\ds CD\)




















\(\ds f\)

\(=\)







\(\ds AD\)










We have that $\triangle CDB$ and $\triangle ADB$ are right triangles.
Hence:




\(\text {(1)}: \quad\)









\(\ds c^2\)

\(=\)







\(\ds h^2 + f^2\)





Pythagoras's Theorem




\(\text {(2)}: \quad\)









\(\ds a^2\)

\(=\)







\(\ds h^2 + e^2\)





Pythagoras's Theorem




\(\text {(3)}: \quad\)









\(\ds e^2\)

\(=\)







\(\ds \paren {b + f}^2\)




















\(\ds \)

\(=\)







\(\ds b^2 + f^2 + 2 b f\)










\(\text {(4)}: \quad\)









\(\ds e\)

\(=\)







\(\ds a \cos C\)





Definition of Cosine of Angle




Then:














\(\ds c^2\)

\(=\)







\(\ds h^2 + f^2\)





from $(1)$














\(\ds \)

\(=\)







\(\ds a^2 - e^2 + f^2\)





from $(2)$














\(\ds \)

\(=\)







\(\ds a^2 - b^2 - f^2 - 2 b f + f^2\)





substituting for $e^2$ from $(3)$














\(\ds \)

\(=\)







\(\ds a^2 - b^2 - 2 b f + 2 b^2 - 2 b^2\)





simplifying and adding and subtracting  $2 b^2$














\(\ds \)

\(=\)







\(\ds a^2 + b^2 - 2 b \paren {b + f}\)





rearranging














\(\ds \)

\(=\)







\(\ds a^2 + b^2 - 2 a b \cos C\)





using $(4)$ to substitute $b + f = e$ with $a \cos C$



$\blacksquare$


Sources
1953: L. Harwood Clarke: A Note Book in Pure Mathematics ... (previous) ... (next): $\text V$. Trigonometry: The cos formula and the sine formula




