# 

Source: https://proofwiki.org/wiki/Law_of_Cosines/Proof_3/Acute_Triangle

Theorem
Let $\triangle ABC$ be a triangle whose sides $a, b, c$ are such that:

$a$ is opposite $A$
$b$ is opposite $B$
$c$ is opposite $C$.
Let $\triangle ABC$ be an acute triangle.

Then:

$c^2 = a^2 + b^2 - 2a b \cos C$


Proof
Let $\triangle ABC$ be an acute triangle.


Let $BD$ be dropped perpendicular to $AC$.
Let:














\(\ds h\)

\(=\)







\(\ds BD\)




















\(\ds e\)

\(=\)







\(\ds CD\)




















\(\ds f\)

\(=\)







\(\ds AD\)










We have that $\triangle CDB$ and $\triangle ADB$ are right triangles.
Hence:




\(\text {(1)}: \quad\)









\(\ds c^2\)

\(=\)







\(\ds h^2 + f^2\)





Pythagoras's Theorem




\(\text {(2)}: \quad\)









\(\ds a^2\)

\(=\)







\(\ds h^2 + e^2\)





Pythagoras's Theorem




\(\text {(3)}: \quad\)









\(\ds b^2\)

\(=\)







\(\ds \paren {e + f}^2\)




















\(\ds \)

\(=\)







\(\ds e^2 + f^2 + 2ef\)










\(\text {(4)}: \quad\)









\(\ds e\)

\(=\)







\(\ds a \cos C\)





Definition of Cosine of Angle




Then:














\(\ds c^2\)

\(=\)







\(\ds h^2 + f^2\)





from $(1)$














\(\ds \)

\(=\)







\(\ds a^2 - e^2 + f^2\)





from $(2)$














\(\ds \)

\(=\)







\(\ds a^2 - e^2 + f^2 + 2 e^2 - 2 e^2 + 2 e f - 2 e f\)





adding and subtracting $2 e^2$ and $2 e f$














\(\ds \)

\(=\)







\(\ds a^2 + \paren {e^2 + f^2 + 2 e f} - 2 e \paren {e + f}\)





rearanging














\(\ds \)

\(=\)







\(\ds a^2 + b^2 - 2 a b \cos C\)





using $(3)$ to substitute for $b^2$ and $b$, and $(4)$ to substitute $e$ for $a \cos C$



$\blacksquare$


Sources
1953: L. Harwood Clarke: A Note Book in Pure Mathematics ... (previous) ... (next): $\text V$. Trigonometry: The cos formula and the sine formula




