# 

Source: https://proofwiki.org/wiki/Left_Coset_by_Identity



Theorem
Let $G$ be a group whose identity is $e$.
Let $H$ be a subgroup of $G$.

Then:

$e H = H$
where $e H$ is the left coset of $H$ by $e$.


Proof
We have:














\(\ds e H\)

\(=\)







\(\ds \set {y \in G: \exists h \in H: y = e h}\)





Definition of Left Coset of $H$ by $e$














\(\ds \)

\(=\)







\(\ds \set {y \in G: \exists h \in H: y = h}\)





Definition of Identity Element














\(\ds \)

\(=\)







\(\ds \set {y \in G: y \in H}\)




















\(\ds \)

\(=\)







\(\ds H\)










So $e H = H$.
$\blacksquare$


Also see
This is consistent with the definition of the concept of coset by means of the subset product:

$e H = \set e H$


Right Coset by Identity


Sources
1965: J.A. Green: Sets and Groups ... (previous) ... (next): $\S 6.1$. The quotient sets of a subgroup: Example $112$
1966: Richard A. Dean: Elements of Abstract Algebra ... (previous) ... (next): $\S 1.9$: Example $30$
1996: John F. Humphreys: A Course in Group Theory ... (previous) ... (next): Chapter $5$: Cosets and Lagrange's Theorem: Definition $5.1$: Remark $1$




