# 

Source: https://proofwiki.org/wiki/Lemmata_for_Euler%27s_Third_Substitution/Lemma_1

Theorem
Let Euler's third substitution be employed in order to evaluate a primitive of the form:

$\ds \map R {x, \sqrt {a x^2 + b x + c} } \rd x$
where $R$ is a rational function of $x$ and $\sqrt {a x^2 + b x + c}$.
Thus:

$\ds \sqrt {a x^2 + b x + c} = \sqrt {a \paren {x - \alpha} \paren {x - \beta} } = \paren {x - \alpha} t$

Then we have:

$x = \dfrac {a \beta - \alpha t^2} {a - t^2}$


Proof













\(\ds \sqrt {a x^2 + b x + c}\)

\(=\)







\(\ds \sqrt {a \paren {x - \alpha} \paren {x - \beta} }\)




















\(\ds \)

\(=\)







\(\ds \paren {x - \alpha} t\)





by hypothesis








\(\ds \leadsto \ \ \)





\(\ds a \paren {x - \alpha} \paren {x - \beta}\)

\(=\)







\(\ds \paren {x - \alpha}^2 t^2\)





squaring both sides








\(\ds \leadsto \ \ \)





\(\ds a \paren {x - \beta}\)

\(=\)







\(\ds \paren {x - \alpha} t^2\)





simplifying








\(\ds \leadsto \ \ \)





\(\ds a x - a \beta\)

\(=\)







\(\ds x t^2 - \alpha t^2\)





multiplying out








\(\ds \leadsto \ \ \)





\(\ds x \paren {a - t^2}\)

\(=\)







\(\ds a \beta - \alpha t^2\)





rearranging








\(\ds \leadsto \ \ \)





\(\ds x\)

\(=\)







\(\ds \dfrac {a \beta - \alpha t^2} {a - t^2}\)





rearranging



$\blacksquare$


Also see
Definition:Euler's Third Substitution




