# 

Source: https://proofwiki.org/wiki/Length_of_Angle_Bisector/Proof_1

Theorem
Let $\triangle ABC$ be a triangle.
Let $AD$ be the angle bisector of $\angle BAC$ in $\triangle ABC$.


Let $d$ be the length of $AD$.

Then $d$ is given by:

$d^2 = \dfrac {b c} {\paren {b + c}^2} \paren {\paren {b + c}^2 - a^2}$
where $a$, $b$, and $c$ are the sides opposite $A$, $B$ and $C$ respectively.


Proof













\(\ds \frac {BD} {DC}\)

\(=\)







\(\ds \frac c b\)





Angle Bisector Theorem








\(\ds \leadsto \ \ \)





\(\ds \frac {BD} {DC} + 1\)

\(=\)







\(\ds \frac c b + 1\)














\(\ds \leadsto \ \ \)





\(\ds \frac {BD + DC} {DC}\)

\(=\)







\(\ds \frac {b + c} b\)














\(\ds \leadsto \ \ \)





\(\ds \frac a {DC}\)

\(=\)







\(\ds \frac {b + c} b\)














\(\ds \leadsto \ \ \)





\(\ds DC\)

\(=\)







\(\ds \frac {a b} {b + c}\)









Similarly, or by symmetry, we get:

$BD = \dfrac {a c} {b + c}$

From Stewart's Theorem, we have:

$b^2 \cdot BD + c^2 \cdot DC = d^2 \cdot a + BD \cdot DC \cdot a$

Substituting the above expressions for $BD$ and $DC$:














\(\ds b^2 \dfrac {a c} {b + c} + c^2 \frac {a b} {b + c}\)

\(=\)







\(\ds d^2 \cdot a + \dfrac {a c} {b + c} \cdot \frac {a b} {b + c} \cdot a\)














\(\ds \leadsto \ \ \)





\(\ds a b c \frac {b + c} {b + c}\)

\(=\)







\(\ds d^2 \cdot a + \frac{a^2 b c} {\paren {b + c}^2} \cdot a\)














\(\ds \leadsto \ \ \)





\(\ds b c\)

\(=\)







\(\ds d^2 + \frac {a^2 b c} {\paren {b + c}^2}\)














\(\ds \leadsto \ \ \)





\(\ds d^2\)

\(=\)







\(\ds b c \paren {1 - \frac {a^2} {\paren {b + c}^2} }\)














\(\ds \leadsto \ \ \)





\(\ds d^2\)

\(=\)







\(\ds \frac {b c} {\paren {b + c}^2} \paren {\paren {b + c}^2 - a^2}\)









$\blacksquare$





