# 

Source: https://proofwiki.org/wiki/Linear_Second_Order_ODE/y%27%27_-_4_y%27_%2B_4_y_%3D_0/Proof_2

Theorem
The second order ODE:

$(1): \quad y - 4 y' + 4 y = 0$
has the general solution:

$y = C_1 e^{2 x} + C_2 x e^{2 x}$


Proof
It can be seen that $(1)$ is a constant coefficient homogeneous linear second order ODE.
Its auxiliary equation is:

$(2): \quad: m^2 - 4 m + 4 = 0$
From Solution to Quadratic Equation with Real Coefficients, the roots of $(2)$ are:

$m_1 = m_2 = 2$

These are real and equal.
So from Solution of Constant Coefficient Homogeneous LSOODE, the general solution of $(1)$ is:

$y = C_1 e^{2 x} + C_2 x e^{2 x}$
$\blacksquare$


Sources
1972: George F. Simmons: Differential Equations ... (previous) ... (next): $\S 3.17$: Problem $1 \ \text{(e)}$




