# 

Source: https://proofwiki.org/wiki/Linear_Second_Order_ODE/y%27%27_%2B_2_y%27_%2B_10_y_%3D_0

Theorem
The second order ODE:

$(1): \quad y + 2 y' + 10 y = 0$
has the general solution:

$y = e^{-x} \paren {C_1 \cos 3 x + C_2 \sin 3 x}$


Proof
It can be seen that $(1)$ is a constant coefficient homogeneous linear second order ODE.
Its auxiliary equation is:

$(2): \quad: m^2 + 2 m + 10 = 0$
From Solution to Quadratic Equation with Real Coefficients, the roots of $(2)$ are:

$m_1 = -1 + 3 i$
$m_2 = -1 - 3 i$

So from Solution of Constant Coefficient Homogeneous LSOODE, the general solution of $(1)$ is:

$y = e^{-x} \paren {C_1 \cos 3 x + C_2 \sin 3 x}$
$\blacksquare$





