# 

Source: https://proofwiki.org/wiki/Linear_Second_Order_ODE/y%27%27_-_k%5E2_y_%3D_0/Proof_2

Theorem
The second order ODE:

$(1): \quad y - k^2 y = 0$
has the general solution:

$y = C_1 e^{k x} + C_2 e^{-k x}$


Proof
It can be seen that $(1)$ is a constant coefficient homogeneous linear second order ODE.
Its auxiliary equation is:

$(2): \quad m^2 - k^2 = 0$
From Solution to Quadratic Equation with Real Coefficients, the roots of $(2)$ are:

$m_1 = k$
$m_2 = -k$

These are real and unequal.
So from Solution of Constant Coefficient Homogeneous LSOODE, the general solution of $(1)$ is:

$y = C_1 e^{k x} + C_2 e^{-k x}$
$\blacksquare$





