# 

Source: https://proofwiki.org/wiki/Linear_Second_Order_ODE/y%27%27_-_5_y%27_%2B_6_y_%3D_0

Theorem
The linear second order ODE:

$(1): \quad y' ' - 5 y' + 6 y = 0$
has the general solution:

$y = C_1 e^{2 x} + C_2 e^{3 x}$


Proof
It can be seen that $(1)$ is a constant coefficient homogeneous linear second order ODE.
Its auxiliary equation is:

$(2): \quad: m^2 - 5 m + 6 = 0$

From Solution to Quadratic Equation with Real Coefficients, the roots of $(2)$ are:

$m_1 = 2$
$m_2 = 3$
These are real and unequal.

So from Solution of Constant Coefficient Homogeneous LSOODE, the general solution of $(1)$ is:

$y = C_1 e^{2 x} + C_2 e^{3 x}$
$\blacksquare$


Sources
1972: George F. Simmons: Differential Equations ... (previous) ... (next): $1$: The Nature of Differential Equations: $\S 1$: Introduction: $(7)$




