# 

Source: https://proofwiki.org/wiki/Linear_Second_Order_ODE/y%27%27_%2B_2_y%27_%2B_2_y_%3D_0



Theorem
The second order ODE:

$(1): \quad y + 2 y' + 2 y = 0$
has the general solution:

$y = e^{-x} \paren {A \cos x + B \sin x}$


Proof
It can be seen that $(1)$ is a constant coefficient homogeneous linear second order ODE.
Its auxiliary equation is:

$(2): \quad: m^2 + 2 m + 2 = 0$
From Solution to Quadratic Equation with Real Coefficients, the roots of $(2)$ are:

$m_1 = -1 + i$
$m_2 = -1 - i$

These are complex conjugates.
So from Solution of Constant Coefficient Homogeneous LSOODE, the general solution of $(1)$ is:

$y = e^{-x} \paren {A \cos x + B \sin x}$
$\blacksquare$


Verification
The equation:

$(1): \quad y = e^{-x} \paren {A \cos x + B \sin x}$
is a set of solutions to the second order ODE:

$y + 2 y' + 2 y = 0$


Sources
1958: G.E.H. Reuter: Elementary Differential Equations & Operators ... (previous) ... (next): Chapter $1$: Linear Differential Equations with Constant Coefficients: $\S 2$. The second order equation: $\S 2.1$ The reduced equation: Example $1$




