# 

Source: https://proofwiki.org/wiki/Linear_Second_Order_ODE/y%27%27_-_y_%3D_0/Proof_2

Theorem
The second order ODE:

$(1): \quad y - y = 0$
has the general solution:

$y = C_1 e^x + C_2 e^{-x}$


Proof
It can be seen that $(1)$ is a constant coefficient homogeneous linear second order ODE.
Its auxiliary equation is:

$(2): \quad: m^2 - 1 = 0$
From Solution to Quadratic Equation with Real Coefficients, the roots of $(2)$ are:

$m_1 = 1$
$m_2 = -1$

These are real and unequal.
So from Solution of Constant Coefficient Homogeneous LSOODE, the general solution of $(1)$ is:

$y = C_1 e^x + C_2 e^{- x}$
$\blacksquare$





