# 

Source: https://proofwiki.org/wiki/Linear_Second_Order_ODE/y%27%27_-_2_y%27_%2B_y_%3D_0

Theorem
The second order ODE:

$(1): \quad y - 2 y' + y = 0$
has the general solution:

$y = C_1 e^x + C_2 x e^x$


Proof
It can be seen that $(1)$ is a constant coefficient homogeneous linear second order ODE.
Its auxiliary equation is:

$(2): \quad: m^2 - 2 m + 1 = 0$
From Solution to Quadratic Equation with Real Coefficients, the roots of $(2)$ are:

$m_1 = m_2 = 1$

These are real and equal.
So from Solution of Constant Coefficient Homogeneous LSOODE, the general solution of $(1)$ is:

$y = C_1 e^x + C_2 x e^x$
$\blacksquare$





