# 

Source: https://proofwiki.org/wiki/Linear_First_Order_ODE/(1_%2B_x%5E2)_y%27_%2B_2_x_y_%3D_4_x%5E3

Theorem
The linear first order ODE:

$\paren {1 + x^2} \dfrac {\d y} {\d x} + 2 x y = 4 x^3$
has the general solution:

$y = \dfrac {x^4} {1 + x^2} + \dfrac C {1 + x^2}$


Proof
It is noticed that:

$\dfrac {\d} {\d x} \paren {1 + x^2} = 2 x$
and so $(1)$ can be rendered in the form:














\(\ds \map \d {\paren {1 + x^2} y}\)

\(=\)







\(\ds 4 x^3\)














\(\ds \leadsto \ \ \)





\(\ds \paren {1 + x^2} y\)

\(=\)







\(\ds \int 4 x^3 \rd x\)




















\(\ds \)

\(=\)







\(\ds x^4 + C\)














\(\ds \leadsto \ \ \)





\(\ds y\)

\(=\)







\(\ds \frac {x^4} {1 + x^2} + \frac C {1 + x^2}\)









$\blacksquare$


Sources
1972: George F. Simmons: Differential Equations ... (previous) ... (next): Miscellaneous Problems for Chapter $2$: Problem $21$




