# 

Source: https://proofwiki.org/wiki/Linear_First_Order_ODE/y%27_%3D_x_%2B_y/y(0)_%3D_1

Theorem
The linear first order ODE:

$(1): \quad \dfrac {\d y} {\d x} = x + y$
with initial condition:

$\map y 0 = 1$
has the particular solution:

$y = 2 e^x - x - 1$


Proof
From Linear First Order ODE: $y' = x + y$, the general solution of $(1)$ is:

$y = C e^x - x - 1$
Setting $y = 1$ when $x = 0$ gives:

$1 = C + 1$
from which $C = 2$.
Hence the result.
$\blacksquare$


Sources
1972: George F. Simmons: Differential Equations ... (previous) ... (next): Miscellaneous Problems for Chapter $2$: Appendix $\text{A}$. Numerical Methods




