# 

Source: https://proofwiki.org/wiki/Linear_Diophantine_Equation/Examples/2x_%2B_3y_%3D_4



Example of Linear Diophantine Equation
The linear diophantine equation:

$2 x + 3 y = 4$
has the general solution:

$x = -4 + 3 t, y = 4 - 2 t$


Graphical Presentation



Proof
We have that:

$\gcd \set {2, 3} = 1$
which is (trivially) a divisor of $4$.
So, from Solution of Linear Diophantine Equation, a solution exists.

First we find a single solution to $2 x + 3 y = 4$:














\(\ds 1\)

\(=\)







\(\ds 1 \times 3 - 1 \times 2\)














\(\ds \leadsto \ \ \)





\(\ds 4\)

\(=\)







\(\ds 4 \times 3 - 4 \times 2\)










and so:














\(\ds x_0\)

\(=\)







\(\ds -4\)




















\(\ds y_0\)

\(=\)







\(\ds 4\)









is a solution.

From Solution of Linear Diophantine Equation, the general solution is:

$\forall t \in \Z: x = x_0 + \dfrac b d t, y = y_0 - \dfrac a d t$
where $d = \gcd \set {a, b}$.
In this case:














\(\ds x_0\)

\(=\)







\(\ds -4\)




















\(\ds y_0\)

\(=\)







\(\ds 4\)




















\(\ds a\)

\(=\)







\(\ds 2\)




















\(\ds b\)

\(=\)







\(\ds 3\)




















\(\ds d\)

\(=\)







\(\ds 1\)










giving:














\(\ds x\)

\(=\)







\(\ds -4 + 3 t\)




















\(\ds y\)

\(=\)







\(\ds 4 - 2 t\)









$\blacksquare$


Sources
1971: George E. Andrews: Number Theory ... (previous) ... (next): $\text {2-3}$ The Linear Diophantine Equation: Exercise $1 \ \text {(a)}$




