# 

Source: https://proofwiki.org/wiki/Linear_Second_Order_ODE/y%27%27_-_2_y%27_-_3_y_%3D_0

Theorem
The second order ODE:

$(1): \quad y - 2 y' - 3 y = 0$
has the general solution:

$y = C_1 e^{3 x} + C_2 e^{-x}$


Proof
It can be seen that $(1)$ is a constant coefficient homogeneous linear second order ODE.
Its auxiliary equation is:

$(2): \quad: m^2 - 2 m - 3 = 0$
From Solution to Quadratic Equation with Real Coefficients, the roots of $(2)$ are:

$m_1 = 3$
$m_2 = -1$

These are real and unequal.
So from Solution of Constant Coefficient Homogeneous LSOODE, the general solution of $(1)$ is:

$y = C_1 e^{3 x} + C_2 e^{-x}$
$\blacksquare$





