# 

Source: https://proofwiki.org/wiki/Logarithm_of_Power/Natural_Logarithm/Proof_2

Theorem
Let $x \in \R$ be a strictly positive real number.
Let $a \in \R$ be a real number such that $a > 1$.
Let $r \in \R$ be any real number.
Let $\ln x$ be the natural logarithm of $x$.

Then:

$\map \ln {x^r} = r \ln x$


Proof













\(\ds \ln a\)

\(=\)







\(\ds b\)














\(\ds \leadstoandfrom \ \ \)





\(\ds e^b\)

\(=\)







\(\ds a\)














\(\ds \leadsto \ \ \)





\(\ds \paren {e^b}^c\)

\(=\)







\(\ds a^c\)














\(\ds \leadsto \ \ \)





\(\ds e^{c b}\)

\(=\)







\(\ds a^c\)





Exponential of Product








\(\ds \leadsto \ \ \)





\(\ds \ln e^{c b}\)

\(=\)







\(\ds \ln a^c\)














\(\ds \leadsto \ \ \)





\(\ds c b\)

\(=\)







\(\ds \ln a^c\)





Exponential of Natural Logarithm




By hypothesis, $\ln a = b$.
Multiplying both sides by $c$:

$c \ln a = c b$
But we proved above that:

$c b = \ln a^c$
$\blacksquare$


Sources
For a video presentation of the contents of this page, visit the Khan Academy.




