# 

Source: https://proofwiki.org/wiki/Median_Formula/Proof_1

Theorem
Let $\triangle ABC$ be a triangle.
Let $CD$ be the median of $\triangle ABC$ which bisects $AB$.


The length $m_c$ of $CD$ is given by:

${m_c}^2 = \dfrac {a^2 + b^2} 2 - \dfrac {c^2} 4$


Proof













\(\ds a^2 \cdot AD + b^2 \cdot DB\)

\(=\)







\(\ds CD^2 \cdot c + AD \cdot DB \cdot c\)





Stewart's Theorem








\(\ds \leadsto \ \ \)





\(\ds a^2 \frac c 2 + b^2 \frac c 2\)

\(=\)







\(\ds {m_c}^2 \cdot c + \paren {\frac c 2}^2 c\)





substituting $AD = DB = \dfrac c 2$ and $CD = m_c$








\(\ds \leadsto \ \ \)





\(\ds \frac c 2 \paren {a^2 + b^2}\)

\(=\)







\(\ds m_c^2 \cdot c + \frac {c^2} 4 \cdot c\)














\(\ds \leadsto \ \ \)





\(\ds \frac {a^2 + b^2} 2\)

\(=\)







\(\ds m_c^2 + \frac {c^2} 4\)














\(\ds \leadsto \ \ \)





\(\ds {m_c}^2\)

\(=\)







\(\ds \frac {a^2 + b^2} 2 - \frac {c^2} 4\)





after algebra



$\blacksquare$





