# 

Source: https://proofwiki.org/wiki/Modulo_Operation/Examples/0.11_mod_0.1/Proof_2

Theorem
$0 \cdotp 11 \bmod 0 \cdotp 1 = 0 \cdotp 01$


Proof
From Modulo Operation: $1 \cdotp 1 \bmod 1$:

$1 \cdotp 1 \bmod 1 = 0 \cdotp 1$

From Product Distributes over Modulo Operation:

$z \left({x \bmod y}\right) = \left({z x}\right) \bmod \left({z y}\right)$
and so:














\(\ds 0 \cdotp 11 \bmod 0 \cdotp 1\)

\(=\)







\(\ds 0 \cdotp 1 \left({1 \cdotp 1 \bmod 1}\right)\)




















\(\ds \)

\(=\)







\(\ds 0 \cdotp 1 \times 0 \cdotp 1\)




















\(\ds \)

\(=\)







\(\ds 0 \cdotp 01\)









$\blacksquare$





