# 

Source: https://proofwiki.org/wiki/Modus_Ponendo_Ponens/Sequent_Form/Proof_1

Theorem













\(\ds p\)

\(\implies\)







\(\ds q\)




















\(\ds p\)

\(\)







\(\ds \)














\(\ds \vdash \ \ \)





\(\ds q\)

\(\)







\(\ds \)











Proof
By the tableau method of natural deduction:


$p \implies q, p \vdash q$


Line


Pool

Formula

Rule

Depends upon

Notes


1


1

$p \implies q$

Premise

(None)




2


2

$p$

Premise

(None)




3


1, 2

$q$

Modus Ponendo Ponens: $\implies \mathcal E$

1, 2


$\blacksquare$


Sources
1965: E.J. Lemmon: Beginning Logic ... (previous) ... (next): Chapter $1$: The Propositional Calculus $1$: $2$ Conditionals and Negation: Theorem $1$




