# 

Source: https://proofwiki.org/wiki/Modulo_Operation/Examples/0.11_mod_0.1/Proof_1

Theorem
$0 \cdotp 11 \bmod 0 \cdotp 1 = 0 \cdotp 01$


Proof
By definition of modulo operation:

$x \bmod yÂ := x - y \floor {\dfrac x y}$
for $y \ne 0$.

We have:














\(\ds \dfrac {0 \cdotp 11} {0 \cdotp 1}\)

\(=\)







\(\ds \dfrac {1 \cdotp 1} 1\)




















\(\ds \)

\(=\)







\(\ds 1 \cdotp 1\)









and so:

$\floor {\dfrac {0 \cdotp 11} {0 \cdotp 1} } = 1$

Thus:














\(\ds 0 \cdotp 11 \bmod 0 \cdotp 1\)

\(=\)







\(\ds 0 \cdotp 11 - 0 \cdotp 1 \times \floor {\dfrac {0 \cdotp 11} {0 \cdotp 1} }\)




















\(\ds \)

\(=\)







\(\ds 0 \cdotp 11 - 0 \cdotp 1 \times 1\)




















\(\ds \)

\(=\)







\(\ds 0 \cdotp 01\)









$\blacksquare$





