# 

Source: https://proofwiki.org/wiki/Multiple_of_Sine_plus_Multiple_of_Cosine/Cosine_Form

Theorem
$p \sin x + q \cos x = \sqrt {p^2 + q^2} \map \cos {x + \arctan \dfrac {-p} q}$


Proof
Let it be assumed that $p \sin x + q \cos x$ can be expressed in the form $M \map \cos {x + \phi}$.

Then:














\(\ds p \sin x + q \cos x\)

\(=\)







\(\ds M \map \cos {x + \phi}\)














\(\ds \leadsto \ \ \)





\(\ds \frac p M \sin x + \frac q M \cos x\)

\(=\)







\(\ds \map \cos {x + \phi}\)




















\(\ds \)

\(=\)







\(\ds \cos x \cos \phi - \sin x \sin \phi\)





Cosine of Sum








\(\ds \leadsto \ \ \)





\(\ds \sin x \sin \phi\)

\(=\)







\(\ds \frac {-p} M \sin x\)





equating terms in $\sin x$














\(\ds \cos x \cos \phi\)

\(=\)







\(\ds \frac q M \cos x\)





and $\cos x$




\(\text {(1)}: \quad\)



\(\ds \leadsto \ \ \)





\(\ds \sin \phi\)

\(=\)







\(\ds \frac {-p} M\)










\(\text {(2)}: \quad\)









\(\ds \cos \phi\)

\(=\)







\(\ds \frac q M\)














\(\ds \leadsto \ \ \)





\(\ds \sin^2 \phi + \cos^2 \phi\)

\(=\)







\(\ds \paren {\frac {-p} M}^2 + \paren {\frac q M}^2\)





squaring and adding $(1)$ and $(2)$








\(\ds \leadsto \ \ \)





\(\ds 1\)

\(=\)







\(\ds \frac {p^2 + q^2} {M^2}\)














\(\ds \leadsto \ \ \)





\(\ds \sqrt {p^2 + q^2}\)

\(=\)







\(\ds M\)










Then:














\(\ds \tan \phi\)

\(=\)







\(\ds \frac {\sin \phi} {\cos \phi}\)





Tangent is Sine divided by Cosine














\(\ds \)

\(=\)







\(\ds \frac {-p / M} {q / M}\)





from $(1)$ and $(2)$














\(\ds \)

\(=\)







\(\ds \frac {-p} q\)





simplifying




Hence the result.
$\blacksquare$





