# 

Source: https://proofwiki.org/wiki/N_less_than_M_to_the_N

Theorem
$\forall m, n \in \Z_{>0}: m > 1 \implies n < m^n$


Proof













\(\ds n\)

\(=\)







\(\ds \underbrace {1 + 1 + \cdots + 1}_{\text {$n$ times} }\)




















\(\ds \)

\(<\)







\(\ds 1 + m + m^2 + \cdots + m^{n - 1}\)





as $m > 1$














\(\ds \)

\(=\)







\(\ds \frac {m^n - 1} {m - 1}\)





Sum of Geometric Sequence














\(\ds \)

\(\le\)







\(\ds m^n - 1\)





as $m - 1 \ge 1$














\(\ds \)

\(<\)







\(\ds m^n\)









$\blacksquare$


Sources
1971: George E. Andrews: Number Theory ... (previous) ... (next): $\text {1-1}$ Principle of Mathematical Induction: Corollary $\text {1-1}$




