# 

Source: https://proofwiki.org/wiki/N_(n_%2B_1)_(2n_%2B_1)_over_6_is_Integer

Theorem
Let $n \in \Z$ be an integer.

Then $\dfrac {n \paren {n + 1} \paren {2 n + 1} } 6$ is also an integer.


Proof
This is equivalent to proving that $n \paren {n + 1} \paren {2 n + 1}$ is a multiple of $6$.

There are $6$ cases to consider:

$(1): \quad n \equiv 0 \pmod 6$: we have $n = 6 k$
$(2): \quad n \equiv 1 \pmod 6$: we have $n = 6 k + 1$
$(3): \quad n \equiv 2 \pmod 6$: we have $n = 6 k + 2$
$(4): \quad n \equiv 3 \pmod 6$: we have $n = 6 k + 3$
$(5): \quad n \equiv 4 \pmod 6$: we have $n = 6 k + 4$
$(6): \quad n \equiv 5 \pmod 6$: we have $n = 6 k + 5$





\(\text {(1)}: \quad\)









\(\ds n\)

\(=\)







\(\ds 6 k\)














\(\ds \leadsto \ \ \)





\(\ds n \paren {n + 1} \paren {2 n + 1}\)

\(=\)







\(\ds \paren {6 k} \paren {6 k + 1} \paren {2 \paren {6 k} + 1}\)




















\(\ds \)

\(=\)







\(\ds 6 \paren {k \paren {6 k + 1} \paren {12 k + 1} }\)














\(\ds \leadsto \ \ \)





\(\ds n \paren {n + 1} \paren {2 n + 1}\)

\(\equiv\)







\(\ds 0 \pmod 6\)









$\Box$





\(\text {(2)}: \quad\)









\(\ds n\)

\(=\)







\(\ds 6 k + 1\)














\(\ds \leadsto \ \ \)





\(\ds n \paren {n + 1} \paren {2 n + 1}\)

\(=\)







\(\ds \paren {6 k + 1} \paren {6 k + 2} \paren {2 \paren {6 k + 1} + 1}\)




















\(\ds \)

\(=\)







\(\ds \paren {6 k + 1} \paren {6 k + 2} \paren {12 k + 3}\)




















\(\ds \)

\(=\)







\(\ds \paren {6 k + 1} \paren {2 \paren {3 k + 1} } \paren {3 \paren {4 k + 1} }\)




















\(\ds \)

\(=\)







\(\ds 6 \paren {6 k + 1} \paren {3 k + 1} \paren {4 k + 1}\)














\(\ds \leadsto \ \ \)





\(\ds n \paren {n + 1} \paren {2 n + 1}\)

\(\equiv\)







\(\ds 0 \pmod 6\)









$\Box$





\(\text {(3)}: \quad\)









\(\ds n\)

\(=\)







\(\ds 6 k + 2\)














\(\ds \leadsto \ \ \)





\(\ds n \paren {n + 1} \paren {2 n + 1}\)

\(=\)







\(\ds \paren {6 k + 2} \paren {6 k + 3} \paren {2 \paren {6 k + 2} + 1}\)




















\(\ds \)

\(=\)







\(\ds \paren {2 \paren {3 k + 1} } \paren {3 \paren {2 k + 1} } \paren {12 k + 5}\)




















\(\ds \)

\(=\)







\(\ds 6 \paren {3 k + 1} \paren {2 k + 1} \paren {12 k + 5}\)














\(\ds \leadsto \ \ \)





\(\ds n \paren {n + 1} \paren {2 n + 1}\)

\(\equiv\)







\(\ds 0 \pmod 6\)









$\Box$





\(\text {(4)}: \quad\)









\(\ds n\)

\(=\)







\(\ds 6 k + 3\)














\(\ds \leadsto \ \ \)





\(\ds n \paren {n + 1} \paren {2 n + 1}\)

\(=\)







\(\ds \paren {6 k + 3} \paren {6 k + 4} \paren {2 \paren {6 k + 3} + 1}\)




















\(\ds \)

\(=\)







\(\ds \paren {3 \paren {2 k + 1} } \paren {2 \paren {3 k + 2} } \paren {12 k + 7}\)




















\(\ds \)

\(=\)







\(\ds 6 \paren {2 k + 1} \paren {3 k + 2} \paren {12 k + 7}\)














\(\ds \leadsto \ \ \)





\(\ds n \paren {n + 1} \paren {2 n + 1}\)

\(\equiv\)







\(\ds 0 \pmod 6\)









$\Box$





\(\text {(5)}: \quad\)









\(\ds n\)

\(=\)







\(\ds 6 k + 4\)














\(\ds \leadsto \ \ \)





\(\ds n \paren {n + 1} \paren {2 n + 1}\)

\(=\)







\(\ds \paren {6 k + 4} \paren {6 k + 5} \paren {2 \paren {6 k + 4} + 1}\)




















\(\ds \)

\(=\)







\(\ds \paren {6 k + 4} \paren {6 k + 5} \paren {12 k + 9}\)




















\(\ds \)

\(=\)







\(\ds \paren {2 \paren {3 k + 2} } \paren {6 k + 5} \paren {3 \paren {4 k + 3} }\)




















\(\ds \)

\(=\)







\(\ds 6 \paren {3 k + 2} \paren {6 k + 5} \paren {4 k + 3}\)














\(\ds \leadsto \ \ \)





\(\ds n \paren {n + 1} \paren {2 n + 1}\)

\(\equiv\)







\(\ds 0 \pmod 6\)









$\Box$





\(\text {(6)}: \quad\)









\(\ds n\)

\(=\)







\(\ds 6 k + 5\)














\(\ds \leadsto \ \ \)





\(\ds n \paren {n + 1} \paren {2 n + 1}\)

\(=\)







\(\ds \paren {6 k + 5} \paren {6 k + 6} \paren {2 \paren {6 k + 5} + 1}\)




















\(\ds \)

\(=\)







\(\ds 6 \paren {6 k + 5} \paren {k + 1} \paren {12 k + 11}\)














\(\ds \leadsto \ \ \)





\(\ds n \paren {n + 1} \paren {2 n + 1}\)

\(\equiv\)







\(\ds 0 \pmod 6\)









$\blacksquare$


Sources
1980: David M. Burton: Elementary Number Theory (revised ed.) ... (previous) ... (next): Chapter $2$: Divisibility Theory in the Integers: $2.1$ The Division Algorithm: Problems $2.1$: $4$




