# 

Source: https://proofwiki.org/wiki/Nakayama%27s_Lemma/Proof_1

Theorem
Let $A$ be a commutative ring with unity.
Let $M$ be a finitely generated $A$-module. 
Let $\map {\operatorname{Jac} } A$ be the Jacobson radical of $A$.
Let $\mathfrak a \subseteq \map {\operatorname{Jac} } A$ be an ideal of $A$.
Suppose $\mathfrak a M = M$.

Then:

$M = 0$


Proof
We induct on the number of generators of $M$. 


Basis for the Induction
Let $M$ have a single generator $m_1 \in M$.
Then $\mathfrak a m_1 = M$.
So:

$m_1 \in \mathfrak a m_1$
That is:

$m_1 = a m_1$
for some $a \in \mathfrak a$.
By Characterisation of Jacobson Radical, $1 - a$ is a unit in $A$.
So:

$\paren {1 - a}^{-1} \paren {1 - a} m = 0$
thus $m = 0$.


Inductive Step
Suppose that $M$ is generated by $n$ elements:

$M = A m_1 + \dotsb + A m_n$
for some $m_1, \dotsc, m_n \in M$.
Then we have:

$M = \mathfrak a M = \mathfrak a m_1 + \dotsb + \mathfrak a m_n $
Thus for some $a_1, \dotsc, a_n \in \mathfrak a$:

$ m_1 = a_1 m_1 + \dotsb + a_n m_n $
Then:

$\paren {1 - a_1} m_1 = a_2 m_2 + \dotsb + a_n m_n$
By Characterisation of Jacobson Radical, $1 - a$ is a unit in $A$.
Multiplying both sides by $\paren {1 - a_1}^{-1}$ gives:

$m_1 = \paren {1 - a_1}^{-1} a_2 m_2 + \dotsb + \paren {1 - a_1}^{-1} a_n m_n$
so we have:

$m_1 \in A m_2 + \cdots + A m_n$
Therefore $M$ has $n - 1$ generators $m_2, \dotsc, m_n$.
By the induction hypothesis:

$\mathfrak a M = M \implies M = 0$
$\blacksquare$





