# 

Source: https://proofwiki.org/wiki/Natural_Logarithm_of_1_is_0



Theorem
$\ln 1 = 0$
where $\ln 1$ denotes the natural logarithm of $1$.


Proof 1
We use the definition of the natural logarithm as an integral:

$\ds \ln x = \int_1^x \frac {\d t} t$
From Integral on Zero Interval:

$\ds \ln 1 = \int_1^1 \frac {\d t} t = 0$
$\blacksquare$


Proof 2
We use the definition of the natural logarithm as the inverse of the exponential:

$\ln x = y \iff e^y = x$

Then:














\(\ds e^0\)

\(=\)







\(\ds 1\)





Exponential of Zero








\(\ds \leadstoandfrom \ \ \)





\(\ds \ln 1\)

\(=\)







\(\ds 0\)









$\blacksquare$


Proof 3
We use the definition of the natural logarithm as the limit of a sequence:

$\ds \ln x = \lim_{n \mathop \to \infty} n \paren {\sqrt [n] x - 1}$
Then:














\(\ds \ln 1\)

\(=\)







\(\ds \lim_{n \mathop \to \infty} n \paren {\sqrt [n] 1 - 1}\)




















\(\ds \)

\(=\)







\(\ds \lim_{n \mathop \to \infty} n \times 0\)




















\(\ds \)

\(=\)







\(\ds \lim_{n \mathop \to \infty} 0\)




















\(\ds \)

\(=\)







\(\ds 0\)









$\blacksquare$





