# 

Source: https://proofwiki.org/wiki/Natural_Logarithm_of_1_is_0/Proof_3

Theorem
$\ln 1 = 0$


Proof
We use the definition of the natural logarithm as the limit of a sequence:

$\ds \ln x = \lim_{n \mathop \to \infty} n \paren {\sqrt [n] x - 1}$
Then:














\(\ds \ln 1\)

\(=\)







\(\ds \lim_{n \mathop \to \infty} n \paren {\sqrt [n] 1 - 1}\)




















\(\ds \)

\(=\)







\(\ds \lim_{n \mathop \to \infty} n \times 0\)




















\(\ds \)

\(=\)







\(\ds \lim_{n \mathop \to \infty} 0\)




















\(\ds \)

\(=\)







\(\ds 0\)









$\blacksquare$





