# 

Source: https://proofwiki.org/wiki/Opposite_Ring_of_Opposite_Ring

Theorem
Let $\struct {R, +, \times}$ be a ring.
Let $\struct {R, +, *}$ be the opposite ring of $\struct {R, +, \times}$.
Let $\struct {R, +, \circ}$ be the opposite ring of $\struct {R, +, *}$.

Then $\struct {R, +, \circ} = \struct {R, +, \times}$.


Proof
By definition of the opposite ring:

$\forall x, y \in S: x * y = y \times x$
$\forall x, y \in S: x \circ y = y * x$
Hence for all $x,y \in S$:

$x \circ y = y * x = x \times y$
The result follows.
$\blacksquare$





