# 

Source: https://proofwiki.org/wiki/P-Product_Metrics_on_Real_Vector_Space_are_Topologically_Equivalent/Inequality_for_General_Case

Theorem
For $n \in \N$, let $\R^n$ be a real vector Space.
Let $r, t \in \R_{\ge 1}$.
Let $d_r$ and $d_t$ be $p$-product metrics on $\R^n$.

Then $d_r$ and $d_t$ are topologically equivalent.


Proof
Without loss of generality, assume that $r \le t$.
We show that $\ds \map {d_r} {x, y} \ge \map {d_t} {x, y}$, which is equivalent to proving that:

$\ds \paren {\sum_{i \mathop = 1}^n \size {x_i - y_i}^r}^{1/r} \ge \paren {\sum_{i \mathop = 1}^n \size {x_i - y_i}^t}^{1/t}$

Let $\forall i \in \closedint 1 n: s_i = \size {x_i - y_i}$.
Suppose $s_k = 0$ for some $k \in \closedint 1 n$.


Although this article appears correct, it's inelegant. There has to be a better way of doing it.In particular: Putting off the analysis of s_k being 0 until near the end of the proof should shorten it without losing any clarity.You can help $\mathsf{Pr} \infty \mathsf{fWiki}$ by redesigning it.To discuss this page in more detail, feel free to use the talk page.When this work has been completed, you may remove this instance of {{Improve}} from the code.If you would welcome a second opinion as to whether your work is correct, add a call to {{Proofread}} the page.
Then the problem reduces to the equivalent one of showing that:

$\ds \paren {\sum_{i \mathop = 1}^{n - 1} \size {x_i - y_i}^r}^{1/r} \ge \paren {\sum_{i \mathop = 1}^{n - 1} \size {x_i - y_i}^t}^{1/t}$
that is, of reducing the index by $1$.
Note that when $n = 1$, from simple algebra $\map {d_r} {x, y} = \map {d_t} {x, y}$.

So, let us start with the assumption that $\forall i \in \closedint 1 n: s_i > 0$.
Let $\ds u = \sum_{i \mathop = 1}^n \size {x_i - y_i}^r = \sum_{i \mathop = 1}^n s_i^r$, and $v = \dfrac 1 r$.
From Derivative of Function to Power of Functionâ€Ž, $\map {D_r} {u^v} = v u^{v - 1} \map {D_r} u + u^v \ln u \map {D_r} v$.
Here:

$\ds \map {D_r} u = \sum_{i \mathop = 1}^n s_i^r \ln s_i$ from Derivative of Exponential Function and Sum Rule for Derivatives
$\map {D_r} v = - \dfrac 1 {r^2}$ from Power Rule for Derivatives
In the case where $r = 1$, we have:

$\map {D_r} {u^v} = 0$
When $r > 1$, we have:














\(\ds \map {D_r} {\paren {\sum_{i \mathop = 1}^n s_i^r}^{1 / r} }\)

\(=\)







\(\ds \dfrac 1 r \paren {\sum_{i \mathop = 1}^n s_i^r}^{1 / \paren {r - 1} } \paren {\sum_{i \mathop = 1}^n s_i^r \ln s_i} - \dfrac {\paren {\sum_{i \mathop = 1}^n s_i^r}^{1/r} \map \ln {\sum_{i \mathop = 1}^n s_i^r} } {r^2}\)




















\(\ds \)

\(=\)







\(\ds \dfrac {\paren {\sum_{i \mathop = 1}^n s_i^r}^{1 / r} } r \paren {\dfrac {\sum_{i \mathop = 1}^n s_i^r \ln s_i} {\sum_{i \mathop = 1}^n s_i^r} - \dfrac {\map \ln {\sum_{i \mathop = 1}^n s_i^r} } r}\)




















\(\ds \)

\(=\)







\(\ds \dfrac {\paren {\sum_{i \mathop = 1}^n s_i^r}^{1 / r} } r \paren {\dfrac {r \paren {\sum_{i \mathop = 1}^n s_i^r \ln s_i} - \paren {\sum_{i \mathop = 1}^n s_i^r} \map \ln {\sum_{i \mathop = 1}^n s_i^r} } {r \paren {\sum_{i \mathop = 1}^n s_i^r} } }\)




















\(\ds \)

\(=\)







\(\ds K \paren {r \paren {\sum_{i \mathop = 1}^n s_i^r \ln s_i} - \paren {\sum_{i \mathop = 1}^n s_i^r} \map \ln {\sum_{i \mathop = 1}^n s_i^r} }\)





where $\ds K = \dfrac {\paren {\sum_{i \mathop = 1}^n s_i^r}^{1 / r} } {r^2 \paren {\sum_{i \mathop = 1}^n s_i^r} } > 0$














\(\ds \)

\(=\)







\(\ds K \paren {\sum_{i \mathop = 1}^n s_i^r \map \ln {s_i^r} - \paren {\sum_{i \mathop = 1}^n s_i^r} \map \ln {\sum_{i \mathop = 1}^n s_i^r} }\)





Logarithms of Powers














\(\ds \)

\(=\)







\(\ds K \paren {\sum_{j \mathop = 1}^n \paren {s_j^r \paren {\map \ln {s_j^r} - \map \ln {\sum_{i \mathop = 1}^n s_i^r} } } }\)




















\(\ds \)

\(=\)







\(\ds K \paren {\sum_{j \mathop = 1}^n \paren {s_j^r \map \ln {\frac {s_j^r} {\sum_{i \mathop = 1}^n s_i^r} } } }\)









where $K > 0$ because all of $s_i, r > 0$.
For the same reason, $\ds \dfrac{s_j^r} {\sum_{i \mathop = 1}^n s_i^r} < 1$ for all $j \in \set {1, \ldots, n}$.
From Logarithm of 1 is 0 and Logarithm is Strictly Increasing, their logarithms are therefore negative.
So for $r > 1$:

$\ds \map {D_r} {\paren {\sum_{i \mathop = 1}^n s_i^r}^{1 / r} } < 0$
So, from Derivative of Monotone Function, it follows that (given the conditions on $r$ and $s_i$) $\ds \paren {\sum_{i \mathop = 1}^n s_i^r}^{1 / r}$ is decreasing.

As we assumed $r \le t$, we have $\map {d_r} {x, y} \ge \map {d_t} {x, y}$.
$\blacksquare$





