# 

Source: https://proofwiki.org/wiki/Partial_Fractions_Expansion/Examples/Arbitrary_Example_1

Example of Partial Fractions Expansion
$\dfrac 1 {x \paren {x + 1}^2} = \dfrac 1 x - \dfrac 1 {\paren {x + 1} } - \dfrac 1 {\paren {x + 1}^2}$


Proof













\(\ds \dfrac 1 {x \paren {x + 1}^2}\)

\(=\)







\(\ds \dfrac A x + \dfrac B {\paren {x + 1} } + \dfrac C {\paren {x + 1}^2}\)




















\(\ds \)

\(=\)







\(\ds \dfrac {A \paren {x + 1}^2 + B x \paren {x + 1} + C x} {x \paren {x + 1}^2}\)




















\(\ds \)

\(=\)







\(\ds \dfrac {A \paren {x^2 + 2x + 1} + B \paren {x^2 + x} + C x} {x \paren {x + 1}^2}\)




















\(\ds \)

\(=\)







\(\ds \dfrac {\paren {A + B} x^2 + \paren {2A + B + C} x + A} {x \paren {x + 1}^2}\)




















\(\ds A\)

\(=\)







\(\ds 1\)




















\(\ds \paren {A + B}\)

\(=\)







\(\ds 0\)





$x^2$ term vanishes








\(\ds \leadsto \ \ \)





\(\ds B\)

\(=\)







\(\ds -1\)




















\(\ds \paren {2A + B + C}\)

\(=\)







\(\ds 0\)





$x$ term vanishes








\(\ds \leadsto \ \ \)





\(\ds C\)

\(=\)







\(\ds -1\)










Therefore:

$\dfrac 1 {x \paren {x + 1}^2} = \dfrac 1 x - \dfrac 1 {\paren {x + 1} } - \dfrac 1 {\paren {x + 1}^2}$
$\blacksquare$





