# 

Source: https://proofwiki.org/wiki/Partial_Fractions_Expansion/Examples/Arbitrary_Example_2

Example of Partial Fractions Expansion
$\dfrac {x + 3} {x^2 + 3 x + 2} = \dfrac 2 {x + 1} -\dfrac 1 {x + 2}$


Proof













\(\ds \dfrac {x + 3} {x^2 + 3 x + 2}\)

\(=\)







\(\ds \dfrac {x + 3} {\paren {x + 1} \paren {x + 2} }\)




















\(\ds \)

\(=\)







\(\ds \dfrac A {x + 1} + \dfrac B {x + 2}\)





where $A$ and $B$ are to be found














\(\ds \)

\(=\)







\(\ds \dfrac {A \paren {x + 1} + B \paren {x + 2} } {\paren {x + 1} \paren {x + 2} }\)





multiplying out








\(\ds \leadsto \ \ \)





\(\ds x + 3\)

\(=\)







\(\ds A \paren {x + 1} + B \paren {x + 2}\)














\(\ds \leadsto \ \ \)





\(\ds 3\)

\(=\)







\(\ds A + 2 B\)





setting $x = 0$














\(\ds 1\)

\(=\)







\(\ds A + B\)





equating coefficients of $x$








\(\ds \leadsto \ \ \)





\(\ds A\)

\(=\)







\(\ds -1\)





solving the simultaneous equations














\(\ds B\)

\(=\)







\(\ds 2\)










Therefore:

$\dfrac {x + 3} {x^2 + 3 x + 2} = \dfrac 2 {x + 1} -\dfrac 1 {x + 2}$
$\blacksquare$


Sources
1998: David Nelson: The Penguin Dictionary of Mathematics (2nd ed.) ... (previous) ... (next): partial fractions
2008: David Nelson: The Penguin Dictionary of Mathematics (4th ed.) ... (previous) ... (next): partial fractions




