# 

Source: https://proofwiki.org/wiki/Partial_Derivatives_of_u%5E2_%2B_x%5E2_%2B_y%5E2,_u_-_v%5E3_%2B_3_x

Theorem
Let:














\(\ds u^2 + x^2 + y^2\)

\(=\)







\(\ds 3\)




















\(\ds u - v^3 + 3 x\)

\(=\)







\(\ds 4\)









Then:














\(\ds \dfrac {\partial u} {\partial x}\)

\(=\)







\(\ds -\dfrac x u\)




















\(\ds \dfrac {\partial u} {\partial y}\)

\(=\)







\(\ds -\dfrac y u\)




















\(\ds \dfrac {\partial v} {\partial x}\)

\(=\)







\(\ds \dfrac {x - 3 u} {3 u v^2}\)




















\(\ds \dfrac {\partial v} {\partial y}\)

\(=\)







\(\ds \dfrac y {3 u v^2}\)











Proof













\(\ds 2 u \dfrac {\partial u} {\partial x} + 2 x\)

\(=\)







\(\ds 0\)










\(\text {(1)}: \quad\)



\(\ds \leadsto \ \ \)





\(\ds \dfrac {\partial u} {\partial x}\)

\(=\)







\(\ds -\dfrac x u\)









$\Box$















\(\ds 2 u \dfrac {\partial u} {\partial y} + 2 y\)

\(=\)







\(\ds 0\)










\(\text {(2)}: \quad\)



\(\ds \leadsto \ \ \)





\(\ds \dfrac {\partial u} {\partial y}\)

\(=\)







\(\ds -\dfrac y u\)









$\Box$















\(\ds \dfrac {\partial u} {\partial x} + 3 v^2 \dfrac {\partial v} {\partial x} + 3\)

\(=\)







\(\ds 0\)














\(\ds \leadsto \ \ \)





\(\ds -\dfrac x u + 3 v^2 \dfrac {\partial v} {\partial x} + 3\)

\(=\)







\(\ds 0\)





substituting for $\dfrac {\partial u} {\partial x}$ from $(1)$








\(\ds \leadsto \ \ \)





\(\ds \dfrac {\partial v} {\partial x}\)

\(=\)







\(\ds \dfrac {x - 3 u} {3 u v^2}\)





rearranging



$\Box$















\(\ds \dfrac {\partial u} {\partial y} + 3 v^2 \dfrac {\partial v} {\partial y}\)

\(=\)







\(\ds 0\)














\(\ds \leadsto \ \ \)





\(\ds -\dfrac y u + 3 v^2 \dfrac {\partial v} {\partial x}\)

\(=\)







\(\ds 0\)





substituting for $\dfrac {\partial u} {\partial y}$ from $(2)$








\(\ds \leadsto \ \ \)





\(\ds \dfrac {\partial v} {\partial y}\)

\(=\)







\(\ds \dfrac y {3 u v^2}\)





rearranging



$\blacksquare$


Sources
1961: David V. Widder: Advanced Calculus (2nd ed.) ... (previous) ... (next): $1$ Partial Differentiation: $\S 1$. Introduction: Exercise $10$




