# 

Source: https://proofwiki.org/wiki/Partial_Derivative/Examples/u%5E2_%2B_v%5E2_%3D_x%5E2,_2_u_v_%3D_2_x_y_%2B_y%5E2/Lemma

Lemma for Example: $u^2 + v^2 = x^2$, $2 u v = 2 x y + y^2$
Consider the simultaneous equations:














\(\ds u^2 + v^2\)

\(=\)







\(\ds x^2\)




















\(\ds 2 u v\)

\(=\)







\(\ds 2 x y + y^2\)









Then:

$x = 1$, $y = -2$ is a solution at $u = 1$, $v = 0$.


Proof
We make sure that $\tuple {1, -2}$ is actually a solution at $u = 1$, $v = 0$:














\(\ds u^2 + v^2\)

\(=\)







\(\ds \paren {-1}^2 + 0^2\)





at $u = 1$, $v = 0$














\(\ds \)

\(=\)







\(\ds x^2\)





at $\tuple {1, -2}$


















\(\ds 2 u v\)

\(=\)







\(\ds 2 \times \paren {-1} \times 0\)





at $u = 1$, $v = 0$














\(\ds \)

\(=\)







\(\ds 2 \times 1 \times \paren {-2} + \paren {-2}^2\)





at $\tuple {1, -2}$














\(\ds \)

\(=\)







\(\ds 2 x y + y^2\)





at $\tuple {1, -2}$



and it is seen that this is the case.
$\blacksquare$


Sources
1961: David V. Widder: Advanced Calculus (2nd ed.) ... (previous) ... (next): $1$ Partial Differentiation: $\S 1$. Introduction: Exercise $15$




