# 

Source: https://proofwiki.org/wiki/Periodicity_of_Hyperbolic_Sine

Theorem
Let $k \in \Z$.
Then:

$\map \sinh {x + 2 k \pi i} = \sinh x$


Proof













\(\ds \map \sinh {x + 2 k \pi i}\)

\(=\)







\(\ds \frac {e^{x + 2 k \pi i} - e^{-\paren {x + 2 k \pi i} } } {2 i}\)





Definition of Hyperbolic Sine














\(\ds \)

\(=\)







\(\ds \frac {e^{i \paren {-i x + 2 k \pi} } - e^{i \paren {i x + 2 \paren {-k} \pi} } } {2 i}\)





$i^2 = -1$ and simplifying














\(\ds \)

\(=\)







\(\ds \frac {e^{i \paren {-i x} } - e^{i \paren {i x} } } {2 i}\)





Periodicity of Complex Exponential Function














\(\ds \)

\(=\)







\(\ds \frac {e^x - e^{- x} } {2 i}\)





$i^2 = -1$














\(\ds \)

\(=\)







\(\ds \sinh x\)





Definition of Hyperbolic Sine



$\blacksquare$


Sources
1968: Murray R. Spiegel: Mathematical Handbook of Formulas and Tables ... (previous) ... (next): $\S 8$: Hyperbolic Functions: $8.86$: Periodicity of Hyperbolic Functions




