# 

Source: https://proofwiki.org/wiki/Power_Reduction_Formulas/Cosine_Squared/Proof_2

Theorem
$\cos^2 x = \dfrac {1 + \cos 2 x} 2$


Proof













\(\ds \dfrac {1 + \cos 2 x} 2\)

\(=\)







\(\ds \dfrac 1 2 \paren {1 + \dfrac {e^{2 i x} + e^{-2 i x} } 2}\)





Euler's Cosine Identity














\(\ds \)

\(=\)







\(\ds \dfrac 1 4 \paren {e^{2 i x} + 2 + e^{-2 i x} }\)





simplifying














\(\ds \)

\(=\)







\(\ds \dfrac 1 4 \paren {e^{2 i x} + 2 \paren {e^{i x} } \paren {e^{-i x} } + e^{-2 i x} }\)




















\(\ds \)

\(=\)







\(\ds \paren {\dfrac {e^{i x} + e^{-i x} } 2}^2\)





Square of Sum














\(\ds \)

\(=\)







\(\ds \cos^2 x\)





Euler's Cosine Identity



$\blacksquare$





