# 

Source: https://proofwiki.org/wiki/Power_Reduction_Formulas/Hyperbolic_Cosine_Cubed/Proof_1

Theorem
$\cosh^3 x = \dfrac {\cosh 3 x + 3 \cosh x} 4$


Proof













\(\ds \cosh 3 x\)

\(=\)







\(\ds 4 \cosh^3 x - 3 \cosh x\)





Triple Angle Formula for Hyperbolic Cosine








\(\ds \leadsto \ \ \)





\(\ds 4 \cosh^3 x\)

\(=\)







\(\ds \cosh 3 x + 3 \cosh x\)





rearranging








\(\ds \leadsto \ \ \)





\(\ds \cosh^3 x\)

\(=\)







\(\ds \dfrac {\cosh 3 x + 3 \cosh x} 4\)





dividing both sides by $4$



$\blacksquare$





