# 

Source: https://proofwiki.org/wiki/Powers_of_Group_Elements/Negative_Index/Additive_Notation

Theorem
Let $\struct {G, +}$ be a group whose identity is $e$.
Let $g \in G$.

Then:

$\forall n \in \Z: -\paren {n g} = \paren {-n} g = n \paren {-g}$


Proof
All elements of a group are invertible, so we can directly use the result from Index Laws for Monoids: Sum of Indices:

$\forall n \in \Z: \paren {g^n}^{-1} = g^{-n} = \paren {g^{-1} }^n$
where in this context:

the group operation is $+$
the $n$th power of $g$ is denoted $n g$
the inverse of $g$ is $-g$.
$\blacksquare$


Sources
1970: B. Hartley and T.O. Hawkes: Rings, Modules and Linear Algebra ... (previous) ... (next): $\S 2.1$: Subrings: Notation $2$




