# 

Source: https://proofwiki.org/wiki/Power_Series_Expansion_for_Reciprocal_of_Square_of_1_%2B_x/Corollary

Corollary to Power Series Expansion for $\frac 1 {\paren {1 + x} }$
Let $x \in \R$ such that $-1 < x < 1$.
Then:














\(\ds \dfrac 1 {\paren {1 - x}^2}\)

\(=\)







\(\ds \sum_{k \mathop = 0}^\infty \paren {k + 1} x^k\)




















\(\ds \)

\(=\)







\(\ds 1 + 2 x + 3 x^2 + 4 x^3 + 5 x^4 + \cdots\)











Proof













\(\ds \dfrac 1 {\paren {1 - x}^2}\)

\(=\)







\(\ds \dfrac 1 {\paren {1 + \paren {-x} }^2}\)




















\(\ds \)

\(=\)







\(\ds \sum_{k \mathop = 0}^\infty \paren {-1}^k \paren {k + 1} \paren {-x}^k\)





Power Series Expansion for $\dfrac 1 {\paren {1 + x}^2}$














\(\ds \)

\(=\)







\(\ds \sum_{k \mathop = 0}^\infty \paren {-1}^k \paren {-1}^k \paren {k + 1} x^k\)




















\(\ds \)

\(=\)







\(\ds \sum_{k \mathop = 0}^\infty \paren {-1}^{2 k} \paren {k + 1} x^k\)




















\(\ds \)

\(=\)







\(\ds \sum_{k \mathop = 0}^\infty \paren {k + 1} x^k\)









$\blacksquare$


Sources
1953: L. Harwood Clarke: A Note Book in Pure Mathematics ... (previous) ... (next): $\text I$. Algebra: The Binomial Theorem: Negative and fractional indices




