# 

Source: https://proofwiki.org/wiki/Power_Series_Expansion_for_Reciprocal_of_Square_of_1_-_z/Proof_2

Theorem













\(\ds \dfrac 1 {\paren {1 - z}^2}\)

\(=\)







\(\ds \sum_{n \mathop = 0}^\infty \paren {n + 1} z^n\)




















\(\ds \)

\(=\)







\(\ds 1 + 2 z + 3 z^2 + 4 z^3 + \cdots\)











Proof













\(\ds \dfrac 1 {\paren {1 - z}^2}\)

\(=\)







\(\ds \paren {\dfrac 1 {1 - z} }^2\)




















\(\ds \)

\(=\)







\(\ds \paren {\sum_{n \mathop = 0}^\infty z^n}^2\)





Sum of Infinite Geometric Sequence














\(\ds \)

\(=\)







\(\ds \sum_{n \mathop = 0}^\infty \paren {\sum_{k \mathop = 0}^n 1 \times 1} z^n\)





Product of Absolutely Convergent Series














\(\ds \)

\(=\)







\(\ds \sum_{n \mathop = 0}^\infty \paren {n + 1} z^n\)









$\blacksquare$


Sources
1960: Walter Ledermann: Complex Numbers ... (previous) ... (next): $\S 4.4$. Power Series: Example




