# 

Source: https://proofwiki.org/wiki/Power_Reduction_Formulas/Hyperbolic_Sine_Squared/Proof_2

Theorem
$\sinh^2 x = \dfrac {\cosh 2 x - 1} 2$


Proof













\(\ds \sinh^2 x\)

\(=\)







\(\ds \paren {\frac {e^x - e^{-x} } 2}^2\)





Definition of Hyperbolic Sine














\(\ds \)

\(=\)







\(\ds \frac 1 4 \paren {e^{2 x} + e^{-2 x} - 2}\)





multiplying out














\(\ds \)

\(=\)







\(\ds \frac 1 2 \paren {\dfrac {e^{2 x} + e^{-2 x} } 2 - 1}\)





rearranging














\(\ds \)

\(=\)







\(\ds \frac {\cosh 2 x - 1} 2\)





Definition of Hyperbolic Cosine



$\blacksquare$





