# 

Source: https://proofwiki.org/wiki/Power_Reduction_Formulas/Hyperbolic_Cosine_to_4th/Proof_1

Theorem
$\cosh^4 x = \dfrac {3 + 4 \cosh 2 x + \cosh 4 x} 8$


Proof













\(\ds \cosh 4 x\)

\(=\)







\(\ds \paren {\cosh^2 x}^2\)




















\(\ds \)

\(=\)







\(\ds \paren {\frac {\cosh 2 x + 1} 2}^2\)





Square of Hyperbolic Cosine














\(\ds \)

\(=\)







\(\ds \frac {\cosh^2 2 x + 2 \cosh 2 x + 1} 4\)





multiplying out














\(\ds \)

\(=\)







\(\ds \frac {\frac {\cosh 4 x + 1} 2 + 2 \cosh 2 x + 1} 4\)





Square of Hyperbolic Cosine














\(\ds \)

\(=\)







\(\ds \frac {\cosh 4 x + 1 + 4 \cosh 2 x + 2} 8\)





multiplying top and bottom by $2$














\(\ds \)

\(=\)







\(\ds \frac {3 + 4 \cosh 2 x + \cosh 4 x} 8\)





rearrangement



$\blacksquare$





