# 

Source: https://proofwiki.org/wiki/Power_Reduction_Formulas/Hyperbolic_Cosine_Cubed/Proof_3

Theorem
$\cosh^3 x = \dfrac {\cosh 3 x + 3 \cosh x} 4$


Proof













\(\ds \cosh^3 x\)

\(=\)







\(\ds \cos^3 i x\)





Hyperbolic Cosine in terms of Cosine














\(\ds \)

\(=\)







\(\ds \frac {\map \cos {3 i x} + 3 \cos i x} 4\)





Cube of Cosine














\(\ds \)

\(=\)







\(\ds \frac {\cosh 3 x + 3 \cosh x} 4\)





Hyperbolic Cosine in terms of Cosine



$\blacksquare$





