# 

Source: https://proofwiki.org/wiki/Power_Reduction_Formulas/Hyperbolic_Cosine_Cubed/Proof_2

Theorem
$\cosh^3 x = \dfrac {\cosh 3 x + 3 \cosh x} 4$


Proof













\(\ds \cosh^3 x\)

\(=\)







\(\ds \frac 1 {2^3} \paren {e^x + e^{-x} }^3\)





Definition of Hyperbolic Cosine














\(\ds \)

\(=\)







\(\ds \frac 1 8 \paren {e^{3x} + e^{-3x} + 3e^{x} + 3e^{-x} }\)




















\(\ds \)

\(=\)







\(\ds \frac 1 4 \paren {\frac{ e^{3x} + e^{-3x} } 2} + \frac 3 4 \paren {\frac{e^{x} + e^{-x} } 2}\)




















\(\ds \)

\(=\)







\(\ds \frac {\cosh 3x} 4 + \frac {3 \cosh x} 4\)





Definition of Hyperbolic Cosine



$\blacksquare$





