# 

Source: https://proofwiki.org/wiki/Power_Reduction_Formulas/Sine_Cubed/Proof_1

Theorem
$\sin^3 x = \dfrac {3 \sin x - \sin 3 x} 4$


Proof













\(\ds \sin 3 x\)

\(=\)







\(\ds 3 \sin x - 4 \sin^3 x\)





Triple Angle Formula for Sine








\(\ds \leadsto \ \ \)





\(\ds 4 \sin^3 x\)

\(=\)







\(\ds 3 \sin x - \sin 3 x\)





rearranging








\(\ds \leadsto \ \ \)





\(\ds \sin^3 x\)

\(=\)







\(\ds \frac {3 \sin x - \sin 3 x} 4\)





dividing both sides by $4$



$\blacksquare$





