# 

Source: https://proofwiki.org/wiki/Power_Series_Expansion_for_Reciprocal_of_1_%2B_x/Proof_1

Theorem
Let $x \in \R$ such that $-1 < x < 1$.
Then:














\(\ds \dfrac 1 {1 + x}\)

\(=\)







\(\ds \sum_{k \mathop = 0}^\infty \paren {-1}^k x^k\)




















\(\ds \)

\(=\)







\(\ds 1 - x + x^2 - x^3 + x^4 - \cdots\)











Proof













\(\ds \frac 1 {1 + x}\)

\(=\)







\(\ds \frac 1 {1 - \paren {-x} }\)




















\(\ds \)

\(=\)







\(\ds \sum_{k \mathop = 0}^\infty \paren {-x}^k\)





Sum of Infinite Geometric Sequence














\(\ds \)

\(=\)







\(\ds \sum_{k \mathop = 0}^\infty \paren {-1}^k x^k\)









$\blacksquare$





