# 

Source: https://proofwiki.org/wiki/Power_of_Golden_Mean_as_Sum_of_Smaller_Powers

Theorem
Let $\phi$ denote the golden mean.
Then:

$\forall z \in \C: \phi^z = \phi^{z - 1} + \phi^{z - 2}$


Proof
Let $z \in \C$.
Let $w \in \C$ such that $w + 2 = z$.
Then:














\(\ds \phi^z\)

\(=\)







\(\ds \phi^{w + 2}\)




















\(\ds \)

\(=\)







\(\ds \phi^w \phi^2\)




















\(\ds \)

\(=\)







\(\ds \phi^w \left({\phi + 1}\right)\)





Square of Golden Mean equals One plus Golden Mean














\(\ds \)

\(=\)







\(\ds \phi^{w + 1} + \phi^w\)




















\(\ds \)

\(=\)







\(\ds \phi^{z - 1} + \phi^{z - 2}\)









$\blacksquare$


Sources
1957: George Bergman: Number System with an Irrational Base (Math. Mag. Vol. 31, no. 2: pp. 98 – 110)  www.jstor.org/stable/3029218




