# 

Source: https://proofwiki.org/wiki/Preimage_of_Subset_under_Composite_Mapping/Proof_1

Theorem
Let $S_1, S_2, S_3$ be sets.
Let $f: S_1 \to S_2$ and $g: S_2 \to S_3$ be mappings.
Denote with $g \circ f: S_1 \to S_3$ the composition of $g$ and $f$.
Let $S_3' \subseteq S_3$ be a subset of $S_3$.

Then:

$\paren {g \circ f}^{-1} \sqbrk {S_3'} = \paren {f^{-1} \circ g^{-1} } \sqbrk {S_3'}$
where $g^{-1} \sqbrk {S_3'}$ denotes the preimage of $S_3'$ under $g$.


Proof
A mapping is a specific kind of relation.
Hence, Inverse of Composite Relation applies, and it follows that:

$\paren {g \circ f}^{-1} \sqbrk {S_3'} = \paren {f^{-1} \circ g^{-1} } \sqbrk {S_3'}$
$\blacksquare$





