# 

Source: https://proofwiki.org/wiki/Primitive_of_Reciprocal_of_x_by_a_x_%2B_b_squared/Partial_Fraction_Expansion

Lemma for Primitive of $\dfrac 1 {x \paren {a x + b}^2}$
$\dfrac 1 {x \paren {a x + b}^2} \equiv \dfrac 1 {b^2 x} - \dfrac a {b^2 \paren {a x + b} } - \dfrac a {b \paren {a x + b}^2}$


Proof













\(\ds \dfrac 1 {x \paren {a x + b}^2}\)

\(\equiv\)







\(\ds \dfrac A x + \dfrac B {a x + b} + \dfrac C {\paren {a x + b}^2}\)










\(\text {(1)}: \quad\)



\(\ds \leadsto \ \ \)





\(\ds 1\)

\(\equiv\)







\(\ds A \paren {a x + b}^2 + B x \paren {a x + b} + C x\)





multiplying through by $x \paren {a x + b}^2$














\(\ds \)

\(\equiv\)







\(\ds A a^2 x^2 + 2 A a b x + A b^2 + B a x^2 + B b x + C x\)





multiplying everything out




Setting $a x + b = 0$ in $(1)$:














\(\ds a x + b\)

\(=\)







\(\ds 0\)














\(\ds \leadsto \ \ \)





\(\ds x\)

\(=\)







\(\ds -\frac b a\)














\(\ds \leadsto \ \ \)





\(\ds C \paren {-\frac b a}\)

\(=\)







\(\ds 1\)





substituting for $x$ in $(1)$: terms in $a x + b$ are all $0$








\(\ds \leadsto \ \ \)





\(\ds C\)

\(=\)







\(\ds -\frac a b\)










Equating constants in $(1)$:














\(\ds 1\)

\(=\)







\(\ds A b^2\)










\(\text {(2)}: \quad\)



\(\ds \leadsto \ \ \)





\(\ds A\)

\(=\)







\(\ds \frac 1 {b^2}\)










Equating $2$nd powers of $x$ in $(1)$:














\(\ds 0\)

\(=\)







\(\ds A a^2 + B a\)














\(\ds \leadsto \ \ \)





\(\ds B\)

\(=\)







\(\ds -\frac a {b^2}\)





substituting for $A$ from $(2)$ and simplifying




Summarising:














\(\ds A\)

\(=\)







\(\ds \frac 1 {b^2}\)




















\(\ds B\)

\(=\)







\(\ds -\frac a {b^2}\)




















\(\ds C\)

\(=\)







\(\ds -\frac a b\)









Hence the result.
$\blacksquare$





