# 

Source: https://proofwiki.org/wiki/Primitive_of_Reciprocal_of_x_by_x_squared_plus_a_squared/Partial_Fraction_Expansion

Lemma for Primitive of Reciprocal of $x \paren {x^2 + a^2}$
$\dfrac 1 {x \paren {x^2 + a^2} } \equiv \dfrac 1 {a^2 x} - \dfrac x {a^2 \paren {x^2 + a^2} }$


Proof













\(\ds \dfrac 1 {x \paren {x^2 + a^2} }\)

\(\equiv\)







\(\ds \dfrac A x + \dfrac {B x + C} {x^2 + a^2}\)










\(\text {(1)}: \quad\)



\(\ds \leadsto \ \ \)





\(\ds 1\)

\(\equiv\)







\(\ds A \paren {x^2 + a^2} + B x^2 + C x\)





multiplying through by $x \paren {x^2 + a^2}$




Setting $x = 0$ in $(1)$:














\(\ds A a^2\)

\(=\)







\(\ds 1\)














\(\ds \leadsto \ \ \)





\(\ds A\)

\(=\)







\(\ds \frac 1 {a^2}\)










Equating coefficients of $x^2$ in $(1)$:














\(\ds 0\)

\(=\)







\(\ds A + B\)














\(\ds \leadsto \ \ \)





\(\ds B\)

\(=\)







\(\ds -\frac 1 {a^2}\)










Equating coefficients of $x$ in $(1)$:














\(\ds 0\)

\(=\)







\(\ds C\)










Summarising:














\(\ds A\)

\(=\)







\(\ds \frac 1 {a^2}\)




















\(\ds B\)

\(=\)







\(\ds -\frac 1 {a^2}\)




















\(\ds C\)

\(=\)







\(\ds 0\)









Hence the result.
$\blacksquare$





