# 

Source: https://proofwiki.org/wiki/Primitive_of_Reciprocal_of_x_squared_minus_a_squared/Logarithm_Form_2/Proof_2/Partial_Fraction_Expansion

Lemma for Primitive of Reciprocal of $\paren {x^2 - a^2}$
$\dfrac 1 {x^2 - a^2} \equiv \dfrac 1 {2 a \paren {x - a} } - \dfrac 1 {2 a \paren {x + a} }$


Proof













\(\ds \frac 1 {\paren {x^2 - a^2} }\)

\(\equiv\)







\(\ds \frac A {x - a} + \frac B {x + a}\)





Difference of Two Squares




\(\text {(1)}: \quad\)



\(\ds \leadsto \ \ \)





\(\ds 1\)

\(\equiv\)







\(\ds A \paren {x + a} + B \paren {x - a}\)





multiplying through by $\paren {x^2 - a^2}$




Setting $x = a$ in $(1)$:














\(\ds A \cdot 2 a + B \cdot 0\)

\(=\)







\(\ds 1\)














\(\ds \leadsto \ \ \)





\(\ds A\)

\(=\)







\(\ds \frac 1 {2 a}\)










Setting $x = -a$ in $(1)$:














\(\ds A \cdot 0 + B \cdot \paren {-2 a}\)

\(=\)







\(\ds 1\)














\(\ds \leadsto \ \ \)





\(\ds B\)

\(=\)







\(\ds \frac {-1} {2 a}\)










Summarising:














\(\ds A\)

\(=\)







\(\ds \frac 1 {2 a}\)




















\(\ds B\)

\(=\)







\(\ds \frac {-1} {2 a}\)










Hence the result.
$\blacksquare$





