# 

Source: https://proofwiki.org/wiki/Primitive_of_Logarithm_of_x/Proof_1

Theorem
$\ds \int \ln x \rd x = x \ln x - x + C$


Proof
With a view to expressing the primitive in the form:

$\ds \int u \frac {\d v} {\d x} \rd x = u v - \int v \frac {\d u} {\d x} \rd x$
let:














\(\ds u\)

\(=\)







\(\ds \ln x\)














\(\ds \leadsto \ \ \)





\(\ds \frac {\d u} {\d x}\)

\(=\)







\(\ds \frac 1 x\)





Derivative of $\ln x$




and let:














\(\ds \frac {\d v} {\d x}\)

\(=\)







\(\ds 1\)














\(\ds \leadsto \ \ \)





\(\ds v\)

\(=\)







\(\ds x\)





Primitive of Constant




Then:














\(\ds \int \ln x \rd x\)

\(=\)







\(\ds x \ln x - \int x \paren {\frac 1 x} \rd x + C\)





Integration by Parts














\(\ds \)

\(=\)







\(\ds x \ln x - \int \rd x + C\)





simplifying














\(\ds \)

\(=\)







\(\ds x \ln x - x + C\)





Primitive of Constant



$\blacksquare$


Sources
1953: L. Harwood Clarke: A Note Book in Pure Mathematics ... (previous) ... (next): $\text {II}$. Calculus: Integration: Integration by Parts: Example




