# 

Source: https://proofwiki.org/wiki/Primitive_of_Reciprocal_of_x_squared_by_a_x_squared_plus_b_x_plus_c/Partial_Fraction_Expansion

Lemma for Primitive of $\dfrac 1 {x^2 \paren {a x^2 + b x + c} }$
$\dfrac 1 {x^2 \paren {a x^2 + b x + c} } \equiv \dfrac {-b} {c^2 x} + \dfrac 1 {c x^2} + \dfrac {a b x + b^2 - a c} {c^2 \paren {a x^2 + b x + c} }$


Proof













\(\ds \dfrac 1 {x \paren {a x^2 + b x + c} }\)

\(\equiv\)







\(\ds \frac A x + \frac B x^2 + \frac {C x + D} {a x^2 + b x + c}\)










\(\text {(1)}: \quad\)



\(\ds \leadsto \ \ \)





\(\ds 1\)

\(\equiv\)







\(\ds A \paren {a x^2 + b x + c} x + B \paren {a x^2 + b x + c} + C x^3 + D x^2\)





multiplying through by $x^2 \paren {a x^2 + b x + c}$




Setting $x = 0$ in $(1)$:














\(\ds B c\)

\(=\)







\(\ds 1\)














\(\ds \leadsto \ \ \)





\(\ds B\)

\(=\)







\(\ds \frac 1 c\)










Equating coefficients of $x$ in $(1)$:














\(\ds A c + B b\)

\(=\)







\(\ds 0\)














\(\ds \leadsto \ \ \)





\(\ds A c\)

\(=\)







\(\ds \frac {-b} c\)














\(\ds \leadsto \ \ \)





\(\ds A\)

\(=\)







\(\ds \frac {-b} {c^2}\)










Equating coefficients of $x^3$ in $(1)$:














\(\ds A a + C\)

\(=\)







\(\ds 0\)














\(\ds \leadsto \ \ \)





\(\ds C\)

\(=\)







\(\ds \frac {a b} {c^2}\)










Equating coefficients of $x^2$ in $(1)$:














\(\ds A b + B a + D\)

\(=\)







\(\ds 0\)














\(\ds \leadsto \ \ \)





\(\ds D\)

\(=\)







\(\ds \frac {b^2 - a c} {c^2}\)










Summarising:














\(\ds A\)

\(=\)







\(\ds \frac {-b} {c^2}\)




















\(\ds B\)

\(=\)







\(\ds \frac 1 c\)




















\(\ds C\)

\(=\)







\(\ds \frac {a b} {c^2}\)




















\(\ds D\)

\(=\)







\(\ds \frac {b^2 - a c} {c^2}\)










Hence the result.
$\blacksquare$





