# 

Source: https://proofwiki.org/wiki/Primitive_of_Reciprocal_of_Root_of_a_x_%2B_b_by_Root_of_p_x_%2B_q/Lemma_1

Lemma for Primitive of $\frac 1 {\sqrt {\paren {a x + b} \paren {p x + q} } }$
Let $u = \sqrt {a x + b}$.
Then:

$\ds \sqrt {p x + q} = \sqrt {\paren {\frac p a} \paren {u^2 - \paren {\frac {b p - a q} p} } }$


Proof
We have:














\(\ds u\)

\(=\)







\(\ds \sqrt {a x + b}\)














\(\ds \leadsto \ \ \)





\(\ds x\)

\(=\)







\(\ds \frac {u^2 - b} a\)














\(\ds \leadsto \ \ \)





\(\ds \sqrt {p x + q}\)

\(=\)







\(\ds \sqrt {p \paren {\frac {u^2 - b} a} + q}\)




















\(\ds \)

\(=\)







\(\ds \sqrt {\frac {p \paren {u^2 - b} + a q} a}\)




















\(\ds \)

\(=\)







\(\ds \sqrt {\frac {p u^2 - b p + a q} a}\)




















\(\ds \)

\(=\)







\(\ds \sqrt {\paren {\frac p a} \paren {u^2 - \paren {\frac {b p - a q} p} } }\)









$\blacksquare$





