# 

Source: https://proofwiki.org/wiki/Primitive_of_Reciprocal_of_a_x_squared_plus_b_x_plus_c/Examples/x%5E2_%2B_4_x_%2B_5

Example of Use of Primitive of $\dfrac 1 {a x^2 + b x + c}$
$\ds \int \dfrac {\d x} {x^2 + 4 x + 5} = \map \arctan {x + 2} + C$


Proof
We aim to use Primitive of $\dfrac 1 {a x^2 + b x + c}$ with:














\(\ds a\)

\(=\)







\(\ds 1\)




















\(\ds b\)

\(=\)







\(\ds 4\)




















\(\ds c\)

\(=\)







\(\ds 5\)









We note that:














\(\ds b^2 - 4 a c\)

\(=\)







\(\ds 4^2 - 4 \times 1 \times 5\)




















\(\ds \)

\(=\)







\(\ds 16 - 20\)




















\(\ds \)

\(=\)







\(\ds -4\)










Hence from Primitive of $\dfrac 1 {a x^2 + b x + c}$:

$\ds \int \frac {\d x} {a x^2 + b x + c} = \dfrac 2 {\sqrt {4 a c - b^2} } \map \arctan {\dfrac {2 a x + b} {\sqrt {4 a c - b^2} } } + C$

Substituting for $a$, $b$ and $c$ and simplifying:














\(\ds \int \frac {\d x} {x^2 + 4 x + 5}\)

\(=\)







\(\ds \dfrac 2 {\sqrt {4 \times 1 \times 5 - 4^2} } \map \arctan {\dfrac {2 \times 1 \cdot x + 4} {\sqrt {4 \times 1 \times 5 - 4^2} } } + C\)




















\(\ds \)

\(=\)







\(\ds \dfrac 2 {\sqrt 4} \map \arctan {\dfrac {2 x + 4} {\sqrt 4} } + C\)





simplifying














\(\ds \)

\(=\)







\(\ds \map \arctan {x + 2} + C\)





simplifying



$\blacksquare$


Sources
1953: L. Harwood Clarke: A Note Book in Pure Mathematics ... (previous) ... (next): $\text {II}$. Calculus: Exercises $\text {XIV}$: $15$.




