# 

Source: https://proofwiki.org/wiki/Primitive_of_Reciprocal_of_x_by_a_x_%2B_b/Partial_Fraction_Expansion

Lemma for Primitive of $\dfrac 1 {x \paren {a x + b} }$
$\dfrac 1 {x \paren {a x + b} } \equiv \dfrac 1 {b x} - \dfrac a {b \paren {a x + b} }$


Proof













\(\ds \dfrac 1 {x \paren {a x + b} }\)

\(\equiv\)







\(\ds \dfrac A x + \dfrac B {a x + b}\)










\(\text {(1)}: \quad\)



\(\ds \leadsto \ \ \)





\(\ds 1\)

\(\equiv\)







\(\ds A \paren {a x + b} + B x\)





multiplying through by $x \paren {a x + b}$














\(\ds \)

\(\equiv\)







\(\ds A a x + A b + B x\)





multiplying out




Setting $a x + b = 0$ in $(1)$:














\(\ds a x + b\)

\(=\)







\(\ds 0\)














\(\ds \leadsto \ \ \)





\(\ds x\)

\(=\)







\(\ds -\frac b a\)














\(\ds \leadsto \ \ \)





\(\ds B \paren {-\frac b a}\)

\(=\)







\(\ds 1\)





substituting for $x$ in $(1)$: terms in $a x + b$ are all $0$








\(\ds \leadsto \ \ \)





\(\ds B\)

\(=\)







\(\ds -\frac a b\)










Equating constants in $(1)$:














\(\ds 1\)

\(=\)







\(\ds A b\)














\(\ds \leadsto \ \ \)





\(\ds A\)

\(=\)







\(\ds \frac 1 b\)










Summarising:














\(\ds A\)

\(=\)







\(\ds \frac 1 b\)




















\(\ds B\)

\(=\)







\(\ds -\frac a b\)









Hence the result.
$\blacksquare$





