# 

Source: https://proofwiki.org/wiki/Primitive_of_Reciprocal_of_x_squared_by_a_squared_minus_x_squared/Partial_Fraction_Expansion

Lemma for Primitive of Reciprocal of $x^2 \paren {a^2 - x^2}$
$\dfrac 1 {x^2 \paren {a^2 - x^2} } \equiv \dfrac 1 {a^2 \paren {a^2 - x^2} } + \dfrac 1 {a^2 x^2}$


Proof













\(\ds \dfrac 1 {x^2 \paren {a^2 - x^2} }\)

\(\equiv\)







\(\ds \dfrac A x + \dfrac B {x^2} + \dfrac {C x + D} {a^2 - x^2}\)










\(\text {(1)}: \quad\)



\(\ds \leadsto \ \ \)





\(\ds 1\)

\(\equiv\)







\(\ds A x \paren {a^2 - x^2} + B \paren {a^2 - x^2} + C x^3 + D x^2\)





multiplying through by $x^2 \paren {a^2 - x^2}$




Setting $x = 0$ in $(1)$:














\(\ds B a^2\)

\(=\)







\(\ds 1\)














\(\ds \leadsto \ \ \)





\(\ds B\)

\(=\)







\(\ds \frac 1 {a^2}\)










Equating coefficients of $x$ in $(1)$:














\(\ds 0\)

\(=\)







\(\ds A a^2\)














\(\ds \leadsto \ \ \)





\(\ds A\)

\(=\)







\(\ds 0\)










Equating coefficients of $x^3$ in $(1)$:














\(\ds 0\)

\(=\)







\(\ds -A + C\)














\(\ds \leadsto \ \ \)





\(\ds C\)

\(=\)







\(\ds 0\)










Equating coefficients of $x^2$ in $(1)$:














\(\ds 0\)

\(=\)







\(\ds -B + D\)














\(\ds \leadsto \ \ \)





\(\ds D\)

\(=\)







\(\ds \frac 1 {a^2}\)










Summarising:














\(\ds A\)

\(=\)







\(\ds 0\)




















\(\ds B\)

\(=\)







\(\ds \frac 1 {a^2}\)




















\(\ds C\)

\(=\)







\(\ds 0\)




















\(\ds D\)

\(=\)







\(\ds \frac 1 {a^2}\)









Hence the result.
$\blacksquare$





