# 

Source: https://proofwiki.org/wiki/Primitive_of_Reciprocal_of_x_by_a_x_squared_plus_b_x_plus_c/Partial_Fraction_Expansion

Lemma for Primitive of $\dfrac 1 {x \paren {a x^2 + b x + c} }$
$\dfrac 1 {x \paren {a x^2 + b x + c} } \equiv \dfrac 1 {c x} - \dfrac {a x + b} {c \paren {a x^2 + b x + c} }$


Proof













\(\ds \dfrac 1 {x \paren {a x^2 + b x + c} }\)

\(\equiv\)







\(\ds \frac A x + \frac {B x + C} {a x^2 + b x + c}\)










\(\text {(1)}: \quad\)



\(\ds \leadsto \ \ \)





\(\ds 1\)

\(\equiv\)







\(\ds A \paren {a x^2 + b x + c} + B x^2 + C x\)





multiplying through by $x \paren {a x^2 + b x + c}$




Setting $x = 0$ in $(1)$:














\(\ds A c\)

\(=\)







\(\ds 1\)














\(\ds \leadsto \ \ \)





\(\ds A\)

\(=\)







\(\ds \frac 1 c\)










Equating coefficients of $x$ in $(1)$:














\(\ds A b + C\)

\(=\)







\(\ds 0\)














\(\ds \leadsto \ \ \)





\(\ds C\)

\(=\)







\(\ds \frac {-b} c\)










Equating coefficients of $x^2$ in $(1)$:














\(\ds A a + B\)

\(=\)







\(\ds 0\)














\(\ds \leadsto \ \ \)





\(\ds B\)

\(=\)







\(\ds \frac {-a} c\)










Summarising:














\(\ds A\)

\(=\)







\(\ds \frac 1 c\)




















\(\ds B\)

\(=\)







\(\ds \frac {-b} c\)




















\(\ds C\)

\(=\)







\(\ds \frac {-a} c\)










Hence the result.
$\blacksquare$





