# 

Source: https://proofwiki.org/wiki/Primitive_of_Power_of_a_x_%2B_b/Proof_2

Theorem
$\ds \int \paren {a x + b}^n \rd x = \frac {\paren {a x + b}^{n + 1} } {\paren {n + 1} a} + C$
where $n \ne 1$.


Proof
Let $u = a x + b$.
Then:

$\dfrac {\d u} {\d x} = a$
Then:














\(\ds \int \paren {a x + b}^n \rd x\)

\(=\)







\(\ds \int \dfrac {u^n} a \rd u\)





Integration by Substitution














\(\ds \)

\(=\)







\(\ds \dfrac 1 a \dfrac {u^{n + 1} } {n + 1}\)





Primitive of Power














\(\ds \)

\(=\)







\(\ds \frac {\paren {a x + b}^{n + 1} } {\paren {n + 1} a} + C\)





substituting back for $u$



$\blacksquare$


Sources
1944: R.P. Gillespie: Integration (2nd ed.) ... (previous) ... (next): Chapter $\text {II}$: Integration of Elementary Functions: $\S 8$. Change of Variable




