# 

Source: https://proofwiki.org/wiki/Primitive_of_Reciprocal_of_x_squared_by_x_squared_plus_a_squared_squared/Partial_Fraction_Expansion

Lemma for Primitive of Reciprocal of $x^2 \paren {x^2 + a^2}^2$
$\dfrac 1 {x^2 \paren {x^2 + a^2}^2} \equiv -\dfrac 1 {a^4 x^2} - \dfrac 1 {a^4 \paren {x^2 + a^2} } - \dfrac 1 {a^2 \paren {x^2 + a^2}^2}$


Proof













\(\ds \dfrac 1 {x^2 \paren {x^2 + a^2}^2}\)

\(\equiv\)







\(\ds \dfrac A x + \dfrac B {x^2} + \dfrac {C x + D} {x^2 + a^2} + \dfrac {E x + F} {\paren {x^2 + a^2}^2}\)














\(\ds \leadsto \ \ \)





\(\ds 1\)

\(\equiv\)







\(\ds A x \paren {x^2 + a^2}^2 + B \paren {x^2 + a^2}^2\)





multiplying through by $x^2 \paren {x^2 + a^2}^2$














\(\ds \)

\(\)





\(\, \ds + \, \)

\(\ds \paren {C x + D} x^2 \paren {x^2 + a^2} + \paren {E x + F} x^2\)










\(\text {(1)}: \quad\)









\(\ds \)

\(\equiv\)







\(\ds A x^5 + 2 A a^2 x^3 + A a^4 x + B x^4 + 2 B a^2 x^2 + B a^4\)





multiplying everything out














\(\ds \)

\(\)





\(\, \ds + \, \)

\(\ds C x^5 + C x^3 a^2 + D x^4 + D x^2 a^2 + E x^3 + F x^2\)










Setting $x = 0$ in $(1)$:














\(\ds B a^4\)

\(=\)







\(\ds 1\)














\(\ds \leadsto \ \ \)





\(\ds B\)

\(=\)







\(\ds \frac 1 {a^4}\)










Equating coefficients of $x^4$ in $(1)$:














\(\ds 0\)

\(=\)







\(\ds B + D\)














\(\ds \leadsto \ \ \)





\(\ds D\)

\(=\)







\(\ds -\frac 1 {a^4}\)










Equating coefficients of $x$ in $(1)$:














\(\ds A\)

\(=\)







\(\ds 0\)










Equating coefficients of $x^5$ in $(1)$:














\(\ds 0\)

\(=\)







\(\ds A + C\)














\(\ds \leadsto \ \ \)





\(\ds C\)

\(=\)







\(\ds 0\)










Equating coefficients of $x^3$ in $(1)$:














\(\ds 2 A a^2 + C a^2 + E\)

\(=\)







\(\ds 0\)














\(\ds \leadsto \ \ \)





\(\ds E\)

\(=\)







\(\ds 0\)










Equating coefficients of $x^2$ in $(1)$:














\(\ds 0\)

\(=\)







\(\ds 2 B a^2 + D a^2 + F\)














\(\ds \leadsto \ \ \)





\(\ds F\)

\(=\)







\(\ds -\frac 1 {a^2}\)










Summarising:














\(\ds A\)

\(=\)







\(\ds 0\)




















\(\ds B\)

\(=\)







\(\ds \frac 1 {a^4}\)




















\(\ds C\)

\(=\)







\(\ds 0\)




















\(\ds D\)

\(=\)







\(\ds -\frac 1 {a^4}\)




















\(\ds E\)

\(=\)







\(\ds 0\)




















\(\ds F\)

\(=\)







\(\ds -\frac 1 {a^2}\)









Hence the result.
$\blacksquare$





