# 

Source: https://proofwiki.org/wiki/Primitive_of_Square_Root

Theorem
$\ds \int \sqrt x \rd x = \dfrac {2 x^{3 / 2} } 3 = \dfrac {2 \sqrt x^3} 3$


Proof
From Primitive of Power:
Let $n \in \R: n \ne -1$.

Then:

$\ds \int x^n \rd x = \frac {x^{n + 1} } {n + 1} + C$
where $C$ is an arbitrary constant.

Hence:














\(\ds \int \sqrt x \rd x\)

\(=\)







\(\ds \int x^{1/2} \rd x\)





Definition of Square Root














\(\ds \)

\(=\)







\(\ds \dfrac {x^{1/2 + 1} } {1/2 + 1} + C\)





Primitive of Power














\(\ds \)

\(=\)







\(\ds \dfrac {x^{3/2} } {3/2} + C\)





simplification














\(\ds \)

\(=\)







\(\ds \dfrac {2 \sqrt x^3} 3 + C\)





simplification



$\blacksquare$





