# 

Source: https://proofwiki.org/wiki/Primitive_of_Reciprocal_of_x_cubed_by_x_squared_plus_a_squared/Partial_Fraction_Expansion

Lemma for Primitive of Reciprocal of $x^3 \paren {x^2 + a^2}$
$\dfrac 1 {x^3 \paren {x^2 + a^2} } \equiv \dfrac 1 {a^2 x^3} - \dfrac 1 {a^4 x} + \dfrac x {a^4 \paren {x^2 + a^2} }$


Proof













\(\ds \dfrac 1 {x^3 \paren {x^2 + a^2} }\)

\(\equiv\)







\(\ds \dfrac A x + \dfrac B {x^2} + \dfrac C {x^3} + \dfrac {D x + E} {x^2 + a^2}\)










\(\text {(1)}: \quad\)



\(\ds \leadsto \ \ \)





\(\ds 1\)

\(\equiv\)







\(\ds A x^2 \paren {x^2 + a^2} + B x \paren {x^2 + a^2} + C \paren {x^2 + a^2} + D x^4 + E x^3\)





multiplying through by $x^3 \paren {x^2 + a^2}$




Setting $x = 0$ in $(1)$:














\(\ds C a^2\)

\(=\)







\(\ds 1\)














\(\ds \leadsto \ \ \)





\(\ds C\)

\(=\)







\(\ds \frac 1 {a^2}\)










Equating coefficients of $x$ in $(1)$:














\(\ds 0\)

\(=\)







\(\ds B a^2\)














\(\ds \leadsto \ \ \)





\(\ds B\)

\(=\)







\(\ds 0\)










Equating coefficients of $x^2$ in $(1)$:














\(\ds 0\)

\(=\)







\(\ds A a^2 + C\)














\(\ds \leadsto \ \ \)





\(\ds A\)

\(=\)







\(\ds -\frac 1 {a^4}\)










Equating coefficients of $x^3$ in $(1)$:














\(\ds 0\)

\(=\)







\(\ds B + E\)














\(\ds \leadsto \ \ \)





\(\ds E\)

\(=\)







\(\ds 0\)










Equating coefficients of $x^4$ in $(1)$:














\(\ds 0\)

\(=\)







\(\ds A + D\)














\(\ds \leadsto \ \ \)





\(\ds D\)

\(=\)







\(\ds \frac 1 {a^4}\)










Summarising:














\(\ds A\)

\(=\)







\(\ds -\frac 1 {a^4}\)




















\(\ds B\)

\(=\)







\(\ds 0\)




















\(\ds C\)

\(=\)







\(\ds \frac 1 {a^2}\)




















\(\ds D\)

\(=\)







\(\ds \frac 1 {a^4}\)




















\(\ds E\)

\(=\)







\(\ds 0\)









Hence the result.
$\blacksquare$





