# 

Source: https://proofwiki.org/wiki/Primitive_of_Reciprocal_of_a_x_%2B_b_cubed/Proof_1

Theorem
$\ds \int \frac {\d x} {\paren {a x + b}^3} = -\frac 1 {2 a \paren {a x + b}^2} + C$


Proof
Let $u = a x + b$.
Then:














\(\ds \int \frac {\rd x} {\paren {a x + b}^3}\)

\(=\)







\(\ds \frac 1 a \int \frac {\rd u} {u^3}\)





Primitive of Function of $a x + b$














\(\ds \)

\(=\)







\(\ds \frac 1 a \frac {-1} {2 u^2} + C\)





Primitive of Power














\(\ds \)

\(=\)







\(\ds -\frac 1 {2 a \paren {a x + b}^2} + C\)





substituting for $u$



$\blacksquare$





