# 

Source: https://proofwiki.org/wiki/Primitive_of_x_squared_by_Exponential_of_a_x/Examples/x_squared_by_e%5E-x

Theorem
$\ds \int x^2 e^{-x} \rd x = -e^{-x} \paren {x^2 + 2 x + 2} + C$


Proof
From Primitive of $x^2 e^{a x}$:

$\ds \int x^2 e^{a x} \rd x = \frac {e^{a x} } a \paren {x^2 - \frac {2 x} a + \frac 2 {a^2} } + C$

So:














\(\ds \int x^2 e^{-x} \rd x\)

\(=\)







\(\ds \frac {e^{-x} } {-1} \paren {x^2 - \frac {2 x} {-1} + \frac 2 {\paren {-1}^2} } + C\)





Primitive of $x^2 e^{a x}$: setting $a = -1$














\(\ds \)

\(=\)







\(\ds -e^{-x} \paren {x^2 + 2 x + 2} + C\)









$\blacksquare$





