# 

Source: https://proofwiki.org/wiki/Primitive_of_Inverse_Hyperbolic_Secant_of_x_over_a_over_x/Lemma

Lemma for Primitive of Inverse Hyperbolic Secant of x over a over x
$\map {\ln^2} {\dfrac x {2 a} } = \map \ln {\dfrac a x} \map \ln {\dfrac {4 a} x} + \map {\ln^2} 2$


Proof
$$\ln \left(\frac{a}{x}\right) \ln \left(\frac{4 a}{x}\right)-\ln ^2\left(\frac{x}{2 a}\right)=
\ln \left(\frac{a}{x}\right) \left[\ln \left(\frac{a}{x}\right)+2 \log (2)\right]-\left[\ln \left(\frac{a}{x}\right)+\ln (2)\right]^2
=-\ln ^2(2)$$














\(\ds \map {\ln^2} {\dfrac x {2 a} }\)

\(=\)







\(\ds \paren {\map \ln {\dfrac x {2 a} } }^2\)




















\(\ds \)

\(=\)







\(\ds \paren {-\map \ln {\dfrac {2 a} x} }^2\)





Logarithm of Reciprocal














\(\ds \)

\(=\)







\(\ds \paren {\map \ln {\dfrac {2 a} x} }^2\)




















\(\ds \)

\(=\)







\(\ds \paren {\map \ln {\dfrac a x} + \ln 2}^2\)




















\(\ds \)

\(=\)







\(\ds \paren {\map \ln {\dfrac a x} }^2 + 2 \ln 2 \map \ln {\dfrac a x} + \paren {\ln 2}^2\)










Then:














\(\ds \map \ln {\dfrac a x} \map \ln {\dfrac {4 a} x}\)

\(=\)







\(\ds \map \ln {\dfrac a x} \paren {\map \ln {\dfrac a x} + \map \ln {2^2} }\)





Sum of Logarithms














\(\ds \)

\(=\)







\(\ds \map \ln {\dfrac a x} \paren {\map \ln {\dfrac a x} + 2 \ln 2}\)




















\(\ds \)

\(=\)







\(\ds \paren {\map \ln {\dfrac a x} }^2 + 2 \ln 2 \map \ln {\dfrac a x}\)









Hence the result.
$\blacksquare$





