# 

Source: https://proofwiki.org/wiki/Primitive_of_Logarithm_of_x/Corollary

Corollary to Primitive of $\map \ln x$
$\ds \int \map \ln {1 - x} \rd x = \paren {x - 1} \map \ln {1 - x} - x + C$


Proof
Let $z = \paren {1 - x}$.














\(\ds z\)

\(=\)







\(\ds 1 - x\)














\(\ds \leadsto \ \ \)





\(\ds \d z\)

\(=\)







\(\ds - \rd x\)














\(\ds \leadsto \ \ \)





\(\ds \int \map \ln {1 - x} \rd x\)

\(=\)







\(\ds -\int \map \ln z \rd z\)





Integration by Substitution: $z = 1 - x$














\(\ds \)

\(=\)







\(\ds - \paren {z \ln z - z} + C\)





Primitive of Logarithm of x














\(\ds \)

\(=\)







\(\ds - z \ln z + z + C\)




















\(\ds \)

\(=\)







\(\ds -\paren {1 - x} \map \ln {1 - x} + \paren {1 - x} + C\)




















\(\ds \)

\(=\)







\(\ds \paren {x - 1} \map \ln {1 - x} - x + C\)









$\blacksquare$





