# 

Source: https://proofwiki.org/wiki/Primitive_of_Reciprocal_of_x_cubed_by_x_squared_plus_a_squared_squared/Partial_Fraction_Expansion

Lemma for Primitive of Reciprocal of $x^3 \paren {x^2 + a^2}^2$
$\dfrac 1 {x^3 \paren {x^2 + a^2}^2} \equiv -\dfrac 2 {a^6 x} + \dfrac 1 {a^4 x^3} + \dfrac {2 x} {a^6 \paren {x^2 + a^2} } + \dfrac x {a^4 \paren {x^2 + a^2}^2}$


Proof













\(\ds \dfrac 1 {x^3 \paren {x^2 + a^2}^2}\)

\(\equiv\)







\(\ds \dfrac A x + \dfrac B {x^2} + \dfrac C {x^3} + \dfrac {D x + E} {x^2 + a^2} + \dfrac {F x + G} {\paren {x^2 + a^2}^2}\)














\(\ds \leadsto \ \ \)





\(\ds 1\)

\(\equiv\)







\(\ds A x^2 \paren {x^2 + a^2}^2 + B x \paren {x^2 + a^2}^2 + C \paren {x^2 + a^2}^2\)





multiplying through by $x^2 \paren {x^2 + a^2}^2$














\(\ds \)

\(\)





\(\, \ds + \, \)

\(\ds \paren {D x + E} x^3 \paren {x^2 + a^2} + \paren {F x + G} x^3\)










\(\text {(1)}: \quad\)









\(\ds \)

\(\equiv\)







\(\ds A x^6 + 2 A a^2 x^4 + A a^4 x^2 + B x^5 + 2 B a^2 x^3 + B a^4 x\)





multiplying everything out














\(\ds \)

\(\)





\(\, \ds + \, \)

\(\ds C x^4 + 2 C a^2 x^2 + C a^4\)




















\(\ds \)

\(\)





\(\, \ds + \, \)

\(\ds D x^6 + D x^4 a^2 + E x^5 + E x^3 a^2 + F x^4 + G x^3\)










Setting $x = 0$ in $(1)$:














\(\ds C a^4\)

\(=\)







\(\ds 1\)














\(\ds \leadsto \ \ \)





\(\ds C\)

\(=\)







\(\ds \frac 1 {a^4}\)










Equating coefficients of $x^2$ in $(1)$:














\(\ds 0\)

\(=\)







\(\ds A a^4 + 2 C a^2\)














\(\ds \leadsto \ \ \)





\(\ds A\)

\(=\)







\(\ds -\frac 2 {a^6}\)










Equating coefficients of $x^6$ in $(1)$:














\(\ds 0\)

\(=\)







\(\ds A + D\)














\(\ds \leadsto \ \ \)





\(\ds D\)

\(=\)







\(\ds \frac 2 {a^6}\)










Equating coefficients of $x$ in $(1)$:














\(\ds B\)

\(=\)







\(\ds 0\)










Equating coefficients of $x^5$ in $(1)$:














\(\ds 0\)

\(=\)







\(\ds B + E\)














\(\ds \leadsto \ \ \)





\(\ds E\)

\(=\)







\(\ds 0\)










Equating coefficients of $x^3$ in $(1)$:














\(\ds 0\)

\(=\)







\(\ds 2 B a^2 + E a^2 + G\)














\(\ds \leadsto \ \ \)





\(\ds G\)

\(=\)







\(\ds 0\)










Equating coefficients of $x^4$ in $(1)$:














\(\ds 2 A a^2 + C + D a^2 + F\)

\(=\)







\(\ds 0\)














\(\ds \leadsto \ \ \)





\(\ds F\)

\(=\)







\(\ds \frac 1 {a^4}\)










Summarising:














\(\ds A\)

\(=\)







\(\ds -\frac 2 {a^6}\)




















\(\ds B\)

\(=\)







\(\ds 0\)




















\(\ds C\)

\(=\)







\(\ds \frac 1 {a^4}\)




















\(\ds D\)

\(=\)







\(\ds \frac 2 {a^6}\)




















\(\ds E\)

\(=\)







\(\ds 0\)




















\(\ds F\)

\(=\)







\(\ds \frac 1 {a^4}\)




















\(\ds G\)

\(=\)







\(\ds 0\)









Hence the result.
$\blacksquare$





