# 

Source: https://proofwiki.org/wiki/Primitive_of_Reciprocal_of_a_squared_minus_x_squared/Logarithm_Form/Partial_Fraction_Expansion

Lemma for Primitive of $\dfrac 1 {a^2 - x^2}$
$\dfrac 1 {a^2 - x^2} \equiv \dfrac 1 {2 a \paren {a + x} } + \dfrac 1 {2 a \paren {a - x} }$


Proof













\(\ds \frac 1 {\paren {a^2 - x^2} }\)

\(\equiv\)







\(\ds \frac A {a - x} + \frac B {a + x}\)





Difference of Two Squares




\(\text {(1)}: \quad\)



\(\ds \leadsto \ \ \)





\(\ds 1\)

\(\equiv\)







\(\ds A \paren {a + x} + B \paren {a - x}\)





multiplying through by $\paren {a^2 - x^2}$




Setting $x = a$ in $(1)$:














\(\ds A \cdot 2 a + B \cdot 0\)

\(=\)







\(\ds 1\)














\(\ds \leadsto \ \ \)





\(\ds A\)

\(=\)







\(\ds \frac 1 {2 a}\)










Setting $x = -a$ in $(1)$:














\(\ds A \cdot 0 + B \cdot \paren {2 a}\)

\(=\)







\(\ds 1\)














\(\ds \leadsto \ \ \)





\(\ds B\)

\(=\)







\(\ds \frac 1 {2 a}\)










Summarising:














\(\ds A\)

\(=\)







\(\ds \frac 1 {2 a}\)




















\(\ds B\)

\(=\)







\(\ds \frac 1 {2 a}\)









Hence the result.
$\blacksquare$





