# 

Source: https://proofwiki.org/wiki/Principle_of_Dilemma/Formulation_1/Reverse_Implication

Theorem
$q \vdash \left({p \implies q}\right) \land \left({\neg p \implies q}\right)$


Proof
By the tableau method of natural deduction:


$q \vdash \left({p \implies q}\right) \land \left({\neg p \implies q}\right)$


Line


Pool

Formula

Rule

Depends upon

Notes


1


1

$q$

Premise

(None)




2


1

$p \implies q$

Sequent Introduction

1

True Statement is implied by Every Statement


3


1

$\neg p \implies q$

Sequent Introduction

1

True Statement is implied by Every Statement


4


1

$\left({p \implies q}\right) \land \left({\neg p \implies q}\right)$

Rule of Conjunction: $\land \II$

2, 3



$\blacksquare$





