# 

Source: https://proofwiki.org/wiki/Principle_of_Dilemma/Formulation_2/Forward_Implication/Proof_1

Theorem
$\vdash \paren {p \implies q} \land \paren {\neg p \implies q} \implies q$


Proof
By the tableau method of natural deduction:


$\vdash \paren {p \implies q} \land \paren {\neg p \implies q} \implies q$


Line


Pool

Formula

Rule

Depends upon

Notes


1


1

$\paren {p \implies q} \land \paren {\neg p \implies q}$

Assumption

(None)




2


1

$q$

Sequent Introduction

1

Principle of Dilemma: Formulation 1


3




$\paren {p \implies q} \land \paren {\neg p \implies q} \implies q$

Rule of Implication: $\implies \II$

1 â€“ 2

Assumption 1 has been discharged
$\blacksquare$




