# 

Source: https://proofwiki.org/wiki/Product_of_Negative_with_Product_Inverse

Theorem
Let $\struct {R, +, \circ}$ be a ring with unity.
Let $z \in U_R$, where $U_R$ is the set of units.
Then:

$(1): \quad \forall x \in R: -\paren {x \circ z^{-1} } = \paren {-x} \circ z^{-1} = x \circ \paren {\paren {-z}^{-1} }$
$(2): \quad \forall x \in R: -\paren {z^{-1} \circ x} = z^{-1} \circ \paren {-x} = \paren {\paren {-z}^{-1} } \circ x$


Proof



\(\text {(1)}: \quad\)









\(\ds -\paren {x \circ z^{-1} }\)

\(=\)







\(\ds \paren {-x} \circ z^{-1}\)





Product with Ring Negative














\(\ds \)

\(=\)







\(\ds x \circ \paren {-\paren {z^{-1} } }\)





Product with Ring Negative














\(\ds \)

\(=\)







\(\ds x \circ \paren {\paren {-z}^{-1} }\)





Negative of Product Inverse



$\Box$





\(\text {(2)}: \quad\)









\(\ds -\paren {z^{-1} \circ x}\)

\(=\)







\(\ds z^{-1} \circ \paren {-x}\)





Product with Ring Negative














\(\ds \)

\(=\)







\(\ds \paren {-\paren {z^{-1} } } \circ x\)





Product with Ring Negative














\(\ds \)

\(=\)







\(\ds \paren {\paren {-z}^{-1} } \circ x\)





Negative of Product Inverse



$\blacksquare$


Sources
1965: Seth Warner: Modern Algebra ... (previous) ... (next): Chapter $\text {IV}$: Rings and Fields: $23$. The Field of Rational Numbers: Theorem $23.7 \ (1)$




