# 

Source: https://proofwiki.org/wiki/Product_Rule_for_Derivatives/Examples/x_squared_times_Arctangent_of_x

Examples of Use of Product Rule for Derivatives
$\map {\dfrac \d {\d x} } {x^2 \arctan x} = 2 x \arctan x + \dfrac {x^2} {1 + x^2}$


Proof
Let $u = x^2$.
Let $v = \arctan x$.
Thus we have:

$y = u v$
and so:














\(\ds \dfrac {\d y} {\d x}\)

\(=\)







\(\ds v \dfrac {\d u} {\d x} + u \dfrac {\d v} {\d x}\)





Product Rule for Derivatives














\(\ds \)

\(=\)







\(\ds \arctan x \cdot 2 x + x^2 \cdot \dfrac 1 {1 + x^2}\)





Power Rule for Derivatives, Derivative of Arctangent Function














\(\ds \)

\(=\)







\(\ds 2 x \arctan x + \dfrac {x^2} {1 + x^2}\)





simplification



$\blacksquare$


Sources
1953: L. Harwood Clarke: A Note Book in Pure Mathematics ... (previous) ... (next): $\text {II}$. Calculus: Differentiation: Exercises $\text {IX}$: $17$.




