# 

Source: https://proofwiki.org/wiki/Product_of_Subgroup_with_Inverse

Theorem
Let $\struct {G, \circ}$ be a group.

Then:

$\forall H \le \struct {G, \circ}:$
$H^{-1} \circ H = H$
$H \circ H^{-1} = H$
where $H \le G$ denotes that $H$ is a subgroup of $G$.


Proof
From Inverse of Subgroup:

$H = H^{-1}$
From Product of Subgroup with Itself:

$H \circ H = H$
The result follows.
$\blacksquare$


Sources
1965: Seth Warner: Modern Algebra ... (previous) ... (next): Chapter $\text {II}$: New Structures from Old: $\S 9$: Compositions Induced on the Set of All Subsets: Exercise $9.10 \ \text {(a)}$




