# 

Source: https://proofwiki.org/wiki/Product_Rule_for_Derivatives/Examples/x_times_Cotangent_of_x

Examples of Use of Product Rule for Derivatives
$\map {\dfrac \d {\d x} } {x \cot x} = \cot x - x \cosec^2 x$


Proof
Let $u = x$.
Let $v = \cot x$.
Thus we have:

$y = u v$
and so:














\(\ds \dfrac {\d y} {\d x}\)

\(=\)







\(\ds v \dfrac {\d u} {\d x} + u \dfrac {\d v} {\d x}\)





Product Rule for Derivatives














\(\ds \)

\(=\)







\(\ds \cot x \cdot 1 + x \cdot \paren {-\cosec^2 x}\)





Power Rule for Derivatives, Derivative of Cotangent Function














\(\ds \)

\(=\)







\(\ds \cot x - x \cosec^2 x\)





simplification



$\blacksquare$


Sources
1953: L. Harwood Clarke: A Note Book in Pure Mathematics ... (previous) ... (next): $\text {II}$. Calculus: Differentiation: Exercises $\text {IX}$: $16$.




