# 

Source: https://proofwiki.org/wiki/Product_of_Number_by_its_Rising_Factorial

Theorem
Let $x^{\overline n}$ denote the $n$th rising factorial power of $x$.
Then:

$x x^{\overline n} = x^{\overline {n + 1} } - n x^{\overline n}$


Proof













\(\ds x x^{\overline n}\)

\(=\)







\(\ds \paren {x + n - n} x^{\overline n}\)




















\(\ds \)

\(=\)







\(\ds \paren {x + n} x^{\overline n} - n x^{\overline n}\)




















\(\ds \)

\(=\)







\(\ds \paren {x + n} \prod_{j \mathop = 0}^{n - 1} \paren {x + j} - n x^{\overline n}\)





Definition of Rising Factorial














\(\ds \)

\(=\)







\(\ds \prod_{j \mathop = 0}^n \paren {x + j} - n x^{\overline n}\)





Definition of Continued Product














\(\ds \)

\(=\)







\(\ds x^{\overline {n + 1} } - n x^{\overline n}\)





Definition of Rising Factorial



$\blacksquare$





