# 

Source: https://proofwiki.org/wiki/Product_Rule_for_Derivatives/Examples/Cotangent_of_x_times_Exponential_of_-x

Examples of Use of Product Rule for Derivatives
$\map {\dfrac \d {\d x} } {\cot x e^{-x} } = -e^{-x} \paren {\cot x + \cosec^2 x}$


Proof
Let $u = \cot x$.
Let $v = e^{-x}$.
Thus we have:

$y = u v$
and so:














\(\ds \dfrac {\d y} {\d x}\)

\(=\)







\(\ds u \dfrac {\d v} {\d x} + v \dfrac {\d u} {\d x}\)





Product Rule for Derivatives














\(\ds \)

\(=\)







\(\ds \cot x \paren {-e^{-x} } + e^{-x} \paren {-\cosec^2 x}\)





Derivative of Exponential Function: Corollary 3, Derivative of Cotangent Function














\(\ds \)

\(=\)







\(\ds -e^{-x} \paren {\cot x + \cosec^2 x}\)





simplification



$\blacksquare$


Sources
1953: L. Harwood Clarke: A Note Book in Pure Mathematics ... (previous) ... (next): $\text {II}$. Calculus: Differentiation: Exercises $\text {IX}$: $22$.




