# 

Source: https://proofwiki.org/wiki/Proportional_Magnitudes_are_Proportional_Alternately



Theorem
In the words of Euclid:

If four magnitudes be proportional, they will also be proportional alternately.
(The Elements: Book $\text{V}$: Proposition $16$)

That is:

$a : b = c : d \implies a : c = b : d$


Proof
Let $A, B, C, D$ be four proportional magnitudes, so that as $A$ is to $B$, then so is $C$ to $D$.
We need to show that as $A$ is to $C$, then $B$ is to $D$.


Let equimultiples $E, F$ be taken of $A, B$.
Let other arbitrary equimultiples $G, H$ be taken of $C, D$.
We have that $E$ is the same multiple of $A$ that $F$ is of $B$.
So from Ratio Equals its Multiples we have that $A : B = E : F$
But $A : B = C : D$.
So from Equality of Ratios is Transitive it follows that $C : D = E : F$.
Similarly, we have that $G, H$ are equimultiples of $C, D$.
So from Ratio Equals its Multiples we have that $C : D = G : H$
So from Equality of Ratios is Transitive it follows that $E : F = G : H$.
But from Relative Sizes of Components of Ratios:

$E > G \implies F > H$
$E = G \implies F = H$
$E < G \implies F < H$
Now:

$E, F$ are equimultiples of $A, B$
$G, H$ are equimultiples of $C, D$.
Therefore from Book $\text{V}$ Definition $5$: Equality of Ratios:

$A : C = B : D$
$\blacksquare$


Historical Note
This proof is Proposition $16$ of Book $\text{V}$ of Euclid's The Elements.


Sources
1926: Sir Thomas L. Heath: Euclid: The Thirteen Books of The Elements: Volume 2 (2nd ed.) ... (previous) ... (next): Book $\text{V}$. Propositions




