# 

Source: https://proofwiki.org/wiki/Properties_of_Limit_at_Minus_Infinity_of_Real_Function/Combined_Sum_Rule

Theorem
Let $a, \alpha, \beta \in \R$. 
Let $f, gÂ : \hointl {-\infty} a \to \R$ be real functions such that: 

$\ds \lim_{x \mathop \to -\infty} \map f x$ and $\ds \lim_{x \mathop \to -\infty} \map g x$ exist
where $\ds \lim_{x \mathop \to -\infty}$ denotes the limit at $-\infty$.

Then: 

$\ds \lim_{x \mathop \to -\infty} \paren {\alpha \map f x + \beta \map g x}$ exists
with: 

$\ds \lim_{x \mathop \to -\infty} \paren {\alpha \map f x + \beta \map g x} = \alpha \lim_{x \mathop \to \infty} \map f x + \beta \lim_{x \mathop \to \infty} \map g x$


Proof
From Properties of Limit at Minus Infinity of Real Function: Multiple Rule:

$\ds \lim_{x \mathop \to -\infty} \paren {\alpha \map f x}$ exists
with:

$\ds \lim_{x \mathop \to -\infty} \paren {\alpha \map f x} = \alpha \lim_{x \mathop \to -\infty} \map f x$
and:

$\ds \lim_{x \mathop \to -\infty} \paren {\beta \map g x}$ exists
with:

$\ds \lim_{x \mathop \to -\infty} \paren {\beta \map g x} = \beta \lim_{x \mathop \to -\infty} \map g x$
From Properties of Limit at Minus Infinity of Real Function: Sum Rule, we then have: 

$\ds \lim_{x \mathop \to -\infty} \paren {\alpha \map f x + \beta \map g x}$ exists
with: 














\(\ds \lim_{x \mathop \to -\infty} \paren {\alpha \map f x + \beta \map g x}\)

\(=\)







\(\ds \lim_{x \mathop \to -\infty} \paren {\alpha \map f x} + \lim_{x \mathop \to -\infty} \paren {\beta \map g x}\)




















\(\ds \)

\(=\)







\(\ds \alpha \lim_{x \mathop \to -\infty} \map f x + \beta \lim_{x \mathop \to -\infty} \map g x\)









$\blacksquare$





