# 

Source: https://proofwiki.org/wiki/Properties_of_Limit_at_Infinity_of_Real_Function/Difference_Rule

Theorem
Let $a \in \R$. 
Let $f, gÂ : \hointr a \infty \to \R$ be real functions such that: 

$\ds \lim_{x \mathop \to \infty} \map f x = L_1$
and:

$\ds \lim_{x \mathop \to \infty} \map g x = L_2$
where $\ds \lim_{x \mathop \to \infty}$ denotes the limit at $+\infty$.

Then: 

$\ds \lim_{x \mathop \to \infty} \paren {\map f x - \map g x} = L_1 - L_2$


Proof
This follows immediately by plugging $\alpha = 1$ and $\beta = -1$ into the combined sum rule.
$\blacksquare$





