# 

Source: https://proofwiki.org/wiki/Pythagoras%27s_Theorem/Algebraic_Proof

Theorem
Let $\triangle ABC$ be a right triangle with $c$ as the hypotenuse.
Then:

$a^2 + b^2 = c^2$


Proof
We start with the algebraic definitions for sine and cosine:

$\ds \sin x = \sum_{n \mathop = 0}^\infty \paren {-1}^n \frac {x^{2 n + 1} } {\paren {2 n + 1}!} = x - \frac {x^3} {3!} + \frac {x^5} {5!} - \cdots$
$\ds \cos x = \sum_{n \mathop = 0}^\infty \paren {-1}^n \frac {x^{2 n} } {\paren {2 n}!} = 1 - \frac {x^2} {2!} + \frac {x^4} {4!} - \cdots$

From these, we derive the proof that $\cos^2 x + \sin^2 x = 1$.
Then from the Equivalence of Definitions of Trigonometric Functions, we can use the geometric interpretation of sine and cosine:


$\sin \theta = \dfrac {\text{Opposite}} {\text{Hypotenuse}}$
$\cos \theta = \dfrac {\text{Adjacent}} {\text{Hypotenuse}}$
Let $\text{Adjacent} = a, \text{Opposite} = b, \text{Hypotenuse} = c$, as in the diagram at the top of the page.

Thus:














\(\ds \cos^2 x + \sin^2 x\)

\(=\)







\(\ds 1\)





Sum of Squares of Sine and Cosine








\(\ds \leadsto \ \ \)





\(\ds \paren {\frac a c}^2 + \paren {\frac b c}^2\)

\(=\)







\(\ds 1\)














\(\ds \leadsto \ \ \)





\(\ds a^2 + b^2\)

\(=\)







\(\ds c^2\)





multiplying both sides by $c^2$



$\blacksquare$


Source of Name
This entry was named for Pythagoras of Samos.





