# 

Source: https://proofwiki.org/wiki/Pythagoras%27s_Theorem/Proof_2



Theorem
Let $\triangle ABC$ be a right triangle with $c$ as the hypotenuse.
Then:

$a^2 + b^2 = c^2$


Proof

We have:

$\dfrac b c = \dfrac d b$
and:

$\dfrac a c = \dfrac e a$
using the fact that all the triangles involved are similar.
That is:

$b^2 = c d$
$a^2 = c e$
Adding, we now get:

$a^2 + b^2 = c d + c e = c \paren {d + e} = c^2$
$\blacksquare$


Source of Name
This entry was named for Pythagoras of Samos.


Historical Note
This proof was demonstrated by Bhaskara II Acharya in the $12$th century.
It was rediscovered in the $17$th century by John Wallis.


Sources
1992: George F. Simmons: Calculus Gems ... (previous) ... (next): Chapter $\text {B}.1$: The Pythagorean Theorem
For a video presentation of the contents of this page, visit the Khan Academy.




