# 

Source: https://proofwiki.org/wiki/Quadratic_Equation/Examples/z%5E2_-_(3%2Bi)z_%2B_4%2B3i_%3D_0

Example of Quadratic Equation
The quadratic equation in $\C$:

$z^2 - \paren {3 + i} z + 4 + 3 i = 0$
has the solutions:

$z = \begin{cases} 1 + 2 i \\ 2 - i \end{cases}$


Proof
From the Quadratic Formula:














\(\ds z^2 - \paren {3 + i} z + 4 + 3 i\)

\(=\)







\(\ds 0\)














\(\ds \leadsto \ \ \)





\(\ds z\)

\(=\)







\(\ds \dfrac {-\paren {-\paren {3 + i} } \pm \sqrt {\paren {-\paren {3 + i} }^2 - 4 \times 1 \times \paren {4 + 3 i} } } {2 \times 1}\)





Quadratic Formula: $a = 1$, $b = -\paren {3 + i}$, $c = 4 + 3 i$














\(\ds \)

\(=\)







\(\ds \dfrac {3 + i} 2 \pm \dfrac {\sqrt {\paren {8 + 6 i} - \paren {16 + 12 i} } } 2\)





simplifying














\(\ds \)

\(=\)







\(\ds \dfrac {3 + i} 2 \pm \dfrac {\sqrt {-8 - 6 i} } 2\)





simplifying














\(\ds \)

\(=\)







\(\ds \dfrac {3 + i} 2 \pm \dfrac {\sqrt {\paren {-1} \paren {8 + 6 i} } } 2\)





simplifying














\(\ds \)

\(=\)







\(\ds \dfrac {3 + i} 2 \pm \dfrac {i \sqrt {\paren {8 + 6 i} } } 2\)





simplifying














\(\ds \)

\(=\)







\(\ds \dfrac {3 + i} 2 \pm \dfrac {i \paren {3 + i} } 2\)





from above: we have established that $\paren {\pm \paren {3 + i} }^2 = \paren {8 + 6 i}$














\(\ds \)

\(=\)







\(\ds \dfrac {3 + i} 2 \pm \dfrac {3 i + i^2} 2\)





simplifying














\(\ds \)

\(=\)







\(\ds \dfrac {3 + i} 2 \pm \dfrac {-1 + 3 i} 2\)





simplifying














\(\ds \)

\(=\)







\(\ds \begin{cases} 1 + 2 i \\ 2 - i \end{cases}\)





simplifying



$\blacksquare$


Sources
1960: Walter Ledermann: Complex Numbers ... (previous) ... (next): $\S 1$. Algebraic Theory of Complex Numbers: Exercise $7$




