# 

Source: https://proofwiki.org/wiki/Quadratic_Equation/Examples/z%5E4_%2B_z%5E2_%2B_1_%3D_0



Example of Quadratic Equation
The quartic equation:

$z^4 + z^2 + 1 = 0$
has the solutions:

$z = \dfrac {\pm 1 \pm i \sqrt 3} 2$


Proof
Although this is a quartic in $z$, it can be solved as a quadratic in $z^2$.














\(\ds z^4 + z^2 + 1\)

\(=\)







\(\ds 0\)














\(\ds \leadsto \ \ \)





\(\ds z^2\)

\(=\)







\(\ds \dfrac {-1 \pm \sqrt {1^2 - 4 \times 1 \times 1} } {2 \times 1}\)





Quadratic Formula: $a = 1$, $b = 1$, $c = 1$














\(\ds \)

\(=\)







\(\ds -1 \pm \dfrac {\sqrt {-3} } 2\)





simplifying














\(\ds \)

\(=\)







\(\ds -\dfrac 1 2 \pm i \dfrac {\sqrt 3} 2\)





Definition of Imaginary Unit



$\Box$

$-\dfrac 1 2 \pm i \dfrac {\sqrt 3} 2$ are recognised as the complex cube roots of unity, and so:














\(\ds z^2\)

\(=\)







\(\ds e^{\pm 2 i \pi / 3}\)




















\(\ds \)

\(=\)







\(\ds \cos \dfrac {2 \pi} 3 \pm i \sin  \dfrac {2 \pi} 3\)










Taking each in turn:














\(\ds z^2\)

\(=\)







\(\ds \cos \dfrac {2 \pi} 3 + i \sin  \dfrac {2 \pi} 3\)




















\(\ds \)

\(=\)







\(\ds \map \cis {\dfrac {2 \pi} 3 + 2 k \pi\)





for $k = 0, 1$








\(\ds \leadsto \ \ \)





\(\ds z\)

\(=\)







\(\ds \map \cis {\dfrac {\pi} 3 + k \pi}\)





for $k = 0, 1$








\(\ds \leadsto \ \ \)





\(\ds z\)

\(=\)







\(\ds \map \cis {\dfrac {\pi} 3} \text { or } \map \cis {\dfrac {4 \pi} 3}\)














\(\ds \leadsto \ \ \)





\(\ds z\)

\(=\)







\(\ds \dfrac 1 2 + \dfrac {\sqrt 3} 2 \text { or } -\dfrac 1 2 - \dfrac {\sqrt 3} 2\)










and:














\(\ds z^2\)

\(=\)







\(\ds \cos \dfrac {2 \pi} 3 - i \sin  \dfrac {2 \pi} 3\)




















\(\ds \)

\(=\)







\(\ds \cos \dfrac {4 \pi} 3 + i \sin  \dfrac {4 \pi} 3\)





for $k = 0, 1$














\(\ds \)

\(=\)







\(\ds \map \cis {\dfrac {4 \pi} 3 + 2 k \pi}\)





for $k = 0, 1$








\(\ds \leadsto \ \ \)





\(\ds z\)

\(=\)







\(\ds \map \cis {\dfrac {2 \pi} 3 + k \pi}\)





for $k = 0, 1$








\(\ds \leadsto \ \ \)





\(\ds z\)

\(=\)







\(\ds \map \cis {\dfrac {2 \pi} 3} \text { or } \map \cis {\dfrac {5 \pi} 3}\)














\(\ds \leadsto \ \ \)





\(\ds z\)

\(=\)







\(\ds -\dfrac 1 2 + \dfrac {\sqrt 3} 2 \text { or } \dfrac 1 2 - \dfrac {\sqrt 3} 2\)









$\blacksquare$


Illustration
The roots of the quartic equation:

$z^4 + z^2 + 1 = 0$
can be depicted as follows:





Sources
1981: Murray R. Spiegel: Theory and Problems of Complex Variables (SI ed.) ... (previous) ... (next): $1$: Complex Numbers: Supplementary Problems: Polynomial Equations: $102$




