# 

Source: https://proofwiki.org/wiki/Quadratic_Equation/Examples/z%5E2_%2B_(2i-3)z_%2B_5-i_%3D_0

Example of Quadratic Equation
The quadratic equation in $\C$:

$z^2 + \paren {2 i - 3} z + 5 - i = 0$
has the solutions:

$z = \begin {cases} 2 - 3 i \\ 1 + i \end {cases}$


Proof
From the Quadratic Formula:














\(\ds z^2 + \paren {2 i - 3} z + 5 - i\)

\(=\)







\(\ds 0\)














\(\ds \leadsto \ \ \)





\(\ds z\)

\(=\)







\(\ds \dfrac {-\paren {2 i - 3} \pm \sqrt {\paren {2 i - 3}^2 - 4 \times 1 \times \paren {5 - i} } } {2 \times 1}\)





Quadratic Formula: $a = 1$, $b = 2 i - 3$, $c = 5 - i$














\(\ds \)

\(=\)







\(\ds \dfrac {3 - 2 i \pm \sqrt {-15 - 8 i} } 2\)





simplifying














\(\ds \)

\(=\)







\(\ds \dfrac {3 - 2 i \pm \paren {1 - 4 i} } 2\)





Square Root of $-15 - 8 i$














\(\ds \)

\(=\)







\(\ds \begin{cases} 2 - 3 i \\ 1 + i \end{cases}\)





simplifying



$\blacksquare$


Sources
1981: Murray R. Spiegel: Theory and Problems of Complex Variables (SI ed.) ... (previous) ... (next): $1$: Complex Numbers: Solved Problems: Polynomial Equations: $32$




