# 

Source: https://proofwiki.org/wiki/Quadratic_Equation/Examples/z%5E4_-_2z%5E2_%2B_4_%3D_0

Example of Quadratic Equation
The quartic equation:

$z^4 - 2 z^2 + 4 = 0$
has the solutions:

$z = \begin {cases} \dfrac {\sqrt 6} 2 + i \dfrac {\sqrt 2} 2 \\
\dfrac {\sqrt 6} 2 - i \dfrac {\sqrt 2} 2 \\
-\dfrac {\sqrt 6} 2 + i \dfrac {\sqrt 2} 2 \\
-\dfrac {\sqrt 6} 2 - i \dfrac {\sqrt 2} 2 \end {cases}$


Proof
Although this is a quartic in $z$, it can be solved as a quadratic in $z^2$.
From the Quadratic Formula:














\(\ds z^4 - 2 z^2 + 4\)

\(=\)







\(\ds 0\)














\(\ds \leadsto \ \ \)





\(\ds z^2\)

\(=\)







\(\ds \dfrac {-\paren {-2} \pm \sqrt {\paren {-2}^2 - 4 \times 1 \times 4} } {2 \times 1}\)





Quadratic Formula: $a = 1$, $b = -2$, $c = 4$














\(\ds \)

\(=\)







\(\ds 1 \pm \dfrac {\sqrt {4 - 16} } 2\)





simplifying














\(\ds \)

\(=\)







\(\ds 1 \pm \sqrt {-3}\)





simplifying














\(\ds \)

\(=\)







\(\ds 1 \pm i \sqrt 3\)





Definition of Imaginary Unit



$\Box$

It remains to solve for $z$.
Let $z = x + i y$.
We have:














\(\ds \paren {x + i y}^2\)

\(=\)







\(\ds 1 \pm i \sqrt 3\)














\(\ds \leadsto \ \ \)





\(\ds x^2\)

\(=\)







\(\ds \dfrac {1 + \sqrt {1^2 + \paren {\sqrt 3}^2} } 2\)





Square Root of Complex Number in Cartesian Form














\(\ds \)

\(=\)







\(\ds \dfrac {1 + \sqrt 4} 2\)




















\(\ds \)

\(=\)







\(\ds \dfrac 3 2\)














\(\ds \leadsto \ \ \)





\(\ds x\)

\(=\)







\(\ds \pm \sqrt {\dfrac 3 2}\)




















\(\ds \)

\(=\)







\(\ds \pm \dfrac {\sqrt 6} 2\)




















\(\ds y^2\)

\(=\)







\(\ds \dfrac {-1 + \sqrt {1^2 + \paren {\sqrt 3}^2} } 2\)





Square Root of Complex Number in Cartesian Form














\(\ds \)

\(=\)







\(\ds \dfrac {-1 + \sqrt 4} 2\)




















\(\ds \)

\(=\)







\(\ds \dfrac 1 2\)














\(\ds \leadsto \ \ \)





\(\ds y\)

\(=\)







\(\ds \pm \dfrac {\sqrt 2} 2\)










Thus we have:

$z = \begin{cases} \dfrac {\sqrt 6} 2 + i \dfrac {\sqrt 2} 2 \\
\dfrac {\sqrt 6} 2 - i \dfrac {\sqrt 2} 2 \\
-\dfrac {\sqrt 6} 2 + i \dfrac {\sqrt 2} 2 \\
-\dfrac {\sqrt 6} 2 - i \dfrac {\sqrt 2} 2 \end{cases}$
$\blacksquare$


Sources
1960: Walter Ledermann: Complex Numbers ... (previous) ... (next): $\S 1$. Algebraic Theory of Complex Numbers: Exercise $10$




