# 

Source: https://proofwiki.org/wiki/Quadratic_Representation_of_Pair_of_Straight_Lines



Theorem
Consider the general quadratic equation in $2$ variables:

$(1): \quad a x^2 + b x y + c y^2 + d x + e y + f = 0$

Then $(1)$ is the locus of $2$ straight lines in the Cartesian plane if and only if it can be expressed in the form:

$\paren {l_1 x + m_1 y + n_1} \paren {l_2 x + m_2 y + n_2} = 0$
where $l_1$, $m_1$, $n_1$, $l_2$, $m_2$ and $n_2$ are real numbers.


Proof
Sufficient Condition
Let $\LL_1$ and $\LL_2$ be straight lines embedded in a cartesian plane $\CC$, expressed in general form as:






\(\ds \LL_1: \ \ \)







\(\ds l_1 x + m_1 y + n_1\)

\(=\)







\(\ds 0\)












\(\ds \LL_2: \ \ \)







\(\ds l_2 x + m_2 y + n_2\)

\(=\)







\(\ds 0\)









Let $\tuple {x, y}$ be a point on either $\LL_1$ or $\LL_2$.
Then because either $l_1 x + m_1 y + n_1 = 0$ or $l_2 x + m_2 y + n_2 = 0$, it is certainly the case that:

$\paren {l_1 x + m_1 y + n_1} \paren {l_2 x + m_2 y + n_2} = 0$
If $\tuple {x, y}$ is not on either $\LL_1$ or $\LL_2$, then neither $l_1 x + m_1 y + n_1 = 0$ nor $l_2 x + m_2 y + n_2 = 0$ hold.
Hence $l_1 x + m_1 y + n_1 \ne 0$ and $l_2 x + m_2 y + n_2 \ne 0$, and so:

$\paren {l_1 x + m_1 y + n_1} \paren {l_2 x + m_2 y + n_2} \ne 0$
Hence two straight lines embedded in $\CC$ can be expressed by an equation in the form:

$\paren {l_1 x + m_1 y + n_1} \paren {l_2 x + m_2 y + n_2} = 0$
as required.
$\Box$


Necessary Condition
Let it be possible to express $(1)$ in the form:

$(2): \quad \paren {l_1 x + m_1 y + n_1} \paren {l_2 x + m_2 y + n_2} = 0$
Let $\tuple {x, y}$ satisfy $(2)$.
Then either $l_1 x + m_1 y + n_1 = 0$ or $l_2 x + m_2 y + n_2 = 0$ or both.
Thus $\tuple {x, y}$ is either:

on the straight line defined by the equation $l_1 x + m_1 y + n_1 = 0$
or:

on the straight line defined by the equation $l_2 x + m_2 y + n_2 = 0$
It follows that $(2)$, and hence $(1)$, is an equation for two straight lines in $\CC$.
$\blacksquare$


Examples
Example: $x^2 - x y - 2 y^2 + 2 x + 5 y = 3$
The equation:

$x^2 - x y - 2 y^2 + 2 x + 5 y = 3$
represents the two straight lines embedded in the Cartesian plane:














\(\ds x + y - 1\)

\(=\)







\(\ds 0\)




















\(\ds x - 2 y + 3\)

\(=\)







\(\ds 0\)











Example: $x^2 + y^2 - 1 = 0$
The equation:

$x^2 + y^2 - 1 = 0$
does not represent two straight lines embedded in the Cartesian plane.


Sources
1933: D.M.Y. Sommerville: Analytical Conics (3rd ed.) ... (previous) ... (next): Chapter $\text {II}$. The Straight Line: $13$. Quadratic equation representing a pair of straight lines




