# 

Source: https://proofwiki.org/wiki/Quasilinear_Differential_Equation/Examples/x_%2B_y_y%27_%3D_0/Explicit_Solution

Theorem
The first order quasilinear ordinary differential equation:

$x + y y' = 0$
has a general solution which can be expressed explicitly as:

$y = \pm \sqrt {C - x^2}$
over the domain:

$-\sqrt C < x < \sqrt C$


Proof
The general solution of $x + y y' = 0$ is implicitly over the real numbers.
We have:














\(\ds x^2 + y^2\)

\(=\)







\(\ds y\)





Quasilinear Differential Equation: $x + y y' = 0$








\(\ds \leadsto \ \ \)





\(\ds y^2\)

\(=\)







\(\ds C - x^2\)





where $C - x^2 \ge 0$








\(\ds \leadsto \ \ \)





\(\ds y\)

\(=\)







\(\ds \pm \sqrt {C - x^2}\)





where $\size {\sqrt C} \ge x$



But when $y = 0$, the derivative $y'$ of the ordinary differential equation $x + y y' = 0$ needs to be infinite for non-zero $x$.
Hence:

$-\sqrt C < x < \sqrt C$
$\blacksquare$


Sources
1978: Garrett Birkhoff and Gian-Carlo Rota: Ordinary Differential Equations (3rd ed.) ... (previous) ... (next): Chapter $1$ First-Order Differential Equations: $1$ Introduction: Example $1$




