# 

Source: https://proofwiki.org/wiki/Quasilinear_Differential_Equation/Examples/x_%2B_y_y%27_%3D_0/Proof_1

Theorem
The first order quasilinear ordinary differential equation over the real numbers $\R$:

$x + y y' = 0$
has the general solution:

$x^2 + y^2 = C$
where:

$C > 0$
$y \ne 0$
$x < \size {\sqrt C}$
with the singular point:

$x = y = 0$


Proof
Let us rearrange the equation in question:














\(\ds x + y y'\)

\(=\)







\(\ds 0\)














\(\ds \leadstoandfrom \ \ \)





\(\ds y \dfrac {\d y} {\d x}\)

\(=\)







\(\ds -x\)














\(\ds \leadstoandfrom \ \ \)





\(\ds y \rd y\)

\(=\)







\(\ds \paren {-1} x \rd x\)









This is in the form:

$y \rd y = k x \rd x$
where $k = 1$.
From First Order ODE: $y \rd y = k x \rd x$:

$y^2 = \paren {-1} x^2 + C$
from which the result follows.
$\blacksquare$





