# 

Source: https://proofwiki.org/wiki/Ramanujan%27s_Arctangent_Sum/Corollary

Corollary to Ramanujan's Arctangent Sum
Let $n > 0$
Then:

$\ds \sum_{k \mathop = 0}^\infty \map \arctan {\dfrac 2 {\paren {n + 2 k + 1}^2} } = \map \arctan {\dfrac 1 n }$


Proof
Letting $r \to \infty$, we have:














\(\ds \lim_{r \mathop \to +\infty} \sum_{k \mathop = 0}^{r - 1} \map \arctan {\dfrac 2 {\paren {n + 2 k + 1}^2} }\)

\(=\)







\(\ds \lim_{r \mathop \to +\infty} \map \arctan {\dfrac {2 r} {\paren {n^2 + 2 n r + 1} } }\)





Ramanujan's Arctangent Sum








\(\ds \leadsto \ \ \)





\(\ds \sum_{k \mathop = 0}^\infty \map \arctan {\dfrac 2 {\paren {n + 2 k + 1}^2} }\)

\(=\)







\(\ds \map \arctan {\dfrac 1 n}\)









$\blacksquare$


Sources
1985:Â Bruce C. Berndt: Ramanujan's Notebooks: Part I: Chapter $\text {2}$. Sums Related to the Harmonic Series or the Inverse Tangent Function




