# 

Source: https://proofwiki.org/wiki/Reciprocal_of_One_Plus_Cosecant

Theorem
$\dfrac {\cos^2 x + 3 \sin x - 1} {\cos^2 x + 2 \sin x + 2} = \dfrac 1 {1 + \csc x}$


Proof













\(\ds \frac {\cos^2 x + 3 \sin x - 1} {\cos^2 x + 2 \sin x + 2}\)

\(=\)







\(\ds \frac {1 - \sin^2 x + 3 \sin x - 1} {1 - \sin^2 x + 2 \sin x + 2}\)





Sum of Squares of Sine and Cosine














\(\ds \)

\(=\)







\(\ds \frac {\sin^2 x - 3 \sin x} {\sin^2 x - 2 \sin x - 3}\)




















\(\ds \)

\(=\)







\(\ds \frac {\sin x \paren {\sin x - 3} } {\paren {\sin x - 3} \paren {\sin x + 1} }\)




















\(\ds \)

\(=\)







\(\ds \frac {\sin x} {\sin x + 1}\)




















\(\ds \)

\(=\)







\(\ds \frac 1 {1 + \dfrac 1 {\sin x} }\)




















\(\ds \)

\(=\)







\(\ds \frac 1 {1 + \csc x}\)





Definition of Real Cosecant Function



$\blacksquare$





