# 

Source: https://proofwiki.org/wiki/Reciprocal_of_One_Minus_Secant

Theorem
$\dfrac {\sin^2 x + 2 \cos x - 1} {\sin^2 x + 3 \cos x - 3} = \dfrac 1 {1 - \sec x}$


Proof













\(\ds \frac {\sin^2 x + 2 \cos x - 1} {\sin^2 x + 3 \cos x - 3}\)

\(=\)







\(\ds \frac {1 - \cos^2 x - 2 \cos x - 1} {1 - \cos^2 x + 3 \cos x - 3}\)





Sum of Squares of Sine and Cosine














\(\ds \)

\(=\)







\(\ds \frac {\cos^2 x - 2 \cos x} {\cos^2 x - 3 \cos x + 2}\)




















\(\ds \)

\(=\)







\(\ds \frac {\cos x \paren {\cos x - 2} } {\paren {\cos x - 1} \paren {\cos x - 2} }\)




















\(\ds \)

\(=\)







\(\ds \frac {\cos x} {\cos x - 1}\)




















\(\ds \)

\(=\)







\(\ds \frac 1 {1 - \frac 1 {\cos x} }\)




















\(\ds \)

\(=\)







\(\ds \frac 1 {1 - \sec x}\)





Definition of Secant Function



$\blacksquare$





