# 

Source: https://proofwiki.org/wiki/Reciprocal_of_i

Theorem
$\dfrac 1 i = -i$
where $i$ denotes the imaginary unit.


Proof













\(\ds i^2\)

\(=\)







\(\ds -1\)





Definition of Imaginary Unit








\(\ds \leadsto \ \ \)





\(\ds \frac {i^2} i\)

\(=\)







\(\ds \frac {-1} i\)














\(\ds \leadsto \ \ \)





\(\ds i\)

\(=\)







\(\ds \frac {-1} i\)














\(\ds \leadsto \ \ \)





\(\ds -i\)

\(=\)







\(\ds \frac 1 i\)









$\blacksquare$





