# 

Source: https://proofwiki.org/wiki/Reciprocal_of_Complex_Exponential

Theorem
Let $z \in \C$.
Let $\exp$ denote the complex exponential function.
Then:

$\dfrac 1 {\map \exp z} = \map \exp {-z}$


Proof













\(\ds \map \exp {-z}\)

\(=\)







\(\ds \dfrac {\map \exp {-z} } {\map \exp 0}\)





as $\map \exp 0 = 1$ by Exponential of Zero














\(\ds \)

\(=\)







\(\ds \dfrac {\map \exp {-z} } {\map \exp {z - z} }\)




















\(\ds \)

\(=\)







\(\ds \dfrac {\map \exp {-z} } {\map \exp z \, \map \exp {-z} }\)





Exponential of Sum: Complex Numbers














\(\ds \)

\(=\)







\(\ds \dfrac 1 {\map \exp z}\)









$\blacksquare$


Sources
2001:Â Christian Berg: Kompleks funktionsteori: $\S 1.5$




