# 

Source: https://proofwiki.org/wiki/Reciprocal_of_Real_Exponential

Theorem
Let $x \in \R$.
Let $\exp$ denotes the real exponential function.
Then:

$\dfrac 1 {\map \exp x} = \map \exp {-x}$


Proof













\(\ds \map \exp 0\)

\(=\)







\(\ds 1\)





Exponential of Zero








\(\ds \leadsto \ \ \)





\(\ds \map \exp {x - x}\)

\(=\)







\(\ds 1\)





as $\forall x \in \RÂ : x - x = 0$








\(\ds \leadsto \ \ \)





\(\ds \map \exp {-x} \, \map \exp x\)

\(=\)







\(\ds 1\)





Exponential of Sum of Real Numbers








\(\ds \leadsto \ \ \)





\(\ds \map \exp {-x}\)

\(=\)







\(\ds \dfrac 1 {\exp x}\)





dividing both sides by $\exp x$, which is non-zero by Exponential of Real Number is Strictly Positive



$\blacksquare$





