# 

Source: https://proofwiki.org/wiki/Recursive_Form_of_Generalized_Termial

Theorem
The termial function as defined on the real numbers fulfils the identity:

$x? = x + \paren {x - 1}?$


Proof
By definition of the termial on the real numbers:

$x? = \dfrac {x \paren {x + 1} } 2$
Thus:














\(\ds x? - x\)

\(=\)







\(\ds \dfrac {x \paren {x + 1} } 2 - x\)





Definition of Termial














\(\ds \)

\(=\)







\(\ds \dfrac {x \paren {x + 1} - 2 x} 2\)




















\(\ds \)

\(=\)







\(\ds \dfrac {x^2 + x - 2 x} 2\)




















\(\ds \)

\(=\)







\(\ds \dfrac {x^2 - x} 2\)




















\(\ds \)

\(=\)







\(\ds \dfrac {\paren {x - 1} x} 2\)




















\(\ds \)

\(=\)







\(\ds \paren {x - 1}?\)









$\blacksquare$


Sources
1997: Donald E. Knuth: The Art of Computer Programming: Volume 1: Fundamental Algorithms (3rd ed.) ... (previous) ... (next): $\S 1.2.5$: Permutations and Factorials: Exercise $7$




