# 

Source: https://proofwiki.org/wiki/Repeated_Fourier_Transform_of_Odd_Function

Theorem
Let $f: \R \to \R$ be an odd real function which is Lebesgue integrable.
Let $\ds \map \FF {\map f t} = \map F s = \int_{-\infty}^\infty e^{-2 \pi i s t} \map f t \rd t$ be the Fourier transform of $f$.
Let $\ds \map \FF {\map F s} = \map g t = \int_{-\infty}^\infty e^{-2 \pi i t s} \map F s \rd s$ be the Fourier transform of $F$.

Then:

$\map g t = -\map f t$


Proof













\(\ds \map g t\)

\(=\)







\(\ds \map f {-t}\)





Repeated Fourier Transform of Real Function














\(\ds \)

\(=\)







\(\ds -\map f t\)





Definition of Odd Function



$\blacksquare$


Sources
1978: Ronald N. Bracewell: The Fourier Transform and its Applications (2nd ed.) ... (previous) ... (next): Chapter $2$: Groundwork: The Fourier transform and Fourier's integral theorem




