# 

Source: https://proofwiki.org/wiki/Repunit_Integer_as_Product_of_Base_-_1_by_Increasing_Digit_Integer



Theorem













\(\ds 9 \times 1 + 2\)

\(=\)







\(\ds 11\)




















\(\ds 9 \times 12 + 3\)

\(=\)







\(\ds 111\)




















\(\ds 9 \times 123 + 4\)

\(=\)







\(\ds 1111\)




















\(\ds 9 \times 1234 + 5\)

\(=\)







\(\ds 11111\)




















\(\ds 9 \times 12345 + 6\)

\(=\)







\(\ds 11111\)




















\(\ds \)

\(\ldots\)







\(\ds \)









That is:

$\ds 9 \sum_{j \mathop = 0}^n \paren {n - j} 10^j + n + 1 = \sum_{j \mathop = 0}^n 10^j$


General Result
$\ds \paren {b - 1} \sum_{j \mathop = 0}^n \paren {n - j} b^j + n + 1 = \sum_{j \mathop = 0}^n b^j$


Proof
A specific instance of the general result:

$\ds \paren {b - 1} \sum_{j \mathop = 0}^n \paren {n - j} b^j + n + 1 = \sum_{j \mathop = 0}^n b^j$

where $b = 10$.
$\blacksquare$


Sources
1997: Donald E. Knuth: The Art of Computer Programming: Volume 1: Fundamental Algorithms (3rd ed.) ... (previous) ... (next): $\S 1.2.3$: Sums and Products: Exercise $20 \ \text({a})$




