# 

Source: https://proofwiki.org/wiki/Riemann_Zeta_Function_at_Even_Integers/Corollary

Corollary to Riemann Zeta Function at Even Integers













\(\ds B_{2 n}\)

\(=\)







\(\ds \paren {-1}^{n + 1} \dfrac {\paren {2 n}!} {2^{2 n - 1} \pi^{2 n} } \sum_{k \mathop = 1}^\infty \frac 1 {k^{2 n} }\)




















\(\ds \)

\(=\)







\(\ds \paren {-1}^{n + 1} \dfrac {\paren {2 n}!} {2^{2 n - 1} \pi^{2 n} } \paren {1 + \frac 1 {2^{2 n} } + \frac 1 {3^{2 n} } + \cdots}\)









where:

$B_n$ are the Bernoulli numbers
$n$ is a positive integer.


Proof













\(\ds \paren {-1}^{n + 1} \dfrac {B_{2 n} 2^{2 n - 1} \pi^{2 n} } {\paren {2 n}!}\)

\(=\)







\(\ds \map \zeta {2 n}\)





Riemann Zeta Function at Even Integers














\(\ds \)

\(=\)







\(\ds \sum_{k \mathop = 1}^\infty \frac 1 {k^{2 n} }\)





Definition of Riemann Zeta Function








\(\ds \leadsto \ \ \)





\(\ds \paren {-1}^{n + 1} B_{2 n}\)

\(=\)







\(\ds \dfrac {\paren {2 n}!} {2^{2 n - 1} \pi^{2 n} } \sum_{k \mathop = 1}^\infty \frac 1 {k^{2 n} }\)





multiplying both sides by $\dfrac {\paren {2 n}!} {2^{2 n - 1} \pi^{2 n} }$








\(\ds \leadsto \ \ \)





\(\ds \paren {-1}^{2 n + 2} B_{2 n}\)

\(=\)







\(\ds \paren {-1}^{n + 1} \dfrac {\paren {2 n}!} {2^{2 n - 1} \pi^{2 n} } \sum_{k \mathop = 1}^\infty \frac 1 {k^{2 n} }\)





multiplying both sides by $\paren {-1}^{n + 1}$








\(\ds \leadsto \ \ \)





\(\ds B_{2 n}\)

\(=\)







\(\ds \paren {-1}^{n + 1} \dfrac {\paren {2 n}!} {2^{2 n - 1} \pi^{2 n} } \sum_{k \mathop = 1}^\infty \frac 1 {k^{2 n} }\)





$\paren {-1}^{2 n + 2} = 1$ as $2 n + 2$ is even



$\blacksquare$


Sources
1968: Murray R. Spiegel: Mathematical Handbook of Formulas and Tables ... (previous) ... (next): $\S 21$: Series involving Bernoulli and Euler Numbers: $21.8$




