# 

Source: https://proofwiki.org/wiki/Ring_Subtraction_equals_Zero_iff_Elements_are_Equal

Theorem
Let $\struct {R, +, \circ}$ be a ring whose zero is $0_R$
Then:

$\forall a, b \in R: a - b = 0_R \iff a = b$
where $a - b$ denotes ring subtraction.


Proof













\(\ds a - b\)

\(=\)







\(\ds 0_R\)














\(\ds \leadstoandfrom \ \ \)





\(\ds a + \paren {-b}\)

\(=\)







\(\ds 0_R\)





Definition of Ring Subtraction








\(\ds \leadstoandfrom \ \ \)





\(\ds \paren {a + \paren {-b} } + b\)

\(=\)







\(\ds 0_R + b\)





Cancellation Laws








\(\ds \leadstoandfrom \ \ \)





\(\ds a + \paren {b^{-1} + b}\)

\(=\)







\(\ds 0_R \circ b\)





Group Axiom $\text G 1$: Associativity








\(\ds \leadstoandfrom \ \ \)





\(\ds a\)

\(=\)







\(\ds b\)





Group Axiom $\text G 2$: Existence of Identity Element and Group Axiom $\text G 3$: Existence of Inverse Element



$\blacksquare$


Sources
1969: C.R.J. Clapham: Introduction to Abstract Algebra ... (previous) ... (next): Chapter $1$: Integral Domains: $\S 4$. Elementary Properties: Theorem $2 \ \text{(ii)}$




