# 

Source: https://proofwiki.org/wiki/Rising_Sum_of_Binomial_Coefficients/Proof_3

Theorem
$\ds \sum_{j \mathop = 0}^m \binom {n + j} n = \binom {n + m + 1} {n + 1} = \binom {n + m + 1} m$


Direct Proof
We have:














\(\ds \binom {n + j} n\)

\(=\)







\(\ds \binom {n + j} {\left({n + j}\right) - n}\)





Symmetry Rule for Binomial Coefficients














\(\ds \)

\(=\)







\(\ds \binom {n + j} j\)









The result follows from Sum of $\dbinom {r + k} k$ up to $n$.
$\blacksquare$





