# 

Source: https://proofwiki.org/wiki/Roots_of_Complex_Number/Examples/Cube_Roots_of_2-11i

Example of Roots of Complex Number
The complex cube roots of $2 - 11 i$ are given by:

$\paren {2 - 11 i}^{1/3} = \set {2 - i, -1 + \dfrac {\sqrt 3} 2 + i \paren {\dfrac 1 2 + \sqrt 3 }, -1 - \dfrac {\sqrt 3} 2 + i \paren {\dfrac 1 2 - \sqrt 3}}$


Proof
Let $z^3 = 2 - 11 i = \paren {p + iq}^3$.
Then:














\(\ds \paren {p + iq}^3\)

\(=\)







\(\ds 2 - 11 i\)














\(\ds \leadsto \ \ \)





\(\ds p^3 + 3 i p^2 q - 3 p q^2 - i q^3\)

\(=\)







\(\ds 2 - 11 i\)














\(\ds \leadsto \ \ \)





\(\ds p^3 - 3 p q^2\)

\(=\)







\(\ds 2\)




















\(\ds 3 p^2 q - q^3\)

\(=\)







\(\ds -11\)










From this we have:














\(\ds p^3 - 3 p q^2\)

\(=\)







\(\ds 2\)














\(\ds \leadsto \ \ \)





\(\ds \frac {p^3} {q^3} - \frac {3 p} q\)

\(=\)







\(\ds \frac 2 {q^3}\)














\(\ds \leadsto \ \ \)





\(\ds \frac {2 p^3} {q^3} - \frac {6 p} q\)

\(=\)







\(\ds \frac 4 {q^3}\)









and:














\(\ds 3 p^2 q - q^3\)

\(=\)







\(\ds -11\)














\(\ds \leadsto \ \ \)





\(\ds \frac {3 p^2} {q^2} - 1\)

\(=\)







\(\ds -\frac {11} {q^3}\)










Thus:














\(\ds \frac {2 p^3} {q^3} - \frac {6 p} q\)

\(=\)







\(\ds \frac 4 {q^3}\)














\(\ds \leadsto \ \ \)





\(\ds \frac {2 p^3} {q^3} - \frac {6 p} q\)

\(=\)







\(\ds -\dfrac 4 {11} \paren {\frac {3 p^2} {q^2} - 1 }\)














\(\ds \leadsto \ \ \)





\(\ds 2 \paren {p/q}^3 + \dfrac{12} {11} \paren {p/q}^2 - 6 \paren {p/q} - \dfrac 4 {11}\)

\(=\)







\(\ds 0\)














\(\ds \leadsto \ \ \)





\(\ds 11 \paren {p/q}^3 + 6 \paren {p/q}^2 - 33 \paren {p/q} - 2\)

\(=\)







\(\ds 0\)





multiplying by $\dfrac {11} 2$




Let $w = \dfrac p q$:














\(\ds 11 w^3 + 6 w^2 - 33 w - 2\)

\(=\)







\(\ds 0\)














\(\ds \leadsto \ \ \)





\(\ds \paren {w + 2} \paren {11w^2 - 16 w - 1}\)

\(=\)







\(\ds 0\)














\(\ds \leadsto \ \ \)





\(\ds w = \dfrac p q\)

\(=\)







\(\ds -2 \textrm { or } \dfrac {8 \pm 5 \sqrt 3 } {11 }\)





Quadratic Formula on $11w^2 + 16 w - 1$




Putting $\dfrac p q = -2$ leads to::

$p = -2q$
and hence:














\(\ds 3 p^2 q - q^3\)

\(=\)







\(\ds -11\)














\(\ds \leadsto \ \ \)





\(\ds 12 q^3 - q^3\)

\(=\)







\(\ds -11\)














\(\ds \leadsto \ \ \)





\(\ds 11 q^3\)

\(=\)







\(\ds -11\)














\(\ds \leadsto \ \ \)





\(\ds q\)

\(=\)







\(\ds -1 \textrm { or } \dfrac 1 2 \pm i \dfrac {\sqrt 3} 2\)





Cube Roots of Unity




So this gives:

$z = \begin {cases} 2 - i \\ -1 + \dfrac {\sqrt 3} 2 + i \paren {\dfrac 1 2 + \sqrt 3 } \\ -1 - \dfrac {\sqrt 3} 2 + i \paren {\dfrac 1 2 - \sqrt 3} \end{cases}$
$\blacksquare$





