# 

Source: https://proofwiki.org/wiki/Roots_of_Complex_Number/Examples/Cube_Roots_of_-11-2i

Example of Roots of Complex Number: Corollary
The complex cube roots of $-11 - 2 i$ are given by:

$\paren {-11 - 2 i}^{1/3} = \set {1 + 2 i, -\dfrac 1 2 + \sqrt 3 + \paren {-1 - \dfrac {\sqrt 3} 2} i, -\dfrac 1 2 - \sqrt 3 + \paren {-1 + \dfrac {\sqrt 3} 2} i}$


Proof
Let $z^3 = -11 - 2 i = \paren {p + iq}^3$.
Then:














\(\ds \paren {p + iq}^3\)

\(=\)







\(\ds -11 - 2 i\)














\(\ds \leadsto \ \ \)





\(\ds p^3 + 3 i p^2 q - 3 p q^2 - i q^3\)

\(=\)







\(\ds -11 - 2 i\)














\(\ds \leadsto \ \ \)





\(\ds p^3 - 3 p q^2\)

\(=\)







\(\ds -11\)




















\(\ds 3 p^2 q - q^3\)

\(=\)







\(\ds -2\)










From this we have:














\(\ds p^3 - 3 p q^2\)

\(=\)







\(\ds -11\)














\(\ds \leadsto \ \ \)





\(\ds \frac {p^3} {q^3} - \frac {3 p} q\)

\(=\)







\(\ds \frac {-11} {q^3}\)














\(\ds \leadsto \ \ \)





\(\ds \frac {2 p^3} {q^3} - \frac {6 p} q\)

\(=\)







\(\ds -11 \frac 2 {q^3}\)









and:














\(\ds 3 p^2 q - q^3\)

\(=\)







\(\ds -2\)














\(\ds \leadsto \ \ \)





\(\ds \frac {3 p^2} {q^2} - 1\)

\(=\)







\(\ds -\frac 2 {q^3}\)










Thus:














\(\ds \frac {2 p^3} {q^3} - \frac {6 p} q\)

\(=\)







\(\ds -11 \frac 2 {q^3}\)














\(\ds \leadsto \ \ \)





\(\ds \frac {2 p^3} {q^3} - \frac {6 p} q\)

\(=\)







\(\ds \frac {33 p^2} {q^2} - 11\)














\(\ds \leadsto \ \ \)





\(\ds 2 \paren {p/q}^3 - 33 \paren {p/q}^2 - 6 \paren {p/q} + 11\)

\(=\)







\(\ds 0\)










Let $w = \dfrac p q$:














\(\ds 2 w^3 - 33 w^2 - 6 w + 11\)

\(=\)







\(\ds 0\)














\(\ds \leadsto \ \ \)





\(\ds \paren {2 w - 1} \paren {w^2 - 16 w - 11}\)

\(=\)







\(\ds 0\)














\(\ds \leadsto \ \ \)





\(\ds w = \dfrac p q\)

\(=\)







\(\ds \dfrac 1 2 \textrm { or } 8 \pm 5 \sqrt 3\)





Quadratic Formula on $w^2 - 16 w - 11$




Putting $\dfrac p q = \dfrac 1 2$ leads to::

$2 p = q$
and hence:














\(\ds 3 p^2 q - q^3\)

\(=\)







\(\ds -2\)














\(\ds \leadsto \ \ \)





\(\ds 6 p^3 - 8 p^3\)

\(=\)







\(\ds -2\)














\(\ds \leadsto \ \ \)





\(\ds p^3\)

\(=\)







\(\ds 1\)














\(\ds \leadsto \ \ \)





\(\ds p\)

\(=\)







\(\ds 1 \textrm { or } -\dfrac 1 2 \pm i \dfrac {\sqrt 3} 2\)










So this gives:

$z = \begin {cases} 1 + 2i \\ -\dfrac 1 2 + \sqrt 3 + i \paren {-1 - \dfrac {\sqrt 3} 2} \\ -\dfrac 1 2 - \sqrt 3 + i \paren {-1 + \dfrac {\sqrt 3} 2} \end{cases}$
$\blacksquare$


Sources
1981: Murray R. Spiegel: Theory and Problems of Complex Variables (SI ed.) ... (previous) ... (next): $1$: Complex Numbers: Supplementary Problems: Roots of Complex Numbers: $99$




