# 

Source: https://proofwiki.org/wiki/Roots_of_Quadratic_with_Rational_Coefficients_of_form_r_plus_s_Root_2

Theorem
Consider the quadratic equation:

$(1): \quad a^2 x + b x + c = 0$
where $a, b, c$ are rational.
Let $\alpha = r + s \sqrt 2$ be one of the roots of $(1)$.

Then $\beta = r - s \sqrt 2$ is the other root of $(1)$.


Proof
We have that:














\(\ds a \paren {r + s \sqrt 2}^2 + b \paren {r + s \sqrt 2} + c\)

\(=\)







\(\ds 0\)














\(\ds \leadsto \ \ \)





\(\ds \paren {a r^2 + 2 a s + br + c} + \paren {2 a + b} s \sqrt 2\)

\(=\)







\(\ds 0\)









Because $a$, $b$, $c$, $r$ and $s$ are rational, it must be that $\paren {2 a + b} s = 0$.
Hence:














\(\ds a \paren {r - s \sqrt 2}^2 + b \paren {r - s \sqrt 2} + c\)

\(=\)







\(\ds \paren {a r^2 + 2 a s + br + c} - \paren {2 a + b} s \sqrt 2\)




















\(\ds \)

\(=\)







\(\ds 0\)









and so $\beta$ is also a root of $(1)$.
$\blacksquare$


Sources
1977: K.G. Binmore: Mathematical Analysis: A Straightforward Approach ... (previous) ... (next): $\S 1$: Real Numbers: Exercise $\S 1.20 \ (5)$




