# 

Source: https://proofwiki.org/wiki/Rule_of_Simplification/Sequent_Form/Formulation_1/Form_2/Proof_by_Truth_Table

Theorem













\(\ds p \land q\)

\(\)







\(\ds \)














\(\ds \vdash \ \ \)





\(\ds q\)

\(\)







\(\ds \)











Proof
We apply the Method of Truth Tables.
$\begin{array}{|ccc||c|} \hline
p & \land & q & q \\
\hline
\F & \F & \F & \F \\
\F & \F & \T & \T \\
\T & \F & \F & \F \\
\T & \T & \T & \T \\
\hline
\end{array}$
As can be seen, when $p \land q$ is true so is $q$.
$\blacksquare$





