# 

Source: https://proofwiki.org/wiki/Rule_of_Conjunction/Sequent_Form/Formulation_1/Proof_1

Theorem













\(\ds p\)

\(\)







\(\ds \)




















\(\ds q\)

\(\)







\(\ds \)














\(\ds \vdash \ \ \)





\(\ds p \land q\)

\(\)







\(\ds \)











Proof
By the tableau method of natural deduction:


$p, q \vdash p \land q$


Line


Pool

Formula

Rule

Depends upon

Notes


1


1

$p$

Premise

(None)




2


2

$q$

Premise

(None)




3


1, 2

$p \land q$

Rule of Conjunction: $\land \II$

1, 2



$\blacksquare$


Sources
1965: E.J. Lemmon: Beginning Logic ... (previous) ... (next): Chapter $1$: The Propositional Calculus $1$: $3$ Conjunction and Disjunction: Theorem $12$




