# 

Source: https://proofwiki.org/wiki/Rule_of_Simplification/Sequent_Form/Formulation_1



Theorem



\(\text {(1)}: \quad\)









\(\ds p \land q\)

\(\)







\(\ds \)














\(\ds \vdash \ \ \)





\(\ds p\)

\(\)







\(\ds \)












\(\text {(2)}: \quad\)









\(\ds p \land q\)

\(\)







\(\ds \)














\(\ds \vdash \ \ \)





\(\ds q\)

\(\)







\(\ds \)











Form 1













\(\ds p \land q\)

\(\)







\(\ds \)














\(\ds \vdash \ \ \)





\(\ds p\)

\(\)







\(\ds \)









Form 2













\(\ds p \land q\)

\(\)







\(\ds \)














\(\ds \vdash \ \ \)





\(\ds q\)

\(\)







\(\ds \)











Proof
We apply the Method of Truth Tables.
$\begin{array}{|ccc||c|c|} \hline
p & \land & q & p & q \\
\hline
F & F & F & F & F \\
F & F & T & F & T \\
T & F & F & T & F \\
T & T & T & T & T \\
\hline
\end{array}$
As can be seen, when $p \land q$ is true so are both $p$ and $q$.
$\blacksquare$





