# 

Source: https://proofwiki.org/wiki/Rule_of_Simplification/Sequent_Form/Formulation_1/Form_1/Proof_by_Truth_Table

Theorem













\(\ds p \land q\)

\(\)







\(\ds \)














\(\ds \vdash \ \ \)





\(\ds p\)

\(\)







\(\ds \)











Proof
We apply the Method of Truth Tables.
$\begin{array}{|ccc||c|} \hline
p & \land & q & p \\
\hline
\F & \F & \F & \F \\
\F & \F & \T & \F \\
\T & \F & \F & \T \\
\T & \T & \T & \T \\
\hline
\end{array}$
As can be seen, when $p \land q$ is true so is $p$.
$\blacksquare$


Sources
1988: Alan G. Hamilton: Logic for Mathematicians (2nd ed.) ... (previous) ... (next): $\S 1$: Informal statement calculus: $\S 1.2$: Truth functions and truth tables: Example $1.8 \ \text{(a)}$




