# 

Source: https://proofwiki.org/wiki/Rule_of_Conjunction/Sequent_Form/Formulation_1/Proof_by_Truth_Table

Theorem













\(\ds p\)

\(\)







\(\ds \)




















\(\ds q\)

\(\)







\(\ds \)














\(\ds \vdash \ \ \)





\(\ds p \land q\)

\(\)







\(\ds \)











Proof
We apply the Method of Truth Tables.
$\begin{array}{|c|c||ccc|} \hline
p & q & p & \land & q\\
\hline
\F & \F & \F & \F & \F \\
\F & \T & \F & \F & \T \\
\T & \F & \T & \F & \F \\
\T & \T & \T & \T & \T \\
\hline
\end{array}$
As can be seen, only when both $p$ and $q$ are true, then so is $p \land q$.
$\blacksquare$





