# 

Source: https://proofwiki.org/wiki/Secant_Plus_One_over_Secant_Squared

Theorem
$\dfrac {\sec x + 1} {\sec^2 x} = \dfrac {\sin^2 x} {\sec x - 1}$


Proof













\(\ds \frac {\sec x + 1} {\sec^2 x}\)

\(=\)







\(\ds \cos^2 x \paren {\frac 1 {\cos x} + 1}\)





Definition of Secant Function














\(\ds \)

\(=\)







\(\ds \cos x + \cos^2x\)




















\(\ds \)

\(=\)







\(\ds \cos x \paren {1 + \cos x}\)




















\(\ds \)

\(=\)







\(\ds \cos x \frac {\paren {1 + \cos x} \paren {1 - \cos x} } {1 - \cos x}\)




















\(\ds \)

\(=\)







\(\ds \frac {1 - \cos^2 x} {\frac {1 - \cos x} {\cos x} }\)





Difference of Two Squares














\(\ds \)

\(=\)







\(\ds \frac {\sin^2 x} {\frac 1 {\cos x} - 1}\)





Sum of Squares of Sine and Cosine














\(\ds \)

\(=\)







\(\ds \frac {\sin^2 x} {\sec x - 1}\)





Definition of Secant Function



$\blacksquare$





