# 

Source: https://proofwiki.org/wiki/Second_Order_ODE/y_y%27%27_%2B_(y%27)%5E2_%3D_0

Theorem
The second order ODE:

$(1): \quad y y + \paren {y'}^2 = 0$
has the general solution:

$y^2 = C_1 x + C_2$


Proof
Using Solution of Second Order Differential Equation with Missing Independent Variable, $(1)$ can be expressed as:














\(\ds y p \frac {\d p} {\d y} + p^2\)

\(=\)







\(\ds 0\)





where $p = \dfrac {\d y} {\d x}$








\(\ds \leadsto \ \ \)





\(\ds y \rd p + p \rd y\)

\(=\)







\(\ds 0\)





multiplying by $\dfrac {\d y} p$








\(\ds \leadsto \ \ \)





\(\ds p y\)

\(=\)







\(\ds C\)





First Order ODE: $y \rd x + x \rd y = 0$








\(\ds \leadsto \ \ \)





\(\ds y \dfrac {\d y} {\d x}\)

\(=\)







\(\ds C\)





substituting $p = \dfrac {\d y} {\d x}$








\(\ds \leadsto \ \ \)





\(\ds y^2\)

\(=\)







\(\ds 2 C x + C_2\)





First Order ODE: $y \dfrac {\d y} {\d x} = k$














\(\ds \)

\(=\)







\(\ds C_1 x + C_2\)





reassigning constant



$\blacksquare$


Sources
1972: George F. Simmons: Differential Equations ... (previous) ... (next): $\S 2.11$: Problem $1 \ \text{(a)}$




